<?xml version="1.0" encoding="utf-8"?>
<rdf:RDF xmlns:cc="http://creativecommons.org/ns#"
   xmlns:dc="http://purl.org/dc/elements/1.1/"
   xmlns:dcat="http://www.w3.org/ns/dcat#"
   xmlns:dct="http://purl.org/dc/terms/"
   xmlns:foaf="http://xmlns.com/foaf/0.1/"
   xmlns:msxml="http://www.ilsp.gr/META-XMLSchema#"
   xmlns:ns="http://purl.org/net/def/metashare#"
   xmlns:odrl="http://www.w3.org/ns/odrl/2/"
   xmlns:owl="http://www.w3.org/2002/07/owl#"
   xmlns:rdf="http://www.w3.org/1999/02/22-rdf-syntax-ns#"
   xmlns:rdfs="http://www.w3.org/2000/01/rdf-schema#"
   xmlns:swrc="http://swrc.ontoware.org/ontology#">
  <owl:Ontology rdf:about="http://purl.org/net/def/metashare">
    <dct:creator rdf:resource="http://john.mccr.ae/"/>
    <dct:creator>John P. McCrae</dct:creator>
    <dct:creator>Jorge Gracia</dct:creator>
    <dct:creator>Marta Villegas</dct:creator>
    <dct:creator>Penny Labropoulou</dct:creator>
    <dct:creator>Philipp Cimiano</dct:creator>
    <dct:creator>Victor Rodriguez Doncel</dct:creator>
    <dct:license rdf:resource="http://purl.org/NET/rdflicense/cc-by4.0"/>
    <dct:modified>2015-03-20</dct:modified>
    <ns1:preferredNamespacePrefix xmlns:ns1="http://purl.org/vocab/vann/">ms</ns1:preferredNamespacePrefix>
    <ns2:preferredNamespaceUri xmlns:ns2="http://purl.org/vocab/vann/"
       rdf:resource="http://purl.org/net/def/metashare#"/>
    <rdfs:label xml:lang="en">Rights Information for Language Resources</rdfs:label>
    <owl:priorVersion rdf:resource="http://lodserver.iula.upf.edu/Metashare/ontology/"/>
    <owl:priorVersion rdf:resource="http://purl.org/ms-lod/MetaShareRights.ttl#"/>
  </owl:Ontology>
  <ns:VisualModelling rdf:about="http://purl.org/net/def/metashare#2D"/>
  <ns:VisualModelling rdf:about="http://purl.org/net/def/metashare#3D"/>
  <ns:SourceChannelType rdf:about="http://purl.org/net/def/metashare#3G"/>
  <ns:ColourSpace rdf:about="http://purl.org/net/def/metashare#4:2:2"/>
  <ns:SignalEncoding rdf:about="http://purl.org/net/def/metashare#ADPCM"/>
  <ns:ConformanceToClassificationScheme rdf:about="http://purl.org/net/def/metashare#ANC_domainClassification"/>
  <ns:ConformanceToClassificationScheme rdf:about="http://purl.org/net/def/metashare#ANC_genreClassification"/>
  <owl:Class rdf:about="http://purl.org/net/def/metashare#Actor">
    <owl:equivalentClass rdf:resource="http://xmlns.com/foaf/0.1/Actor"/>
  </owl:Class>
  <owl:Class rdf:about="http://purl.org/net/def/metashare#ActualUseInfo">
    <rdfs:comment xml:lang="en">Groups information on how the resource has already been used</rdfs:comment>
  </owl:Class>
  <owl:Class rdf:about="http://purl.org/net/def/metashare#AgeGroup">
    <rdfs:comment xml:lang="en">The age group to which the participant belongs</rdfs:comment>
  </owl:Class>
  <owl:Class rdf:about="http://purl.org/net/def/metashare#AgeOfPersons">
    <rdfs:comment xml:lang="en">The age range of the group of participants; repeat the element if needed</rdfs:comment>
  </owl:Class>
  <owl:Class rdf:about="http://purl.org/net/def/metashare#AnnotatedElements">
    <rdfs:comment xml:lang="en">Specifies the elements annotated in each annotation level</rdfs:comment>
  </owl:Class>
  <owl:Class rdf:about="http://purl.org/net/def/metashare#AnnotationInfo">
    <rdfs:comment xml:lang="en">Groups information on the annotated part(s) of a resource</rdfs:comment>
  </owl:Class>
  <owl:Class rdf:about="http://purl.org/net/def/metashare#AnnotationMode">
    <rdfs:comment xml:lang="en">Indicates whether the resource is annotated manually or by automatic processes</rdfs:comment>
  </owl:Class>
  <owl:Class rdf:about="http://purl.org/net/def/metashare#AnnotationType">
    <rdfs:comment xml:lang="en">Specifies the annotation level of the resource or the annotation type a tool/ service requires or produces as an output</rdfs:comment>
  </owl:Class>
  <owl:Class rdf:about="http://purl.org/net/def/metashare#Audience">
    <rdfs:comment xml:lang="en">Indication of the intended audience size</rdfs:comment>
  </owl:Class>
  <owl:Class rdf:about="http://purl.org/net/def/metashare#AudioClassificationInfo">
    <rdfs:comment xml:lang="en">Groups together information on audio type/genre of the resource</rdfs:comment>
    <rdfs:subClassOf rdf:resource="http://purl.org/net/def/metashare#ClassificationInfo"/>
  </owl:Class>
  <owl:Class rdf:about="http://purl.org/net/def/metashare#AudioFormatInfo">
    <rdfs:comment xml:lang="en">Groups together information on the format of the audio part of a resource</rdfs:comment>
  </owl:Class>
  <owl:Class rdf:about="http://purl.org/net/def/metashare#AudioQualityMeasuresIncluded">
    <rdfs:comment xml:lang="en">Specifies the audio quality measures</rdfs:comment>
  </owl:Class>
  <owl:Class rdf:about="http://purl.org/net/def/metashare#AudioSizeInfo">
    <rdfs:comment xml:lang="en">SizeInfo Element for Audio parts of a resource</rdfs:comment>
  </owl:Class>
  <owl:Class rdf:about="http://purl.org/net/def/metashare#Availability">
    <rdfs:comment xml:lang="en">Availability status of the resource; conditionsOfUse can be further used to indicate the specific terms of availability</rdfs:comment>
    <rdfs:comment xml:lang="en">Specifies the availability status of the resource; restrictionsOfUse can be further used to indicate the specific terms of availability</rdfs:comment>
  </owl:Class>
  <ns:ConformanceToStandardsBestPractices rdf:about="http://purl.org/net/def/metashare#BLM"/>
  <ns:ConformanceToClassificationScheme rdf:about="http://purl.org/net/def/metashare#BNC_domainClassification"/>
  <ns:ConformanceToClassificationScheme rdf:about="http://purl.org/net/def/metashare#BNC_textTypeClassification"/>
  <owl:Class rdf:about="http://purl.org/net/def/metashare#BaseItem">
    <rdfs:comment xml:lang="en">Type of item that is represented in the n-gram resource</rdfs:comment>
  </owl:Class>
  <ns:CharacterEncoding rdf:about="http://purl.org/net/def/metashare#Big5"/>
  <ns:CharacterEncoding rdf:about="http://purl.org/net/def/metashare#Big5-HKSCS"/>
  <ns:CharacterEncoding rdf:about="http://purl.org/net/def/metashare#Big5_Solaris"/>
  <owl:Class rdf:about="http://purl.org/net/def/metashare#BodyParts">
    <rdfs:comment xml:lang="en">The body parts visible in the video or image part of the resource</rdfs:comment>
  </owl:Class>
  <owl:Class rdf:about="http://purl.org/net/def/metashare#ByteOrder">
    <rdfs:comment xml:lang="en">The byte order of 2 or more bytes sample</rdfs:comment>
  </owl:Class>
  <ns:SourceChannelType rdf:about="http://purl.org/net/def/metashare#C"/>
  <ns:DistributionAccessMedium rdf:about="http://purl.org/net/def/metashare#CD-ROM">
    <rdfs:comment xml:lang="en">CD-ROM refers to a kind of distribution/access medium used for delivering a language resource; intended for resources delivered on CD-ROM</rdfs:comment>
  </ns:DistributionAccessMedium>
  <ns:SourceChannelType rdf:about="http://purl.org/net/def/metashare#CDMA"/>
  <ns:ConformanceToStandardsBestPractices rdf:about="http://purl.org/net/def/metashare#CES"/>
  <ns:ColourSpace rdf:about="http://purl.org/net/def/metashare#CMYK"/>
  <owl:Class rdf:about="http://purl.org/net/def/metashare#CapturingDeviceType">
    <rdfs:comment xml:lang="en">The transducers through which the data is captured</rdfs:comment>
  </owl:Class>
  <owl:Class rdf:about="http://purl.org/net/def/metashare#CapturingEnvironment">
    <rdfs:comment xml:lang="en">Type of capturing environment</rdfs:comment>
  </owl:Class>
  <owl:Class rdf:about="http://purl.org/net/def/metashare#CharacterEncoding">
    <rdfs:comment xml:lang="en">The name of the character encoding used in the resource or accepted by the tool/service</rdfs:comment>
  </owl:Class>
  <owl:Class rdf:about="http://purl.org/net/def/metashare#CharacterEncodingInfo">
    <rdfs:comment xml:lang="en">Groups together information on character encoding of the resource</rdfs:comment>
  </owl:Class>
  <rdf:Description rdf:about="http://purl.org/net/def/metashare#CharacterEncodingSet">
    <dct:replaces rdf:resource="http://www.ilsp.gr/META-XMLSchema#characterEncoding"/>
  </rdf:Description>
  <owl:Class rdf:about="http://purl.org/net/def/metashare#ClassificationInfo"/>
  <owl:Class rdf:about="http://purl.org/net/def/metashare#ColourSpace">
    <rdfs:comment xml:lang="en">Defines the colour space for the video</rdfs:comment>
  </owl:Class>
  <owl:Class rdf:about="http://purl.org/net/def/metashare#CompatibleLexiconType">
    <rdfs:comment xml:lang="en">Type of (external) lexicon that can be used with the grammar</rdfs:comment>
  </owl:Class>
  <owl:Class rdf:about="http://purl.org/net/def/metashare#CompressionName">
    <rdfs:comment xml:lang="en">The name of the compression applied</rdfs:comment>
  </owl:Class>
  <owl:Class rdf:about="http://purl.org/net/def/metashare#ComputationalLexicon">
    <rdfs:subClassOf rdf:resource="http://purl.org/net/def/metashare#LexicalConceptualResourceInfo"/>
    <owl:equivalentClass>
      <rdf:Description>
        <owl:hasValue rdf:resource="http://purl.org/net/def/metashare#computationalLexicon"/>
        <owl:onProperty rdf:resource="http://purl.org/net/def/metashare#lexicalConcepturalResourceType"/>
      </rdf:Description>
    </owl:equivalentClass>
  </owl:Class>
  <owl:Class rdf:about="http://purl.org/net/def/metashare#ConditionsOfUse">
    <dct:replaces rdf:resource="http://www.ilsp.gr/META-XMLSchema#restrictionsOfUse"/>
    <rdfs:comment xml:lang="en">The conditionsOfUse optional element in the metadata is only to be taken as providing brief human readable information on the fact that the LR is provided under a specific set of conditions. These correspond to the most frequently used conditions imposed by the licensor of the LR (via the specified licence). The proper exposition of all conditions and possible exceptions is to be found inside the licence text. LR depositors should, hence, carefully choose the values of this field to match the licence chosen and users should carefully read that licence before using the LR.</rdfs:comment>
  </owl:Class>
  <owl:Class rdf:about="http://purl.org/net/def/metashare#ConformanceToClassificationScheme">
    <rdfs:comment xml:lang="en">Specifies the external classification schemes</rdfs:comment>
  </owl:Class>
  <owl:Class rdf:about="http://purl.org/net/def/metashare#ConformanceToStandardsBestPractices">
    <rdfs:comment xml:lang="en">Specifies the standards or the best practices to which the tagset used for the annotation conforms </rdfs:comment>
  </owl:Class>
  <owl:Class rdf:about="http://purl.org/net/def/metashare#ContactPerson">
    <rdfs:comment xml:lang="en">Groups information on the person(s) that is/are responsible for providing further information regarding the resource</rdfs:comment>
  </owl:Class>
  <owl:Class rdf:about="http://purl.org/net/def/metashare#ConversationalType">
    <rdfs:comment xml:lang="en">Specifies the conversational type of the resource</rdfs:comment>
  </owl:Class>
  <owl:Class rdf:about="http://purl.org/net/def/metashare#Corpus">
    <rdfs:subClassOf rdf:resource="http://purl.org/net/def/metashare#LanguageResource"/>
    <owl:equivalentClass>
      <owl:Restriction>
        <owl:onProperty rdf:resource="http://purl.org/net/def/metashare#corpusInfo"/>
        <owl:someValuesFrom rdf:resource="http://purl.org/net/def/metashare#CorpusInfo"/>
      </owl:Restriction>
    </owl:equivalentClass>
  </owl:Class>
  <owl:Class rdf:about="http://purl.org/net/def/metashare#CorpusAudio">
    <rdfs:subClassOf rdf:resource="http://purl.org/net/def/metashare#CorpusMediaPart"/>
    <rdfs:subclassOf rdf:resource="http://purl.org/net/def/metashare#CorpusInfo"/>
    <owl:equivalentClass>
      <owl:Restriction>
        <owl:onProperty rdf:resource="http://purl.org/net/def/metashare#corpusAudioInfo"/>
        <owl:someValuesFrom rdf:resource="http://purl.org/net/def/metashare#CorpusAudioInfo"/>
      </owl:Restriction>
    </owl:equivalentClass>
  </owl:Class>
  <owl:Class rdf:about="http://purl.org/net/def/metashare#CorpusAudioInfo">
    <rdfs:comment xml:lang="en">Groups together information on the audio module of a corpus</rdfs:comment>
  </owl:Class>
  <owl:Class rdf:about="http://purl.org/net/def/metashare#CorpusImage">
    <rdfs:subClassOf rdf:resource="http://purl.org/net/def/metashare#CorpusMediaPart"/>
    <rdfs:subclassOf rdf:resource="http://purl.org/net/def/metashare#CorpusInfo"/>
    <owl:equivalentClass>
      <owl:Restriction>
        <owl:onProperty rdf:resource="http://purl.org/net/def/metashare#corpusImageInfo"/>
        <owl:someValuesFrom rdf:resource="http://purl.org/net/def/metashare#CorpusImageInfo"/>
      </owl:Restriction>
    </owl:equivalentClass>
  </owl:Class>
  <owl:Class rdf:about="http://purl.org/net/def/metashare#CorpusImageInfo">
    <rdfs:comment xml:lang="en">Groups together information on the image component of a resource</rdfs:comment>
  </owl:Class>
  <owl:Class rdf:about="http://purl.org/net/def/metashare#CorpusInfo">
    <rdfs:comment xml:lang="en">Groups together information on corpora of all media types</rdfs:comment>
  </owl:Class>
  <owl:Class rdf:about="http://purl.org/net/def/metashare#CorpusMediaPart">
    <rdfs:subClassOf rdf:resource="http://purl.org/net/def/metashare#MediaPart"/>
  </owl:Class>
  <owl:Class rdf:about="http://purl.org/net/def/metashare#CorpusText">
    <rdfs:subClassOf rdf:resource="http://purl.org/net/def/metashare#CorpusMediaPart"/>
    <rdfs:subclassOf rdf:resource="http://purl.org/net/def/metashare#CorpusInfo"/>
    <owl:equivalentClass>
      <owl:Restriction>
        <owl:onProperty rdf:resource="http://purl.org/net/def/metashare#corpusTextInfo"/>
        <owl:someValuesFrom rdf:resource="http://purl.org/net/def/metashare#CorpusTextInfo"/>
      </owl:Restriction>
    </owl:equivalentClass>
  </owl:Class>
  <owl:Class rdf:about="http://purl.org/net/def/metashare#CorpusTextInfo">
    <rdfs:comment xml:lang="en">Groups together information on the text component of a resource</rdfs:comment>
  </owl:Class>
  <owl:Class rdf:about="http://purl.org/net/def/metashare#CorpusTextNgram">
    <rdfs:subClassOf rdf:resource="http://purl.org/net/def/metashare#CorpusMediaPart"/>
    <rdfs:subclassOf rdf:resource="http://purl.org/net/def/metashare#CorpusInfo"/>
    <owl:equivalentClass>
      <owl:Restriction>
        <owl:onProperty rdf:resource="http://purl.org/net/def/metashare#corpusTextNgramInfo"/>
        <owl:someValuesFrom rdf:resource="http://purl.org/net/def/metashare#CorpusTextNgramInfo"/>
      </owl:Restriction>
    </owl:equivalentClass>
  </owl:Class>
  <owl:Class rdf:about="http://purl.org/net/def/metashare#CorpusTextNgramInfo">
    <rdfs:comment xml:lang="en">Groups together information required for n-gram resources; information can be provided both as regards features drawn from the source corpus (e.g. language coverage, size, format, domains etc.) and features pertaining to the n-gram output itself (e.g. range of n-grams, type of item included, etc.)</rdfs:comment>
  </owl:Class>
  <owl:Class rdf:about="http://purl.org/net/def/metashare#CorpusTextNumerical">
    <rdfs:subClassOf rdf:resource="http://purl.org/net/def/metashare#CorpusMediaPart"/>
    <rdfs:subclassOf rdf:resource="http://purl.org/net/def/metashare#CorpusInfo"/>
    <owl:equivalentClass>
      <owl:Restriction>
        <owl:onProperty rdf:resource="http://purl.org/net/def/metashare#corpusTextNumericalInfo"/>
        <owl:someValuesFrom rdf:resource="http://purl.org/net/def/metashare#CorpusTextNumericalInfo"/>
      </owl:Restriction>
    </owl:equivalentClass>
  </owl:Class>
  <owl:Class rdf:about="http://purl.org/net/def/metashare#CorpusTextNumericalInfo">
    <rdfs:comment xml:lang="en">Groups together information on the textNumerical component of a corpus. It is used basically for the textual representation of measurements and observations linked to sensorimotor recordings</rdfs:comment>
  </owl:Class>
  <owl:Class rdf:about="http://purl.org/net/def/metashare#CorpusVideo">
    <rdfs:subClassOf rdf:resource="http://purl.org/net/def/metashare#CorpusMediaPart"/>
    <rdfs:subclassOf rdf:resource="http://purl.org/net/def/metashare#CorpusInfo"/>
    <owl:equivalentClass>
      <owl:Restriction>
        <owl:onProperty rdf:resource="http://purl.org/net/def/metashare#corpusVideoInfo"/>
        <owl:someValuesFrom rdf:resource="http://purl.org/net/def/metashare#CorpusVideoInfo"/>
      </owl:Restriction>
    </owl:equivalentClass>
  </owl:Class>
  <owl:Class rdf:about="http://purl.org/net/def/metashare#CorpusVideoInfo">
    <rdfs:comment xml:lang="en">Groups together information on the video component of a corpus</rdfs:comment>
  </owl:Class>
  <ns:CharacterEncoding rdf:about="http://purl.org/net/def/metashare#Cp037"/>
  <ns:CharacterEncoding rdf:about="http://purl.org/net/def/metashare#Cp1006"/>
  <ns:CharacterEncoding rdf:about="http://purl.org/net/def/metashare#Cp1025"/>
  <ns:CharacterEncoding rdf:about="http://purl.org/net/def/metashare#Cp1026"/>
  <ns:CharacterEncoding rdf:about="http://purl.org/net/def/metashare#Cp1046"/>
  <ns:CharacterEncoding rdf:about="http://purl.org/net/def/metashare#Cp1047"/>
  <ns:CharacterEncoding rdf:about="http://purl.org/net/def/metashare#Cp1097"/>
  <ns:CharacterEncoding rdf:about="http://purl.org/net/def/metashare#Cp1098"/>
  <ns:CharacterEncoding rdf:about="http://purl.org/net/def/metashare#Cp1112"/>
  <ns:CharacterEncoding rdf:about="http://purl.org/net/def/metashare#Cp1122"/>
  <ns:CharacterEncoding rdf:about="http://purl.org/net/def/metashare#Cp1123"/>
  <ns:CharacterEncoding rdf:about="http://purl.org/net/def/metashare#Cp1124"/>
  <ns:CharacterEncoding rdf:about="http://purl.org/net/def/metashare#Cp1140"/>
  <ns:CharacterEncoding rdf:about="http://purl.org/net/def/metashare#Cp1141"/>
  <ns:CharacterEncoding rdf:about="http://purl.org/net/def/metashare#Cp1142"/>
  <ns:CharacterEncoding rdf:about="http://purl.org/net/def/metashare#Cp1143"/>
  <ns:CharacterEncoding rdf:about="http://purl.org/net/def/metashare#Cp1144"/>
  <ns:CharacterEncoding rdf:about="http://purl.org/net/def/metashare#Cp1145"/>
  <ns:CharacterEncoding rdf:about="http://purl.org/net/def/metashare#Cp1146"/>
  <ns:CharacterEncoding rdf:about="http://purl.org/net/def/metashare#Cp1147"/>
  <ns:CharacterEncoding rdf:about="http://purl.org/net/def/metashare#Cp1148"/>
  <ns:CharacterEncoding rdf:about="http://purl.org/net/def/metashare#Cp1149"/>
  <ns:CharacterEncoding rdf:about="http://purl.org/net/def/metashare#Cp1381"/>
  <ns:CharacterEncoding rdf:about="http://purl.org/net/def/metashare#Cp1383"/>
  <ns:CharacterEncoding rdf:about="http://purl.org/net/def/metashare#Cp273"/>
  <ns:CharacterEncoding rdf:about="http://purl.org/net/def/metashare#Cp277"/>
  <ns:CharacterEncoding rdf:about="http://purl.org/net/def/metashare#Cp278"/>
  <ns:CharacterEncoding rdf:about="http://purl.org/net/def/metashare#Cp280"/>
  <ns:CharacterEncoding rdf:about="http://purl.org/net/def/metashare#Cp284"/>
  <ns:CharacterEncoding rdf:about="http://purl.org/net/def/metashare#Cp285"/>
  <ns:CharacterEncoding rdf:about="http://purl.org/net/def/metashare#Cp297"/>
  <ns:CharacterEncoding rdf:about="http://purl.org/net/def/metashare#Cp33722"/>
  <ns:CharacterEncoding rdf:about="http://purl.org/net/def/metashare#Cp420"/>
  <ns:CharacterEncoding rdf:about="http://purl.org/net/def/metashare#Cp424"/>
  <ns:CharacterEncoding rdf:about="http://purl.org/net/def/metashare#Cp437"/>
  <ns:CharacterEncoding rdf:about="http://purl.org/net/def/metashare#Cp500"/>
  <ns:CharacterEncoding rdf:about="http://purl.org/net/def/metashare#Cp737"/>
  <ns:CharacterEncoding rdf:about="http://purl.org/net/def/metashare#Cp775"/>
  <ns:CharacterEncoding rdf:about="http://purl.org/net/def/metashare#Cp838"/>
  <ns:CharacterEncoding rdf:about="http://purl.org/net/def/metashare#Cp850"/>
  <ns:CharacterEncoding rdf:about="http://purl.org/net/def/metashare#Cp852"/>
  <ns:CharacterEncoding rdf:about="http://purl.org/net/def/metashare#Cp855"/>
  <ns:CharacterEncoding rdf:about="http://purl.org/net/def/metashare#Cp856"/>
  <ns:CharacterEncoding rdf:about="http://purl.org/net/def/metashare#Cp857"/>
  <ns:CharacterEncoding rdf:about="http://purl.org/net/def/metashare#Cp858"/>
  <ns:CharacterEncoding rdf:about="http://purl.org/net/def/metashare#Cp860"/>
  <ns:CharacterEncoding rdf:about="http://purl.org/net/def/metashare#Cp861"/>
  <ns:CharacterEncoding rdf:about="http://purl.org/net/def/metashare#Cp862"/>
  <ns:CharacterEncoding rdf:about="http://purl.org/net/def/metashare#Cp863"/>
  <ns:CharacterEncoding rdf:about="http://purl.org/net/def/metashare#Cp864"/>
  <ns:CharacterEncoding rdf:about="http://purl.org/net/def/metashare#Cp865"/>
  <ns:CharacterEncoding rdf:about="http://purl.org/net/def/metashare#Cp866"/>
  <ns:CharacterEncoding rdf:about="http://purl.org/net/def/metashare#Cp868"/>
  <ns:CharacterEncoding rdf:about="http://purl.org/net/def/metashare#Cp869"/>
  <ns:CharacterEncoding rdf:about="http://purl.org/net/def/metashare#Cp870"/>
  <ns:CharacterEncoding rdf:about="http://purl.org/net/def/metashare#Cp871"/>
  <ns:CharacterEncoding rdf:about="http://purl.org/net/def/metashare#Cp874"/>
  <ns:CharacterEncoding rdf:about="http://purl.org/net/def/metashare#Cp875"/>
  <ns:CharacterEncoding rdf:about="http://purl.org/net/def/metashare#Cp918"/>
  <ns:CharacterEncoding rdf:about="http://purl.org/net/def/metashare#Cp921"/>
  <ns:CharacterEncoding rdf:about="http://purl.org/net/def/metashare#Cp922"/>
  <ns:CharacterEncoding rdf:about="http://purl.org/net/def/metashare#Cp930"/>
  <ns:CharacterEncoding rdf:about="http://purl.org/net/def/metashare#Cp933"/>
  <ns:CharacterEncoding rdf:about="http://purl.org/net/def/metashare#Cp935"/>
  <ns:CharacterEncoding rdf:about="http://purl.org/net/def/metashare#Cp937"/>
  <ns:CharacterEncoding rdf:about="http://purl.org/net/def/metashare#Cp939"/>
  <ns:CharacterEncoding rdf:about="http://purl.org/net/def/metashare#Cp942"/>
  <ns:CharacterEncoding rdf:about="http://purl.org/net/def/metashare#Cp942C"/>
  <ns:CharacterEncoding rdf:about="http://purl.org/net/def/metashare#Cp943"/>
  <ns:CharacterEncoding rdf:about="http://purl.org/net/def/metashare#Cp943C"/>
  <ns:CharacterEncoding rdf:about="http://purl.org/net/def/metashare#Cp948"/>
  <ns:CharacterEncoding rdf:about="http://purl.org/net/def/metashare#Cp949"/>
  <ns:CharacterEncoding rdf:about="http://purl.org/net/def/metashare#Cp949C"/>
  <ns:CharacterEncoding rdf:about="http://purl.org/net/def/metashare#Cp950"/>
  <ns:CharacterEncoding rdf:about="http://purl.org/net/def/metashare#Cp964"/>
  <ns:CharacterEncoding rdf:about="http://purl.org/net/def/metashare#Cp970"/>
  <owl:Class rdf:about="http://purl.org/net/def/metashare#CreationMode">
    <rdfs:comment xml:lang="en">Specifies whether the resource is created automatically or in a manual or interactive mode </rdfs:comment>
  </owl:Class>
  <ns:RecordingDeviceType rdf:about="http://purl.org/net/def/metashare#DAT"/>
  <ns:ConformanceToClassificationScheme rdf:about="http://purl.org/net/def/metashare#DDC_classification"/>
  <ns:DistributionAccessMedium rdf:about="http://purl.org/net/def/metashare#DVD-R"/>
  <rdf:Description rdf:about="http://purl.org/net/def/metashare#DiscourseAnnotation">
    <rdfs:subClassOf rdf:resource="http://purl.org/net/def/metashare#AnnotationType"/>
  </rdf:Description>
  <owl:Class rdf:about="http://purl.org/net/def/metashare#DistributionAccessMedium">
    <rdfs:comment xml:lang="en">Specifies the medium (channel) used for delivery or providing access to the resource</rdfs:comment>
    <rdfs:comment xml:lang="en">Specifies the medium (channel) used for delivery or providing access to the resource.</rdfs:comment>
  </owl:Class>
  <rdf:Description rdf:about="http://purl.org/net/def/metashare#DistributionInfo">
    <owl:equivalentClass rdf:resource="http://www.w3.org/ns/dcat#Distribution"/>
  </rdf:Description>
  <rdf:Description rdf:about="http://purl.org/net/def/metashare#Document">
    <owl:equivalentClass rdf:resource="http://swrc.ontoware.org/ontology#Publication"/>
  </rdf:Description>
  <owl:Class rdf:about="http://purl.org/net/def/metashare#DocumentInfo"/>
  <owl:Class rdf:about="http://purl.org/net/def/metashare#Documentation">
    <rdfs:comment xml:lang="en">Refers to papers, manuals, reports etc. describing the resource</rdfs:comment>
  </owl:Class>
  <rdf:Description rdf:about="http://purl.org/net/def/metashare#DomainClassification">
    <dct:replaces rdf:resource="http://www.ilsp.gr/META-XMLSchema#domainInfo"/>
  </rdf:Description>
  <owl:Class rdf:about="http://purl.org/net/def/metashare#DomainInfo">
    <rdfs:comment xml:lang="en">Groups together information on domains represented in the resource; can be repeated for parts of the resource with distinct domain</rdfs:comment>
  </owl:Class>
  <owl:Class rdf:about="http://purl.org/net/def/metashare#DurationOfAudioInfoUnit"/>
  <owl:Class rdf:about="http://purl.org/net/def/metashare#DurationOfEffectiveSpeechInfoUnit"/>
  <owl:Class rdf:about="http://purl.org/net/def/metashare#DynamicElementInfo">
    <rdfs:comment xml:lang="en">Groups information on the dynamic elements that are represented in the video part of the resource</rdfs:comment>
  </owl:Class>
  <ns:ConformanceToStandardsBestPractices rdf:about="http://purl.org/net/def/metashare#EAGLES"/>
  <ns:MembershipInstitution rdf:about="http://purl.org/net/def/metashare#ELRA"/>
  <ns:SourceChannel rdf:about="http://purl.org/net/def/metashare#EMA"/>
  <ns:ConformanceToStandardsBestPractices rdf:about="http://purl.org/net/def/metashare#EML"/>
  <ns:ConformanceToStandardsBestPractices rdf:about="http://purl.org/net/def/metashare#EMMA"/>
  <ns:CharacterEncoding rdf:about="http://purl.org/net/def/metashare#EUC-JP"/>
  <ns:CharacterEncoding rdf:about="http://purl.org/net/def/metashare#EUC-KR"/>
  <owl:Class rdf:about="http://purl.org/net/def/metashare#EncodingLevel">
    <rdfs:comment xml:lang="en">Information on the contents of the lexicalConceptualResource as regards the linguistic level of analysis</rdfs:comment>
  </owl:Class>
  <owl:Class rdf:about="http://purl.org/net/def/metashare#EvaluationCriteria">
    <rdfs:comment xml:lang="en">Defines the criteria of the evaluation of a tool</rdfs:comment>
  </owl:Class>
  <owl:Class rdf:about="http://purl.org/net/def/metashare#EvaluationLevel">
    <rdfs:comment xml:lang="en">Indicates the evaluation level</rdfs:comment>
  </owl:Class>
  <owl:Class rdf:about="http://purl.org/net/def/metashare#EvaluationMeasure">
    <rdfs:comment xml:lang="en">Defines whether the evaluation measure is human or automatic</rdfs:comment>
  </owl:Class>
  <owl:Class rdf:about="http://purl.org/net/def/metashare#EvaluationType">
    <rdfs:comment xml:lang="en">Indicates the evaluation type</rdfs:comment>
  </owl:Class>
  <owl:Class rdf:about="http://purl.org/net/def/metashare#ExtraTextualInformationUnit">
    <rdfs:comment xml:lang="en">The unit of the extratextual information contained in the lexical conceptual resource</rdfs:comment>
  </owl:Class>
  <owl:Class rdf:about="http://purl.org/net/def/metashare#ExtratextualInformation">
    <rdfs:comment xml:lang="en">An indication of the extratextual information contained in the lexicalConceptualResouce; can be used as an alternative to audio, image, videos etc. for cases where these are not considered an important part of the lcr</rdfs:comment>
  </owl:Class>
  <owl:Class rdf:about="http://purl.org/net/def/metashare#ForeseenUseInfo">
    <rdfs:comment xml:lang="en">Groups information on the use for which the resource is created</rdfs:comment>
  </owl:Class>
  <owl:Class rdf:about="http://purl.org/net/def/metashare#FrameNet">
    <rdfs:subClassOf rdf:resource="http://purl.org/net/def/metashare#LexicalConceptualResourceInfo"/>
    <owl:equivalentClass>
      <rdf:Description>
        <owl:hasValue rdf:resource="http://purl.org/net/def/metashare#frameNet"/>
        <owl:onProperty rdf:resource="http://purl.org/net/def/metashare#lexicalConcepturalResourceType"/>
      </rdf:Description>
    </owl:equivalentClass>
  </owl:Class>
  <owl:Class rdf:about="http://purl.org/net/def/metashare#FundingType">
    <rdfs:comment xml:lang="en">Specifies the type of funding of the project</rdfs:comment>
  </owl:Class>
  <ns:CharacterEncoding rdf:about="http://purl.org/net/def/metashare#GB18030"/>
  <ns:CharacterEncoding rdf:about="http://purl.org/net/def/metashare#GBK"/>
  <ns:ConformanceToStandardsBestPractices rdf:about="http://purl.org/net/def/metashare#GMX"/>
  <ns:SourceChannelType rdf:about="http://purl.org/net/def/metashare#GSM"/>
  <rdf:Description rdf:about="http://purl.org/net/def/metashare#GeographicCoverageClassification">
    <dct:replaces rdf:resource="http://www.ilsp.gr/META-XMLSchema#geographicCoverageInfo"/>
  </rdf:Description>
  <owl:Class rdf:about="http://purl.org/net/def/metashare#GeographicCoverageInfo">
    <rdfs:comment xml:lang="en">Groups information on geographic classification of the resource</rdfs:comment>
  </owl:Class>
  <ns:ConformanceToStandardsBestPractices rdf:about="http://purl.org/net/def/metashare#GrAF"/>
  <owl:Class rdf:about="http://purl.org/net/def/metashare#GrammaticalPhenomenaCoverage">
    <rdfs:comment xml:lang="en">An indication of the grammatical phenomena covered by the grammar</rdfs:comment>
  </owl:Class>
  <ns:ResolutionStandard rdf:about="http://purl.org/net/def/metashare#HD.1080"/>
  <ns:ResolutionStandard rdf:about="http://purl.org/net/def/metashare#HD.720"/>
  <ns:ConformanceToStandardsBestPractices rdf:about="http://purl.org/net/def/metashare#HamNoSys"/>
  <owl:Class rdf:about="http://purl.org/net/def/metashare#HearingImpairmentOfPersons">
    <rdfs:comment xml:lang="en">Whether the group of participants contains persons with hearing impairments</rdfs:comment>
  </owl:Class>
  <ns:CharacterEncoding rdf:about="http://purl.org/net/def/metashare#ISCII91"/>
  <ns:SourceChannelType rdf:about="http://purl.org/net/def/metashare#ISDN"/>
  <ns:CharacterEncoding rdf:about="http://purl.org/net/def/metashare#ISO-2022-JP"/>
  <ns:CharacterEncoding rdf:about="http://purl.org/net/def/metashare#ISO-2022-KR"/>
  <ns:CharacterEncoding rdf:about="http://purl.org/net/def/metashare#ISO-8859-1"/>
  <ns:CharacterEncoding rdf:about="http://purl.org/net/def/metashare#ISO-8859-15"/>
  <ns:CharacterEncoding rdf:about="http://purl.org/net/def/metashare#ISO-8859-2"/>
  <ns:CharacterEncoding rdf:about="http://purl.org/net/def/metashare#ISO-8859-3"/>
  <ns:CharacterEncoding rdf:about="http://purl.org/net/def/metashare#ISO-8859-4"/>
  <ns:CharacterEncoding rdf:about="http://purl.org/net/def/metashare#ISO-8859-5"/>
  <ns:CharacterEncoding rdf:about="http://purl.org/net/def/metashare#ISO-8859-6"/>
  <ns:CharacterEncoding rdf:about="http://purl.org/net/def/metashare#ISO-8859-7"/>
  <ns:CharacterEncoding rdf:about="http://purl.org/net/def/metashare#ISO-8859-8"/>
  <ns:CharacterEncoding rdf:about="http://purl.org/net/def/metashare#ISO-8859-9"/>
  <ns:CharacterEncoding rdf:about="http://purl.org/net/def/metashare#ISO-8860-13"/>
  <ns:ConformanceToStandardsBestPractices rdf:about="http://purl.org/net/def/metashare#ISO12620"/>
  <ns:ConformanceToStandardsBestPractices rdf:about="http://purl.org/net/def/metashare#ISO16642"/>
  <ns:ConformanceToStandardsBestPractices rdf:about="http://purl.org/net/def/metashare#ISO1987"/>
  <ns:CharacterEncoding rdf:about="http://purl.org/net/def/metashare#ISO2022_CN_CNS"/>
  <ns:CharacterEncoding rdf:about="http://purl.org/net/def/metashare#ISO2022_CN_GB"/>
  <ns:ConformanceToStandardsBestPractices rdf:about="http://purl.org/net/def/metashare#ISO26162"/>
  <ns:ConformanceToStandardsBestPractices rdf:about="http://purl.org/net/def/metashare#ISO30042"/>
  <ns:ConformanceToStandardsBestPractices rdf:about="http://purl.org/net/def/metashare#ISO704"/>
  <owl:Class rdf:about="http://purl.org/net/def/metashare#ImageClassificationInfo">
    <rdfs:comment xml:lang="en">Groups together information on image type/genre of the resource</rdfs:comment>
    <rdfs:subClassOf rdf:resource="http://purl.org/net/def/metashare#ClassificationInfo"/>
  </owl:Class>
  <owl:Class rdf:about="http://purl.org/net/def/metashare#ImageFormatInfo">
    <rdfs:comment xml:lang="en">Groups together information on the format of the image part of a resource</rdfs:comment>
  </owl:Class>
  <ns:ConformanceToStandardsBestPractices rdf:about="http://purl.org/net/def/metashare#InkML"/>
  <owl:Class rdf:about="http://purl.org/net/def/metashare#InputInfo">
    <rdfs:comment xml:lang="en">Groups together information on the requirements set on the input resource of a tool or service</rdfs:comment>
  </owl:Class>
  <owl:Class rdf:about="http://purl.org/net/def/metashare#Interactivity">
    <rdfs:comment xml:lang="en">Indicates the level of conversational interaction between speakers (for audio component) or participants (for video component)</rdfs:comment>
  </owl:Class>
  <ns:CharacterEncoding rdf:about="http://purl.org/net/def/metashare#JISAutoDetect"/>
  <ns:CharacterEncoding rdf:about="http://purl.org/net/def/metashare#KOI8-R"/>
  <ns:MembershipInstitution rdf:about="http://purl.org/net/def/metashare#LDC"/>
  <ns:ConformanceToStandardsBestPractices rdf:about="http://purl.org/net/def/metashare#LMF"/>
  <owl:Class rdf:about="http://purl.org/net/def/metashare#LanguageDescription">
    <rdfs:subClassOf rdf:resource="http://purl.org/net/def/metashare#LanguageResource"/>
    <owl:equivalentClass>
      <owl:Restriction>
        <owl:onProperty rdf:resource="http://purl.org/net/def/metashare#languageDescriptionInfo"/>
        <owl:someValuesFrom rdf:resource="http://purl.org/net/def/metashare#LanguageDescriptionInfo"/>
      </owl:Restriction>
    </owl:equivalentClass>
  </owl:Class>
  <owl:Class rdf:about="http://purl.org/net/def/metashare#LanguageDescriptionImage">
    <rdf:type rdf:resource="http://www.w3.org/2002/07/owl#Class"/>
    <rdfs:subClassOf rdf:resource="http://purl.org/net/def/metashare#LanguageDescriptionInfo"/>
    <rdfs:subClassOf rdf:resource="http://purl.org/net/def/metashare#LanguageDescriptionMediaPart"/>
    <rdfs:subclassOf rdf:resource="http://purl.org/net/def/metashare#LanguageDescriptionInfo"/>
    <owl:equivalentClass>
      <owl:Restriction>
        <owl:onProperty rdf:resource="http://purl.org/net/def/metashare#languageDescriptionImageInfo"/>
        <owl:someValuesFrom rdf:resource="http://purl.org/net/def/metashare#LanguageDescriptionImageInfo"/>
      </owl:Restriction>
    </owl:equivalentClass>
    <owl:equivalentClass>
      <rdf:Description>
        <owl:onProperty rdf:resource="http://purl.org/net/def/metashare#languageDescriptionImageInfo"/>
        <owl:someValuesFrom rdf:resource="http://purl.org/net/def/metashare#LanguageDescriptionImageInfo"/>
      </rdf:Description>
    </owl:equivalentClass>
  </owl:Class>
  <owl:Class rdf:about="http://purl.org/net/def/metashare#LanguageDescriptionImageInfo">
    <rdfs:comment xml:lang="en">Groups together all information relevant to the image module of a language description (e.g. format, languages, size etc.), if there are any (e.g. for sign language grammars)</rdfs:comment>
  </owl:Class>
  <owl:Class rdf:about="http://purl.org/net/def/metashare#LanguageDescriptionInfo">
    <rdfs:comment xml:lang="en">Groups together information on language descriptions (grammars)</rdfs:comment>
  </owl:Class>
  <owl:Class rdf:about="http://purl.org/net/def/metashare#LanguageDescriptionMediaPart">
    <rdfs:subClassOf rdf:resource="http://purl.org/net/def/metashare#MediaPart"/>
  </owl:Class>
  <owl:Class rdf:about="http://purl.org/net/def/metashare#LanguageDescriptionText">
    <rdf:type rdf:resource="http://www.w3.org/2002/07/owl#Class"/>
    <rdfs:subClassOf rdf:resource="http://purl.org/net/def/metashare#LanguageDescriptionInfo"/>
    <rdfs:subClassOf rdf:resource="http://purl.org/net/def/metashare#LanguageDescriptionMediaPart"/>
    <rdfs:subclassOf rdf:resource="http://purl.org/net/def/metashare#LanguageDescriptionInfo"/>
    <owl:equivalentClass>
      <owl:Restriction>
        <owl:onProperty rdf:resource="http://purl.org/net/def/metashare#languageDescriptionTextInfo"/>
        <owl:someValuesFrom rdf:resource="http://purl.org/net/def/metashare#LanguageDescriptionTextInfo"/>
      </owl:Restriction>
    </owl:equivalentClass>
    <owl:equivalentClass>
      <rdf:Description>
        <owl:onProperty rdf:resource="http://purl.org/net/def/metashare#languageDescriptionTextInfo"/>
        <owl:someValuesFrom rdf:resource="http://purl.org/net/def/metashare#LanguageDescriptionTextInfo"/>
      </rdf:Description>
    </owl:equivalentClass>
  </owl:Class>
  <owl:Class rdf:about="http://purl.org/net/def/metashare#LanguageDescriptionTextInfo">
    <rdfs:comment xml:lang="en">Groups together all information relevant to the text module of a language description (e.g. format, languages, size etc.); it is obligatory for all language descriptions</rdfs:comment>
  </owl:Class>
  <owl:Class rdf:about="http://purl.org/net/def/metashare#LanguageDescriptionType">
    <rdfs:comment xml:lang="en">The type of the language description</rdfs:comment>
  </owl:Class>
  <owl:Class rdf:about="http://purl.org/net/def/metashare#LanguageDescriptionVideo">
    <rdf:type rdf:resource="http://www.w3.org/2002/07/owl#Class"/>
    <rdfs:subClassOf rdf:resource="http://purl.org/net/def/metashare#LanguageDescriptionInfo"/>
    <rdfs:subClassOf rdf:resource="http://purl.org/net/def/metashare#LanguageDescriptionMediaPart"/>
    <rdfs:subclassOf rdf:resource="http://purl.org/net/def/metashare#LanguageDescriptionInfo"/>
    <owl:equivalentClass>
      <owl:Restriction>
        <owl:onProperty rdf:resource="http://purl.org/net/def/metashare#languageDescriptionVideoInfo"/>
        <owl:someValuesFrom rdf:resource="http://purl.org/net/def/metashare#LanguageDescriptionVideoInfo"/>
      </owl:Restriction>
    </owl:equivalentClass>
    <owl:equivalentClass>
      <rdf:Description>
        <owl:onProperty rdf:resource="http://purl.org/net/def/metashare#languageDescriptionVideoInfo"/>
        <owl:someValuesFrom rdf:resource="http://purl.org/net/def/metashare#LanguageDescriptionVideoInfo"/>
      </rdf:Description>
    </owl:equivalentClass>
  </owl:Class>
  <owl:Class rdf:about="http://purl.org/net/def/metashare#LanguageDescriptionVideoInfo">
    <rdfs:comment xml:lang="en">Groups together all information relevant to the video parts of a language description (e.g. format, languages, size etc.), if there are any (e.g. for sign language grammars)</rdfs:comment>
  </owl:Class>
  <owl:Class rdf:about="http://purl.org/net/def/metashare#LanguageInfo">
    <rdfs:comment xml:lang="en">Groups information on the languages represented in the resource</rdfs:comment>
  </owl:Class>
  <owl:Class rdf:about="http://purl.org/net/def/metashare#LanguageResource">
    <dct:replaces rdf:resource="http://www.ilsp.gr/META-XMLSchema#resourceInfo"/>
    <owl:equivalentClass rdf:resource="http://www.w3.org/ns/dcat#Dataset"/>
  </owl:Class>
  <owl:Class rdf:about="http://purl.org/net/def/metashare#LanguageVarietyInfo">
    <rdfs:comment xml:lang="en">Groups information on language varieties occurred in the resource (e.g. dialects)</rdfs:comment>
  </owl:Class>
  <owl:Class rdf:about="http://purl.org/net/def/metashare#LanguageVarietyType">
    <rdfs:comment xml:lang="en">Specifies the type of the language variety that occurs in the resource or is supported by a tool/service</rdfs:comment>
  </owl:Class>
  <owl:Class rdf:about="http://purl.org/net/def/metashare#LexicalConceptualResource">
    <rdfs:subClassOf rdf:resource="http://purl.org/net/def/metashare#LanguageResource"/>
    <owl:equivalentClass>
      <owl:Restriction>
        <owl:onProperty rdf:resource="http://purl.org/net/def/metashare#lexicalConceptualResourceInfo"/>
        <owl:someValuesFrom rdf:resource="http://purl.org/net/def/metashare#LexicalConceptualResourceInfo"/>
      </owl:Restriction>
    </owl:equivalentClass>
  </owl:Class>
  <owl:Class rdf:about="http://purl.org/net/def/metashare#LexicalConceptualResourceAudio">
    <rdfs:subClassOf rdf:resource="http://purl.org/net/def/metashare#LexicalConceptualResourceInfo"/>
    <rdfs:subClassOf rdf:resource="http://purl.org/net/def/metashare#LexicalConceptualResourceMediaPart"/>
    <owl:equivalentClass>
      <rdf:Description>
        <owl:onProperty rdf:resource="http://purl.org/net/def/metashare#lexicalConceptualResourceAudioInfo"/>
        <owl:someValuesFrom rdf:resource="http://purl.org/net/def/metashare#LexicalConceptualResourceAudioInfo"/>
      </rdf:Description>
    </owl:equivalentClass>
  </owl:Class>
  <owl:Class rdf:about="http://purl.org/net/def/metashare#LexicalConceptualResourceAudioInfo">
    <rdfs:comment xml:lang="en">Groups information on the audio part of the lexical/conceptual resource</rdfs:comment>
  </owl:Class>
  <owl:Class rdf:about="http://purl.org/net/def/metashare#LexicalConceptualResourceImage">
    <rdfs:subClassOf rdf:resource="http://purl.org/net/def/metashare#LexicalConceptualResourceInfo"/>
    <rdfs:subClassOf rdf:resource="http://purl.org/net/def/metashare#LexicalConceptualResourceMediaPart"/>
    <owl:equivalentClass>
      <rdf:Description>
        <owl:onProperty rdf:resource="http://purl.org/net/def/metashare#lexicalConceptualResourceImageInfo"/>
        <owl:someValuesFrom rdf:resource="http://purl.org/net/def/metashare#LexicalConceptualResourceImageInfo"/>
      </rdf:Description>
    </owl:equivalentClass>
  </owl:Class>
  <owl:Class rdf:about="http://purl.org/net/def/metashare#LexicalConceptualResourceImageInfo">
    <rdfs:comment xml:lang="en">Groups information on the image part of the lexical/conceptual resource</rdfs:comment>
  </owl:Class>
  <owl:Class rdf:about="http://purl.org/net/def/metashare#LexicalConceptualResourceInfo">
    <rdfs:comment xml:lang="en">Groups together information specific to lexical/conceptual resources</rdfs:comment>
  </owl:Class>
  <owl:Class rdf:about="http://purl.org/net/def/metashare#LexicalConceptualResourceMediaPart">
    <rdfs:subClassOf rdf:resource="http://purl.org/net/def/metashare#MediaPart"/>
  </owl:Class>
  <owl:Class rdf:about="http://purl.org/net/def/metashare#LexicalConceptualResourceText">
    <rdfs:subClassOf rdf:resource="http://purl.org/net/def/metashare#LexicalConceptualResourceInfo"/>
    <rdfs:subClassOf rdf:resource="http://purl.org/net/def/metashare#LexicalConceptualResourceMediaPart"/>
    <owl:equivalentClass>
      <rdf:Description>
        <owl:onProperty rdf:resource="http://purl.org/net/def/metashare#lexicalConceptualResourceTextInfo"/>
        <owl:someValuesFrom rdf:resource="http://purl.org/net/def/metashare#LexicalConceptualResourceTextInfo"/>
      </rdf:Description>
    </owl:equivalentClass>
  </owl:Class>
  <owl:Class rdf:about="http://purl.org/net/def/metashare#LexicalConceptualResourceTextInfo">
    <rdfs:comment xml:lang="en">Groups information on the textual part of the lexical/conceptual resource</rdfs:comment>
  </owl:Class>
  <owl:Class rdf:about="http://purl.org/net/def/metashare#LexicalConceptualResourceType">
    <rdfs:comment xml:lang="en">Specifies the subtype of lexicalConceptualResource</rdfs:comment>
    <owl:equivalentClass rdf:resource="http://purl.org/net/def/metashare#CompatibleLexiconType"/>
  </owl:Class>
  <owl:Class rdf:about="http://purl.org/net/def/metashare#LexicalConceptualResourceVideo">
    <rdfs:subClassOf rdf:resource="http://purl.org/net/def/metashare#LexicalConceptualResourceInfo"/>
    <rdfs:subClassOf rdf:resource="http://purl.org/net/def/metashare#LexicalConceptualResourceMediaPart"/>
    <owl:equivalentClass>
      <rdf:Description>
        <owl:onProperty rdf:resource="http://purl.org/net/def/metashare#lexicalConceptualResourceVideoInfo"/>
        <owl:someValuesFrom rdf:resource="http://purl.org/net/def/metashare#LexicalConceptualResourceVideoInfo"/>
      </rdf:Description>
    </owl:equivalentClass>
  </owl:Class>
  <owl:Class rdf:about="http://purl.org/net/def/metashare#LexicalConceptualResourceVideoInfo">
    <rdfs:comment xml:lang="en">Groups information on the video part of the lexical conceptual resource</rdfs:comment>
  </owl:Class>
  <owl:Class rdf:about="http://purl.org/net/def/metashare#Lexicon">
    <rdfs:subClassOf rdf:resource="http://purl.org/net/def/metashare#LexicalConceptualResourceInfo"/>
    <owl:equivalentClass>
      <rdf:Description>
        <owl:hasValue rdf:resource="http://purl.org/net/def/metashare#lexicon"/>
        <owl:onProperty rdf:resource="http://purl.org/net/def/metashare#lexicalConcepturalResourceType"/>
      </rdf:Description>
    </owl:equivalentClass>
  </owl:Class>
  <owl:Class rdf:about="http://purl.org/net/def/metashare#LicenceInfo">
    <rdfs:comment xml:lang="en">Groups information on licences for the resource; can be repeated to allow for different modes of access and restrictions of use (e.g. free for academic use, on-a-fee basis for commercial use, download of a sample for free use etc.)</rdfs:comment>
  </owl:Class>
  <owl:Class rdf:about="http://purl.org/net/def/metashare#LicenseCategory">
    <rdfs:comment xml:lang="en">A way of classifying licences according to their conditions of use (CLARIN recommendation)</rdfs:comment>
    <rdfs:label xml:lang="en">License Category</rdfs:label>
  </owl:Class>
  <rdf:Description rdf:about="http://purl.org/net/def/metashare#LicenseInfo">
    <rdfs:comment xml:lang="en">Links a resource to the licence under which it is distributed; values are taken from a list of standard licences</rdfs:comment>
  </rdf:Description>
  <owl:Class rdf:about="http://purl.org/net/def/metashare#LingualityType">
    <rdfs:comment xml:lang="en">Indicates whether the resource includes one, two or more languages</rdfs:comment>
  </owl:Class>
  <owl:Class rdf:about="http://purl.org/net/def/metashare#LinguisticInformation">
    <rdfs:comment xml:lang="en">A more detailed account of the linguistic information contained in the lexicalConceptualResource</rdfs:comment>
  </owl:Class>
  <owl:Class rdf:about="http://purl.org/net/def/metashare#LinkToOtherMediaInfo">
    <rdfs:comment xml:lang="en">Groups information on the way different media of the resource interact with or link to each other. To be used for multimodal resources or for resources representing sensorimotor data</rdfs:comment>
  </owl:Class>
  <ns:ConformanceToStandardsBestPractices rdf:about="http://purl.org/net/def/metashare#MAF"/>
  <ns:ConformanceToStandardsBestPractices rdf:about="http://purl.org/net/def/metashare#MLIF"/>
  <ns:CharacterEncoding rdf:about="http://purl.org/net/def/metashare#MS874"/>
  <ns:ConformanceToStandardsBestPractices rdf:about="http://purl.org/net/def/metashare#MULTEXT"/>
  <ns:ConformanceToStandardsBestPractices rdf:about="http://purl.org/net/def/metashare#MUMIN"/>
  <ns:CharacterEncoding rdf:about="http://purl.org/net/def/metashare#MacArabic"/>
  <ns:CharacterEncoding rdf:about="http://purl.org/net/def/metashare#MacCentralEurope"/>
  <ns:CharacterEncoding rdf:about="http://purl.org/net/def/metashare#MacCroatian"/>
  <ns:CharacterEncoding rdf:about="http://purl.org/net/def/metashare#MacCyrillic"/>
  <ns:CharacterEncoding rdf:about="http://purl.org/net/def/metashare#MacDingbat"/>
  <ns:CharacterEncoding rdf:about="http://purl.org/net/def/metashare#MacGreek"/>
  <ns:CharacterEncoding rdf:about="http://purl.org/net/def/metashare#MacHebrew"/>
  <ns:CharacterEncoding rdf:about="http://purl.org/net/def/metashare#MacIceland"/>
  <ns:CharacterEncoding rdf:about="http://purl.org/net/def/metashare#MacRoman"/>
  <ns:CharacterEncoding rdf:about="http://purl.org/net/def/metashare#MacRomania"/>
  <ns:CharacterEncoding rdf:about="http://purl.org/net/def/metashare#MacSymbol"/>
  <ns:CharacterEncoding rdf:about="http://purl.org/net/def/metashare#MacThai"/>
  <ns:CharacterEncoding rdf:about="http://purl.org/net/def/metashare#MacTurkish"/>
  <ns:CharacterEncoding rdf:about="http://purl.org/net/def/metashare#MacUkraine"/>
  <owl:Class rdf:about="http://purl.org/net/def/metashare#MachineReadableDictionary">
    <rdfs:subClassOf rdf:resource="http://purl.org/net/def/metashare#LexicalConceptualResourceInfo"/>
    <owl:equivalentClass>
      <rdf:Description>
        <owl:hasValue rdf:resource="http://purl.org/net/def/metashare#machineReadableDictionary"/>
        <owl:onProperty rdf:resource="http://purl.org/net/def/metashare#lexicalConcepturalResourceType"/>
      </rdf:Description>
    </owl:equivalentClass>
  </owl:Class>
  <ns:ConformanceToClassificationScheme rdf:about="http://purl.org/net/def/metashare#MeSH_classification"/>
  <owl:Class rdf:about="http://purl.org/net/def/metashare#MediaPart"/>
  <owl:Class rdf:about="http://purl.org/net/def/metashare#MediaType">
    <rdfs:comment xml:lang="en">Specifies the media type of the resource and basically corresponds to the physical medium of the content representation. Each media type is described through a 				distinctive set of features. A resource may consist of parts attributed to different types of media.</rdfs:comment>
  </owl:Class>
  <owl:Class rdf:about="http://purl.org/net/def/metashare#MembershipInfo">
    <rdfs:comment xml:lang="en">The conditions imposed by the user being member of some association/institution (e.g., ELRA, LDC) distributing the resource. This indicates the availability conditions (and prices) for users who are members or not</rdfs:comment>
  </owl:Class>
  <owl:Class rdf:about="http://purl.org/net/def/metashare#MembershipInstitution">
    <rdfs:comment xml:lang="en">This lists the different institutions releasing the resources and establishing membership conditions</rdfs:comment>
  </owl:Class>
  <owl:Class rdf:about="http://purl.org/net/def/metashare#MetadataInfo">
    <rdfs:comment xml:lang="en">Groups information on the metadata record itself</rdfs:comment>
    <owl:equivalentClass rdf:resource="http://www.w3.org/ns/dcat#CatalogRecord"/>
  </owl:Class>
  <rdf:Description rdf:about="http://purl.org/net/def/metashare#ModalityAnnotation">
    <rdfs:subClassOf rdf:resource="http://purl.org/net/def/metashare#AnnotationType"/>
  </rdf:Description>
  <owl:Class rdf:about="http://purl.org/net/def/metashare#ModalityInfo">
    <rdfs:comment xml:lang="en">Groups information on the modalities represented in the resource</rdfs:comment>
  </owl:Class>
  <owl:Class rdf:about="http://purl.org/net/def/metashare#ModalityType">
    <rdfs:comment xml:lang="en">Specifies the type of the modality represented in the resource or processed by a tool/service</rdfs:comment>
  </owl:Class>
  <rdf:Description rdf:about="http://purl.org/net/def/metashare#MorphosyntacticAnnotation">
    <rdfs:subClassOf rdf:resource="http://purl.org/net/def/metashare#AnnotationType"/>
  </rdf:Description>
  <owl:Class rdf:about="http://purl.org/net/def/metashare#MultilingualityType">
    <rdfs:comment xml:lang="en">Indicates whether the corpus is parallel, comparable or mixed</rdfs:comment>
  </owl:Class>
  <ns:ConformanceToClassificationScheme rdf:about="http://purl.org/net/def/metashare#NLK_classification"/>
  <owl:Class rdf:about="http://purl.org/net/def/metashare#Naturality">
    <rdfs:comment xml:lang="en">Specifies the level of naturality for multimodal/multimedia resources</rdfs:comment>
  </owl:Class>
  <owl:Class rdf:about="http://purl.org/net/def/metashare#NgramInfo">
    <rdfs:comment xml:lang="en">Groups information specific to n-gram resources (e.g. range of n-grams, base item etc.)</rdfs:comment>
  </owl:Class>
  <owl:Class rdf:about="http://purl.org/net/def/metashare#NoiseLevel">
    <rdfs:comment xml:lang="en">Specifies the  level of background noise</rdfs:comment>
  </owl:Class>
  <owl:Class rdf:about="http://purl.org/net/def/metashare#NonSpeechItems">
    <rdfs:comment xml:lang="en">Specifies the distinct elements that maybe included in the audio corpus</rdfs:comment>
  </owl:Class>
  <ns:ConformanceToStandardsBestPractices rdf:about="http://purl.org/net/def/metashare#OAXAL"/>
  <ns:ConformanceToStandardsBestPractices rdf:about="http://purl.org/net/def/metashare#OWL"/>
  <owl:Class rdf:about="http://purl.org/net/def/metashare#Ontology">
    <rdfs:subClassOf rdf:resource="http://purl.org/net/def/metashare#LexicalConceptualResourceInfo"/>
    <owl:equivalentClass>
      <rdf:Description>
        <owl:hasValue rdf:resource="http://purl.org/net/def/metashare#ontology"/>
        <owl:onProperty rdf:resource="http://purl.org/net/def/metashare#lexicalConcepturalResourceType"/>
      </rdf:Description>
    </owl:equivalentClass>
  </owl:Class>
  <owl:Class rdf:about="http://purl.org/net/def/metashare#OperatingSystem">
    <rdfs:comment xml:lang="en">The operating system on which the tool will be running</rdfs:comment>
  </owl:Class>
  <owl:Class rdf:about="http://purl.org/net/def/metashare#Organization">
    <owl:equivalentClass rdf:resource="http://xmlns.com/foaf/0.1/Organization"/>
  </owl:Class>
  <owl:Class rdf:about="http://purl.org/net/def/metashare#Origin">
    <rdfs:comment xml:lang="en">The language origin of the participant</rdfs:comment>
  </owl:Class>
  <owl:Class rdf:about="http://purl.org/net/def/metashare#OriginOfPersons">
    <rdfs:comment xml:lang="en">The language origin of the group of participants</rdfs:comment>
  </owl:Class>
  <owl:Class rdf:about="http://purl.org/net/def/metashare#OtherMedia">
    <rdfs:comment xml:lang="en">Specifies the media types that are linked to the media type described within the same resource</rdfs:comment>
  </owl:Class>
  <owl:Class rdf:about="http://purl.org/net/def/metashare#OutputInfo">
    <rdfs:comment xml:lang="en">Groups together information on the requirements set on the output of a tool or service</rdfs:comment>
  </owl:Class>
  <ns:ConformanceToClassificationScheme rdf:about="http://purl.org/net/def/metashare#PAROLE_genreClassification"/>
  <ns:ConformanceToClassificationScheme rdf:about="http://purl.org/net/def/metashare#PAROLE_topicClassification"/>
  <owl:Class rdf:about="http://purl.org/net/def/metashare#ParticipantInfo">
    <rdfs:comment xml:lang="en">Groups information on the individual person(s) participating in the audio, video, sensorimotor (textNumerical) part of the resource</rdfs:comment>
  </owl:Class>
  <owl:Class rdf:about="http://purl.org/net/def/metashare#Person">
    <owl:equivalentClass rdf:resource="http://xmlns.com/foaf/0.1/Actor"/>
  </owl:Class>
  <owl:Class rdf:about="http://purl.org/net/def/metashare#Project">
    <owl:equivalentClass rdf:resource="http://xmlns.com/foaf/0.1/Project"/>
  </owl:Class>
  <owl:Class rdf:about="http://purl.org/net/def/metashare#Quality">
    <rdfs:comment xml:lang="en">Specifies the quality level of image resource</rdfs:comment>
  </owl:Class>
  <ns:ConformanceToStandardsBestPractices rdf:about="http://purl.org/net/def/metashare#RDF"/>
  <ns:ColourSpace rdf:about="http://purl.org/net/def/metashare#RGB"/>
  <owl:Class rdf:about="http://purl.org/net/def/metashare#RasterOrVectorGraphics">
    <rdfs:comment xml:lang="en">Indicates if the image is stored as raster or vector graphics</rdfs:comment>
  </owl:Class>
  <owl:Class rdf:about="http://purl.org/net/def/metashare#RecordingDeviceType">
    <rdfs:comment xml:lang="en">The nature of the recording platform hardware and the storage medium</rdfs:comment>
  </owl:Class>
  <owl:Class rdf:about="http://purl.org/net/def/metashare#RecordingEnvironment">
    <rdfs:comment xml:lang="en">Where the recording took place</rdfs:comment>
  </owl:Class>
  <owl:Class rdf:about="http://purl.org/net/def/metashare#RecordingQuality">
    <rdfs:comment xml:lang="en">Indication of the audio or video recording quality</rdfs:comment>
  </owl:Class>
  <owl:Class rdf:about="http://purl.org/net/def/metashare#RelatedLexiconType">
    <rdfs:comment xml:lang="en">Indicates the position of the lexica that must or can be used with the grammar</rdfs:comment>
  </owl:Class>
  <owl:Class rdf:about="http://purl.org/net/def/metashare#RelationInfo"/>
  <owl:Class rdf:about="http://purl.org/net/def/metashare#RequiredHardware">
    <rdfs:comment xml:lang="en">Hardware required for running a tool and/or computational grammar</rdfs:comment>
  </owl:Class>
  <owl:Class rdf:about="http://purl.org/net/def/metashare#ResolutionInfo">
    <rdfs:comment xml:lang="en">Groups together information on the image resolution</rdfs:comment>
  </owl:Class>
  <owl:Class rdf:about="http://purl.org/net/def/metashare#ResolutionStandard">
    <rdfs:comment xml:lang="en">The standard to which  the resolution conforms</rdfs:comment>
  </owl:Class>
  <owl:Class rdf:about="http://purl.org/net/def/metashare#ResourceType">
    <rdfs:comment xml:lang="en">Specifies the type of the resource being described</rdfs:comment>
  </owl:Class>
  <ns:SourceChannelType rdf:about="http://purl.org/net/def/metashare#S"/>
  <ns:ConformanceToStandardsBestPractices rdf:about="http://purl.org/net/def/metashare#SKOS"/>
  <ns:AudioQualityMeasuresIncluded rdf:about="http://purl.org/net/def/metashare#SNR"/>
  <ns:ConformanceToStandardsBestPractices rdf:about="http://purl.org/net/def/metashare#SRX"/>
  <owl:Class rdf:about="http://purl.org/net/def/metashare#ScenarioType">
    <rdfs:comment xml:lang="en">Indicates the task defined for the conversation or the interaction of participants</rdfs:comment>
  </owl:Class>
  <owl:Class rdf:about="http://purl.org/net/def/metashare#SceneIllumination">
    <rdfs:comment xml:lang="en">Information on the illumination of the scene</rdfs:comment>
  </owl:Class>
  <owl:Class rdf:about="http://purl.org/net/def/metashare#SegmentationLevel">
    <rdfs:comment xml:lang="en">Specifies the segmentation unit in terms of which the resource has been segmented or the level of segmentation a tool/service requires/outputs</rdfs:comment>
  </owl:Class>
  <ns:ConformanceToStandardsBestPractices rdf:about="http://purl.org/net/def/metashare#SemAF"/>
  <ns:ConformanceToStandardsBestPractices rdf:about="http://purl.org/net/def/metashare#SemAF_DA"/>
  <ns:ConformanceToStandardsBestPractices rdf:about="http://purl.org/net/def/metashare#SemAF_DS"/>
  <ns:ConformanceToStandardsBestPractices rdf:about="http://purl.org/net/def/metashare#SemAF_NE"/>
  <ns:ConformanceToStandardsBestPractices rdf:about="http://purl.org/net/def/metashare#SemAF_SRL"/>
  <rdf:Description rdf:about="http://purl.org/net/def/metashare#SemanticAnnotation">
    <rdfs:subClassOf rdf:resource="http://purl.org/net/def/metashare#AnnotationType"/>
  </rdf:Description>
  <owl:Class rdf:about="http://purl.org/net/def/metashare#SexOfPersons">
    <rdfs:comment xml:lang="en">The gender of the group of participants</rdfs:comment>
  </owl:Class>
  <ns:CharacterEncoding rdf:about="http://purl.org/net/def/metashare#Shift_JIS"/>
  <owl:Class rdf:about="http://purl.org/net/def/metashare#SignConvention">
    <rdfs:comment xml:lang="en">Binary representation of numbers</rdfs:comment>
  </owl:Class>
  <owl:Class rdf:about="http://purl.org/net/def/metashare#SignalEncoding">
    <rdfs:comment xml:lang="en">Specifies the  encoding the audio type uses</rdfs:comment>
  </owl:Class>
  <owl:Class rdf:about="http://purl.org/net/def/metashare#Size">
    <rdfs:comment xml:lang="en">Specifies the size of the resource with regard to the SizeUnit measurement in form of a number</rdfs:comment>
  </owl:Class>
  <owl:Class rdf:about="http://purl.org/net/def/metashare#SizeUnit">
    <rdfs:comment xml:lang="en">Specifies the unit that is used when providing information on the size of the resource or of resource parts</rdfs:comment>
  </owl:Class>
  <owl:Class rdf:about="http://purl.org/net/def/metashare#SourceChannel">
    <rdfs:comment xml:lang="en">Information on the source channel</rdfs:comment>
  </owl:Class>
  <owl:Class rdf:about="http://purl.org/net/def/metashare#SourceChannelType">
    <rdfs:comment xml:lang="en">Type of the source channel</rdfs:comment>
  </owl:Class>
  <owl:Class rdf:about="http://purl.org/net/def/metashare#SpeakingImpairmentOfPersons">
    <rdfs:comment xml:lang="en">Whether the group of participants contains persons withwith speakingimpairments</rdfs:comment>
  </owl:Class>
  <rdf:Description rdf:about="http://purl.org/net/def/metashare#SpeechAnnotation">
    <rdfs:subClassOf rdf:resource="http://purl.org/net/def/metashare#AnnotationType"/>
  </rdf:Description>
  <owl:Class rdf:about="http://purl.org/net/def/metashare#SpeechInfluences">
    <rdfs:comment xml:lang="en">Specifies the factors influencing speech</rdfs:comment>
  </owl:Class>
  <owl:Class rdf:about="http://purl.org/net/def/metashare#SpeechItems">
    <rdfs:comment xml:lang="en">Specifies the distinct elements that are pronounced and annotated as such</rdfs:comment>
  </owl:Class>
  <owl:Class rdf:about="http://purl.org/net/def/metashare#StaticElementInfo">
    <rdfs:comment xml:lang="en">Groups information on the static element visible on the images</rdfs:comment>
  </owl:Class>
  <ns:ConformanceToStandardsBestPractices rdf:about="http://purl.org/net/def/metashare#SynAF"/>
  <rdf:Description rdf:about="http://purl.org/net/def/metashare#SyntacticAnnotation">
    <rdfs:subClassOf rdf:resource="http://purl.org/net/def/metashare#AnnotationType"/>
  </rdf:Description>
  <ns:SourceChannelType rdf:about="http://purl.org/net/def/metashare#T"/>
  <ns:SizeUnit rdf:about="http://purl.org/net/def/metashare#T-HPairs"/>
  <ns:ConformanceToStandardsBestPractices rdf:about="http://purl.org/net/def/metashare#TBX"/>
  <ns:ConformanceToStandardsBestPractices rdf:about="http://purl.org/net/def/metashare#TEI"/>
  <ns:ConformanceToStandardsBestPractices rdf:about="http://purl.org/net/def/metashare#TEI_P3"/>
  <ns:ConformanceToStandardsBestPractices rdf:about="http://purl.org/net/def/metashare#TEI_P4"/>
  <ns:ConformanceToStandardsBestPractices rdf:about="http://purl.org/net/def/metashare#TEI_P5"/>
  <ns:CharacterEncoding rdf:about="http://purl.org/net/def/metashare#TIS-620"/>
  <ns:ConformanceToStandardsBestPractices rdf:about="http://purl.org/net/def/metashare#TMX"/>
  <ns:MembershipInstitution rdf:about="http://purl.org/net/def/metashare#TST-CENTRALE"/>
  <owl:Class rdf:about="http://purl.org/net/def/metashare#Task">
    <rdfs:comment xml:lang="en">An indication of the task performed by the grammar</rdfs:comment>
  </owl:Class>
  <owl:Class rdf:about="http://purl.org/net/def/metashare#TerminologicalResource">
    <rdfs:subClassOf rdf:resource="http://purl.org/net/def/metashare#LexicalConceptualResourceInfo"/>
    <owl:equivalentClass>
      <rdf:Description>
        <owl:hasValue rdf:resource="http://purl.org/net/def/metashare#terminologicalResource"/>
        <owl:onProperty rdf:resource="http://purl.org/net/def/metashare#lexicalConcepturalResourceType"/>
      </rdf:Description>
    </owl:equivalentClass>
  </owl:Class>
  <owl:Class rdf:about="http://purl.org/net/def/metashare#TextClassificationInfo">
    <rdfs:comment xml:lang="en">Groups together information on text type/genre of the resource</rdfs:comment>
    <rdfs:subClassOf rdf:resource="http://purl.org/net/def/metashare#ClassificationInfo"/>
  </owl:Class>
  <owl:Class rdf:about="http://purl.org/net/def/metashare#TextFormatInfo">
    <rdfs:comment xml:lang="en">Groups information on the text format(s) of a resource</rdfs:comment>
  </owl:Class>
  <owl:Class rdf:about="http://purl.org/net/def/metashare#TextIncludedInImage">
    <rdfs:comment xml:lang="en">Provides information on the type of text that may be on the image</rdfs:comment>
  </owl:Class>
  <owl:Class rdf:about="http://purl.org/net/def/metashare#TextIncludedInVideo">
    <rdfs:comment xml:lang="en">Indicates if text is present in or in conjunction with the video</rdfs:comment>
  </owl:Class>
  <owl:Class rdf:about="http://purl.org/net/def/metashare#TextNumericalFormatInfo">
    <rdfs:comment xml:lang="en">Groups information on the format(s) of the textNumerical part of the resource</rdfs:comment>
  </owl:Class>
  <owl:Class rdf:about="http://purl.org/net/def/metashare#Thesaurus">
    <rdfs:subClassOf rdf:resource="http://purl.org/net/def/metashare#LexicalConceptualResourceInfo"/>
    <owl:equivalentClass>
      <rdf:Description>
        <owl:hasValue rdf:resource="http://purl.org/net/def/metashare#thesaurus"/>
        <owl:onProperty rdf:resource="http://purl.org/net/def/metashare#lexicalConcepturalResourceType"/>
      </rdf:Description>
    </owl:equivalentClass>
  </owl:Class>
  <rdf:Description rdf:about="http://purl.org/net/def/metashare#TimeCoverageClassification">
    <dct:replaces rdf:resource="http://www.ilsp.gr/META-XMLSchema#timeCoverageInfo"/>
  </rdf:Description>
  <owl:Class rdf:about="http://purl.org/net/def/metashare#TimeCoverageInfo">
    <rdfs:comment xml:lang="en">Groups together information on time classification of the resource</rdfs:comment>
  </owl:Class>
  <ns:ConformanceToStandardsBestPractices rdf:about="http://purl.org/net/def/metashare#TimeML"/>
  <owl:Class rdf:about="http://purl.org/net/def/metashare#ToolDocumentationType">
    <rdfs:comment xml:lang="en">Specifies the type of documentation for tool or service</rdfs:comment>
  </owl:Class>
  <owl:Class rdf:about="http://purl.org/net/def/metashare#ToolService">
    <rdfs:subClassOf rdf:resource="http://purl.org/net/def/metashare#LanguageResource"/>
    <owl:equivalentClass>
      <owl:Restriction>
        <owl:onProperty rdf:resource="http://purl.org/net/def/metashare#toolServiceInfo"/>
        <owl:someValuesFrom rdf:resource="http://purl.org/net/def/metashare#ToolServiceInfo"/>
      </owl:Restriction>
    </owl:equivalentClass>
  </owl:Class>
  <owl:Class rdf:about="http://purl.org/net/def/metashare#ToolServiceInfo">
    <rdfs:comment xml:lang="en">Groups together elements required for the description of tools and services</rdfs:comment>
  </owl:Class>
  <owl:Class rdf:about="http://purl.org/net/def/metashare#ToolServiceType">
    <rdfs:comment xml:lang="en">Specifies the type of the tool or service</rdfs:comment>
  </owl:Class>
  <ns:ConformanceToClassificationScheme rdf:about="http://purl.org/net/def/metashare#UDC_classification"/>
  <ns:CharacterEncoding rdf:about="http://purl.org/net/def/metashare#US-ASCII"/>
  <ns:CharacterEncoding rdf:about="http://purl.org/net/def/metashare#UTF-16"/>
  <ns:CharacterEncoding rdf:about="http://purl.org/net/def/metashare#UTF-16BE"/>
  <ns:CharacterEncoding rdf:about="http://purl.org/net/def/metashare#UTF-16LE"/>
  <ns:CharacterEncoding rdf:about="http://purl.org/net/def/metashare#UTF-8"/>
  <owl:Class rdf:about="http://purl.org/net/def/metashare#Use">
    <dct:replaces rdf:resource="http://www.ilsp.gr/META-XMLSchema#actualUse"/>
    <dct:replaces rdf:resource="http://www.ilsp.gr/META-XMLSchema#foreseenUse"/>
  </owl:Class>
  <owl:Class rdf:about="http://purl.org/net/def/metashare#UseNLPSpecific">
    <rdfs:comment xml:lang="en">Specifies the NLP application for which the resource iscreated or the application in which it has actually been used.</rdfs:comment>
  </owl:Class>
  <owl:Class rdf:about="http://purl.org/net/def/metashare#UserNature">
    <rdfs:comment xml:lang="en">Identifies the type of user of the resource (e.g. affiliated with a commercial vs. academic institution, member of an organisation/network etc.); the user type may have implications on the licensing or pricing of a resource</rdfs:comment>
    <rdfs:comment xml:lang="en">The conditions imposed by the nature of the user (for instance, a research use may have different implications depending on this)</rdfs:comment>
  </owl:Class>
  <ns:ResolutionStandard rdf:about="http://purl.org/net/def/metashare#VGA"/>
  <ns:SourceChannelType rdf:about="http://purl.org/net/def/metashare#VOIP"/>
  <owl:Class rdf:about="http://purl.org/net/def/metashare#ValidationExtent">
    <rdfs:comment xml:lang="en">The resource coverage in terms of validated data</rdfs:comment>
  </owl:Class>
  <owl:Class rdf:about="http://purl.org/net/def/metashare#ValidationInfo">
    <rdfs:comment xml:lang="en">Groups information on validation of a resource; it can be repeated to allow for different validations (e.g. formal validation of the whole resource; content validation of one part of the resource etc.). </rdfs:comment>
  </owl:Class>
  <owl:Class rdf:about="http://purl.org/net/def/metashare#ValidationMode">
    <rdfs:comment xml:lang="en">Specifies the validation methodology applied</rdfs:comment>
  </owl:Class>
  <owl:Class rdf:about="http://purl.org/net/def/metashare#ValidationType">
    <rdfs:comment xml:lang="en">Specifies the type of the validation that have been performed </rdfs:comment>
  </owl:Class>
  <owl:Class rdf:about="http://purl.org/net/def/metashare#VideoClassificationInfo">
    <rdfs:comment xml:lang="en">Groups together information on video genre of the resource</rdfs:comment>
    <rdfs:subClassOf rdf:resource="http://purl.org/net/def/metashare#ClassificationInfo"/>
  </owl:Class>
  <owl:Class rdf:about="http://purl.org/net/def/metashare#VideoFormatInfo">
    <rdfs:comment xml:lang="en">Groups information on the format(s) of a resource; repeated if parts of the resource are in different formats</rdfs:comment>
  </owl:Class>
  <owl:Class rdf:about="http://purl.org/net/def/metashare#VisualModelling">
    <rdfs:comment xml:lang="en">The dimensional form applied on video or image corpus</rdfs:comment>
  </owl:Class>
  <owl:Class rdf:about="http://purl.org/net/def/metashare#WordList">
    <rdfs:subClassOf rdf:resource="http://purl.org/net/def/metashare#LexicalConceptualResourceInfo"/>
    <owl:equivalentClass>
      <rdf:Description>
        <owl:hasValue rdf:resource="http://purl.org/net/def/metashare#wordList"/>
        <owl:onProperty rdf:resource="http://purl.org/net/def/metashare#lexicalConceptualResourceType"/>
      </rdf:Description>
    </owl:equivalentClass>
  </owl:Class>
  <owl:Class rdf:about="http://purl.org/net/def/metashare#WordNet">
    <rdf:type rdf:resource="http://purl.org/net/def/metashare#ConformanceToStandardsBestPractices"/>
    <rdfs:subClassOf rdf:resource="http://purl.org/net/def/metashare#LexicalConceptualResourceInfo"/>
    <owl:equivalentClass>
      <rdf:Description>
        <owl:hasValue rdf:resource="http://purl.org/net/def/metashare#wordNet"/>
        <owl:onProperty rdf:resource="http://purl.org/net/def/metashare#lexicalConcepturalResourceType"/>
      </rdf:Description>
    </owl:equivalentClass>
  </owl:Class>
  <ns:ConformanceToStandardsBestPractices rdf:about="http://purl.org/net/def/metashare#XCES"/>
  <ns:ConformanceToStandardsBestPractices rdf:about="http://purl.org/net/def/metashare#XLIFF"/>
  <ns:ColourSpace rdf:about="http://purl.org/net/def/metashare#YUV"/>
  <ns:SignalEncoding rdf:about="http://purl.org/net/def/metashare#aLaw"/>
  <ns:CompressionName rdf:about="http://purl.org/net/def/metashare#aac"/>
  <ns:UserNature rdf:about="http://purl.org/net/def/metashare#academic"/>
  <odrl:Set rdf:about="http://purl.org/net/def/metashare#academic-nonCommercialUse">
    <rdf:type rdf:resource="http://purl.org/net/def/metashare#ConditionsOfUse"/>
    <odrl:permission>
      <rdf:Description>
        <odrl:constraint>
          <rdf:Description>
            <odrl:operator rdf:resource="http://www.w3.org/ns/odrl/2/eq"/>
            <odrl:purpose rdf:resource="http://purl.org/net/def/metashare#academic"/>
          </rdf:Description>
        </odrl:constraint>
      </rdf:Description>
    </odrl:permission>
    <odrl:prohibition>
      <rdf:Description>
        <odrl:action rdf:resource="http://creativecommons.org/ns#CommericalUse"/>
        <odrl:action rdf:resource="http://creativecommons.org/ns#Distribution"/>
      </rdf:Description>
    </odrl:prohibition>
  </odrl:Set>
  <ns:LinguisticInformation rdf:about="http://purl.org/net/def/metashare#accentuation"/>
  <owl:DatatypeProperty rdf:about="http://purl.org/net/def/metashare#accessTool">
    <rdfs:comment xml:lang="en">The name or the identifier or the url of the tool used to access a resource (e.g. a corpus workbench)</rdfs:comment>
    <rdfs:domain rdf:resource="http://purl.org/net/def/metashare#LanguageResource"/>
    <rdfs:range rdf:resource="http://www.w3.org/2001/XMLSchema#string"/>
  </owl:DatatypeProperty>
  <ns:DistributionAccessMedium rdf:about="http://purl.org/net/def/metashare#accessibleThroughInterface"/>
  <owl:DatatypeProperty rdf:about="http://purl.org/net/def/metashare#actualUseDetails">
    <rdfs:comment xml:lang="en">Reports on the usage of the resource in free text</rdfs:comment>
    <rdfs:domain rdf:resource="http://purl.org/net/def/metashare#ActualUseInfo"/>
    <rdfs:range rdf:resource="http://www.w3.org/2001/XMLSchema#string"/>
  </owl:DatatypeProperty>
  <owl:ObjectProperty rdf:about="http://purl.org/net/def/metashare#actualUseInfo">
    <rdfs:comment xml:lang="en">Groups information on how the resource has already been used</rdfs:comment>
    <rdfs:domain rdf:resource="http://purl.org/net/def/metashare#LanguageResource"/>
    <rdfs:range rdf:resource="http://purl.org/net/def/metashare#ActualUseInfo"/>
  </owl:ObjectProperty>
  <owl:DatatypeProperty rdf:about="http://purl.org/net/def/metashare#address">
    <rdfs:comment xml:lang="en">The street and the number of the postal address of a person or organization</rdfs:comment>
    <rdfs:domain>
      <owl:Class>
        <owl:unionOf>
          <rdf:Description>
            <rdf:first rdf:resource="http://purl.org/net/def/metashare#Person"/>
            <rdf:rest>
              <rdf:Description>
                <rdf:first rdf:resource="http://purl.org/net/def/metashare#Organization"/>
                <rdf:rest rdf:resource="http://www.w3.org/1999/02/22-rdf-syntax-ns#nil"/>
              </rdf:Description>
            </rdf:rest>
          </rdf:Description>
        </owl:unionOf>
      </owl:Class>
    </rdfs:domain>
    <rdfs:range rdf:resource="http://www.w3.org/2001/XMLSchema#string"/>
  </owl:DatatypeProperty>
  <ns:AgeGroup rdf:about="http://purl.org/net/def/metashare#adult">
    <rdf:type rdf:resource="http://purl.org/net/def/metashare#AgeOfPersons"/>
  </ns:AgeGroup>
  <owl:ObjectProperty rdf:about="http://purl.org/net/def/metashare#affiliation">
    <rdfs:comment xml:lang="en">Groups information on organization to whomtheperson is affiliated</rdfs:comment>
    <rdfs:domain rdf:resource="http://purl.org/net/def/metashare#Person"/>
    <rdfs:range rdf:resource="http://purl.org/net/def/metashare#Organization"/>
  </owl:ObjectProperty>
  <owl:ObjectProperty rdf:about="http://purl.org/net/def/metashare#ageGroup">
    <rdfs:comment xml:lang="en">The age group to which the participant belongs</rdfs:comment>
    <rdfs:domain rdf:resource="http://purl.org/net/def/metashare#ParticipantInfo"/>
    <rdfs:range rdf:resource="http://purl.org/net/def/metashare#AgeGroup"/>
  </owl:ObjectProperty>
  <owl:ObjectProperty rdf:about="http://purl.org/net/def/metashare#ageOfPersons">
    <rdfs:comment xml:lang="en">The age range of the group of participants; repeat the element if needed</rdfs:comment>
    <rdfs:domain>
      <owl:Class>
        <owl:unionOf>
          <rdf:Description>
            <rdf:first rdf:resource="http://purl.org/net/def/metashare#CorpusAudioInfo"/>
            <rdf:rest>
              <rdf:Description>
                <rdf:first rdf:resource="http://purl.org/net/def/metashare#CorpusTextNumericalInfo"/>
                <rdf:rest>
                  <rdf:Description>
                    <rdf:first rdf:resource="http://purl.org/net/def/metashare#CorpusVideoInfo"/>
                    <rdf:rest>
                      <rdf:Description>
                        <rdf:first rdf:resource="http://purl.org/net/def/metashare#CorpusImageInfo"/>
                        <rdf:rest rdf:resource="http://www.w3.org/1999/02/22-rdf-syntax-ns#nil"/>
                      </rdf:Description>
                    </rdf:rest>
                  </rdf:Description>
                </rdf:rest>
              </rdf:Description>
            </rdf:rest>
          </rdf:Description>
        </owl:unionOf>
      </owl:Class>
    </rdfs:domain>
    <rdfs:range>
      <owl:Class>
        <owl:unionOf>
          <rdf:Description>
            <rdf:first rdf:resource="http://purl.org/net/def/metashare#AgeOfPersons"/>
            <rdf:rest>
              <rdf:Description>
                <rdf:first rdf:resource="http://purl.org/net/def/metashare#AgeOfPersons"/>
                <rdf:rest>
                  <rdf:Description>
                    <rdf:first rdf:resource="http://purl.org/net/def/metashare#AgeOfPersons"/>
                    <rdf:rest>
                      <rdf:Description>
                        <rdf:first rdf:resource="http://purl.org/net/def/metashare#AgeOfPersons"/>
                        <rdf:rest rdf:resource="http://www.w3.org/1999/02/22-rdf-syntax-ns#nil"/>
                      </rdf:Description>
                    </rdf:rest>
                  </rdf:Description>
                </rdf:rest>
              </rdf:Description>
            </rdf:rest>
          </rdf:Description>
        </owl:unionOf>
      </owl:Class>
    </rdfs:range>
  </owl:ObjectProperty>
  <owl:DatatypeProperty rdf:about="http://purl.org/net/def/metashare#ageRangeEnd">
    <rdfs:comment xml:lang="en">End of age range of the group of participants</rdfs:comment>
    <rdfs:domain>
      <owl:Class>
        <owl:unionOf>
          <rdf:Description>
            <rdf:first rdf:resource="http://purl.org/net/def/metashare#CorpusTextNumericalInfo"/>
            <rdf:rest>
              <rdf:Description>
                <rdf:first rdf:resource="http://purl.org/net/def/metashare#CorpusVideoInfo"/>
                <rdf:rest>
                  <rdf:Description>
                    <rdf:first rdf:resource="http://purl.org/net/def/metashare#CorpusAudioInfo"/>
                    <rdf:rest>
                      <rdf:Description>
                        <rdf:first rdf:resource="http://purl.org/net/def/metashare#CorpusImageInfo"/>
                        <rdf:rest rdf:resource="http://www.w3.org/1999/02/22-rdf-syntax-ns#nil"/>
                      </rdf:Description>
                    </rdf:rest>
                  </rdf:Description>
                </rdf:rest>
              </rdf:Description>
            </rdf:rest>
          </rdf:Description>
        </owl:unionOf>
      </owl:Class>
    </rdfs:domain>
    <rdfs:range rdf:resource="http://www.w3.org/2001/XMLSchema#int"/>
  </owl:DatatypeProperty>
  <owl:DatatypeProperty rdf:about="http://purl.org/net/def/metashare#ageRangeStart">
    <rdfs:comment xml:lang="en">Start of age range of the group of participants</rdfs:comment>
    <rdfs:domain>
      <owl:Class>
        <owl:unionOf>
          <rdf:Description>
            <rdf:first rdf:resource="http://purl.org/net/def/metashare#CorpusAudioInfo"/>
            <rdf:rest>
              <rdf:Description>
                <rdf:first rdf:resource="http://purl.org/net/def/metashare#CorpusImageInfo"/>
                <rdf:rest>
                  <rdf:Description>
                    <rdf:first rdf:resource="http://purl.org/net/def/metashare#CorpusTextNumericalInfo"/>
                    <rdf:rest>
                      <rdf:Description>
                        <rdf:first rdf:resource="http://purl.org/net/def/metashare#CorpusVideoInfo"/>
                        <rdf:rest rdf:resource="http://www.w3.org/1999/02/22-rdf-syntax-ns#nil"/>
                      </rdf:Description>
                    </rdf:rest>
                  </rdf:Description>
                </rdf:rest>
              </rdf:Description>
            </rdf:rest>
          </rdf:Description>
        </owl:unionOf>
      </owl:Class>
    </rdfs:domain>
    <rdfs:range rdf:resource="http://www.w3.org/2001/XMLSchema#int"/>
  </owl:DatatypeProperty>
  <ns:SourceChannel rdf:about="http://purl.org/net/def/metashare#airflow"/>
  <ns:SpeechInfluences rdf:about="http://purl.org/net/def/metashare#alcohol"/>
  <owl:DatatypeProperty rdf:about="http://purl.org/net/def/metashare#alias">
    <rdfs:comment xml:lang="en">The name of the person used instead of the real one</rdfs:comment>
    <rdfs:domain rdf:resource="http://purl.org/net/def/metashare#ParticipantInfo"/>
    <rdfs:range rdf:resource="http://www.w3.org/1999/02/22-rdf-syntax-ns#langString"/>
  </owl:DatatypeProperty>
  <ns:AnnotationType rdf:about="http://purl.org/net/def/metashare#alignment"/>
  <rdf:Description rdf:about="http://purl.org/net/def/metashare#amount">
    <dct:replaces rdf:resource="http://www.ilsp.gr/META-XMLSchema#size"/>
  </rdf:Description>
  <ns:Task rdf:about="http://purl.org/net/def/metashare#analysis"/>
  <ns:GrammaticalPhenomenaCoverage rdf:about="http://purl.org/net/def/metashare#anaphora"/>
  <ns:Task rdf:about="http://purl.org/net/def/metashare#anaphoraResolution"/>
  <ns:RecordingEnvironment rdf:about="http://purl.org/net/def/metashare#anechoicChamber"/>
  <owl:ObjectProperty rdf:about="http://purl.org/net/def/metashare#annotatedElements">
    <rdfs:comment xml:lang="en">Specifies the elements annotated in each annotation level</rdfs:comment>
    <rdfs:domain rdf:resource="http://purl.org/net/def/metashare#AnnotationInfo"/>
    <rdfs:range rdf:resource="http://purl.org/net/def/metashare#AnnotatedElements"/>
  </owl:ObjectProperty>
  <ns:UseNLPSpecific rdf:about="http://purl.org/net/def/metashare#annotation"/>
  <owl:DatatypeProperty rdf:about="http://purl.org/net/def/metashare#annotationEndDate">
    <rdfs:comment xml:lang="en">The date in which the annotation process has ended</rdfs:comment>
    <rdfs:domain rdf:resource="http://purl.org/net/def/metashare#AnnotationInfo"/>
    <rdfs:range rdf:resource="http://www.w3.org/2001/XMLSchema#date"/>
  </owl:DatatypeProperty>
  <owl:DatatypeProperty rdf:about="http://purl.org/net/def/metashare#annotationFormat">
    <rdfs:comment xml:lang="en">Specifies the format that is used in the annotation process since often the mime type will not be sufficient for machine processing</rdfs:comment>
    <rdfs:domain>
      <owl:Class>
        <owl:unionOf>
          <rdf:Description>
            <rdf:first rdf:resource="http://purl.org/net/def/metashare#OutputInfo"/>
            <rdf:rest>
              <rdf:Description>
                <rdf:first rdf:resource="http://purl.org/net/def/metashare#InputInfo"/>
                <rdf:rest>
                  <rdf:Description>
                    <rdf:first rdf:resource="http://purl.org/net/def/metashare#AnnotationInfo"/>
                    <rdf:rest rdf:resource="http://www.w3.org/1999/02/22-rdf-syntax-ns#nil"/>
                  </rdf:Description>
                </rdf:rest>
              </rdf:Description>
            </rdf:rest>
          </rdf:Description>
        </owl:unionOf>
      </owl:Class>
    </rdfs:domain>
    <rdfs:range rdf:resource="http://www.w3.org/2001/XMLSchema#string"/>
  </owl:DatatypeProperty>
  <owl:ObjectProperty rdf:about="http://purl.org/net/def/metashare#annotationInfo">
    <rdfs:comment xml:lang="en">Groups information on the annotated part(s) of a resource</rdfs:comment>
    <rdfs:domain>
      <owl:Class>
        <owl:unionOf>
          <rdf:Description>
            <rdf:first rdf:resource="http://purl.org/net/def/metashare#CorpusTextInfo"/>
            <rdf:rest>
              <rdf:Description>
                <rdf:first rdf:resource="http://purl.org/net/def/metashare#CorpusTextNumericalInfo"/>
                <rdf:rest>
                  <rdf:Description>
                    <rdf:first rdf:resource="http://purl.org/net/def/metashare#CorpusTextNgramInfo"/>
                    <rdf:rest>
                      <rdf:Description>
                        <rdf:first rdf:resource="http://purl.org/net/def/metashare#CorpusImageInfo"/>
                        <rdf:rest>
                          <rdf:Description>
                            <rdf:first rdf:resource="http://purl.org/net/def/metashare#CorpusVideoInfo"/>
                            <rdf:rest>
                              <rdf:Description>
                                <rdf:first rdf:resource="http://purl.org/net/def/metashare#CorpusAudioInfo"/>
                                <rdf:rest rdf:resource="http://www.w3.org/1999/02/22-rdf-syntax-ns#nil"/>
                              </rdf:Description>
                            </rdf:rest>
                          </rdf:Description>
                        </rdf:rest>
                      </rdf:Description>
                    </rdf:rest>
                  </rdf:Description>
                </rdf:rest>
              </rdf:Description>
            </rdf:rest>
          </rdf:Description>
        </owl:unionOf>
      </owl:Class>
    </rdfs:domain>
    <rdfs:range>
      <owl:Class>
        <owl:unionOf>
          <rdf:Description>
            <rdf:first rdf:resource="http://purl.org/net/def/metashare#AnnotationInfo"/>
            <rdf:rest>
              <rdf:Description>
                <rdf:first rdf:resource="http://purl.org/net/def/metashare#AnnotationInfo"/>
                <rdf:rest>
                  <rdf:Description>
                    <rdf:first rdf:resource="http://purl.org/net/def/metashare#AnnotationInfo"/>
                    <rdf:rest>
                      <rdf:Description>
                        <rdf:first rdf:resource="http://purl.org/net/def/metashare#AnnotationInfo"/>
                        <rdf:rest>
                          <rdf:Description>
                            <rdf:first rdf:resource="http://purl.org/net/def/metashare#AnnotationInfo"/>
                            <rdf:rest>
                              <rdf:Description>
                                <rdf:first rdf:resource="http://purl.org/net/def/metashare#AnnotationInfo"/>
                                <rdf:rest rdf:resource="http://www.w3.org/1999/02/22-rdf-syntax-ns#nil"/>
                              </rdf:Description>
                            </rdf:rest>
                          </rdf:Description>
                        </rdf:rest>
                      </rdf:Description>
                    </rdf:rest>
                  </rdf:Description>
                </rdf:rest>
              </rdf:Description>
            </rdf:rest>
          </rdf:Description>
        </owl:unionOf>
      </owl:Class>
    </rdfs:range>
  </owl:ObjectProperty>
  <owl:ObjectProperty rdf:about="http://purl.org/net/def/metashare#annotationManual">
    <rdfs:comment xml:lang="en">A bibliographic reference or ms:httpURI link to the annotation manual</rdfs:comment>
    <rdfs:domain rdf:resource="http://purl.org/net/def/metashare#AnnotationInfo"/>
    <rdfs:range rdf:resource="http://purl.org/net/def/metashare#Documentation"/>
  </owl:ObjectProperty>
  <owl:ObjectProperty rdf:about="http://purl.org/net/def/metashare#annotationMode">
    <rdfs:comment xml:lang="en">Indicates whether the resource is annotated manually or by automatic processes</rdfs:comment>
    <rdfs:domain rdf:resource="http://purl.org/net/def/metashare#AnnotationInfo"/>
    <rdfs:range rdf:resource="http://purl.org/net/def/metashare#AnnotationMode"/>
  </owl:ObjectProperty>
  <owl:DatatypeProperty rdf:about="http://purl.org/net/def/metashare#annotationModeDetails">
    <rdfs:comment xml:lang="en">Provides further information on annotation process </rdfs:comment>
    <rdfs:domain rdf:resource="http://purl.org/net/def/metashare#AnnotationInfo"/>
    <rdfs:range rdf:resource="http://www.w3.org/2001/XMLSchema#string"/>
  </owl:DatatypeProperty>
  <owl:DatatypeProperty rdf:about="http://purl.org/net/def/metashare#annotationStandoff">
    <rdfs:comment xml:lang="en">Indicates whether the annotation is created inline or in a stand-off fashion</rdfs:comment>
    <rdfs:domain rdf:resource="http://purl.org/net/def/metashare#AnnotationInfo"/>
    <rdfs:range rdf:resource="http://www.w3.org/2001/XMLSchema#boolean"/>
  </owl:DatatypeProperty>
  <owl:DatatypeProperty rdf:about="http://purl.org/net/def/metashare#annotationStartDate">
    <rdfs:comment xml:lang="en">The date in which the annotation process has started</rdfs:comment>
    <rdfs:domain rdf:resource="http://purl.org/net/def/metashare#AnnotationInfo"/>
    <rdfs:range rdf:resource="http://www.w3.org/2001/XMLSchema#date"/>
  </owl:DatatypeProperty>
  <owl:DatatypeProperty rdf:about="http://purl.org/net/def/metashare#annotationTool">
    <rdfs:comment xml:lang="en">The name, the identifier or the url of the tool used for the annotation of the resource</rdfs:comment>
    <rdfs:domain rdf:resource="http://purl.org/net/def/metashare#AnnotationInfo"/>
    <rdfs:range rdf:resource="http://www.w3.org/2001/XMLSchema#string"/>
  </owl:DatatypeProperty>
  <owl:ObjectProperty rdf:about="http://purl.org/net/def/metashare#annotationType">
    <rdfs:comment xml:lang="en">Specifies the annotation level of the resource or the annotation type a tool/ service requires or produces as an output</rdfs:comment>
    <rdfs:domain>
      <owl:Class>
        <owl:unionOf>
          <rdf:Description>
            <rdf:first rdf:resource="http://purl.org/net/def/metashare#OutputInfo"/>
            <rdf:rest>
              <rdf:Description>
                <rdf:first rdf:resource="http://purl.org/net/def/metashare#InputInfo"/>
                <rdf:rest>
                  <rdf:Description>
                    <rdf:first rdf:resource="http://purl.org/net/def/metashare#AnnotationInfo"/>
                    <rdf:rest rdf:resource="http://www.w3.org/1999/02/22-rdf-syntax-ns#nil"/>
                  </rdf:Description>
                </rdf:rest>
              </rdf:Description>
            </rdf:rest>
          </rdf:Description>
        </owl:unionOf>
      </owl:Class>
    </rdfs:domain>
    <rdfs:range>
      <owl:Class>
        <owl:unionOf>
          <rdf:Description>
            <rdf:first rdf:resource="http://purl.org/net/def/metashare#AnnotationType"/>
            <rdf:rest>
              <rdf:Description>
                <rdf:first rdf:resource="http://purl.org/net/def/metashare#AnnotationType"/>
                <rdf:rest>
                  <rdf:Description>
                    <rdf:first rdf:resource="http://purl.org/net/def/metashare#AnnotationType"/>
                    <rdf:rest rdf:resource="http://www.w3.org/1999/02/22-rdf-syntax-ns#nil"/>
                  </rdf:Description>
                </rdf:rest>
              </rdf:Description>
            </rdf:rest>
          </rdf:Description>
        </owl:unionOf>
      </owl:Class>
    </rdfs:range>
  </owl:ObjectProperty>
  <owl:ObjectProperty rdf:about="http://purl.org/net/def/metashare#annotator">
    <rdfs:comment xml:lang="en">Groups information on the annotators of the specific annotation type</rdfs:comment>
    <rdfs:domain rdf:resource="http://purl.org/net/def/metashare#AnnotationInfo"/>
    <rdfs:range rdf:resource="http://purl.org/net/def/metashare#Actor"/>
  </owl:ObjectProperty>
  <ns:SpeechItems rdf:about="http://purl.org/net/def/metashare#applicationWords"/>
  <ns:ToolServiceType rdf:about="http://purl.org/net/def/metashare#architecture"/>
  <ns:BodyParts rdf:about="http://purl.org/net/def/metashare#arms"/>
  <ns:SizeUnit rdf:about="http://purl.org/net/def/metashare#articles"/>
  <owl:DatatypeProperty rdf:about="http://purl.org/net/def/metashare#artifactParts">
    <rdfs:comment xml:lang="en">Indicates the parts of the artifacts represented in the image corpus</rdfs:comment>
    <rdfs:domain rdf:resource="http://purl.org/net/def/metashare#StaticElementInfo"/>
    <rdfs:range rdf:resource="http://www.w3.org/2001/XMLSchema#string"/>
  </owl:DatatypeProperty>
  <ns:Naturality rdf:about="http://purl.org/net/def/metashare#assisted"/>
  <ns:CompressionName rdf:about="http://purl.org/net/def/metashare#atrac"/>
  <ns:RelatedLexiconType rdf:about="http://purl.org/net/def/metashare#attached"/>
  <owl:DatatypeProperty rdf:about="http://purl.org/net/def/metashare#attachedLexiconPosition">
    <rdfs:comment xml:lang="en">Indicates the position of the lexicon, if attached to the grammar</rdfs:comment>
    <rdfs:domain rdf:resource="http://purl.org/net/def/metashare#LanguageDescriptionInfo"/>
    <rdfs:range rdf:resource="http://www.w3.org/2001/XMLSchema#string"/>
  </owl:DatatypeProperty>
  <odrl:Set rdf:about="http://purl.org/net/def/metashare#attribution">
    <rdf:type rdf:resource="http://purl.org/net/def/metashare#ConditionsOfUse"/>
    <odrl:permission>
      <rdf:Description>
        <odrl:duty>
          <rdf:Description>
            <odrl:action rdf:resource="http://creativecommons.org/ns#Attribution"/>
          </rdf:Description>
        </odrl:duty>
      </rdf:Description>
    </odrl:permission>
  </odrl:Set>
  <owl:DatatypeProperty rdf:about="http://purl.org/net/def/metashare#attributionText">
    <rdfs:comment xml:lang="en">The text that must be quoted for attribution purposes when using a resource - for cases where a resource is provided with a restriction on attribution</rdfs:comment>
    <rdfs:domain rdf:resource="http://purl.org/net/def/metashare#LicenceInfo"/>
    <rdfs:range rdf:resource="http://www.w3.org/1999/02/22-rdf-syntax-ns#langString"/>
  </owl:DatatypeProperty>
  <owl:ObjectProperty rdf:about="http://purl.org/net/def/metashare#audience">
    <rdfs:comment xml:lang="en">Indication of the intended audience size</rdfs:comment>
    <rdfs:domain>
      <owl:Class>
        <owl:unionOf>
          <rdf:Description>
            <rdf:first rdf:resource="http://purl.org/net/def/metashare#CorpusAudioInfo"/>
            <rdf:rest>
              <rdf:Description>
                <rdf:first rdf:resource="http://purl.org/net/def/metashare#CorpusVideoInfo"/>
                <rdf:rest rdf:resource="http://www.w3.org/1999/02/22-rdf-syntax-ns#nil"/>
              </rdf:Description>
            </rdf:rest>
          </rdf:Description>
        </owl:unionOf>
      </owl:Class>
    </rdfs:domain>
    <rdfs:range>
      <owl:Class>
        <owl:unionOf>
          <rdf:Description>
            <rdf:first rdf:resource="http://purl.org/net/def/metashare#Audience"/>
            <rdf:rest>
              <rdf:Description>
                <rdf:first rdf:resource="http://purl.org/net/def/metashare#Audience"/>
                <rdf:rest rdf:resource="http://www.w3.org/1999/02/22-rdf-syntax-ns#nil"/>
              </rdf:Description>
            </rdf:rest>
          </rdf:Description>
        </owl:unionOf>
      </owl:Class>
    </rdfs:range>
  </owl:ObjectProperty>
  <ns:MediaType rdf:about="http://purl.org/net/def/metashare#audio">
    <rdf:type rdf:resource="http://purl.org/net/def/metashare#OtherMedia"/>
  </ns:MediaType>
  <owl:ObjectProperty rdf:about="http://purl.org/net/def/metashare#audioClassificationInfo">
    <rdfs:comment xml:lang="en">Groups together information on audio type/genre of the resource</rdfs:comment>
    <rdfs:domain rdf:resource="http://purl.org/net/def/metashare#CorpusAudioInfo"/>
    <rdfs:range rdf:resource="http://purl.org/net/def/metashare#AudioClassificationInfo"/>
  </owl:ObjectProperty>
  <owl:ObjectProperty rdf:about="http://purl.org/net/def/metashare#audioFormatInfo">
    <rdfs:comment xml:lang="en">Groups together information on the format of the audio part of a resource</rdfs:comment>
    <rdfs:domain>
      <owl:Class>
        <owl:unionOf>
          <rdf:Description>
            <rdf:first rdf:resource="http://purl.org/net/def/metashare#LexicalConceptualResourceAudioInfo"/>
            <rdf:rest>
              <rdf:Description>
                <rdf:first rdf:resource="http://purl.org/net/def/metashare#CorpusAudioInfo"/>
                <rdf:rest rdf:resource="http://www.w3.org/1999/02/22-rdf-syntax-ns#nil"/>
              </rdf:Description>
            </rdf:rest>
          </rdf:Description>
        </owl:unionOf>
      </owl:Class>
    </rdfs:domain>
    <rdfs:range>
      <owl:Class>
        <owl:unionOf>
          <rdf:Description>
            <rdf:first rdf:resource="http://purl.org/net/def/metashare#AudioFormatInfo"/>
            <rdf:rest>
              <rdf:Description>
                <rdf:first rdf:resource="http://purl.org/net/def/metashare#AudioFormatInfo"/>
                <rdf:rest rdf:resource="http://www.w3.org/1999/02/22-rdf-syntax-ns#nil"/>
              </rdf:Description>
            </rdf:rest>
          </rdf:Description>
        </owl:unionOf>
      </owl:Class>
    </rdfs:range>
  </owl:ObjectProperty>
  <owl:DatatypeProperty rdf:about="http://purl.org/net/def/metashare#audioGenre">
    <rdfs:comment xml:lang="en">A first indication of type of sounds recorded</rdfs:comment>
    <rdfs:domain rdf:resource="http://purl.org/net/def/metashare#AudioClassificationInfo"/>
    <rdfs:range rdf:resource="http://www.w3.org/2001/XMLSchema#string"/>
    <rdfs:subPropertyOf rdf:resource="http://purl.org/net/def/metashare#genre"/>
  </owl:DatatypeProperty>
  <owl:ObjectProperty rdf:about="http://purl.org/net/def/metashare#audioQualityMeasuresIncluded">
    <rdfs:comment xml:lang="en">Specifies the audio quality measures</rdfs:comment>
    <rdfs:domain rdf:resource="http://purl.org/net/def/metashare#AudioFormatInfo"/>
    <rdfs:range rdf:resource="http://purl.org/net/def/metashare#AudioQualityMeasuresIncluded"/>
  </owl:ObjectProperty>
  <owl:ObjectProperty rdf:about="http://purl.org/net/def/metashare#audioSizeInfo">
    <rdfs:comment xml:lang="en">SizeInfo Element for Audio parts of a resource</rdfs:comment>
    <rdfs:domain rdf:resource="http://purl.org/net/def/metashare#CorpusAudioInfo"/>
    <rdfs:range rdf:resource="http://purl.org/net/def/metashare#AudioSizeInfo"/>
  </owl:ObjectProperty>
  <owl:DatatypeProperty rdf:about="http://purl.org/net/def/metashare#authenticated">
    <rdfs:comment xml:lang="en">Specifies if the user has been identified/authenticated.</rdfs:comment>
    <rdfs:label xml:lang="en">Authenticated</rdfs:label>
    <rdfs:range rdf:resource="http://www.w3.org/2001/XMLSchema#boolean"/>
  </owl:DatatypeProperty>
  <ns:AnnotationMode rdf:about="http://purl.org/net/def/metashare#automatic">
    <rdf:type rdf:resource="http://purl.org/net/def/metashare#CreationMode"/>
    <rdf:type rdf:resource="http://purl.org/net/def/metashare#EvaluationMeasure"/>
    <rdf:type rdf:resource="http://purl.org/net/def/metashare#ValidationMode"/>
  </ns:AnnotationMode>
  <owl:ObjectProperty rdf:about="http://purl.org/net/def/metashare#availability">
    <rdfs:comment xml:lang="en">Specifies the availability status of the resource; restrictionsOfUse can be further used to indicate the specific terms of availability</rdfs:comment>
    <rdfs:range rdf:resource="http://purl.org/net/def/metashare#Availability"/>
  </owl:ObjectProperty>
  <owl:DatatypeProperty rdf:about="http://purl.org/net/def/metashare#availabilityEndDate">
    <rdfs:comment xml:lang="en">Identifies the Availability End Date of the resource.</rdfs:comment>
    <rdfs:comment xml:lang="en">Specifies the end date of availability of a resource - only for cases where a resource is available for a restricted time period.</rdfs:comment>
    <rdfs:range rdf:resource="http://www.w3.org/2001/XMLSchema#date"/>
  </owl:DatatypeProperty>
  <owl:DatatypeProperty rdf:about="http://purl.org/net/def/metashare#availabilityStartDate">
    <rdfs:comment xml:lang="en">Identifies the Availability Start Date of the resource.</rdfs:comment>
    <rdfs:comment xml:lang="en">Specifies the start date of availability of a resource - only for cases where a resource is available for a restricted time period.</rdfs:comment>
    <rdfs:range rdf:resource="http://www.w3.org/2001/XMLSchema#date"/>
  </owl:DatatypeProperty>
  <ns:Availability rdf:about="http://purl.org/net/def/metashare#available-restrictedUse">
    <rdfs:comment xml:lang="en">For resources available but with conditions of use imposed by the type of licence.</rdfs:comment>
  </ns:Availability>
  <ns:Availability rdf:about="http://purl.org/net/def/metashare#available-unrestrictedUse">
    <rdfs:comment xml:lang="en">For resources available with no restrictions of use (e.g. public domain resources).</rdfs:comment>
  </ns:Availability>
  <rdf:Description rdf:about="http://purl.org/net/def/metashare#availableThroughOtherDistributor">
    <dct:replaces rdf:resource="http://www.ilsp.gr/META-XMLSchema#notAvailableThroughMetashare"/>
    <rdfs:comment xml:lang="en">For resources that are documented in the catalogue but the contents of which can only be accessed through other distribution channels.</rdfs:comment>
    <rdfs:label xml:lang="en">Available Through Other Distributor</rdfs:label>
  </rdf:Description>
  <ns:Availability rdf:about="http://purl.org/net/def/metashare#availableThroughOtherDistributors"/>
  <ns:UseNLPSpecific rdf:about="http://purl.org/net/def/metashare#avatarSynthesis"/>
  <ns:CompressionName rdf:about="http://purl.org/net/def/metashare#avi"/>
  <ns:AnnotatedElements rdf:about="http://purl.org/net/def/metashare#backgroundNoise">
    <rdf:type rdf:resource="http://purl.org/net/def/metashare#AudioQualityMeasuresIncluded"/>
  </ns:AnnotatedElements>
  <owl:ObjectProperty rdf:about="http://purl.org/net/def/metashare#baseItem">
    <rdfs:comment xml:lang="en">Type of item that is represented in the n-gram resource</rdfs:comment>
    <rdfs:domain rdf:resource="http://purl.org/net/def/metashare#NgramInfo"/>
    <rdfs:range rdf:resource="http://purl.org/net/def/metashare#BaseItem"/>
  </owl:ObjectProperty>
  <ns:ByteOrder rdf:about="http://purl.org/net/def/metashare#bigEndian"/>
  <ns:SizeUnit rdf:about="http://purl.org/net/def/metashare#bigrams"/>
  <ns:LingualityType rdf:about="http://purl.org/net/def/metashare#bilingual"/>
  <ns:UseNLPSpecific rdf:about="http://purl.org/net/def/metashare#bilingualLexiconInduction"/>
  <ns:EvaluationType rdf:about="http://purl.org/net/def/metashare#blackBox"/>
  <ns:DistributionAccessMedium rdf:about="http://purl.org/net/def/metashare#bluRay">
    <rdfs:comment xml:lang="en">bluRay refers to a kind of distribution/access medium used for delivering a language resource; intended for resources delivered on bluRay disks</rdfs:comment>
  </ns:DistributionAccessMedium>
  <ns:ModalityType rdf:about="http://purl.org/net/def/metashare#bodyGesture"/>
  <owl:DatatypeProperty rdf:about="http://purl.org/net/def/metashare#bodyMovement">
    <rdfs:comment xml:lang="en">Indicates the body parts that move in the video part of the resource</rdfs:comment>
    <rdfs:domain rdf:resource="http://purl.org/net/def/metashare#DynamicElementInfo"/>
    <rdfs:range rdf:resource="http://www.w3.org/2001/XMLSchema#string"/>
  </owl:DatatypeProperty>
  <owl:ObjectProperty rdf:about="http://purl.org/net/def/metashare#bodyParts">
    <rdfs:comment xml:lang="en">The body parts visible in the video or image part of the resource</rdfs:comment>
    <rdfs:domain>
      <owl:Class>
        <owl:unionOf>
          <rdf:Description>
            <rdf:first rdf:resource="http://purl.org/net/def/metashare#StaticElementInfo"/>
            <rdf:rest>
              <rdf:Description>
                <rdf:first rdf:resource="http://purl.org/net/def/metashare#DynamicElementInfo"/>
                <rdf:rest rdf:resource="http://www.w3.org/1999/02/22-rdf-syntax-ns#nil"/>
              </rdf:Description>
            </rdf:rest>
          </rdf:Description>
        </owl:unionOf>
      </owl:Class>
    </rdfs:domain>
    <rdfs:range>
      <owl:Class>
        <owl:unionOf>
          <rdf:Description>
            <rdf:first rdf:resource="http://purl.org/net/def/metashare#BodyParts"/>
            <rdf:rest>
              <rdf:Description>
                <rdf:first rdf:resource="http://purl.org/net/def/metashare#BodyParts"/>
                <rdf:rest rdf:resource="http://www.w3.org/1999/02/22-rdf-syntax-ns#nil"/>
              </rdf:Description>
            </rdf:rest>
          </rdf:Description>
        </owl:unionOf>
      </owl:Class>
    </rdfs:range>
  </owl:ObjectProperty>
  <owl:ObjectProperty rdf:about="http://purl.org/net/def/metashare#byteOrder">
    <rdfs:comment xml:lang="en">The byte order of 2 or more bytes sample</rdfs:comment>
    <rdfs:domain rdf:resource="http://purl.org/net/def/metashare#AudioFormatInfo"/>
    <rdfs:range rdf:resource="http://purl.org/net/def/metashare#ByteOrder"/>
  </owl:ObjectProperty>
  <ns:SizeUnit rdf:about="http://purl.org/net/def/metashare#bytes"/>
  <ns:SourceChannel rdf:about="http://purl.org/net/def/metashare#camcorder"/>
  <ns:CapturingDeviceType rdf:about="http://purl.org/net/def/metashare#camera"/>
  <ns:TextIncludedInImage rdf:about="http://purl.org/net/def/metashare#captions">
    <rdf:type rdf:resource="http://purl.org/net/def/metashare#TextIncludedInVideo"/>
  </ns:TextIncludedInImage>
  <ns:TextIncludedInImage rdf:about="http://purl.org/net/def/metashare#captureTime"/>
  <owl:DatatypeProperty rdf:about="http://purl.org/net/def/metashare#capturingDetails">
    <rdfs:comment xml:lang="en">Provides further information on the capturing method and procedure</rdfs:comment>
    <rdfs:domain>
      <owl:Class>
        <owl:unionOf>
          <rdf:Description>
            <rdf:first rdf:resource="http://purl.org/net/def/metashare#CorpusTextNumericalInfo"/>
            <rdf:rest>
              <rdf:Description>
                <rdf:first rdf:resource="http://purl.org/net/def/metashare#CorpusVideoInfo"/>
                <rdf:rest>
                  <rdf:Description>
                    <rdf:first rdf:resource="http://purl.org/net/def/metashare#CorpusImageInfo"/>
                    <rdf:rest>
                      <rdf:Description>
                        <rdf:first rdf:resource="http://purl.org/net/def/metashare#CorpusAudioInfo"/>
                        <rdf:rest rdf:resource="http://www.w3.org/1999/02/22-rdf-syntax-ns#nil"/>
                      </rdf:Description>
                    </rdf:rest>
                  </rdf:Description>
                </rdf:rest>
              </rdf:Description>
            </rdf:rest>
          </rdf:Description>
        </owl:unionOf>
      </owl:Class>
    </rdfs:domain>
    <rdfs:range rdf:resource="http://www.w3.org/2001/XMLSchema#string"/>
  </owl:DatatypeProperty>
  <owl:ObjectProperty rdf:about="http://purl.org/net/def/metashare#capturingDeviceType">
    <rdfs:comment xml:lang="en">The transducers through which the data is captured</rdfs:comment>
    <rdfs:domain>
      <owl:Class>
        <owl:unionOf>
          <rdf:Description>
            <rdf:first rdf:resource="http://purl.org/net/def/metashare#CorpusTextNumericalInfo"/>
            <rdf:rest>
              <rdf:Description>
                <rdf:first rdf:resource="http://purl.org/net/def/metashare#CorpusVideoInfo"/>
                <rdf:rest>
                  <rdf:Description>
                    <rdf:first rdf:resource="http://purl.org/net/def/metashare#CorpusAudioInfo"/>
                    <rdf:rest>
                      <rdf:Description>
                        <rdf:first rdf:resource="http://purl.org/net/def/metashare#CorpusImageInfo"/>
                        <rdf:rest rdf:resource="http://www.w3.org/1999/02/22-rdf-syntax-ns#nil"/>
                      </rdf:Description>
                    </rdf:rest>
                  </rdf:Description>
                </rdf:rest>
              </rdf:Description>
            </rdf:rest>
          </rdf:Description>
        </owl:unionOf>
      </owl:Class>
    </rdfs:domain>
    <rdfs:range>
      <owl:Class>
        <owl:unionOf>
          <rdf:Description>
            <rdf:first rdf:resource="http://purl.org/net/def/metashare#CapturingDeviceType"/>
            <rdf:rest>
              <rdf:Description>
                <rdf:first rdf:resource="http://purl.org/net/def/metashare#CapturingDeviceType"/>
                <rdf:rest>
                  <rdf:Description>
                    <rdf:first rdf:resource="http://purl.org/net/def/metashare#CapturingDeviceType"/>
                    <rdf:rest>
                      <rdf:Description>
                        <rdf:first rdf:resource="http://purl.org/net/def/metashare#CapturingDeviceType"/>
                        <rdf:rest rdf:resource="http://www.w3.org/1999/02/22-rdf-syntax-ns#nil"/>
                      </rdf:Description>
                    </rdf:rest>
                  </rdf:Description>
                </rdf:rest>
              </rdf:Description>
            </rdf:rest>
          </rdf:Description>
        </owl:unionOf>
      </owl:Class>
    </rdfs:range>
  </owl:ObjectProperty>
  <owl:DatatypeProperty rdf:about="http://purl.org/net/def/metashare#capturingDeviceTypeDetails">
    <rdfs:comment xml:lang="en">Provides further information on the capturing device</rdfs:comment>
    <rdfs:domain>
      <owl:Class>
        <owl:unionOf>
          <rdf:Description>
            <rdf:first rdf:resource="http://purl.org/net/def/metashare#CorpusImageInfo"/>
            <rdf:rest>
              <rdf:Description>
                <rdf:first rdf:resource="http://purl.org/net/def/metashare#CorpusVideoInfo"/>
                <rdf:rest>
                  <rdf:Description>
                    <rdf:first rdf:resource="http://purl.org/net/def/metashare#CorpusTextNumericalInfo"/>
                    <rdf:rest>
                      <rdf:Description>
                        <rdf:first rdf:resource="http://purl.org/net/def/metashare#CorpusAudioInfo"/>
                        <rdf:rest rdf:resource="http://www.w3.org/1999/02/22-rdf-syntax-ns#nil"/>
                      </rdf:Description>
                    </rdf:rest>
                  </rdf:Description>
                </rdf:rest>
              </rdf:Description>
            </rdf:rest>
          </rdf:Description>
        </owl:unionOf>
      </owl:Class>
    </rdfs:domain>
    <rdfs:range rdf:resource="http://www.w3.org/2001/XMLSchema#string"/>
  </owl:DatatypeProperty>
  <owl:ObjectProperty rdf:about="http://purl.org/net/def/metashare#capturingEnvironment">
    <rdfs:comment xml:lang="en">Type of capturing environment</rdfs:comment>
    <rdfs:domain>
      <owl:Class>
        <owl:unionOf>
          <rdf:Description>
            <rdf:first rdf:resource="http://purl.org/net/def/metashare#CorpusImageInfo"/>
            <rdf:rest>
              <rdf:Description>
                <rdf:first rdf:resource="http://purl.org/net/def/metashare#CorpusVideoInfo"/>
                <rdf:rest>
                  <rdf:Description>
                    <rdf:first rdf:resource="http://purl.org/net/def/metashare#CorpusTextNumericalInfo"/>
                    <rdf:rest>
                      <rdf:Description>
                        <rdf:first rdf:resource="http://purl.org/net/def/metashare#CorpusAudioInfo"/>
                        <rdf:rest rdf:resource="http://www.w3.org/1999/02/22-rdf-syntax-ns#nil"/>
                      </rdf:Description>
                    </rdf:rest>
                  </rdf:Description>
                </rdf:rest>
              </rdf:Description>
            </rdf:rest>
          </rdf:Description>
        </owl:unionOf>
      </owl:Class>
    </rdfs:domain>
    <rdfs:range>
      <owl:Class>
        <owl:unionOf>
          <rdf:Description>
            <rdf:first rdf:resource="http://purl.org/net/def/metashare#CapturingEnvironment"/>
            <rdf:rest>
              <rdf:Description>
                <rdf:first rdf:resource="http://purl.org/net/def/metashare#CapturingEnvironment"/>
                <rdf:rest>
                  <rdf:Description>
                    <rdf:first rdf:resource="http://purl.org/net/def/metashare#CapturingEnvironment"/>
                    <rdf:rest>
                      <rdf:Description>
                        <rdf:first rdf:resource="http://purl.org/net/def/metashare#CapturingEnvironment"/>
                        <rdf:rest rdf:resource="http://www.w3.org/1999/02/22-rdf-syntax-ns#nil"/>
                      </rdf:Description>
                    </rdf:rest>
                  </rdf:Description>
                </rdf:rest>
              </rdf:Description>
            </rdf:rest>
          </rdf:Description>
        </owl:unionOf>
      </owl:Class>
    </rdfs:range>
  </owl:ObjectProperty>
  <owl:ObjectProperty rdf:about="http://purl.org/net/def/metashare#characterEncoding">
    <rdfs:comment xml:lang="en">The name of the character encoding used in the resource or accepted by the tool/service</rdfs:comment>
    <rdfs:domain>
      <owl:Class>
        <owl:unionOf>
          <rdf:Description>
            <rdf:first rdf:resource="http://purl.org/net/def/metashare#CharacterEncodingInfo"/>
            <rdf:rest>
              <rdf:Description>
                <rdf:first rdf:resource="http://purl.org/net/def/metashare#OutputInfo"/>
                <rdf:rest>
                  <rdf:Description>
                    <rdf:first rdf:resource="http://purl.org/net/def/metashare#InputInfo"/>
                    <rdf:rest rdf:resource="http://www.w3.org/1999/02/22-rdf-syntax-ns#nil"/>
                  </rdf:Description>
                </rdf:rest>
              </rdf:Description>
            </rdf:rest>
          </rdf:Description>
        </owl:unionOf>
      </owl:Class>
    </rdfs:domain>
    <rdfs:range>
      <owl:Class>
        <owl:unionOf>
          <rdf:Description>
            <rdf:first rdf:resource="http://purl.org/net/def/metashare#CharacterEncoding"/>
            <rdf:rest>
              <rdf:Description>
                <rdf:first rdf:resource="http://purl.org/net/def/metashare#CharacterEncoding"/>
                <rdf:rest>
                  <rdf:Description>
                    <rdf:first rdf:resource="http://purl.org/net/def/metashare#CharacterEncoding"/>
                    <rdf:rest rdf:resource="http://www.w3.org/1999/02/22-rdf-syntax-ns#nil"/>
                  </rdf:Description>
                </rdf:rest>
              </rdf:Description>
            </rdf:rest>
          </rdf:Description>
        </owl:unionOf>
      </owl:Class>
    </rdfs:range>
  </owl:ObjectProperty>
  <owl:ObjectProperty rdf:about="http://purl.org/net/def/metashare#characterEncodingInfo">
    <rdfs:comment xml:lang="en">Groups together information on character encoding of the resource</rdfs:comment>
    <rdfs:domain>
      <owl:Class>
        <owl:unionOf>
          <rdf:Description>
            <rdf:first rdf:resource="http://purl.org/net/def/metashare#LanguageDescriptionTextInfo"/>
            <rdf:rest>
              <rdf:Description>
                <rdf:first rdf:resource="http://purl.org/net/def/metashare#CorpusTextInfo"/>
                <rdf:rest>
                  <rdf:Description>
                    <rdf:first rdf:resource="http://purl.org/net/def/metashare#LexicalConceptualResourceTextInfo"/>
                    <rdf:rest>
                      <rdf:Description>
                        <rdf:first rdf:resource="http://purl.org/net/def/metashare#CorpusTextNgramInfo"/>
                        <rdf:rest rdf:resource="http://www.w3.org/1999/02/22-rdf-syntax-ns#nil"/>
                      </rdf:Description>
                    </rdf:rest>
                  </rdf:Description>
                </rdf:rest>
              </rdf:Description>
            </rdf:rest>
          </rdf:Description>
        </owl:unionOf>
      </owl:Class>
    </rdfs:domain>
    <rdfs:range>
      <owl:Class>
        <owl:unionOf>
          <rdf:Description>
            <rdf:first rdf:resource="http://purl.org/net/def/metashare#CharacterEncodingInfo"/>
            <rdf:rest>
              <rdf:Description>
                <rdf:first rdf:resource="http://purl.org/net/def/metashare#CharacterEncodingInfo"/>
                <rdf:rest>
                  <rdf:Description>
                    <rdf:first rdf:resource="http://purl.org/net/def/metashare#CharacterEncodingInfo"/>
                    <rdf:rest>
                      <rdf:Description>
                        <rdf:first rdf:resource="http://purl.org/net/def/metashare#CharacterEncodingInfo"/>
                        <rdf:rest rdf:resource="http://www.w3.org/1999/02/22-rdf-syntax-ns#nil"/>
                      </rdf:Description>
                    </rdf:rest>
                  </rdf:Description>
                </rdf:rest>
              </rdf:Description>
            </rdf:rest>
          </rdf:Description>
        </owl:unionOf>
      </owl:Class>
    </rdfs:range>
  </owl:ObjectProperty>
  <ns:AgeGroup rdf:about="http://purl.org/net/def/metashare#child">
    <rdf:type rdf:resource="http://purl.org/net/def/metashare#AgeOfPersons"/>
  </ns:AgeGroup>
  <ns:Task rdf:about="http://purl.org/net/def/metashare#chunking"/>
  <owl:DatatypeProperty rdf:about="http://purl.org/net/def/metashare#city">
    <rdfs:comment xml:lang="en">The name of the city, town or village as mentioned in the postal address of a person or organization </rdfs:comment>
    <rdfs:domain>
      <owl:Class>
        <owl:unionOf>
          <rdf:Description>
            <rdf:first rdf:resource="http://purl.org/net/def/metashare#Organization"/>
            <rdf:rest>
              <rdf:Description>
                <rdf:first rdf:resource="http://purl.org/net/def/metashare#Person"/>
                <rdf:rest rdf:resource="http://www.w3.org/1999/02/22-rdf-syntax-ns#nil"/>
              </rdf:Description>
            </rdf:rest>
          </rdf:Description>
        </owl:unionOf>
      </owl:Class>
    </rdfs:domain>
    <rdfs:range rdf:resource="http://www.w3.org/2001/XMLSchema#string"/>
  </owl:DatatypeProperty>
  <ns:SizeUnit rdf:about="http://purl.org/net/def/metashare#classes"/>
  <ns:SegmentationLevel rdf:about="http://purl.org/net/def/metashare#clause"/>
  <ns:GrammaticalPhenomenaCoverage rdf:about="http://purl.org/net/def/metashare#clauseStructure"/>
  <ns:AudioQualityMeasuresIncluded rdf:about="http://purl.org/net/def/metashare#clippingRate"/>
  <ns:CapturingDeviceType rdf:about="http://purl.org/net/def/metashare#closeTalkMicrophone"/>
  <ns:RecordingEnvironment rdf:about="http://purl.org/net/def/metashare#closedPublicPlace"/>
  <owl:DatatypeProperty rdf:about="http://purl.org/net/def/metashare#colourDepth">
    <rdfs:comment xml:lang="en">The number of bits used to represent the colour of a single pixel</rdfs:comment>
    <rdfs:domain>
      <owl:Class>
        <owl:unionOf>
          <rdf:Description>
            <rdf:first rdf:resource="http://purl.org/net/def/metashare#ImageFormatInfo"/>
            <rdf:rest>
              <rdf:Description>
                <rdf:first rdf:resource="http://purl.org/net/def/metashare#VideoFormatInfo"/>
                <rdf:rest rdf:resource="http://www.w3.org/1999/02/22-rdf-syntax-ns#nil"/>
              </rdf:Description>
            </rdf:rest>
          </rdf:Description>
        </owl:unionOf>
      </owl:Class>
    </rdfs:domain>
    <rdfs:range rdf:resource="http://www.w3.org/2001/XMLSchema#string"/>
  </owl:DatatypeProperty>
  <owl:ObjectProperty rdf:about="http://purl.org/net/def/metashare#colourSpace">
    <rdfs:comment xml:lang="en">Defines the colour space for the video</rdfs:comment>
    <rdfs:domain>
      <owl:Class>
        <owl:unionOf>
          <rdf:Description>
            <rdf:first rdf:resource="http://purl.org/net/def/metashare#VideoFormatInfo"/>
            <rdf:rest>
              <rdf:Description>
                <rdf:first rdf:resource="http://purl.org/net/def/metashare#ImageFormatInfo"/>
                <rdf:rest rdf:resource="http://www.w3.org/1999/02/22-rdf-syntax-ns#nil"/>
              </rdf:Description>
            </rdf:rest>
          </rdf:Description>
        </owl:unionOf>
      </owl:Class>
    </rdfs:domain>
    <rdfs:range>
      <owl:Class>
        <owl:unionOf>
          <rdf:Description>
            <rdf:first rdf:resource="http://purl.org/net/def/metashare#ColourSpace"/>
            <rdf:rest>
              <rdf:Description>
                <rdf:first rdf:resource="http://purl.org/net/def/metashare#ColourSpace"/>
                <rdf:rest rdf:resource="http://www.w3.org/1999/02/22-rdf-syntax-ns#nil"/>
              </rdf:Description>
            </rdf:rest>
          </rdf:Description>
        </owl:unionOf>
      </owl:Class>
    </rdfs:range>
  </owl:ObjectProperty>
  <ns:ModalityType rdf:about="http://purl.org/net/def/metashare#combinationOfModalities"/>
  <ns:NonSpeechItems rdf:about="http://purl.org/net/def/metashare#commercial">
    <rdf:type rdf:resource="http://purl.org/net/def/metashare#UserNature"/>
    <rdfs:comment xml:lang="en">It refers to resource users affiliated with a commercial institution</rdfs:comment>
  </ns:NonSpeechItems>
  <ns:ConditionsOfUse rdf:about="http://purl.org/net/def/metashare#commercialUse"/>
  <odrl:Set rdf:about="http://purl.org/net/def/metashare#commericalUse">
    <odrl:permission>
      <rdf:Description>
        <odrl:action rdf:resource="http://creativecommons.org/ns#CommercialUse"/>
      </rdf:Description>
    </odrl:permission>
  </odrl:Set>
  <ns3:concept xmlns:ns3="http://www.w3.org/2004/02/skos/core#"
     rdf:about="http://purl.org/net/def/metashare#communicate">
    <rdfs:comment xml:lang="en">The Assigner permits/prohibits the Assignees to communicate the Asset to the public</rdfs:comment>
    <rdfs:label xml:lang="en">communicate</rdfs:label>
    <ns3:closeMatch rdf:resource="http://www.w3.org/ns/odrl/2/present"/>
  </ns3:concept>
  <ns:MultilingualityType rdf:about="http://purl.org/net/def/metashare#comparable"/>
  <ns:RelatedLexiconType rdf:about="http://purl.org/net/def/metashare#compatible"/>
  <owl:ObjectProperty rdf:about="http://purl.org/net/def/metashare#compatibleLexiconType">
    <rdfs:comment xml:lang="en">Type of (external) lexicon that can be used with the grammar</rdfs:comment>
    <rdfs:domain rdf:resource="http://purl.org/net/def/metashare#LanguageDescriptionInfo"/>
    <rdfs:range rdf:resource="http://purl.org/net/def/metashare#CompatibleLexiconType"/>
  </owl:ObjectProperty>
  <ns:CapturingEnvironment rdf:about="http://purl.org/net/def/metashare#complex"/>
  <owl:DatatypeProperty rdf:about="http://purl.org/net/def/metashare#compression">
    <rdfs:comment xml:lang="en">Whether the audio, video or image is compressed or not</rdfs:comment>
    <rdfs:domain>
      <owl:Class>
        <owl:unionOf>
          <rdf:Description>
            <rdf:first rdf:resource="http://purl.org/net/def/metashare#ImageFormatInfo"/>
            <rdf:rest>
              <rdf:Description>
                <rdf:first rdf:resource="http://purl.org/net/def/metashare#VideoFormatInfo"/>
                <rdf:rest>
                  <rdf:Description>
                    <rdf:first rdf:resource="http://purl.org/net/def/metashare#AudioFormatInfo"/>
                    <rdf:rest rdf:resource="http://www.w3.org/1999/02/22-rdf-syntax-ns#nil"/>
                  </rdf:Description>
                </rdf:rest>
              </rdf:Description>
            </rdf:rest>
          </rdf:Description>
        </owl:unionOf>
      </owl:Class>
    </rdfs:domain>
    <rdfs:range rdf:resource="http://www.w3.org/2001/XMLSchema#boolean"/>
  </owl:DatatypeProperty>
  <owl:DatatypeProperty rdf:about="http://purl.org/net/def/metashare#compressionLoss">
    <rdfs:comment xml:lang="en">Whether there is loss due to compression</rdfs:comment>
    <rdfs:domain>
      <owl:Class>
        <owl:unionOf>
          <rdf:Description>
            <rdf:first rdf:resource="http://purl.org/net/def/metashare#VideoFormatInfo"/>
            <rdf:rest>
              <rdf:Description>
                <rdf:first rdf:resource="http://purl.org/net/def/metashare#AudioFormatInfo"/>
                <rdf:rest>
                  <rdf:Description>
                    <rdf:first rdf:resource="http://purl.org/net/def/metashare#ImageFormatInfo"/>
                    <rdf:rest rdf:resource="http://www.w3.org/1999/02/22-rdf-syntax-ns#nil"/>
                  </rdf:Description>
                </rdf:rest>
              </rdf:Description>
            </rdf:rest>
          </rdf:Description>
        </owl:unionOf>
      </owl:Class>
    </rdfs:domain>
    <rdfs:range rdf:resource="http://www.w3.org/2001/XMLSchema#boolean"/>
  </owl:DatatypeProperty>
  <owl:ObjectProperty rdf:about="http://purl.org/net/def/metashare#compressionName">
    <rdfs:comment xml:lang="en">The name of the compression applied</rdfs:comment>
    <rdfs:domain>
      <owl:Class>
        <owl:unionOf>
          <rdf:Description>
            <rdf:first rdf:resource="http://purl.org/net/def/metashare#VideoFormatInfo"/>
            <rdf:rest>
              <rdf:Description>
                <rdf:first rdf:resource="http://purl.org/net/def/metashare#AudioFormatInfo"/>
                <rdf:rest>
                  <rdf:Description>
                    <rdf:first rdf:resource="http://purl.org/net/def/metashare#ImageFormatInfo"/>
                    <rdf:rest rdf:resource="http://www.w3.org/1999/02/22-rdf-syntax-ns#nil"/>
                  </rdf:Description>
                </rdf:rest>
              </rdf:Description>
            </rdf:rest>
          </rdf:Description>
        </owl:unionOf>
      </owl:Class>
    </rdfs:domain>
    <rdfs:range>
      <owl:Class>
        <owl:unionOf>
          <rdf:Description>
            <rdf:first rdf:resource="http://purl.org/net/def/metashare#CompressionName"/>
            <rdf:rest>
              <rdf:Description>
                <rdf:first rdf:resource="http://purl.org/net/def/metashare#CompressionName"/>
                <rdf:rest>
                  <rdf:Description>
                    <rdf:first rdf:resource="http://purl.org/net/def/metashare#CompressionName"/>
                    <rdf:rest rdf:resource="http://www.w3.org/1999/02/22-rdf-syntax-ns#nil"/>
                  </rdf:Description>
                </rdf:rest>
              </rdf:Description>
            </rdf:rest>
          </rdf:Description>
        </owl:unionOf>
      </owl:Class>
    </rdfs:range>
  </owl:ObjectProperty>
  <ns:CompatibleLexiconType rdf:about="http://purl.org/net/def/metashare#computationalLexicon">
    <rdf:type rdf:resource="http://purl.org/net/def/metashare#LexicalConceptualResourceType"/>
  </ns:CompatibleLexiconType>
  <ns:SizeUnit rdf:about="http://purl.org/net/def/metashare#concepts"/>
  <owl:ObjectProperty rdf:about="http://purl.org/net/def/metashare#conditionsOfUse">
    <rdfs:domain rdf:resource="http://purl.org/net/def/metashare#LicenceInfo"/>
    <rdfs:range rdf:resource="http://purl.org/net/def/metashare#ConditionsOfUse"/>
  </owl:ObjectProperty>
  <ns:RecordingEnvironment rdf:about="http://purl.org/net/def/metashare#conferenceRoom"/>
  <owl:ObjectProperty rdf:about="http://purl.org/net/def/metashare#conformanceToClassificationScheme">
    <rdfs:comment xml:lang="en">Specifies the external classification schemes</rdfs:comment>
    <rdfs:domain>
      <owl:Class>
        <owl:unionOf>
          <rdf:Description>
            <rdf:first rdf:resource="http://purl.org/net/def/metashare#VideoClassificationInfo"/>
            <rdf:rest>
              <rdf:Description>
                <rdf:first rdf:resource="http://purl.org/net/def/metashare#TextClassificationInfo"/>
                <rdf:rest>
                  <rdf:Description>
                    <rdf:first rdf:resource="http://purl.org/net/def/metashare#DomainInfo"/>
                    <rdf:rest>
                      <rdf:Description>
                        <rdf:first rdf:resource="http://purl.org/net/def/metashare#ImageClassificationInfo"/>
                        <rdf:rest>
                          <rdf:Description>
                            <rdf:first rdf:resource="http://purl.org/net/def/metashare#AudioClassificationInfo"/>
                            <rdf:rest rdf:resource="http://www.w3.org/1999/02/22-rdf-syntax-ns#nil"/>
                          </rdf:Description>
                        </rdf:rest>
                      </rdf:Description>
                    </rdf:rest>
                  </rdf:Description>
                </rdf:rest>
              </rdf:Description>
            </rdf:rest>
          </rdf:Description>
        </owl:unionOf>
      </owl:Class>
    </rdfs:domain>
    <rdfs:range>
      <owl:Class>
        <owl:unionOf>
          <rdf:Description>
            <rdf:first rdf:resource="http://purl.org/net/def/metashare#ConformanceToClassificationScheme"/>
            <rdf:rest>
              <rdf:Description>
                <rdf:first rdf:resource="http://purl.org/net/def/metashare#ConformanceToClassificationScheme"/>
                <rdf:rest>
                  <rdf:Description>
                    <rdf:first rdf:resource="http://purl.org/net/def/metashare#ConformanceToClassificationScheme"/>
                    <rdf:rest>
                      <rdf:Description>
                        <rdf:first rdf:resource="http://purl.org/net/def/metashare#ConformanceToClassificationScheme"/>
                        <rdf:rest>
                          <rdf:Description>
                            <rdf:first rdf:resource="http://purl.org/net/def/metashare#ConformanceToClassificationScheme"/>
                            <rdf:rest rdf:resource="http://www.w3.org/1999/02/22-rdf-syntax-ns#nil"/>
                          </rdf:Description>
                        </rdf:rest>
                      </rdf:Description>
                    </rdf:rest>
                  </rdf:Description>
                </rdf:rest>
              </rdf:Description>
            </rdf:rest>
          </rdf:Description>
        </owl:unionOf>
      </owl:Class>
    </rdfs:range>
  </owl:ObjectProperty>
  <owl:ObjectProperty rdf:about="http://purl.org/net/def/metashare#conformanceToStandardsBestPractices">
    <rdfs:comment xml:lang="en">Specifies the standards or the best practices to which the tagset used for the annotation conforms </rdfs:comment>
    <rdfs:domain>
      <owl:Class>
        <owl:unionOf>
          <rdf:Description>
            <rdf:first rdf:resource="http://purl.org/net/def/metashare#InputInfo"/>
            <rdf:rest>
              <rdf:Description>
                <rdf:first rdf:resource="http://purl.org/net/def/metashare#AnnotationInfo"/>
                <rdf:rest>
                  <rdf:Description>
                    <rdf:first rdf:resource="http://purl.org/net/def/metashare#OutputInfo"/>
                    <rdf:rest rdf:resource="http://www.w3.org/1999/02/22-rdf-syntax-ns#nil"/>
                  </rdf:Description>
                </rdf:rest>
              </rdf:Description>
            </rdf:rest>
          </rdf:Description>
        </owl:unionOf>
      </owl:Class>
    </rdfs:domain>
    <rdfs:range>
      <owl:Class>
        <owl:unionOf>
          <rdf:Description>
            <rdf:first rdf:resource="http://purl.org/net/def/metashare#ConformanceToStandardsBestPractices"/>
            <rdf:rest>
              <rdf:Description>
                <rdf:first rdf:resource="http://purl.org/net/def/metashare#ConformanceToStandardsBestPractices"/>
                <rdf:rest>
                  <rdf:Description>
                    <rdf:first rdf:resource="http://purl.org/net/def/metashare#ConformanceToStandardsBestPractices"/>
                    <rdf:rest rdf:resource="http://www.w3.org/1999/02/22-rdf-syntax-ns#nil"/>
                  </rdf:Description>
                </rdf:rest>
              </rdf:Description>
            </rdf:rest>
          </rdf:Description>
        </owl:unionOf>
      </owl:Class>
    </rdfs:range>
  </owl:ObjectProperty>
  <ns:ValidationType rdf:about="http://purl.org/net/def/metashare#content"/>
  <ns:UseNLPSpecific rdf:about="http://purl.org/net/def/metashare#contradictionDetection"/>
  <owl:ObjectProperty rdf:about="http://purl.org/net/def/metashare#conversationalType">
    <rdfs:comment xml:lang="en">Specifies the conversational type of the resource</rdfs:comment>
    <rdfs:domain>
      <owl:Class>
        <owl:unionOf>
          <rdf:Description>
            <rdf:first rdf:resource="http://purl.org/net/def/metashare#CorpusVideoInfo"/>
            <rdf:rest>
              <rdf:Description>
                <rdf:first rdf:resource="http://purl.org/net/def/metashare#CorpusAudioInfo"/>
                <rdf:rest rdf:resource="http://www.w3.org/1999/02/22-rdf-syntax-ns#nil"/>
              </rdf:Description>
            </rdf:rest>
          </rdf:Description>
        </owl:unionOf>
      </owl:Class>
    </rdfs:domain>
    <rdfs:range>
      <owl:Class>
        <owl:unionOf>
          <rdf:Description>
            <rdf:first rdf:resource="http://purl.org/net/def/metashare#ConversationalType"/>
            <rdf:rest>
              <rdf:Description>
                <rdf:first rdf:resource="http://purl.org/net/def/metashare#ConversationalType"/>
                <rdf:rest rdf:resource="http://www.w3.org/1999/02/22-rdf-syntax-ns#nil"/>
              </rdf:Description>
            </rdf:rest>
          </rdf:Description>
        </owl:unionOf>
      </owl:Class>
    </rdfs:range>
  </owl:ObjectProperty>
  <ns:GrammaticalPhenomenaCoverage rdf:about="http://purl.org/net/def/metashare#coordination"/>
  <ns:UseNLPSpecific rdf:about="http://purl.org/net/def/metashare#coreferenceResolution"/>
  <ns:ResourceType rdf:about="http://purl.org/net/def/metashare#corpus"/>
  <owl:ObjectProperty rdf:about="http://purl.org/net/def/metashare#corpusAudioInfo">
    <rdfs:comment xml:lang="en">Groups together information on the audio module of a corpus</rdfs:comment>
    <rdfs:domain rdf:resource="http://purl.org/net/def/metashare#CorpusInfo"/>
    <rdfs:range rdf:resource="http://purl.org/net/def/metashare#CorpusAudioInfo"/>
    <rdfs:subPropertyOf rdf:resource="http://purl.org/net/def/metashare#corpusMediaPartInfo"/>
  </owl:ObjectProperty>
  <owl:ObjectProperty rdf:about="http://purl.org/net/def/metashare#corpusImageInfo">
    <rdfs:comment xml:lang="en">Groups together information on the image component of a resource</rdfs:comment>
    <rdfs:domain rdf:resource="http://purl.org/net/def/metashare#CorpusInfo"/>
    <rdfs:range rdf:resource="http://purl.org/net/def/metashare#CorpusImageInfo"/>
    <rdfs:subPropertyOf rdf:resource="http://purl.org/net/def/metashare#corpusMediaPartInfo"/>
  </owl:ObjectProperty>
  <owl:ObjectProperty rdf:about="http://purl.org/net/def/metashare#corpusInfo">
    <rdfs:comment xml:lang="en">Groups together information on corpora of all media types</rdfs:comment>
    <rdfs:domain rdf:resource="http://purl.org/net/def/metashare#LanguageResource"/>
    <rdfs:range rdf:resource="http://purl.org/net/def/metashare#CorpusInfo"/>
  </owl:ObjectProperty>
  <owl:ObjectProperty rdf:about="http://purl.org/net/def/metashare#corpusMediaPartInfo">
    <rdfs:domain rdf:resource="http://purl.org/net/def/metashare#CorpusInfo"/>
    <rdfs:range rdf:resource="http://purl.org/net/def/metashare#CorpusMediaPart"/>
    <rdfs:subPropertyOf rdf:resource="http://purl.org/net/def/metashare#mediaPartInfo"/>
  </owl:ObjectProperty>
  <owl:ObjectProperty rdf:about="http://purl.org/net/def/metashare#corpusTextInfo">
    <rdfs:comment xml:lang="en">Groups together information on the text component of a resource</rdfs:comment>
    <rdfs:domain rdf:resource="http://purl.org/net/def/metashare#CorpusInfo"/>
    <rdfs:range rdf:resource="http://purl.org/net/def/metashare#CorpusTextInfo"/>
    <rdfs:subPropertyOf rdf:resource="http://purl.org/net/def/metashare#corpusMediaPartInfo"/>
  </owl:ObjectProperty>
  <owl:ObjectProperty rdf:about="http://purl.org/net/def/metashare#corpusTextNgramInfo">
    <rdfs:comment xml:lang="en">Groups together information required for n-gram resources; information can be provided both as regards features drawn from the source corpus (e.g. language coverage, size, format, domains etc.) and features pertaining to the n-gram output itself (e.g. range of n-grams, type of item included, etc.)</rdfs:comment>
    <rdfs:domain rdf:resource="http://purl.org/net/def/metashare#CorpusInfo"/>
    <rdfs:range rdf:resource="http://purl.org/net/def/metashare#CorpusTextNgramInfo"/>
    <rdfs:subPropertyOf rdf:resource="http://purl.org/net/def/metashare#corpusMediaPartInfo"/>
  </owl:ObjectProperty>
  <owl:ObjectProperty rdf:about="http://purl.org/net/def/metashare#corpusTextNumericalInfo">
    <rdfs:comment xml:lang="en">Groups together information on the textNumerical component of a corpus. It is used basically for the textual representation of measurements and observations linked to sensorimotor recordings</rdfs:comment>
    <rdfs:domain rdf:resource="http://purl.org/net/def/metashare#CorpusInfo"/>
    <rdfs:range rdf:resource="http://purl.org/net/def/metashare#CorpusTextNumericalInfo"/>
    <rdfs:subPropertyOf rdf:resource="http://purl.org/net/def/metashare#corpusMediaPartInfo"/>
  </owl:ObjectProperty>
  <owl:ObjectProperty rdf:about="http://purl.org/net/def/metashare#corpusVideoInfo">
    <rdfs:comment xml:lang="en">Groups together information on the video component of a corpus</rdfs:comment>
    <rdfs:domain rdf:resource="http://purl.org/net/def/metashare#CorpusInfo"/>
    <rdfs:range rdf:resource="http://purl.org/net/def/metashare#CorpusVideoInfo"/>
    <rdfs:subPropertyOf rdf:resource="http://purl.org/net/def/metashare#corpusMediaPartInfo"/>
  </owl:ObjectProperty>
  <owl:DatatypeProperty rdf:about="http://purl.org/net/def/metashare#country">
    <rdfs:comment xml:lang="en">The name of the country mentioned in the postal address of a person or organization as defined in the list of values of ISO 3166</rdfs:comment>
    <rdfs:domain>
      <owl:Class>
        <owl:unionOf>
          <rdf:Description>
            <rdf:first rdf:resource="http://purl.org/net/def/metashare#Organization"/>
            <rdf:rest>
              <rdf:Description>
                <rdf:first rdf:resource="http://purl.org/net/def/metashare#Person"/>
                <rdf:rest rdf:resource="http://www.w3.org/1999/02/22-rdf-syntax-ns#nil"/>
              </rdf:Description>
            </rdf:rest>
          </rdf:Description>
        </owl:unionOf>
      </owl:Class>
    </rdfs:domain>
    <rdfs:range rdf:resource="http://www.w3.org/2001/XMLSchema#string"/>
  </owl:DatatypeProperty>
  <owl:DatatypeProperty rdf:about="http://purl.org/net/def/metashare#creationDetails">
    <rdfs:comment xml:lang="en">Provides additional information on the creation of a tool or service</rdfs:comment>
    <rdfs:domain rdf:resource="http://purl.org/net/def/metashare#ToolServiceInfo"/>
    <rdfs:range rdf:resource="http://www.w3.org/2001/XMLSchema#string"/>
  </owl:DatatypeProperty>
  <owl:DatatypeProperty rdf:about="http://purl.org/net/def/metashare#creationEndDate">
    <rdfs:comment xml:lang="en">The date in which the creation process was completed</rdfs:comment>
    <rdfs:domain rdf:resource="http://purl.org/net/def/metashare#LanguageResource"/>
    <rdfs:range rdf:resource="http://www.w3.org/2001/XMLSchema#date"/>
  </owl:DatatypeProperty>
  <owl:ObjectProperty rdf:about="http://purl.org/net/def/metashare#creationMode">
    <rdfs:comment xml:lang="en">Specifies whether the resource is created automatically or in a manual or interactive mode </rdfs:comment>
    <rdfs:domain>
      <owl:Class>
        <owl:unionOf>
          <rdf:Description>
            <rdf:first rdf:resource="http://purl.org/net/def/metashare#CorpusTextInfo"/>
            <rdf:rest>
              <rdf:Description>
                <rdf:first rdf:resource="http://purl.org/net/def/metashare#LexicalConceptualResourceInfo"/>
                <rdf:rest>
                  <rdf:Description>
                    <rdf:first rdf:resource="http://purl.org/net/def/metashare#CorpusVideoInfo"/>
                    <rdf:rest>
                      <rdf:Description>
                        <rdf:first rdf:resource="http://purl.org/net/def/metashare#CorpusAudioInfo"/>
                        <rdf:rest>
                          <rdf:Description>
                            <rdf:first rdf:resource="http://purl.org/net/def/metashare#LanguageDescriptionVideoInfo"/>
                            <rdf:rest>
                              <rdf:Description>
                                <rdf:first rdf:resource="http://purl.org/net/def/metashare#LanguageDescriptionImageInfo"/>
                                <rdf:rest>
                                  <rdf:Description>
                                    <rdf:first rdf:resource="http://purl.org/net/def/metashare#CorpusTextNumericalInfo"/>
                                    <rdf:rest>
                                      <rdf:Description>
                                        <rdf:first rdf:resource="http://purl.org/net/def/metashare#CorpusTextNgramInfo"/>
                                        <rdf:rest>
                                          <rdf:Description>
                                            <rdf:first rdf:resource="http://purl.org/net/def/metashare#LanguageDescriptionTextInfo"/>
                                            <rdf:rest>
                                              <rdf:Description>
                                                <rdf:first rdf:resource="http://purl.org/net/def/metashare#CorpusImageInfo"/>
                                                <rdf:rest>
                                                  <rdf:Description>
                                                    <rdf:first rdf:resource="http://purl.org/net/def/metashare#LanguageDescriptionInfo"/>
                                                    <rdf:rest rdf:resource="http://www.w3.org/1999/02/22-rdf-syntax-ns#nil"/>
                                                  </rdf:Description>
                                                </rdf:rest>
                                              </rdf:Description>
                                            </rdf:rest>
                                          </rdf:Description>
                                        </rdf:rest>
                                      </rdf:Description>
                                    </rdf:rest>
                                  </rdf:Description>
                                </rdf:rest>
                              </rdf:Description>
                            </rdf:rest>
                          </rdf:Description>
                        </rdf:rest>
                      </rdf:Description>
                    </rdf:rest>
                  </rdf:Description>
                </rdf:rest>
              </rdf:Description>
            </rdf:rest>
          </rdf:Description>
        </owl:unionOf>
      </owl:Class>
    </rdfs:domain>
    <rdfs:range>
      <owl:Class>
        <owl:unionOf>
          <rdf:Description>
            <rdf:first rdf:resource="http://purl.org/net/def/metashare#CreationMode"/>
            <rdf:rest>
              <rdf:Description>
                <rdf:first rdf:resource="http://purl.org/net/def/metashare#CreationMode"/>
                <rdf:rest>
                  <rdf:Description>
                    <rdf:first rdf:resource="http://purl.org/net/def/metashare#CreationMode"/>
                    <rdf:rest>
                      <rdf:Description>
                        <rdf:first rdf:resource="http://purl.org/net/def/metashare#CreationMode"/>
                        <rdf:rest>
                          <rdf:Description>
                            <rdf:first rdf:resource="http://purl.org/net/def/metashare#CreationMode"/>
                            <rdf:rest>
                              <rdf:Description>
                                <rdf:first rdf:resource="http://purl.org/net/def/metashare#CreationMode"/>
                                <rdf:rest>
                                  <rdf:Description>
                                    <rdf:first rdf:resource="http://purl.org/net/def/metashare#CreationMode"/>
                                    <rdf:rest>
                                      <rdf:Description>
                                        <rdf:first rdf:resource="http://purl.org/net/def/metashare#CreationMode"/>
                                        <rdf:rest>
                                          <rdf:Description>
                                            <rdf:first rdf:resource="http://purl.org/net/def/metashare#CreationMode"/>
                                            <rdf:rest>
                                              <rdf:Description>
                                                <rdf:first rdf:resource="http://purl.org/net/def/metashare#CreationMode"/>
                                                <rdf:rest>
                                                  <rdf:Description>
                                                    <rdf:first rdf:resource="http://purl.org/net/def/metashare#CreationMode"/>
                                                    <rdf:rest rdf:resource="http://www.w3.org/1999/02/22-rdf-syntax-ns#nil"/>
                                                  </rdf:Description>
                                                </rdf:rest>
                                              </rdf:Description>
                                            </rdf:rest>
                                          </rdf:Description>
                                        </rdf:rest>
                                      </rdf:Description>
                                    </rdf:rest>
                                  </rdf:Description>
                                </rdf:rest>
                              </rdf:Description>
                            </rdf:rest>
                          </rdf:Description>
                        </rdf:rest>
                      </rdf:Description>
                    </rdf:rest>
                  </rdf:Description>
                </rdf:rest>
              </rdf:Description>
            </rdf:rest>
          </rdf:Description>
        </owl:unionOf>
      </owl:Class>
    </rdfs:range>
  </owl:ObjectProperty>
  <owl:DatatypeProperty rdf:about="http://purl.org/net/def/metashare#creationModeDetails">
    <rdfs:comment xml:lang="en">Provides further information on the creation methods and processes</rdfs:comment>
    <rdfs:domain>
      <owl:Class>
        <owl:unionOf>
          <rdf:Description>
            <rdf:first rdf:resource="http://purl.org/net/def/metashare#LexicalConceptualResourceInfo"/>
            <rdf:rest>
              <rdf:Description>
                <rdf:first rdf:resource="http://purl.org/net/def/metashare#LanguageDescriptionTextInfo"/>
                <rdf:rest>
                  <rdf:Description>
                    <rdf:first rdf:resource="http://purl.org/net/def/metashare#LanguageDescriptionImageInfo"/>
                    <rdf:rest>
                      <rdf:Description>
                        <rdf:first rdf:resource="http://purl.org/net/def/metashare#CorpusTextNgramInfo"/>
                        <rdf:rest>
                          <rdf:Description>
                            <rdf:first rdf:resource="http://purl.org/net/def/metashare#LanguageDescriptionVideoInfo"/>
                            <rdf:rest>
                              <rdf:Description>
                                <rdf:first rdf:resource="http://purl.org/net/def/metashare#CorpusTextInfo"/>
                                <rdf:rest>
                                  <rdf:Description>
                                    <rdf:first rdf:resource="http://purl.org/net/def/metashare#CorpusVideoInfo"/>
                                    <rdf:rest>
                                      <rdf:Description>
                                        <rdf:first rdf:resource="http://purl.org/net/def/metashare#LanguageDescriptionInfo"/>
                                        <rdf:rest>
                                          <rdf:Description>
                                            <rdf:first rdf:resource="http://purl.org/net/def/metashare#CorpusImageInfo"/>
                                            <rdf:rest>
                                              <rdf:Description>
                                                <rdf:first rdf:resource="http://purl.org/net/def/metashare#CorpusTextNumericalInfo"/>
                                                <rdf:rest>
                                                  <rdf:Description>
                                                    <rdf:first rdf:resource="http://purl.org/net/def/metashare#CorpusAudioInfo"/>
                                                    <rdf:rest rdf:resource="http://www.w3.org/1999/02/22-rdf-syntax-ns#nil"/>
                                                  </rdf:Description>
                                                </rdf:rest>
                                              </rdf:Description>
                                            </rdf:rest>
                                          </rdf:Description>
                                        </rdf:rest>
                                      </rdf:Description>
                                    </rdf:rest>
                                  </rdf:Description>
                                </rdf:rest>
                              </rdf:Description>
                            </rdf:rest>
                          </rdf:Description>
                        </rdf:rest>
                      </rdf:Description>
                    </rdf:rest>
                  </rdf:Description>
                </rdf:rest>
              </rdf:Description>
            </rdf:rest>
          </rdf:Description>
        </owl:unionOf>
      </owl:Class>
    </rdfs:domain>
    <rdfs:range rdf:resource="http://www.w3.org/2001/XMLSchema#string"/>
  </owl:DatatypeProperty>
  <owl:DatatypeProperty rdf:about="http://purl.org/net/def/metashare#creationStartDate">
    <rdfs:comment xml:lang="en">The date in which the creation process was started</rdfs:comment>
    <rdfs:domain rdf:resource="http://purl.org/net/def/metashare#LanguageResource"/>
    <rdfs:range rdf:resource="http://www.w3.org/2001/XMLSchema#date"/>
  </owl:DatatypeProperty>
  <owl:DatatypeProperty rdf:about="http://purl.org/net/def/metashare#creationTool">
    <rdfs:comment xml:lang="en">The name, the identifier or the url of the tool used in the creation process</rdfs:comment>
    <rdfs:domain>
      <owl:Class>
        <owl:unionOf>
          <rdf:Description>
            <rdf:first rdf:resource="http://purl.org/net/def/metashare#LanguageDescriptionVideoInfo"/>
            <rdf:rest>
              <rdf:Description>
                <rdf:first rdf:resource="http://purl.org/net/def/metashare#CorpusTextInfo"/>
                <rdf:rest>
                  <rdf:Description>
                    <rdf:first rdf:resource="http://purl.org/net/def/metashare#CorpusTextNgramInfo"/>
                    <rdf:rest>
                      <rdf:Description>
                        <rdf:first rdf:resource="http://purl.org/net/def/metashare#LexicalConceptualResourceInfo"/>
                        <rdf:rest>
                          <rdf:Description>
                            <rdf:first rdf:resource="http://purl.org/net/def/metashare#CorpusAudioInfo"/>
                            <rdf:rest>
                              <rdf:Description>
                                <rdf:first rdf:resource="http://purl.org/net/def/metashare#LanguageDescriptionInfo"/>
                                <rdf:rest>
                                  <rdf:Description>
                                    <rdf:first rdf:resource="http://purl.org/net/def/metashare#CorpusTextNumericalInfo"/>
                                    <rdf:rest>
                                      <rdf:Description>
                                        <rdf:first rdf:resource="http://purl.org/net/def/metashare#LanguageDescriptionTextInfo"/>
                                        <rdf:rest>
                                          <rdf:Description>
                                            <rdf:first rdf:resource="http://purl.org/net/def/metashare#CorpusVideoInfo"/>
                                            <rdf:rest>
                                              <rdf:Description>
                                                <rdf:first rdf:resource="http://purl.org/net/def/metashare#CorpusImageInfo"/>
                                                <rdf:rest>
                                                  <rdf:Description>
                                                    <rdf:first rdf:resource="http://purl.org/net/def/metashare#LanguageDescriptionImageInfo"/>
                                                    <rdf:rest rdf:resource="http://www.w3.org/1999/02/22-rdf-syntax-ns#nil"/>
                                                  </rdf:Description>
                                                </rdf:rest>
                                              </rdf:Description>
                                            </rdf:rest>
                                          </rdf:Description>
                                        </rdf:rest>
                                      </rdf:Description>
                                    </rdf:rest>
                                  </rdf:Description>
                                </rdf:rest>
                              </rdf:Description>
                            </rdf:rest>
                          </rdf:Description>
                        </rdf:rest>
                      </rdf:Description>
                    </rdf:rest>
                  </rdf:Description>
                </rdf:rest>
              </rdf:Description>
            </rdf:rest>
          </rdf:Description>
        </owl:unionOf>
      </owl:Class>
    </rdfs:domain>
    <rdfs:range rdf:resource="http://www.w3.org/2001/XMLSchema#string"/>
  </owl:DatatypeProperty>
  <ns:SpeechItems rdf:about="http://purl.org/net/def/metashare#creditCardNumbers"/>
  <ns:AudioQualityMeasuresIncluded rdf:about="http://purl.org/net/def/metashare#crossTalk"/>
  <ns:SceneIllumination rdf:about="http://purl.org/net/def/metashare#daylight"/>
  <ns:LinguisticInformation rdf:about="http://purl.org/net/def/metashare#definition-gloss"/>
  <ns:Task rdf:about="http://purl.org/net/def/metashare#definitionsParsing"/>
  <owl:DatatypeProperty rdf:about="http://purl.org/net/def/metashare#departmentName">
    <rdfs:comment xml:lang="en">The name of the department or unit (e.g. specific university faculty/department, department/unit of a research organization or private company etc.)</rdfs:comment>
    <rdfs:domain rdf:resource="http://purl.org/net/def/metashare#Organization"/>
    <rdfs:range rdf:resource="http://www.w3.org/1999/02/22-rdf-syntax-ns#langString"/>
  </owl:DatatypeProperty>
  <ns:UseNLPSpecific rdf:about="http://purl.org/net/def/metashare#derivationalMorphologicalAnalysis"/>
  <owl:DatatypeProperty rdf:about="http://purl.org/net/def/metashare#derivedResource">
    <rdfs:comment xml:lang="en">The name, the identifier or the url of the outcome or product of the resource.</rdfs:comment>
    <rdfs:domain rdf:resource="http://purl.org/net/def/metashare#ActualUseInfo"/>
    <rdfs:range rdf:resource="http://www.w3.org/2001/XMLSchema#string"/>
  </owl:DatatypeProperty>
  <ns:EvaluationLevel rdf:about="http://purl.org/net/def/metashare#diagnostic"/>
  <ns:LanguageVarietyType rdf:about="http://purl.org/net/def/metashare#dialect"/>
  <owl:DatatypeProperty rdf:about="http://purl.org/net/def/metashare#dialectAccent">
    <rdfs:comment xml:lang="en">Provides information on the dialect of the participant</rdfs:comment>
    <rdfs:domain rdf:resource="http://purl.org/net/def/metashare#ParticipantInfo"/>
    <rdfs:range rdf:resource="http://www.w3.org/1999/02/22-rdf-syntax-ns#langString"/>
  </owl:DatatypeProperty>
  <owl:DatatypeProperty rdf:about="http://purl.org/net/def/metashare#dialectAccentOfPersons">
    <rdfs:comment xml:lang="en">Provides information on the dialect of the group of participants</rdfs:comment>
    <rdfs:domain>
      <owl:Class>
        <owl:unionOf>
          <rdf:Description>
            <rdf:first rdf:resource="http://purl.org/net/def/metashare#CorpusImageInfo"/>
            <rdf:rest>
              <rdf:Description>
                <rdf:first rdf:resource="http://purl.org/net/def/metashare#CorpusTextNumericalInfo"/>
                <rdf:rest>
                  <rdf:Description>
                    <rdf:first rdf:resource="http://purl.org/net/def/metashare#CorpusVideoInfo"/>
                    <rdf:rest>
                      <rdf:Description>
                        <rdf:first rdf:resource="http://purl.org/net/def/metashare#CorpusAudioInfo"/>
                        <rdf:rest rdf:resource="http://www.w3.org/1999/02/22-rdf-syntax-ns#nil"/>
                      </rdf:Description>
                    </rdf:rest>
                  </rdf:Description>
                </rdf:rest>
              </rdf:Description>
            </rdf:rest>
          </rdf:Description>
        </owl:unionOf>
      </owl:Class>
    </rdfs:domain>
    <rdfs:range rdf:resource="http://www.w3.org/2001/XMLSchema#string"/>
  </owl:DatatypeProperty>
  <ns:ConversationalType rdf:about="http://purl.org/net/def/metashare#dialogue"/>
  <ns:SegmentationLevel rdf:about="http://purl.org/net/def/metashare#diphone"/>
  <ns:SizeUnit rdf:about="http://purl.org/net/def/metashare#diphones"/>
  <ns:UseNLPSpecific rdf:about="http://purl.org/net/def/metashare#discourseAnalysis"/>
  <ns:DiscourseAnnotation rdf:about="http://purl.org/net/def/metashare#discourseAnnotation">
    <rdf:type rdf:resource="http://purl.org/net/def/metashare#AnnotationType"/>
  </ns:DiscourseAnnotation>
  <ns:DiscourseAnnotation rdf:about="http://purl.org/net/def/metashare#discourseAnnotation-audienceReactions">
    <rdf:type rdf:resource="http://purl.org/net/def/metashare#AnnotationType"/>
  </ns:DiscourseAnnotation>
  <ns:DiscourseAnnotation rdf:about="http://purl.org/net/def/metashare#discourseAnnotation-coreference">
    <rdf:type rdf:resource="http://purl.org/net/def/metashare#AnnotationType"/>
  </ns:DiscourseAnnotation>
  <ns:DiscourseAnnotation rdf:about="http://purl.org/net/def/metashare#discourseAnnotation-dialogueActs">
    <rdf:type rdf:resource="http://purl.org/net/def/metashare#AnnotationType"/>
  </ns:DiscourseAnnotation>
  <ns:DiscourseAnnotation rdf:about="http://purl.org/net/def/metashare#discourseAnnotation-discourseRelations">
    <rdf:type rdf:resource="http://purl.org/net/def/metashare#AnnotationType"/>
  </ns:DiscourseAnnotation>
  <ns:AnnotatedElements rdf:about="http://purl.org/net/def/metashare#discourseMarkers"/>
  <owl:DatatypeProperty rdf:about="http://purl.org/net/def/metashare#distractors">
    <rdfs:comment xml:lang="en">Any distractors visible in the resource</rdfs:comment>
    <rdfs:domain rdf:resource="http://purl.org/net/def/metashare#DynamicElementInfo"/>
    <rdfs:range rdf:resource="http://www.w3.org/2001/XMLSchema#string"/>
  </owl:DatatypeProperty>
  <owl:ObjectProperty rdf:about="http://purl.org/net/def/metashare#distributionAccessMedium">
    <rdfs:comment xml:lang="en">Specifies the medium (channel) used for delivery or providing access to the resource</rdfs:comment>
    <rdfs:comment xml:lang="en">Specifies the medium (channel) used for delivery or providing access to the resource.</rdfs:comment>
    <rdfs:domain rdf:resource="http://purl.org/net/def/metashare#LanguageResource"/>
    <rdfs:range rdf:resource="http://purl.org/net/def/metashare#DistributionAccessMedium"/>
  </owl:ObjectProperty>
  <owl:ObjectProperty rdf:about="http://purl.org/net/def/metashare#distributionRightsHolder">
    <rdfs:comment xml:lang="en">Groups information on a person or an organization that holds the distribution rights. The range and scope of distribution rights is defined in the distribution agreement. The distributor in most cases only has a limited licence to distribute the work and collect royalties on behalf of the licensor or the IPR holder and cannot give to any recipient of the work permissions that exceed the scope of the distribution agreement (e.g. to allow uses of the work that are not defined in the distribution agreement)</rdfs:comment>
    <rdfs:comment xml:lang="en">Identifies a person or an organization that holds the distribution rights. The range and scope of distribution rights is defined in the distribution agreement. The distributor in most cases only has a limited licence to distribute the work and collect royalties on behalf of the licensor or the IPR holder and cannot give to any recipient of the work permissions that exceed the scope of the distribution agreement (e.g. to allow uses of the work that are not defined in the distribution agreement)</rdfs:comment>
    <rdfs:domain rdf:resource="http://purl.org/net/def/metashare#LicenceInfo"/>
    <rdfs:range rdf:resource="http://purl.org/net/def/metashare#Actor"/>
  </owl:ObjectProperty>
  <ns:UseNLPSpecific rdf:about="http://purl.org/net/def/metashare#documentClassification"/>
  <owl:ObjectProperty rdf:about="http://purl.org/net/def/metashare#documentInfo">
    <rdfs:domain rdf:resource="http://purl.org/net/def/metashare#Documentation"/>
    <rdfs:range rdf:resource="http://purl.org/net/def/metashare#DocumentInfo"/>
  </owl:ObjectProperty>
  <owl:DatatypeProperty rdf:about="http://purl.org/net/def/metashare#documentUnstructured">
    <rdfs:comment xml:lang="en">Used either as a free text description or as an unstructured (free form) presentation of a bibliographic record; alternative to the structured presentation of a document (cf. documentInfo)</rdfs:comment>
    <rdfs:domain rdf:resource="http://purl.org/net/def/metashare#Documentation"/>
    <rdfs:range rdf:resource="http://www.w3.org/2001/XMLSchema#string"/>
  </owl:DatatypeProperty>
  <owl:ObjectProperty rdf:about="http://purl.org/net/def/metashare#documentation">
    <rdfs:comment xml:lang="en">Refers to papers, manuals, reports etc. describing the resource</rdfs:comment>
    <rdfs:domain rdf:resource="http://purl.org/net/def/metashare#LanguageResource"/>
    <rdfs:range rdf:resource="http://purl.org/net/def/metashare#Documentation"/>
  </owl:ObjectProperty>
  <owl:DatatypeProperty rdf:about="http://purl.org/net/def/metashare#domain">
    <rdfs:comment xml:lang="en">Specifies the application domain of the resource or the tool/service</rdfs:comment>
    <rdfs:domain rdf:resource="http://purl.org/net/def/metashare#DomainInfo"/>
    <rdfs:range rdf:resource="http://www.w3.org/2001/XMLSchema#string"/>
  </owl:DatatypeProperty>
  <owl:ObjectProperty rdf:about="http://purl.org/net/def/metashare#domainInfo">
    <rdfs:comment xml:lang="en">Groups together information on domains represented in the resource; can be repeated for parts of the resource with distinct domain</rdfs:comment>
    <rdfs:domain>
      <owl:Class>
        <owl:unionOf>
          <rdf:Description>
            <rdf:first rdf:resource="http://purl.org/net/def/metashare#CorpusAudioInfo"/>
            <rdf:rest>
              <rdf:Description>
                <rdf:first rdf:resource="http://purl.org/net/def/metashare#CorpusImageInfo"/>
                <rdf:rest>
                  <rdf:Description>
                    <rdf:first rdf:resource="http://purl.org/net/def/metashare#LanguageDescriptionTextInfo"/>
                    <rdf:rest>
                      <rdf:Description>
                        <rdf:first rdf:resource="http://purl.org/net/def/metashare#CorpusTextNgramInfo"/>
                        <rdf:rest>
                          <rdf:Description>
                            <rdf:first rdf:resource="http://purl.org/net/def/metashare#LexicalConceptualResourceImageInfo"/>
                            <rdf:rest>
                              <rdf:Description>
                                <rdf:first rdf:resource="http://purl.org/net/def/metashare#LexicalConceptualResourceVideoInfo"/>
                                <rdf:rest>
                                  <rdf:Description>
                                    <rdf:first rdf:resource="http://purl.org/net/def/metashare#LanguageDescriptionVideoInfo"/>
                                    <rdf:rest>
                                      <rdf:Description>
                                        <rdf:first rdf:resource="http://purl.org/net/def/metashare#LexicalConceptualResourceTextInfo"/>
                                        <rdf:rest>
                                          <rdf:Description>
                                            <rdf:first rdf:resource="http://purl.org/net/def/metashare#LexicalConceptualResourceAudioInfo"/>
                                            <rdf:rest>
                                              <rdf:Description>
                                                <rdf:first rdf:resource="http://purl.org/net/def/metashare#CorpusVideoInfo"/>
                                                <rdf:rest>
                                                  <rdf:Description>
                                                    <rdf:first rdf:resource="http://purl.org/net/def/metashare#CorpusTextInfo"/>
                                                    <rdf:rest>
                                                      <rdf:Description>
                                                        <rdf:first rdf:resource="http://purl.org/net/def/metashare#LanguageDescriptionImageInfo"/>
                                                        <rdf:rest rdf:resource="http://www.w3.org/1999/02/22-rdf-syntax-ns#nil"/>
                                                      </rdf:Description>
                                                    </rdf:rest>
                                                  </rdf:Description>
                                                </rdf:rest>
                                              </rdf:Description>
                                            </rdf:rest>
                                          </rdf:Description>
                                        </rdf:rest>
                                      </rdf:Description>
                                    </rdf:rest>
                                  </rdf:Description>
                                </rdf:rest>
                              </rdf:Description>
                            </rdf:rest>
                          </rdf:Description>
                        </rdf:rest>
                      </rdf:Description>
                    </rdf:rest>
                  </rdf:Description>
                </rdf:rest>
              </rdf:Description>
            </rdf:rest>
          </rdf:Description>
        </owl:unionOf>
      </owl:Class>
    </rdfs:domain>
    <rdfs:range>
      <owl:Class>
        <owl:unionOf>
          <rdf:Description>
            <rdf:first rdf:resource="http://purl.org/net/def/metashare#DomainInfo"/>
            <rdf:rest>
              <rdf:Description>
                <rdf:first rdf:resource="http://purl.org/net/def/metashare#DomainInfo"/>
                <rdf:rest>
                  <rdf:Description>
                    <rdf:first rdf:resource="http://purl.org/net/def/metashare#DomainInfo"/>
                    <rdf:rest>
                      <rdf:Description>
                        <rdf:first rdf:resource="http://purl.org/net/def/metashare#DomainInfo"/>
                        <rdf:rest>
                          <rdf:Description>
                            <rdf:first rdf:resource="http://purl.org/net/def/metashare#DomainInfo"/>
                            <rdf:rest>
                              <rdf:Description>
                                <rdf:first rdf:resource="http://purl.org/net/def/metashare#DomainInfo"/>
                                <rdf:rest>
                                  <rdf:Description>
                                    <rdf:first rdf:resource="http://purl.org/net/def/metashare#DomainInfo"/>
                                    <rdf:rest>
                                      <rdf:Description>
                                        <rdf:first rdf:resource="http://purl.org/net/def/metashare#DomainInfo"/>
                                        <rdf:rest>
                                          <rdf:Description>
                                            <rdf:first rdf:resource="http://purl.org/net/def/metashare#DomainInfo"/>
                                            <rdf:rest>
                                              <rdf:Description>
                                                <rdf:first rdf:resource="http://purl.org/net/def/metashare#DomainInfo"/>
                                                <rdf:rest>
                                                  <rdf:Description>
                                                    <rdf:first rdf:resource="http://purl.org/net/def/metashare#DomainInfo"/>
                                                    <rdf:rest>
                                                      <rdf:Description>
                                                        <rdf:first rdf:resource="http://purl.org/net/def/metashare#DomainInfo"/>
                                                        <rdf:rest rdf:resource="http://www.w3.org/1999/02/22-rdf-syntax-ns#nil"/>
                                                      </rdf:Description>
                                                    </rdf:rest>
                                                  </rdf:Description>
                                                </rdf:rest>
                                              </rdf:Description>
                                            </rdf:rest>
                                          </rdf:Description>
                                        </rdf:rest>
                                      </rdf:Description>
                                    </rdf:rest>
                                  </rdf:Description>
                                </rdf:rest>
                              </rdf:Description>
                            </rdf:rest>
                          </rdf:Description>
                        </rdf:rest>
                      </rdf:Description>
                    </rdf:rest>
                  </rdf:Description>
                </rdf:rest>
              </rdf:Description>
            </rdf:rest>
          </rdf:Description>
        </owl:unionOf>
      </owl:Class>
    </rdfs:range>
  </owl:ObjectProperty>
  <ns:DistributionAccessMedium rdf:about="http://purl.org/net/def/metashare#downloadable"/>
  <owl:DatatypeProperty rdf:about="http://purl.org/net/def/metashare#duration"/>
  <owl:DatatypeProperty rdf:about="http://purl.org/net/def/metashare#durationOfAudioInfo">
    <rdfs:comment xml:lang="en">Groups together information on the size of audio parts; for silences, music etc.</rdfs:comment>
    <rdfs:domain rdf:resource="http://purl.org/net/def/metashare#AudioSizeInfo"/>
    <rdfs:range rdf:resource="http://www.w3.org/2001/XMLSchema#int"/>
    <rdfs:subPropertyOf rdf:resource="http://purl.org/net/def/metashare#duration"/>
  </owl:DatatypeProperty>
  <owl:ObjectProperty rdf:about="http://purl.org/net/def/metashare#durationOfAudioInfoUnit">
    <rdfs:domain rdf:resource="http://purl.org/net/def/metashare#AudioSizeInfo"/>
    <rdfs:range rdf:resource="http://purl.org/net/def/metashare#DurationOfAudioInfoUnit"/>
    <rdfs:subPropertyOf rdf:resource="http://purl.org/net/def/metashare#durationUnit"/>
  </owl:ObjectProperty>
  <owl:DatatypeProperty rdf:about="http://purl.org/net/def/metashare#durationOfEffectiveSpeechInfo">
    <rdfs:comment xml:lang="en">Groups together information on the duration of effective speech</rdfs:comment>
    <rdfs:domain rdf:resource="http://purl.org/net/def/metashare#AudioSizeInfo"/>
    <rdfs:range rdf:resource="http://www.w3.org/2001/XMLSchema#int"/>
    <rdfs:subPropertyOf rdf:resource="http://purl.org/net/def/metashare#duration"/>
  </owl:DatatypeProperty>
  <owl:ObjectProperty rdf:about="http://purl.org/net/def/metashare#durationOfEffectiveSpeechInfoUnit">
    <rdfs:domain rdf:resource="http://purl.org/net/def/metashare#AudioSizeInfo"/>
    <rdfs:range rdf:resource="http://purl.org/net/def/metashare#DurationOfEffectiveSpeechInfoUnit"/>
    <rdfs:subPropertyOf rdf:resource="http://purl.org/net/def/metashare#durationUnit"/>
  </owl:ObjectProperty>
  <owl:DatatypeProperty rdf:about="http://purl.org/net/def/metashare#durationUnit"/>
  <ns:RecordingDeviceType rdf:about="http://purl.org/net/def/metashare#dv"/>
  <owl:ObjectProperty rdf:about="http://purl.org/net/def/metashare#dynamicElementInfo">
    <rdfs:comment xml:lang="en">Groups information on the dynamic elements that are represented in the video part of the resource</rdfs:comment>
    <rdfs:domain>
      <owl:Class>
        <owl:unionOf>
          <rdf:Description>
            <rdf:first rdf:resource="http://purl.org/net/def/metashare#LanguageDescriptionVideoInfo"/>
            <rdf:rest>
              <rdf:Description>
                <rdf:first rdf:resource="http://purl.org/net/def/metashare#CorpusVideoInfo"/>
                <rdf:rest>
                  <rdf:Description>
                    <rdf:first rdf:resource="http://purl.org/net/def/metashare#LexicalConceptualResourceVideoInfo"/>
                    <rdf:rest rdf:resource="http://www.w3.org/1999/02/22-rdf-syntax-ns#nil"/>
                  </rdf:Description>
                </rdf:rest>
              </rdf:Description>
            </rdf:rest>
          </rdf:Description>
        </owl:unionOf>
      </owl:Class>
    </rdfs:domain>
    <rdfs:range>
      <owl:Class>
        <owl:unionOf>
          <rdf:Description>
            <rdf:first rdf:resource="http://purl.org/net/def/metashare#DynamicElementInfo"/>
            <rdf:rest>
              <rdf:Description>
                <rdf:first rdf:resource="http://purl.org/net/def/metashare#DynamicElementInfo"/>
                <rdf:rest>
                  <rdf:Description>
                    <rdf:first rdf:resource="http://purl.org/net/def/metashare#DynamicElementInfo"/>
                    <rdf:rest rdf:resource="http://www.w3.org/1999/02/22-rdf-syntax-ns#nil"/>
                  </rdf:Description>
                </rdf:rest>
              </rdf:Description>
            </rdf:rest>
          </rdf:Description>
        </owl:unionOf>
      </owl:Class>
    </rdfs:range>
  </owl:ObjectProperty>
  <ns:ConditionsOfUse rdf:about="http://purl.org/net/def/metashare#education">
    <rdf:type rdf:resource="http://www.w3.org/2002/07/owl#NamedIndividual"/>
    <rdfs:comment xml:lang="en">Education refers to a kind of 'ConditionsOfUse' imposed by the licence; the resource can only be used for educational purposes.</rdfs:comment>
    <rdfs:label xml:lang="en">Education</rdfs:label>
  </ns:ConditionsOfUse>
  <owl:DatatypeProperty rdf:about="http://purl.org/net/def/metashare#educationLevel">
    <rdfs:comment xml:lang="en">Provides information on the education level of the participant</rdfs:comment>
    <rdfs:domain rdf:resource="http://purl.org/net/def/metashare#ParticipantInfo"/>
    <rdfs:range rdf:resource="http://www.w3.org/2001/XMLSchema#string"/>
  </owl:DatatypeProperty>
  <ns:AgeGroup rdf:about="http://purl.org/net/def/metashare#elderly">
    <rdf:type rdf:resource="http://purl.org/net/def/metashare#AgeOfPersons"/>
  </ns:AgeGroup>
  <ns:SizeUnit rdf:about="http://purl.org/net/def/metashare#elements"/>
  <ns:Naturality rdf:about="http://purl.org/net/def/metashare#elicited"/>
  <owl:DatatypeProperty rdf:about="http://purl.org/net/def/metashare#email">
    <rdfs:comment xml:lang="en">The email address of a person or an organization</rdfs:comment>
    <rdfs:domain>
      <owl:Class>
        <owl:unionOf>
          <rdf:Description>
            <rdf:first rdf:resource="http://purl.org/net/def/metashare#Organization"/>
            <rdf:rest>
              <rdf:Description>
                <rdf:first rdf:resource="http://purl.org/net/def/metashare#Person"/>
                <rdf:rest rdf:resource="http://www.w3.org/1999/02/22-rdf-syntax-ns#nil"/>
              </rdf:Description>
            </rdf:rest>
          </rdf:Description>
        </owl:unionOf>
      </owl:Class>
    </rdfs:domain>
    <rdfs:range rdf:resource="http://www.w3.org/2001/XMLSchema#string"/>
  </owl:DatatypeProperty>
  <ns:CapturingDeviceType rdf:about="http://purl.org/net/def/metashare#embeddedMicrophone"/>
  <ns:UseNLPSpecific rdf:about="http://purl.org/net/def/metashare#emotionGeneration"/>
  <ns:UseNLPSpecific rdf:about="http://purl.org/net/def/metashare#emotionRecognition"/>
  <owl:ObjectProperty rdf:about="http://purl.org/net/def/metashare#encodingLevel">
    <rdfs:comment xml:lang="en">Information on the contents of the lexicalConceptualResource as regards the linguistic level of analysis</rdfs:comment>
    <rdfs:domain>
      <owl:Class>
        <owl:unionOf>
          <rdf:Description>
            <rdf:first rdf:resource="http://purl.org/net/def/metashare#LanguageDescriptionInfo"/>
            <rdf:rest>
              <rdf:Description>
                <rdf:first rdf:resource="http://purl.org/net/def/metashare#LexicalConceptualResourceInfo"/>
                <rdf:rest rdf:resource="http://www.w3.org/1999/02/22-rdf-syntax-ns#nil"/>
              </rdf:Description>
            </rdf:rest>
          </rdf:Description>
        </owl:unionOf>
      </owl:Class>
    </rdfs:domain>
    <rdfs:range>
      <owl:Class>
        <owl:unionOf>
          <rdf:Description>
            <rdf:first rdf:resource="http://purl.org/net/def/metashare#EncodingLevel"/>
            <rdf:rest>
              <rdf:Description>
                <rdf:first rdf:resource="http://purl.org/net/def/metashare#EncodingLevel"/>
                <rdf:rest rdf:resource="http://www.w3.org/1999/02/22-rdf-syntax-ns#nil"/>
              </rdf:Description>
            </rdf:rest>
          </rdf:Description>
        </owl:unionOf>
      </owl:Class>
    </rdfs:range>
  </owl:ObjectProperty>
  <ns:UseNLPSpecific rdf:about="http://purl.org/net/def/metashare#entityMentionRecognition"/>
  <ns:SizeUnit rdf:about="http://purl.org/net/def/metashare#entries"/>
  <ns:FundingType rdf:about="http://purl.org/net/def/metashare#euFunds"/>
  <owl:DatatypeProperty rdf:about="http://purl.org/net/def/metashare#evaluated">
    <rdfs:comment xml:lang="en">Indicates whether the tool or service has been evaluated</rdfs:comment>
    <rdfs:domain rdf:resource="http://purl.org/net/def/metashare#ToolServiceInfo"/>
    <rdfs:range rdf:resource="http://www.w3.org/2001/XMLSchema#boolean"/>
  </owl:DatatypeProperty>
  <ns:ConditionsOfUse rdf:about="http://purl.org/net/def/metashare#evaluation">
    <rdf:type rdf:resource="http://www.w3.org/2002/07/owl#NamedIndividual"/>
    <rdfs:comment xml:lang="en">Evaluation refers to a kind of 'ConditionsOfUse' imposed by the licence; use for evaluation purposes (cf. ELRA_EVALUATION license)</rdfs:comment>
    <rdfs:label xml:lang="en">Evaluation</rdfs:label>
  </ns:ConditionsOfUse>
  <owl:ObjectProperty rdf:about="http://purl.org/net/def/metashare#evaluationCriteria">
    <rdfs:comment xml:lang="en">Defines the criteria of the evaluation of a tool</rdfs:comment>
    <rdfs:domain rdf:resource="http://purl.org/net/def/metashare#ToolServiceInfo"/>
    <rdfs:range rdf:resource="http://purl.org/net/def/metashare#EvaluationCriteria"/>
  </owl:ObjectProperty>
  <owl:DatatypeProperty rdf:about="http://purl.org/net/def/metashare#evaluationDetails">
    <rdfs:comment xml:lang="en">Provides further information on the evaluation process of a tool or service</rdfs:comment>
    <rdfs:domain rdf:resource="http://purl.org/net/def/metashare#ToolServiceInfo"/>
    <rdfs:range rdf:resource="http://www.w3.org/2001/XMLSchema#string"/>
  </owl:DatatypeProperty>
  <owl:ObjectProperty rdf:about="http://purl.org/net/def/metashare#evaluationLevel">
    <rdfs:comment xml:lang="en">Indicates the evaluation level</rdfs:comment>
    <rdfs:domain rdf:resource="http://purl.org/net/def/metashare#ToolServiceInfo"/>
    <rdfs:range rdf:resource="http://purl.org/net/def/metashare#EvaluationLevel"/>
  </owl:ObjectProperty>
  <owl:ObjectProperty rdf:about="http://purl.org/net/def/metashare#evaluationMeasure">
    <rdfs:comment xml:lang="en">Defines whether the evaluation measure is human or automatic</rdfs:comment>
    <rdfs:domain rdf:resource="http://purl.org/net/def/metashare#ToolServiceInfo"/>
    <rdfs:range rdf:resource="http://purl.org/net/def/metashare#EvaluationMeasure"/>
  </owl:ObjectProperty>
  <owl:ObjectProperty rdf:about="http://purl.org/net/def/metashare#evaluationReport">
    <rdfs:comment xml:lang="en">A bibliographical record of or link to a report describing the evaluation process, tool, method etc. of the tool or service</rdfs:comment>
    <rdfs:domain rdf:resource="http://purl.org/net/def/metashare#ToolServiceInfo"/>
    <rdfs:range rdf:resource="http://purl.org/net/def/metashare#Documentation"/>
  </owl:ObjectProperty>
  <owl:DatatypeProperty rdf:about="http://purl.org/net/def/metashare#evaluationTool">
    <rdfs:comment xml:lang="en">The name or id or url of the tool used for the evaluation of the tool or service</rdfs:comment>
    <rdfs:domain rdf:resource="http://purl.org/net/def/metashare#ToolServiceInfo"/>
    <rdfs:range rdf:resource="http://www.w3.org/2001/XMLSchema#string"/>
  </owl:DatatypeProperty>
  <owl:ObjectProperty rdf:about="http://purl.org/net/def/metashare#evaluationType">
    <rdfs:comment xml:lang="en">Indicates the evaluation type</rdfs:comment>
    <rdfs:domain rdf:resource="http://purl.org/net/def/metashare#ToolServiceInfo"/>
    <rdfs:range rdf:resource="http://purl.org/net/def/metashare#EvaluationType"/>
  </owl:ObjectProperty>
  <ns:ConditionsOfUse rdf:about="http://purl.org/net/def/metashare#evaluationUse"/>
  <owl:ObjectProperty rdf:about="http://purl.org/net/def/metashare#evaluator">
    <rdfs:comment xml:lang="en">Groups information on person or organization that evaluated the tool or service</rdfs:comment>
    <rdfs:domain rdf:resource="http://purl.org/net/def/metashare#ToolServiceInfo"/>
    <rdfs:range rdf:resource="http://purl.org/net/def/metashare#Actor"/>
  </owl:ObjectProperty>
  <owl:DatatypeProperty rdf:about="http://purl.org/net/def/metashare#eventDescription">
    <rdfs:comment xml:lang="en">Provides description of any events represented in the image corpus</rdfs:comment>
    <rdfs:domain rdf:resource="http://purl.org/net/def/metashare#StaticElementInfo"/>
    <rdfs:range rdf:resource="http://www.w3.org/2001/XMLSchema#string"/>
  </owl:DatatypeProperty>
  <ns:UseNLPSpecific rdf:about="http://purl.org/net/def/metashare#eventExtraction"/>
  <ns:ExtraTextualInformationUnit rdf:about="http://purl.org/net/def/metashare#example"/>
  <owl:DatatypeProperty rdf:about="http://purl.org/net/def/metashare#executionLocation">
    <rdfs:comment xml:lang="en">Any url where the service providing access to a resource is being executed</rdfs:comment>
    <rdfs:domain rdf:resource="http://purl.org/net/def/metashare#LicenceInfo"/>
    <rdfs:range rdf:resource="http://www.w3.org/2001/XMLSchema#string"/>
  </owl:DatatypeProperty>
  <ns:UseNLPSpecific rdf:about="http://purl.org/net/def/metashare#expressionRecognition"/>
  <ns:SizeUnit rdf:about="http://purl.org/net/def/metashare#expressions"/>
  <owl:DatatypeProperty rdf:about="http://purl.org/net/def/metashare#externalRef">
    <rdfs:comment xml:lang="en">Another resource to which the lexicalConceptualResource is linked (e.g. link to a wordnet or ontology)</rdfs:comment>
    <rdfs:domain rdf:resource="http://purl.org/net/def/metashare#LexicalConceptualResourceInfo"/>
    <rdfs:range rdf:resource="http://www.w3.org/2001/XMLSchema#string"/>
  </owl:DatatypeProperty>
  <owl:ObjectProperty rdf:about="http://purl.org/net/def/metashare#extraTextualInformationUnit">
    <rdfs:comment xml:lang="en">The unit of the extratextual information contained in the lexical conceptual resource</rdfs:comment>
    <rdfs:domain rdf:resource="http://purl.org/net/def/metashare#LexicalConceptualResourceInfo"/>
    <rdfs:range rdf:resource="http://purl.org/net/def/metashare#ExtraTextualInformationUnit"/>
  </owl:ObjectProperty>
  <owl:ObjectProperty rdf:about="http://purl.org/net/def/metashare#extratextualInformation">
    <rdfs:comment xml:lang="en">An indication of the extratextual information contained in the lexicalConceptualResouce; can be used as an alternative to audio, image, videos etc. for cases where these are not considered an important part of the lcr</rdfs:comment>
    <rdfs:domain rdf:resource="http://purl.org/net/def/metashare#LexicalConceptualResourceInfo"/>
    <rdfs:range rdf:resource="http://purl.org/net/def/metashare#ExtratextualInformation"/>
  </owl:ObjectProperty>
  <ns:EvaluationCriteria rdf:about="http://purl.org/net/def/metashare#extrinsic"/>
  <owl:DatatypeProperty rdf:about="http://purl.org/net/def/metashare#eyeMovement">
    <rdfs:comment xml:lang="en">Indicates the movement of the eyes visible in the resource</rdfs:comment>
    <rdfs:domain rdf:resource="http://purl.org/net/def/metashare#DynamicElementInfo"/>
    <rdfs:range rdf:resource="http://www.w3.org/2001/XMLSchema#string"/>
  </owl:DatatypeProperty>
  <ns:BodyParts rdf:about="http://purl.org/net/def/metashare#face"/>
  <owl:DatatypeProperty rdf:about="http://purl.org/net/def/metashare#faceExpressions">
    <rdfs:comment xml:lang="en">Indicates the facial expressions visible in the resource</rdfs:comment>
    <rdfs:domain>
      <owl:Class>
        <owl:unionOf>
          <rdf:Description>
            <rdf:first rdf:resource="http://purl.org/net/def/metashare#StaticElementInfo"/>
            <rdf:rest>
              <rdf:Description>
                <rdf:first rdf:resource="http://purl.org/net/def/metashare#DynamicElementInfo"/>
                <rdf:rest rdf:resource="http://www.w3.org/1999/02/22-rdf-syntax-ns#nil"/>
              </rdf:Description>
            </rdf:rest>
          </rdf:Description>
        </owl:unionOf>
      </owl:Class>
    </rdfs:domain>
    <rdfs:range rdf:resource="http://www.w3.org/2001/XMLSchema#string"/>
  </owl:DatatypeProperty>
  <ns:UseNLPSpecific rdf:about="http://purl.org/net/def/metashare#faceRecognition"/>
  <ns:UseNLPSpecific rdf:about="http://purl.org/net/def/metashare#faceVerification"/>
  <owl:DatatypeProperty rdf:about="http://purl.org/net/def/metashare#faceViews">
    <rdfs:comment xml:lang="en">Indicates the view of the face(s) that appear in the video or on the image part of the resource</rdfs:comment>
    <rdfs:domain>
      <owl:Class>
        <owl:unionOf>
          <rdf:Description>
            <rdf:first rdf:resource="http://purl.org/net/def/metashare#DynamicElementInfo"/>
            <rdf:rest>
              <rdf:Description>
                <rdf:first rdf:resource="http://purl.org/net/def/metashare#StaticElementInfo"/>
                <rdf:rest rdf:resource="http://www.w3.org/1999/02/22-rdf-syntax-ns#nil"/>
              </rdf:Description>
            </rdf:rest>
          </rdf:Description>
        </owl:unionOf>
      </owl:Class>
    </rdfs:domain>
    <rdfs:range rdf:resource="http://www.w3.org/2001/XMLSchema#string"/>
  </owl:DatatypeProperty>
  <ns:ModalityType rdf:about="http://purl.org/net/def/metashare#facialExpression"/>
  <owl:DatatypeProperty rdf:about="http://purl.org/net/def/metashare#factors">
    <rdfs:comment xml:lang="en">The list of factors that have been used for the n-gram model</rdfs:comment>
    <rdfs:domain rdf:resource="http://purl.org/net/def/metashare#NgramInfo"/>
    <rdfs:range rdf:resource="http://www.w3.org/2001/XMLSchema#string"/>
  </owl:DatatypeProperty>
  <ns:CapturingDeviceType rdf:about="http://purl.org/net/def/metashare#farfieldMicrophone"/>
  <owl:DatatypeProperty rdf:about="http://purl.org/net/def/metashare#faxNumber">
    <rdfs:comment xml:lang="en">The fax number of a person or an organization; recommended format: +_international code_city code_number</rdfs:comment>
    <rdfs:domain>
      <owl:Class>
        <owl:unionOf>
          <rdf:Description>
            <rdf:first rdf:resource="http://purl.org/net/def/metashare#Person"/>
            <rdf:rest>
              <rdf:Description>
                <rdf:first rdf:resource="http://purl.org/net/def/metashare#Organization"/>
                <rdf:rest rdf:resource="http://www.w3.org/1999/02/22-rdf-syntax-ns#nil"/>
              </rdf:Description>
            </rdf:rest>
          </rdf:Description>
        </owl:unionOf>
      </owl:Class>
    </rdfs:domain>
    <rdfs:range rdf:resource="http://www.w3.org/2001/XMLSchema#string"/>
  </owl:DatatypeProperty>
  <owl:DatatypeProperty rdf:about="http://purl.org/net/def/metashare#fee">
    <rdfs:comment xml:lang="en">Specifies the costs that are required to access the resource, a fragment of the resource or to use a tool or service</rdfs:comment>
    <rdfs:domain rdf:resource="http://purl.org/net/def/metashare#LicenceInfo"/>
    <rdfs:range rdf:resource="http://www.w3.org/2001/XMLSchema#string"/>
  </owl:DatatypeProperty>
  <ns:BodyParts rdf:about="http://purl.org/net/def/metashare#feet"/>
  <ns:SexOfPersons rdf:about="http://purl.org/net/def/metashare#female"/>
  <ns:Audience rdf:about="http://purl.org/net/def/metashare#few"/>
  <owl:DatatypeProperty rdf:about="http://purl.org/net/def/metashare#fidelity">
    <rdfs:comment xml:lang="en">Defines whether blur is present in the moving sequences</rdfs:comment>
    <rdfs:domain rdf:resource="http://purl.org/net/def/metashare#VideoFormatInfo"/>
    <rdfs:range rdf:resource="http://www.w3.org/2001/XMLSchema#boolean"/>
  </owl:DatatypeProperty>
  <ns:SizeUnit rdf:about="http://purl.org/net/def/metashare#files"/>
  <ns:SceneIllumination rdf:about="http://purl.org/net/def/metashare#fix"/>
  <ns:CompressionName rdf:about="http://purl.org/net/def/metashare#flac"/>
  <ns:RecordingDeviceType rdf:about="http://purl.org/net/def/metashare#flash"/>
  <ns:SignConvention rdf:about="http://purl.org/net/def/metashare#floatingPoint"/>
  <owl:ObjectProperty rdf:about="http://purl.org/net/def/metashare#foreseenUseInfo">
    <rdfs:comment xml:lang="en">Groups information on the use for which the resource is created</rdfs:comment>
    <rdfs:domain rdf:resource="http://purl.org/net/def/metashare#LanguageResource"/>
    <rdfs:range rdf:resource="http://purl.org/net/def/metashare#ForeseenUseInfo"/>
  </owl:ObjectProperty>
  <ns:ValidationType rdf:about="http://purl.org/net/def/metashare#formal"/>
  <owl:DatatypeProperty rdf:about="http://purl.org/net/def/metashare#formalism">
    <rdfs:comment xml:lang="en">Reference (name, bibliographic reference or link to url) for the formalism used for the creation/enrichment of the resource (grammar or tool/service)</rdfs:comment>
    <rdfs:domain rdf:resource="http://purl.org/net/def/metashare#ToolServiceInfo"/>
    <rdfs:range rdf:resource="http://www.w3.org/2001/XMLSchema#string"/>
  </owl:DatatypeProperty>
  <ns:SegmentationLevel rdf:about="http://purl.org/net/def/metashare#frame"/>
  <rdf:Description rdf:about="http://purl.org/net/def/metashare#frameNet">
    <dct:replaces rdf:resource="http://www.ilsp.gr/META-XMLSchema#framenet"/>
  </rdf:Description>
  <owl:DatatypeProperty rdf:about="http://purl.org/net/def/metashare#frameRate">
    <rdfs:comment xml:lang="en">The number of frames per second</rdfs:comment>
    <rdfs:domain rdf:resource="http://purl.org/net/def/metashare#VideoFormatInfo"/>
    <rdfs:range rdf:resource="http://www.w3.org/2001/XMLSchema#int"/>
  </owl:DatatypeProperty>
  <ns:CompatibleLexiconType rdf:about="http://purl.org/net/def/metashare#framenet">
    <rdf:type rdf:resource="http://purl.org/net/def/metashare#LexicalConceptualResourceType"/>
  </ns:CompatibleLexiconType>
  <ns:SizeUnit rdf:about="http://purl.org/net/def/metashare#frames"/>
  <ns:SpeechItems rdf:about="http://purl.org/net/def/metashare#freeSpeech"/>
  <ns:ScenarioType rdf:about="http://purl.org/net/def/metashare#frogStory"/>
  <ns:ValidationExtent rdf:about="http://purl.org/net/def/metashare#full"/>
  <owl:DatatypeProperty rdf:about="http://purl.org/net/def/metashare#funder">
    <rdfs:comment xml:lang="en">The full name of the funder of the project </rdfs:comment>
    <rdfs:domain rdf:resource="http://purl.org/net/def/metashare#Project"/>
    <rdfs:range rdf:resource="http://www.w3.org/2001/XMLSchema#string"/>
  </owl:DatatypeProperty>
  <owl:DatatypeProperty rdf:about="http://purl.org/net/def/metashare#fundingCountry">
    <rdfs:comment xml:lang="en">The name of the funding country, in case of national funding as mentioned in ISO3166</rdfs:comment>
    <rdfs:domain rdf:resource="http://purl.org/net/def/metashare#Project"/>
    <rdfs:range rdf:resource="http://www.w3.org/2001/XMLSchema#string"/>
  </owl:DatatypeProperty>
  <owl:ObjectProperty rdf:about="http://purl.org/net/def/metashare#fundingProject">
    <rdfs:comment xml:lang="en">Groups information on the project that has funded the resource</rdfs:comment>
    <rdfs:domain rdf:resource="http://purl.org/net/def/metashare#LanguageResource"/>
    <rdfs:range rdf:resource="http://purl.org/net/def/metashare#Project"/>
  </owl:ObjectProperty>
  <owl:ObjectProperty rdf:about="http://purl.org/net/def/metashare#fundingType">
    <rdfs:comment xml:lang="en">Specifies the type of funding of the project</rdfs:comment>
    <rdfs:domain rdf:resource="http://purl.org/net/def/metashare#Project"/>
    <rdfs:range rdf:resource="http://purl.org/net/def/metashare#FundingType"/>
  </owl:ObjectProperty>
  <ns:SizeUnit rdf:about="http://purl.org/net/def/metashare#gb"/>
  <ns:Task rdf:about="http://purl.org/net/def/metashare#generation"/>
  <owl:DatatypeProperty rdf:about="http://purl.org/net/def/metashare#genre">
    <rdfs:domain rdf:resource="http://purl.org/net/def/metashare#ClassificationInfo"/>
    <rdfs:range rdf:resource="http://www.w3.org/2001/XMLSchema#string"/>
  </owl:DatatypeProperty>
  <owl:DatatypeProperty rdf:about="http://purl.org/net/def/metashare#geographicCoverage">
    <rdfs:comment xml:lang="en">The geographic region that the content of a resource is about; for countries, recommended use of ISO-3166</rdfs:comment>
    <rdfs:domain rdf:resource="http://purl.org/net/def/metashare#GeographicCoverageInfo"/>
    <rdfs:range rdf:resource="http://www.w3.org/2001/XMLSchema#string"/>
  </owl:DatatypeProperty>
  <owl:ObjectProperty rdf:about="http://purl.org/net/def/metashare#geographicCoverageInfo">
    <rdfs:comment xml:lang="en">Groups information on geographic classification of the resource</rdfs:comment>
    <rdfs:domain>
      <owl:Class>
        <owl:unionOf>
          <rdf:Description>
            <rdf:first rdf:resource="http://purl.org/net/def/metashare#CorpusTextInfo"/>
            <rdf:rest>
              <rdf:Description>
                <rdf:first rdf:resource="http://purl.org/net/def/metashare#CorpusImageInfo"/>
                <rdf:rest>
                  <rdf:Description>
                    <rdf:first rdf:resource="http://purl.org/net/def/metashare#LanguageDescriptionVideoInfo"/>
                    <rdf:rest>
                      <rdf:Description>
                        <rdf:first rdf:resource="http://purl.org/net/def/metashare#CorpusVideoInfo"/>
                        <rdf:rest>
                          <rdf:Description>
                            <rdf:first rdf:resource="http://purl.org/net/def/metashare#CorpusAudioInfo"/>
                            <rdf:rest>
                              <rdf:Description>
                                <rdf:first rdf:resource="http://purl.org/net/def/metashare#CorpusTextNgramInfo"/>
                                <rdf:rest>
                                  <rdf:Description>
                                    <rdf:first rdf:resource="http://purl.org/net/def/metashare#LanguageDescriptionImageInfo"/>
                                    <rdf:rest>
                                      <rdf:Description>
                                        <rdf:first rdf:resource="http://purl.org/net/def/metashare#LexicalConceptualResourceAudioInfo"/>
                                        <rdf:rest>
                                          <rdf:Description>
                                            <rdf:first rdf:resource="http://purl.org/net/def/metashare#LexicalConceptualResourceVideoInfo"/>
                                            <rdf:rest>
                                              <rdf:Description>
                                                <rdf:first rdf:resource="http://purl.org/net/def/metashare#LexicalConceptualResourceImageInfo"/>
                                                <rdf:rest>
                                                  <rdf:Description>
                                                    <rdf:first rdf:resource="http://purl.org/net/def/metashare#LanguageDescriptionTextInfo"/>
                                                    <rdf:rest>
                                                      <rdf:Description>
                                                        <rdf:first rdf:resource="http://purl.org/net/def/metashare#LexicalConceptualResourceTextInfo"/>
                                                        <rdf:rest rdf:resource="http://www.w3.org/1999/02/22-rdf-syntax-ns#nil"/>
                                                      </rdf:Description>
                                                    </rdf:rest>
                                                  </rdf:Description>
                                                </rdf:rest>
                                              </rdf:Description>
                                            </rdf:rest>
                                          </rdf:Description>
                                        </rdf:rest>
                                      </rdf:Description>
                                    </rdf:rest>
                                  </rdf:Description>
                                </rdf:rest>
                              </rdf:Description>
                            </rdf:rest>
                          </rdf:Description>
                        </rdf:rest>
                      </rdf:Description>
                    </rdf:rest>
                  </rdf:Description>
                </rdf:rest>
              </rdf:Description>
            </rdf:rest>
          </rdf:Description>
        </owl:unionOf>
      </owl:Class>
    </rdfs:domain>
    <rdfs:range>
      <owl:Class>
        <owl:unionOf>
          <rdf:Description>
            <rdf:first rdf:resource="http://purl.org/net/def/metashare#GeographicCoverageInfo"/>
            <rdf:rest>
              <rdf:Description>
                <rdf:first rdf:resource="http://purl.org/net/def/metashare#GeographicCoverageInfo"/>
                <rdf:rest>
                  <rdf:Description>
                    <rdf:first rdf:resource="http://purl.org/net/def/metashare#GeographicCoverageInfo"/>
                    <rdf:rest>
                      <rdf:Description>
                        <rdf:first rdf:resource="http://purl.org/net/def/metashare#GeographicCoverageInfo"/>
                        <rdf:rest>
                          <rdf:Description>
                            <rdf:first rdf:resource="http://purl.org/net/def/metashare#GeographicCoverageInfo"/>
                            <rdf:rest>
                              <rdf:Description>
                                <rdf:first rdf:resource="http://purl.org/net/def/metashare#GeographicCoverageInfo"/>
                                <rdf:rest>
                                  <rdf:Description>
                                    <rdf:first rdf:resource="http://purl.org/net/def/metashare#GeographicCoverageInfo"/>
                                    <rdf:rest>
                                      <rdf:Description>
                                        <rdf:first rdf:resource="http://purl.org/net/def/metashare#GeographicCoverageInfo"/>
                                        <rdf:rest>
                                          <rdf:Description>
                                            <rdf:first rdf:resource="http://purl.org/net/def/metashare#GeographicCoverageInfo"/>
                                            <rdf:rest>
                                              <rdf:Description>
                                                <rdf:first rdf:resource="http://purl.org/net/def/metashare#GeographicCoverageInfo"/>
                                                <rdf:rest>
                                                  <rdf:Description>
                                                    <rdf:first rdf:resource="http://purl.org/net/def/metashare#GeographicCoverageInfo"/>
                                                    <rdf:rest>
                                                      <rdf:Description>
                                                        <rdf:first rdf:resource="http://purl.org/net/def/metashare#GeographicCoverageInfo"/>
                                                        <rdf:rest rdf:resource="http://www.w3.org/1999/02/22-rdf-syntax-ns#nil"/>
                                                      </rdf:Description>
                                                    </rdf:rest>
                                                  </rdf:Description>
                                                </rdf:rest>
                                              </rdf:Description>
                                            </rdf:rest>
                                          </rdf:Description>
                                        </rdf:rest>
                                      </rdf:Description>
                                    </rdf:rest>
                                  </rdf:Description>
                                </rdf:rest>
                              </rdf:Description>
                            </rdf:rest>
                          </rdf:Description>
                        </rdf:rest>
                      </rdf:Description>
                    </rdf:rest>
                  </rdf:Description>
                </rdf:rest>
              </rdf:Description>
            </rdf:rest>
          </rdf:Description>
        </owl:unionOf>
      </owl:Class>
    </rdfs:range>
  </owl:ObjectProperty>
  <owl:DatatypeProperty rdf:about="http://purl.org/net/def/metashare#geographicDistributionOfPersons">
    <rdfs:comment xml:lang="en">Gives information on the geographic distribution of the participants</rdfs:comment>
    <rdfs:domain>
      <owl:Class>
        <owl:unionOf>
          <rdf:Description>
            <rdf:first rdf:resource="http://purl.org/net/def/metashare#CorpusTextNumericalInfo"/>
            <rdf:rest>
              <rdf:Description>
                <rdf:first rdf:resource="http://purl.org/net/def/metashare#CorpusAudioInfo"/>
                <rdf:rest>
                  <rdf:Description>
                    <rdf:first rdf:resource="http://purl.org/net/def/metashare#CorpusImageInfo"/>
                    <rdf:rest>
                      <rdf:Description>
                        <rdf:first rdf:resource="http://purl.org/net/def/metashare#CorpusVideoInfo"/>
                        <rdf:rest rdf:resource="http://www.w3.org/1999/02/22-rdf-syntax-ns#nil"/>
                      </rdf:Description>
                    </rdf:rest>
                  </rdf:Description>
                </rdf:rest>
              </rdf:Description>
            </rdf:rest>
          </rdf:Description>
        </owl:unionOf>
      </owl:Class>
    </rdfs:domain>
    <rdfs:range rdf:resource="http://www.w3.org/2001/XMLSchema#string"/>
  </owl:DatatypeProperty>
  <owl:DatatypeProperty rdf:about="http://purl.org/net/def/metashare#gestures">
    <rdfs:comment xml:lang="en">Indicates the type of gestures visible in the resource</rdfs:comment>
    <rdfs:domain rdf:resource="http://purl.org/net/def/metashare#DynamicElementInfo"/>
    <rdfs:range rdf:resource="http://www.w3.org/2001/XMLSchema#string"/>
  </owl:DatatypeProperty>
  <ns:EvaluationType rdf:about="http://purl.org/net/def/metashare#glassBox"/>
  <ns:LanguageDescriptionType rdf:about="http://purl.org/net/def/metashare#grammar"/>
  <owl:ObjectProperty rdf:about="http://purl.org/net/def/metashare#grammaticalPhenomenaCoverage">
    <rdfs:comment xml:lang="en">An indication of the grammatical phenomena covered by the grammar</rdfs:comment>
    <rdfs:domain rdf:resource="http://purl.org/net/def/metashare#LanguageDescriptionInfo"/>
    <rdfs:range rdf:resource="http://purl.org/net/def/metashare#GrammaticalPhenomenaCoverage"/>
  </owl:ObjectProperty>
  <ns:SizeUnit rdf:about="http://purl.org/net/def/metashare#grams"/>
  <ns:RequiredHardware rdf:about="http://purl.org/net/def/metashare#graphicCard"/>
  <owl:DatatypeProperty rdf:about="http://purl.org/net/def/metashare#handArmMovement">
    <rdfs:comment xml:lang="en">Indicates the movement of hands and/or arms visible in the resource</rdfs:comment>
    <rdfs:domain rdf:resource="http://purl.org/net/def/metashare#DynamicElementInfo"/>
    <rdfs:range rdf:resource="http://www.w3.org/2001/XMLSchema#string"/>
  </owl:DatatypeProperty>
  <owl:DatatypeProperty rdf:about="http://purl.org/net/def/metashare#handManipulation">
    <rdfs:comment xml:lang="en">Gives information on the manipulation of objects by hand</rdfs:comment>
    <rdfs:domain rdf:resource="http://purl.org/net/def/metashare#DynamicElementInfo"/>
    <rdfs:range rdf:resource="http://www.w3.org/2001/XMLSchema#string"/>
  </owl:DatatypeProperty>
  <ns:BodyParts rdf:about="http://purl.org/net/def/metashare#hands"/>
  <ns:DistributionAccessMedium rdf:about="http://purl.org/net/def/metashare#hardDisk">
    <rdf:type rdf:resource="http://purl.org/net/def/metashare#RecordingDeviceType"/>
  </ns:DistributionAccessMedium>
  <ns:BodyParts rdf:about="http://purl.org/net/def/metashare#head"/>
  <owl:DatatypeProperty rdf:about="http://purl.org/net/def/metashare#headMovement">
    <rdfs:comment xml:lang="en">Indicates the movements of the head visible in the resource</rdfs:comment>
    <rdfs:domain rdf:resource="http://purl.org/net/def/metashare#DynamicElementInfo"/>
    <rdfs:range rdf:resource="http://www.w3.org/2001/XMLSchema#string"/>
  </owl:DatatypeProperty>
  <owl:DatatypeProperty rdf:about="http://purl.org/net/def/metashare#hearingImpairment">
    <rdfs:comment xml:lang="en">Provides information on any hearing impairment the participant may have</rdfs:comment>
    <rdfs:domain rdf:resource="http://purl.org/net/def/metashare#ParticipantInfo"/>
    <rdfs:range rdf:resource="http://www.w3.org/2001/XMLSchema#string"/>
  </owl:DatatypeProperty>
  <owl:ObjectProperty rdf:about="http://purl.org/net/def/metashare#hearingImpairmentOfPersons">
    <rdfs:comment xml:lang="en">Whether the group of participants contains persons with hearing impairments</rdfs:comment>
    <rdfs:domain>
      <owl:Class>
        <owl:unionOf>
          <rdf:Description>
            <rdf:first rdf:resource="http://purl.org/net/def/metashare#CorpusAudioInfo"/>
            <rdf:rest>
              <rdf:Description>
                <rdf:first rdf:resource="http://purl.org/net/def/metashare#CorpusTextNumericalInfo"/>
                <rdf:rest>
                  <rdf:Description>
                    <rdf:first rdf:resource="http://purl.org/net/def/metashare#CorpusVideoInfo"/>
                    <rdf:rest>
                      <rdf:Description>
                        <rdf:first rdf:resource="http://purl.org/net/def/metashare#CorpusImageInfo"/>
                        <rdf:rest rdf:resource="http://www.w3.org/1999/02/22-rdf-syntax-ns#nil"/>
                      </rdf:Description>
                    </rdf:rest>
                  </rdf:Description>
                </rdf:rest>
              </rdf:Description>
            </rdf:rest>
          </rdf:Description>
        </owl:unionOf>
      </owl:Class>
    </rdfs:domain>
    <rdfs:range>
      <owl:Class>
        <owl:unionOf>
          <rdf:Description>
            <rdf:first rdf:resource="http://purl.org/net/def/metashare#HearingImpairmentOfPersons"/>
            <rdf:rest>
              <rdf:Description>
                <rdf:first rdf:resource="http://purl.org/net/def/metashare#HearingImpairmentOfPersons"/>
                <rdf:rest>
                  <rdf:Description>
                    <rdf:first rdf:resource="http://purl.org/net/def/metashare#HearingImpairmentOfPersons"/>
                    <rdf:rest>
                      <rdf:Description>
                        <rdf:first rdf:resource="http://purl.org/net/def/metashare#HearingImpairmentOfPersons"/>
                        <rdf:rest rdf:resource="http://www.w3.org/1999/02/22-rdf-syntax-ns#nil"/>
                      </rdf:Description>
                    </rdf:rest>
                  </rdf:Description>
                </rdf:rest>
              </rdf:Description>
            </rdf:rest>
          </rdf:Description>
        </owl:unionOf>
      </owl:Class>
    </rdfs:range>
  </owl:ObjectProperty>
  <owl:DatatypeProperty rdf:about="http://purl.org/net/def/metashare#height">
    <rdfs:comment xml:lang="en">Provides information on the height of the participant in cm</rdfs:comment>
    <rdfs:domain rdf:resource="http://purl.org/net/def/metashare#ParticipantInfo"/>
    <rdfs:range rdf:resource="http://www.w3.org/2001/XMLSchema#int"/>
  </owl:DatatypeProperty>
  <ns:ToolDocumentationType rdf:about="http://purl.org/net/def/metashare#helpFunctions"/>
  <ns:NoiseLevel rdf:about="http://purl.org/net/def/metashare#high">
    <rdf:type rdf:resource="http://purl.org/net/def/metashare#Quality"/>
    <rdf:type rdf:resource="http://purl.org/net/def/metashare#RecordingQuality"/>
  </ns:NoiseLevel>
  <ns:DurationOfAudioInfoUnit rdf:about="http://purl.org/net/def/metashare#hours">
    <rdf:type rdf:resource="http://purl.org/net/def/metashare#DurationOfEffectiveSpeechInfoUnit"/>
    <rdf:type rdf:resource="http://purl.org/net/def/metashare#SizeUnit"/>
  </ns:DurationOfAudioInfoUnit>
  <ns:EvaluationMeasure rdf:about="http://purl.org/net/def/metashare#human"/>
  <ns:Use rdf:about="http://purl.org/net/def/metashare#humanUse"/>
  <ns:UseNLPSpecific rdf:about="http://purl.org/net/def/metashare#humanoidAgentSynthesis"/>
  <ns:SpeechInfluences rdf:about="http://purl.org/net/def/metashare#hyperbaric"/>
  <ns:SizeUnit rdf:about="http://purl.org/net/def/metashare#idiomaticExpressions"/>
  <ns:MediaType rdf:about="http://purl.org/net/def/metashare#image">
    <rdf:type rdf:resource="http://purl.org/net/def/metashare#OtherMedia"/>
  </ns:MediaType>
  <owl:ObjectProperty rdf:about="http://purl.org/net/def/metashare#imageClassificationInfo">
    <rdfs:comment xml:lang="en">Groups together information on image type/genre of the resource</rdfs:comment>
    <rdfs:domain rdf:resource="http://purl.org/net/def/metashare#CorpusImageInfo"/>
    <rdfs:range rdf:resource="http://purl.org/net/def/metashare#ImageClassificationInfo"/>
  </owl:ObjectProperty>
  <owl:ObjectProperty rdf:about="http://purl.org/net/def/metashare#imageFormatInfo">
    <rdfs:comment xml:lang="en">Groups together information on the format of the image part of a resource</rdfs:comment>
    <rdfs:domain>
      <owl:Class>
        <owl:unionOf>
          <rdf:Description>
            <rdf:first rdf:resource="http://purl.org/net/def/metashare#LexicalConceptualResourceImageInfo"/>
            <rdf:rest>
              <rdf:Description>
                <rdf:first rdf:resource="http://purl.org/net/def/metashare#LanguageDescriptionImageInfo"/>
                <rdf:rest>
                  <rdf:Description>
                    <rdf:first rdf:resource="http://purl.org/net/def/metashare#CorpusImageInfo"/>
                    <rdf:rest rdf:resource="http://www.w3.org/1999/02/22-rdf-syntax-ns#nil"/>
                  </rdf:Description>
                </rdf:rest>
              </rdf:Description>
            </rdf:rest>
          </rdf:Description>
        </owl:unionOf>
      </owl:Class>
    </rdfs:domain>
    <rdfs:range>
      <owl:Class>
        <owl:unionOf>
          <rdf:Description>
            <rdf:first rdf:resource="http://purl.org/net/def/metashare#ImageFormatInfo"/>
            <rdf:rest>
              <rdf:Description>
                <rdf:first rdf:resource="http://purl.org/net/def/metashare#ImageFormatInfo"/>
                <rdf:rest>
                  <rdf:Description>
                    <rdf:first rdf:resource="http://purl.org/net/def/metashare#ImageFormatInfo"/>
                    <rdf:rest rdf:resource="http://www.w3.org/1999/02/22-rdf-syntax-ns#nil"/>
                  </rdf:Description>
                </rdf:rest>
              </rdf:Description>
            </rdf:rest>
          </rdf:Description>
        </owl:unionOf>
      </owl:Class>
    </rdfs:range>
  </owl:ObjectProperty>
  <owl:DatatypeProperty rdf:about="http://purl.org/net/def/metashare#imageGenre">
    <rdfs:comment xml:lang="en">A first indication of the genre of images</rdfs:comment>
    <rdfs:domain rdf:resource="http://purl.org/net/def/metashare#ImageClassificationInfo"/>
    <rdfs:range rdf:resource="http://www.w3.org/2001/XMLSchema#string"/>
    <rdfs:subPropertyOf rdf:resource="http://purl.org/net/def/metashare#genre"/>
  </owl:DatatypeProperty>
  <ns:ExtratextualInformation rdf:about="http://purl.org/net/def/metashare#images">
    <rdf:type rdf:resource="http://purl.org/net/def/metashare#SizeUnit"/>
  </ns:ExtratextualInformation>
  <ns:EvaluationLevel rdf:about="http://purl.org/net/def/metashare#impact"/>
  <owl:DatatypeProperty rdf:about="http://purl.org/net/def/metashare#implementationLanguage">
    <rdfs:comment xml:lang="en">The programming languages needed for allowing user contributions, or for running the tools, in case no executables are available</rdfs:comment>
    <rdfs:domain rdf:resource="http://purl.org/net/def/metashare#ToolServiceInfo"/>
    <rdfs:range rdf:resource="http://www.w3.org/2001/XMLSchema#string"/>
  </owl:DatatypeProperty>
  <ns:RecordingEnvironment rdf:about="http://purl.org/net/def/metashare#inCar"/>
  <ns:RelatedLexiconType rdf:about="http://purl.org/net/def/metashare#included"/>
  <ns4:concept xmlns:ns4="http://www.w3.org/2004/02/skos/core#"
     rdf:about="http://purl.org/net/def/metashare#incorporate">
    <rdfs:comment xml:lang="en">The Assigner permits/prohibits the Assignees to incorporate the Asset unmodified into a Collective Work.</rdfs:comment>
    <rdfs:label xml:lang="en">incorporate</rdfs:label>
    <ns4:broaderTransitive rdf:resource="http://www.w3.org/ns/odrl/2/use"/>
  </ns4:concept>
  <ns:RecordingEnvironment rdf:about="http://purl.org/net/def/metashare#industrial"/>
  <odrl:Set rdf:about="http://purl.org/net/def/metashare#informLicensor">
    <rdf:type rdf:resource="http://purl.org/net/def/metashare#ConditionsOfUse"/>
    <rdfs:comment xml:lang="en">Inform Licensor refers to a kind of 'ConditionsOfUse' imposed by the licence; users must inform the licensor as to the kind of use they make of the resource</rdfs:comment>
    <odrl:permission>
      <rdf:Description>
        <odrl:duty>
          <rdf:Description>
            <odrl:action rdf:resource="http://creativecommons.org/ns#Notify"/>
          </rdf:Description>
        </odrl:duty>
      </rdf:Description>
    </odrl:permission>
  </odrl:Set>
  <ns:UseNLPSpecific rdf:about="http://purl.org/net/def/metashare#informationExtraction"/>
  <ns:UseNLPSpecific rdf:about="http://purl.org/net/def/metashare#informationRetrieval"/>
  <ns:ToolServiceType rdf:about="http://purl.org/net/def/metashare#infrastructure"/>
  <owl:ObjectProperty rdf:about="http://purl.org/net/def/metashare#inputInfo">
    <rdfs:comment xml:lang="en">Groups together information on the requirements set on the input resource of a tool or service</rdfs:comment>
    <rdfs:domain rdf:resource="http://purl.org/net/def/metashare#ToolServiceInfo"/>
    <rdfs:range rdf:resource="http://purl.org/net/def/metashare#InputInfo"/>
  </owl:ObjectProperty>
  <owl:DatatypeProperty rdf:about="http://purl.org/net/def/metashare#interaction">
    <rdfs:comment xml:lang="en">Specifies the parts that interact in an audio or video component</rdfs:comment>
    <rdfs:domain>
      <owl:Class>
        <owl:unionOf>
          <rdf:Description>
            <rdf:first rdf:resource="http://purl.org/net/def/metashare#CorpusVideoInfo"/>
            <rdf:rest>
              <rdf:Description>
                <rdf:first rdf:resource="http://purl.org/net/def/metashare#CorpusAudioInfo"/>
                <rdf:rest rdf:resource="http://www.w3.org/1999/02/22-rdf-syntax-ns#nil"/>
              </rdf:Description>
            </rdf:rest>
          </rdf:Description>
        </owl:unionOf>
      </owl:Class>
    </rdfs:domain>
    <rdfs:range rdf:resource="http://www.w3.org/2001/XMLSchema#string"/>
  </owl:DatatypeProperty>
  <ns:AnnotationMode rdf:about="http://purl.org/net/def/metashare#interactive">
    <rdf:type rdf:resource="http://purl.org/net/def/metashare#CreationMode"/>
    <rdf:type rdf:resource="http://purl.org/net/def/metashare#Interactivity"/>
    <rdf:type rdf:resource="http://purl.org/net/def/metashare#ValidationMode"/>
  </ns:AnnotationMode>
  <owl:DatatypeProperty rdf:about="http://purl.org/net/def/metashare#interactiveMedia">
    <rdfs:comment xml:lang="en">Any interactive media visible in the resource</rdfs:comment>
    <rdfs:domain rdf:resource="http://purl.org/net/def/metashare#DynamicElementInfo"/>
    <rdfs:range rdf:resource="http://www.w3.org/2001/XMLSchema#string"/>
  </owl:DatatypeProperty>
  <owl:ObjectProperty rdf:about="http://purl.org/net/def/metashare#interactivity">
    <rdfs:comment xml:lang="en">Indicates the level of conversational interaction between speakers (for audio component) or participants (for video component)</rdfs:comment>
    <rdfs:domain>
      <owl:Class>
        <owl:unionOf>
          <rdf:Description>
            <rdf:first rdf:resource="http://purl.org/net/def/metashare#CorpusAudioInfo"/>
            <rdf:rest>
              <rdf:Description>
                <rdf:first rdf:resource="http://purl.org/net/def/metashare#CorpusVideoInfo"/>
                <rdf:rest rdf:resource="http://www.w3.org/1999/02/22-rdf-syntax-ns#nil"/>
              </rdf:Description>
            </rdf:rest>
          </rdf:Description>
        </owl:unionOf>
      </owl:Class>
    </rdfs:domain>
    <rdfs:range>
      <owl:Class>
        <owl:unionOf>
          <rdf:Description>
            <rdf:first rdf:resource="http://purl.org/net/def/metashare#Interactivity"/>
            <rdf:rest>
              <rdf:Description>
                <rdf:first rdf:resource="http://purl.org/net/def/metashare#Interactivity"/>
                <rdf:rest rdf:resource="http://www.w3.org/1999/02/22-rdf-syntax-ns#nil"/>
              </rdf:Description>
            </rdf:rest>
          </rdf:Description>
        </owl:unionOf>
      </owl:Class>
    </rdfs:range>
  </owl:ObjectProperty>
  <owl:DatatypeProperty rdf:about="http://purl.org/net/def/metashare#interannotatorAgreement">
    <rdfs:comment xml:lang="en">Provides information on the interannotator agreement and the methods/metrics applied </rdfs:comment>
    <rdfs:domain rdf:resource="http://purl.org/net/def/metashare#AnnotationInfo"/>
    <rdfs:range rdf:resource="http://www.w3.org/2001/XMLSchema#string"/>
  </owl:DatatypeProperty>
  <ns:SourceChannel rdf:about="http://purl.org/net/def/metashare#internet"/>
  <owl:DatatypeProperty rdf:about="http://purl.org/net/def/metashare#interpolated">
    <rdfs:comment xml:lang="en">Interpolated language models are constructed by 2 or more corpora. Each corpus is represented in the model according to a predefined weight.</rdfs:comment>
    <rdfs:domain rdf:resource="http://purl.org/net/def/metashare#NgramInfo"/>
    <rdfs:range rdf:resource="http://www.w3.org/2001/XMLSchema#boolean"/>
  </owl:DatatypeProperty>
  <ns:UseNLPSpecific rdf:about="http://purl.org/net/def/metashare#intra-documentCoreferenceResolution"/>
  <owl:DatatypeProperty rdf:about="http://purl.org/net/def/metashare#intraannotatorAgreement">
    <rdfs:comment xml:lang="en">Provides information on the intra-annotator agreement and the methods/metrics applied  </rdfs:comment>
    <rdfs:domain rdf:resource="http://purl.org/net/def/metashare#AnnotationInfo"/>
    <rdfs:range rdf:resource="http://www.w3.org/2001/XMLSchema#string"/>
  </owl:DatatypeProperty>
  <ns:EvaluationCriteria rdf:about="http://purl.org/net/def/metashare#intrinsic"/>
  <owl:ObjectProperty rdf:about="http://purl.org/net/def/metashare#iprHolder">
    <rdfs:comment xml:lang="en">A person or an organization who holds the full Intellectual Property Rights (Copyright, trademark etc) that subsist in the resource. The IPR holder could be different from the creator that may have assigned the rights to the IPR holder (e.g. an author as a creator assigns her rights to the publisher who is the IPR holder) and the distributor that holds a specific licence (i.e. a permission) to distribute the work via a specific distributor.</rdfs:comment>
    <rdfs:comment xml:lang="en">Groups information on a person or an organization who holds the full Intellectual Property Rights (Copyright, trademark etc) that subsist in the resource. The IPR holder could be different from the creator that may have assigned the rights to the IPR holder (e.g. an author as a creator assigns her rights to the publisher who is the IPR holder) and the distributor that holds a specific licence (i.e. a permission) to distribute the work within the META-SHARE network.</rdfs:comment>
    <rdfs:range rdf:resource="http://purl.org/net/def/metashare#Actor"/>
  </owl:ObjectProperty>
  <owl:DatatypeProperty rdf:about="http://purl.org/net/def/metashare#isFactored">
    <rdfs:comment xml:lang="en">Specifies whether the model is factored or not</rdfs:comment>
    <rdfs:domain rdf:resource="http://purl.org/net/def/metashare#NgramInfo"/>
    <rdfs:range rdf:resource="http://www.w3.org/2001/XMLSchema#boolean"/>
  </owl:DatatypeProperty>
  <ns:SpeechItems rdf:about="http://purl.org/net/def/metashare#isolatedDigits"/>
  <ns:SpeechItems rdf:about="http://purl.org/net/def/metashare#isolatedWords"/>
  <owl:DatatypeProperty rdf:about="http://purl.org/net/def/metashare#issn">
    <rdfs:domain rdf:resource="http://purl.org/net/def/metashare#DocumentInfo"/>
    <rdfs:range rdf:resource="http://www.w3.org/2001/XMLSchema#string"/>
  </owl:DatatypeProperty>
  <ns:SizeUnit rdf:about="http://purl.org/net/def/metashare#items"/>
  <ns:LanguageVarietyType rdf:about="http://purl.org/net/def/metashare#jargon"/>
  <ns:SizeUnit rdf:about="http://purl.org/net/def/metashare#kb"/>
  <ns:SizeUnit rdf:about="http://purl.org/net/def/metashare#keywords">
    <rdfs:comment xml:lang="en">The keyword(s) for indexing and classification of the document</rdfs:comment>
  </ns:SizeUnit>
  <ns:UseNLPSpecific rdf:about="http://purl.org/net/def/metashare#knowledgeDiscovery"/>
  <ns:UseNLPSpecific rdf:about="http://purl.org/net/def/metashare#knowledgeRepresentation"/>
  <owl:DatatypeProperty rdf:about="http://purl.org/net/def/metashare#landscapeParts">
    <rdfs:comment xml:lang="en">landscape parts represented in the image corpus</rdfs:comment>
    <rdfs:domain rdf:resource="http://purl.org/net/def/metashare#StaticElementInfo"/>
    <rdfs:range rdf:resource="http://www.w3.org/2001/XMLSchema#string"/>
  </owl:DatatypeProperty>
  <owl:DatatypeProperty rdf:about="http://purl.org/net/def/metashare#languageDependent">
    <rdfs:comment xml:lang="en">Indicates whether the operation of the tool or service is language dependent or not</rdfs:comment>
    <rdfs:domain rdf:resource="http://purl.org/net/def/metashare#ToolServiceInfo"/>
    <rdfs:range rdf:resource="http://www.w3.org/2001/XMLSchema#boolean"/>
  </owl:DatatypeProperty>
  <ns:ResourceType rdf:about="http://purl.org/net/def/metashare#languageDescription"/>
  <owl:ObjectProperty rdf:about="http://purl.org/net/def/metashare#languageDescriptionImageInfo">
    <rdfs:comment xml:lang="en">Groups together all information relevant to the image module of a language description (e.g. format, languages, size etc.), if there are any (e.g. for sign language grammars)</rdfs:comment>
    <rdfs:domain rdf:resource="http://purl.org/net/def/metashare#LanguageDescriptionInfo"/>
    <rdfs:range rdf:resource="http://purl.org/net/def/metashare#LanguageDescriptionImageInfo"/>
    <rdfs:subPropertyOf rdf:resource="http://purl.org/net/def/metashare#languageDescriptionMediaPartInfo"/>
  </owl:ObjectProperty>
  <owl:ObjectProperty rdf:about="http://purl.org/net/def/metashare#languageDescriptionInfo">
    <rdfs:comment xml:lang="en">Groups together information on language descriptions (grammars)</rdfs:comment>
    <rdfs:domain rdf:resource="http://purl.org/net/def/metashare#LanguageResource"/>
    <rdfs:range rdf:resource="http://purl.org/net/def/metashare#LanguageDescriptionInfo"/>
  </owl:ObjectProperty>
  <owl:ObjectProperty rdf:about="http://purl.org/net/def/metashare#languageDescriptionMediaPartInfo">
    <rdfs:domain rdf:resource="http://purl.org/net/def/metashare#LanguageDescriptionInfo"/>
    <rdfs:range rdf:resource="http://purl.org/net/def/metashare#LanguageDescriptionMediaPart"/>
    <rdfs:subClassOf rdf:resource="http://purl.org/net/def/metashare#mediaPartInfo"/>
  </owl:ObjectProperty>
  <owl:ObjectProperty rdf:about="http://purl.org/net/def/metashare#languageDescriptionTextInfo">
    <rdfs:comment xml:lang="en">Groups together all information relevant to the text module of a language description (e.g. format, languages, size etc.); it is obligatory for all language descriptions</rdfs:comment>
    <rdfs:domain rdf:resource="http://purl.org/net/def/metashare#LanguageDescriptionInfo"/>
    <rdfs:range rdf:resource="http://purl.org/net/def/metashare#LanguageDescriptionTextInfo"/>
    <rdfs:subPropertyOf rdf:resource="http://purl.org/net/def/metashare#languageDescriptionMediaPartInfo"/>
  </owl:ObjectProperty>
  <owl:ObjectProperty rdf:about="http://purl.org/net/def/metashare#languageDescriptionType">
    <rdfs:comment xml:lang="en">The type of the language description</rdfs:comment>
    <rdfs:domain rdf:resource="http://purl.org/net/def/metashare#LanguageDescriptionInfo"/>
    <rdfs:range rdf:resource="http://purl.org/net/def/metashare#LanguageDescriptionType"/>
  </owl:ObjectProperty>
  <owl:ObjectProperty rdf:about="http://purl.org/net/def/metashare#languageDescriptionVideoInfo">
    <rdfs:comment xml:lang="en">Groups together all information relevant to the video parts of a language description (e.g. format, languages, size etc.), if there are any (e.g. for sign language grammars)</rdfs:comment>
    <rdfs:domain rdf:resource="http://purl.org/net/def/metashare#LanguageDescriptionInfo"/>
    <rdfs:range rdf:resource="http://purl.org/net/def/metashare#LanguageDescriptionVideoInfo"/>
    <rdfs:subPropertyOf rdf:resource="http://purl.org/net/def/metashare#languageDescriptionMediaPartInfo"/>
  </owl:ObjectProperty>
  <ns:ConditionsOfUse rdf:about="http://purl.org/net/def/metashare#languageEngineeringResearch">
    <rdf:type rdf:resource="http://www.w3.org/2002/07/owl#NamedIndividual"/>
    <rdfs:comment xml:lang="en">Language engineering research refers to a kind of 'ConditionsOfUse' imposed by the licence; the resource can only be used for research purposes in the Language Enginnering / Language Technology domain.</rdfs:comment>
    <rdfs:label xml:lang="en">Language Engineering Research</rdfs:label>
  </ns:ConditionsOfUse>
  <ns:UseNLPSpecific rdf:about="http://purl.org/net/def/metashare#languageIdentification"/>
  <owl:ObjectProperty rdf:about="http://purl.org/net/def/metashare#languageInfo">
    <rdfs:comment xml:lang="en">Groups information on the languages represented in the resource</rdfs:comment>
    <rdfs:domain>
      <owl:Class>
        <owl:unionOf>
          <rdf:Description>
            <rdf:first rdf:resource="http://purl.org/net/def/metashare#LexicalConceptualResourceAudioInfo"/>
            <rdf:rest>
              <rdf:Description>
                <rdf:first rdf:resource="http://purl.org/net/def/metashare#LanguageDescriptionTextInfo"/>
                <rdf:rest>
                  <rdf:Description>
                    <rdf:first rdf:resource="http://purl.org/net/def/metashare#LexicalConceptualResourceVideoInfo"/>
                    <rdf:rest>
                      <rdf:Description>
                        <rdf:first rdf:resource="http://purl.org/net/def/metashare#LanguageDescriptionImageInfo"/>
                        <rdf:rest>
                          <rdf:Description>
                            <rdf:first rdf:resource="http://purl.org/net/def/metashare#LexicalConceptualResourceImageInfo"/>
                            <rdf:rest>
                              <rdf:Description>
                                <rdf:first rdf:resource="http://purl.org/net/def/metashare#LexicalConceptualResourceTextInfo"/>
                                <rdf:rest>
                                  <rdf:Description>
                                    <rdf:first rdf:resource="http://purl.org/net/def/metashare#CorpusVideoInfo"/>
                                    <rdf:rest>
                                      <rdf:Description>
                                        <rdf:first rdf:resource="http://purl.org/net/def/metashare#LanguageDescriptionVideoInfo"/>
                                        <rdf:rest>
                                          <rdf:Description>
                                            <rdf:first rdf:resource="http://purl.org/net/def/metashare#CorpusImageInfo"/>
                                            <rdf:rest>
                                              <rdf:Description>
                                                <rdf:first rdf:resource="http://purl.org/net/def/metashare#CorpusTextInfo"/>
                                                <rdf:rest>
                                                  <rdf:Description>
                                                    <rdf:first rdf:resource="http://purl.org/net/def/metashare#CorpusTextNgramInfo"/>
                                                    <rdf:rest>
                                                      <rdf:Description>
                                                        <rdf:first rdf:resource="http://purl.org/net/def/metashare#CorpusAudioInfo"/>
                                                        <rdf:rest rdf:resource="http://www.w3.org/1999/02/22-rdf-syntax-ns#nil"/>
                                                      </rdf:Description>
                                                    </rdf:rest>
                                                  </rdf:Description>
                                                </rdf:rest>
                                              </rdf:Description>
                                            </rdf:rest>
                                          </rdf:Description>
                                        </rdf:rest>
                                      </rdf:Description>
                                    </rdf:rest>
                                  </rdf:Description>
                                </rdf:rest>
                              </rdf:Description>
                            </rdf:rest>
                          </rdf:Description>
                        </rdf:rest>
                      </rdf:Description>
                    </rdf:rest>
                  </rdf:Description>
                </rdf:rest>
              </rdf:Description>
            </rdf:rest>
          </rdf:Description>
        </owl:unionOf>
      </owl:Class>
    </rdfs:domain>
    <rdfs:range>
      <owl:Class>
        <owl:unionOf>
          <rdf:Description>
            <rdf:first rdf:resource="http://purl.org/net/def/metashare#LanguageInfo"/>
            <rdf:rest>
              <rdf:Description>
                <rdf:first rdf:resource="http://purl.org/net/def/metashare#LanguageInfo"/>
                <rdf:rest>
                  <rdf:Description>
                    <rdf:first rdf:resource="http://purl.org/net/def/metashare#LanguageInfo"/>
                    <rdf:rest>
                      <rdf:Description>
                        <rdf:first rdf:resource="http://purl.org/net/def/metashare#LanguageInfo"/>
                        <rdf:rest>
                          <rdf:Description>
                            <rdf:first rdf:resource="http://purl.org/net/def/metashare#LanguageInfo"/>
                            <rdf:rest>
                              <rdf:Description>
                                <rdf:first rdf:resource="http://purl.org/net/def/metashare#LanguageInfo"/>
                                <rdf:rest>
                                  <rdf:Description>
                                    <rdf:first rdf:resource="http://purl.org/net/def/metashare#LanguageInfo"/>
                                    <rdf:rest>
                                      <rdf:Description>
                                        <rdf:first rdf:resource="http://purl.org/net/def/metashare#LanguageInfo"/>
                                        <rdf:rest>
                                          <rdf:Description>
                                            <rdf:first rdf:resource="http://purl.org/net/def/metashare#LanguageInfo"/>
                                            <rdf:rest>
                                              <rdf:Description>
                                                <rdf:first rdf:resource="http://purl.org/net/def/metashare#LanguageInfo"/>
                                                <rdf:rest>
                                                  <rdf:Description>
                                                    <rdf:first rdf:resource="http://purl.org/net/def/metashare#LanguageInfo"/>
                                                    <rdf:rest>
                                                      <rdf:Description>
                                                        <rdf:first rdf:resource="http://purl.org/net/def/metashare#LanguageInfo"/>
                                                        <rdf:rest rdf:resource="http://www.w3.org/1999/02/22-rdf-syntax-ns#nil"/>
                                                      </rdf:Description>
                                                    </rdf:rest>
                                                  </rdf:Description>
                                                </rdf:rest>
                                              </rdf:Description>
                                            </rdf:rest>
                                          </rdf:Description>
                                        </rdf:rest>
                                      </rdf:Description>
                                    </rdf:rest>
                                  </rdf:Description>
                                </rdf:rest>
                              </rdf:Description>
                            </rdf:rest>
                          </rdf:Description>
                        </rdf:rest>
                      </rdf:Description>
                    </rdf:rest>
                  </rdf:Description>
                </rdf:rest>
              </rdf:Description>
            </rdf:rest>
          </rdf:Description>
        </owl:unionOf>
      </owl:Class>
    </rdfs:range>
  </owl:ObjectProperty>
  <ns:UseNLPSpecific rdf:about="http://purl.org/net/def/metashare#languageModelling"/>
  <ns:UseNLPSpecific rdf:about="http://purl.org/net/def/metashare#languageModelsTraining"/>
  <owl:DatatypeProperty rdf:about="http://purl.org/net/def/metashare#languageName">
    <rdfs:comment xml:lang="en">A human understandable name of the language that is used in the resource or supported by the tool/service; an autocompletion mechanism with values from the ISO 639 is provided in the editor, but the values can be subsequently edited for further specification (according to the IETF BCP47 guidelines)</rdfs:comment>
    <rdfs:domain>
      <owl:Class>
        <owl:unionOf>
          <rdf:Description>
            <rdf:first rdf:resource="http://purl.org/net/def/metashare#OutputInfo"/>
            <rdf:rest>
              <rdf:Description>
                <rdf:first rdf:resource="http://purl.org/net/def/metashare#MetadataInfo"/>
                <rdf:rest>
                  <rdf:Description>
                    <rdf:first rdf:resource="http://purl.org/net/def/metashare#DocumentInfo"/>
                    <rdf:rest>
                      <rdf:Description>
                        <rdf:first rdf:resource="http://purl.org/net/def/metashare#InputInfo"/>
                        <rdf:rest>
                          <rdf:Description>
                            <rdf:first rdf:resource="http://purl.org/net/def/metashare#LanguageInfo"/>
                            <rdf:rest rdf:resource="http://www.w3.org/1999/02/22-rdf-syntax-ns#nil"/>
                          </rdf:Description>
                        </rdf:rest>
                      </rdf:Description>
                    </rdf:rest>
                  </rdf:Description>
                </rdf:rest>
              </rdf:Description>
            </rdf:rest>
          </rdf:Description>
        </owl:unionOf>
      </owl:Class>
    </rdfs:domain>
    <rdfs:range rdf:resource="http://www.w3.org/2001/XMLSchema#string"/>
  </owl:DatatypeProperty>
  <owl:DatatypeProperty rdf:about="http://purl.org/net/def/metashare#languageScript">
    <rdfs:comment xml:lang="en">Specifies the writing system used to represent the language in form of a four letter code as it is defined in ISO-15924</rdfs:comment>
    <rdfs:domain rdf:resource="http://purl.org/net/def/metashare#LanguageInfo"/>
    <rdfs:range rdf:resource="http://www.w3.org/2001/XMLSchema#string"/>
  </owl:DatatypeProperty>
  <owl:ObjectProperty rdf:about="http://purl.org/net/def/metashare#languageVarietyInfo">
    <rdfs:comment xml:lang="en">Groups information on language varieties occurred in the resource (e.g. dialects)</rdfs:comment>
    <rdfs:domain rdf:resource="http://purl.org/net/def/metashare#LanguageInfo"/>
    <rdfs:range rdf:resource="http://purl.org/net/def/metashare#LanguageVarietyInfo"/>
  </owl:ObjectProperty>
  <owl:DatatypeProperty rdf:about="http://purl.org/net/def/metashare#languageVarietyName">
    <rdfs:comment xml:lang="en">The name of the language variety that occurs in the resource or is supported by a tool/service</rdfs:comment>
    <rdfs:domain>
      <owl:Class>
        <owl:unionOf>
          <rdf:Description>
            <rdf:first rdf:resource="http://purl.org/net/def/metashare#LanguageVarietyInfo"/>
            <rdf:rest>
              <rdf:Description>
                <rdf:first rdf:resource="http://purl.org/net/def/metashare#InputInfo"/>
                <rdf:rest>
                  <rdf:Description>
                    <rdf:first rdf:resource="http://purl.org/net/def/metashare#OutputInfo"/>
                    <rdf:rest rdf:resource="http://www.w3.org/1999/02/22-rdf-syntax-ns#nil"/>
                  </rdf:Description>
                </rdf:rest>
              </rdf:Description>
            </rdf:rest>
          </rdf:Description>
        </owl:unionOf>
      </owl:Class>
    </rdfs:domain>
    <rdfs:range rdf:resource="http://www.w3.org/2001/XMLSchema#string"/>
  </owl:DatatypeProperty>
  <owl:ObjectProperty rdf:about="http://purl.org/net/def/metashare#languageVarietyType">
    <rdfs:comment xml:lang="en">Specifies the type of the language variety that occurs in the resource or is supported by a tool/service</rdfs:comment>
    <rdfs:domain rdf:resource="http://purl.org/net/def/metashare#LanguageVarietyInfo"/>
    <rdfs:range rdf:resource="http://purl.org/net/def/metashare#LanguageVarietyType"/>
  </owl:ObjectProperty>
  <ns:CapturingDeviceType rdf:about="http://purl.org/net/def/metashare#largeMembraneMicrophone"/>
  <ns:Audience rdf:about="http://purl.org/net/def/metashare#largePublic"/>
  <ns:CapturingDeviceType rdf:about="http://purl.org/net/def/metashare#laryngograph">
    <rdf:type rdf:resource="http://purl.org/net/def/metashare#SourceChannel"/>
  </ns:CapturingDeviceType>
  <ns:CapturingDeviceType rdf:about="http://purl.org/net/def/metashare#lavalierMicrophone"/>
  <ns:RecordingEnvironment rdf:about="http://purl.org/net/def/metashare#lectureRoom"/>
  <ns:BodyParts rdf:about="http://purl.org/net/def/metashare#legs"/>
  <ns:ExtraTextualInformationUnit rdf:about="http://purl.org/net/def/metashare#lemma">
    <rdf:type rdf:resource="http://purl.org/net/def/metashare#LinguisticInformation"/>
  </ns:ExtraTextualInformationUnit>
  <ns:LinguisticInformation rdf:about="http://purl.org/net/def/metashare#lemma-Abbreviations"/>
  <ns:LinguisticInformation rdf:about="http://purl.org/net/def/metashare#lemma-CliticForms"/>
  <ns:LinguisticInformation rdf:about="http://purl.org/net/def/metashare#lemma-Compounds"/>
  <ns:LinguisticInformation rdf:about="http://purl.org/net/def/metashare#lemma-MultiWordUnits"/>
  <ns:LinguisticInformation rdf:about="http://purl.org/net/def/metashare#lemma-Variants"/>
  <ns:AnnotationType rdf:about="http://purl.org/net/def/metashare#lemmatization">
    <rdf:type rdf:resource="http://purl.org/net/def/metashare#UseNLPSpecific"/>
  </ns:AnnotationType>
  <ns:BaseItem rdf:about="http://purl.org/net/def/metashare#letter"/>
  <ns:ResourceType rdf:about="http://purl.org/net/def/metashare#lexicalConceptualResource"/>
  <owl:ObjectProperty rdf:about="http://purl.org/net/def/metashare#lexicalConceptualResourceAudioInfo">
    <rdfs:comment xml:lang="en">Groups information on the audio part of the lexical/conceptual resource</rdfs:comment>
    <rdfs:domain rdf:resource="http://purl.org/net/def/metashare#LexicalConceptualResourceInfo"/>
    <rdfs:range rdf:resource="http://purl.org/net/def/metashare#LexicalConceptualResourceAudioInfo"/>
    <rdfs:subPropertyOf rdf:resource="http://purl.org/net/def/metashare#lexicalConceptualResourceMediaPartInfo"/>
  </owl:ObjectProperty>
  <owl:ObjectProperty rdf:about="http://purl.org/net/def/metashare#lexicalConceptualResourceImageInfo">
    <rdfs:comment xml:lang="en">Groups information on the image part of the lexical/conceptual resource</rdfs:comment>
    <rdfs:domain rdf:resource="http://purl.org/net/def/metashare#LexicalConceptualResourceInfo"/>
    <rdfs:range rdf:resource="http://purl.org/net/def/metashare#LexicalConceptualResourceImageInfo"/>
    <rdfs:subPropertyOf rdf:resource="http://purl.org/net/def/metashare#lexicalConceptualResourceMediaPartInfo"/>
  </owl:ObjectProperty>
  <owl:ObjectProperty rdf:about="http://purl.org/net/def/metashare#lexicalConceptualResourceInfo">
    <rdfs:comment xml:lang="en">Groups together information specific to lexical/conceptual resources</rdfs:comment>
    <rdfs:domain rdf:resource="http://purl.org/net/def/metashare#LanguageResource"/>
    <rdfs:range rdf:resource="http://purl.org/net/def/metashare#LexicalConceptualResourceInfo"/>
  </owl:ObjectProperty>
  <owl:ObjectProperty rdf:about="http://purl.org/net/def/metashare#lexicalConceptualResourceMediaPartInfo">
    <rdfs:domain rdf:resource="http://purl.org/net/def/metashare#LexicalConceptualResourceInfo"/>
    <rdfs:range rdf:resource="http://purl.org/net/def/metashare#LexicalConceptualResourceMediaPart"/>
    <rdfs:subPropertyOf rdf:resource="http://purl.org/net/def/metashare#mediaPartInfo"/>
  </owl:ObjectProperty>
  <owl:ObjectProperty rdf:about="http://purl.org/net/def/metashare#lexicalConceptualResourceTextInfo">
    <rdfs:comment xml:lang="en">Groups information on the textual part of the lexical/conceptual resource</rdfs:comment>
    <rdfs:domain rdf:resource="http://purl.org/net/def/metashare#LexicalConceptualResourceInfo"/>
    <rdfs:range rdf:resource="http://purl.org/net/def/metashare#LexicalConceptualResourceTextInfo"/>
    <rdfs:subPropertyOf rdf:resource="http://purl.org/net/def/metashare#lexicalConceptualResourceMediaPartInfo"/>
  </owl:ObjectProperty>
  <owl:ObjectProperty rdf:about="http://purl.org/net/def/metashare#lexicalConceptualResourceType">
    <rdfs:comment xml:lang="en">Specifies the subtype of lexicalConceptualResource</rdfs:comment>
    <rdfs:domain rdf:resource="http://purl.org/net/def/metashare#LexicalConceptualResourceInfo"/>
    <rdfs:range rdf:resource="http://purl.org/net/def/metashare#LexicalConceptualResourceType"/>
  </owl:ObjectProperty>
  <owl:ObjectProperty rdf:about="http://purl.org/net/def/metashare#lexicalConceptualResourceVideoInfo">
    <rdfs:comment xml:lang="en">Groups information on the video part of the lexical conceptual resource</rdfs:comment>
    <rdfs:domain rdf:resource="http://purl.org/net/def/metashare#LexicalConceptualResourceInfo"/>
    <rdfs:range rdf:resource="http://purl.org/net/def/metashare#LexicalConceptualResourceVideoInfo"/>
    <rdfs:subPropertyOf rdf:resource="http://purl.org/net/def/metashare#lexicalConceptualResourceMediaPartInfo"/>
  </owl:ObjectProperty>
  <ns:SizeUnit rdf:about="http://purl.org/net/def/metashare#lexicalTypes"/>
  <ns:ExtraTextualInformationUnit rdf:about="http://purl.org/net/def/metashare#lexicalUnit"/>
  <ns:CompatibleLexiconType rdf:about="http://purl.org/net/def/metashare#lexicon">
    <rdf:type rdf:resource="http://purl.org/net/def/metashare#LexicalConceptualResourceType"/>
  </ns:CompatibleLexiconType>
  <ns:UseNLPSpecific rdf:about="http://purl.org/net/def/metashare#lexiconAccess"/>
  <ns:UseNLPSpecific rdf:about="http://purl.org/net/def/metashare#lexiconAcquisitionFromCorpora"/>
  <ns:UseNLPSpecific rdf:about="http://purl.org/net/def/metashare#lexiconEnhancement"/>
  <ns:UseNLPSpecific rdf:about="http://purl.org/net/def/metashare#lexiconExtractionFromLexica"/>
  <ns:UseNLPSpecific rdf:about="http://purl.org/net/def/metashare#lexiconFormatConversion"/>
  <ns:UseNLPSpecific rdf:about="http://purl.org/net/def/metashare#lexiconMerging"/>
  <ns:UseNLPSpecific rdf:about="http://purl.org/net/def/metashare#lexiconVisualization"/>
  <ns:ConformanceToClassificationScheme rdf:about="http://purl.org/net/def/metashare#libraryOfCongress_domainClassification"/>
  <ns:ConformanceToClassificationScheme rdf:about="http://purl.org/net/def/metashare#libraryofCongressSubjectHeadings_classification"/>
  <owl:ObjectProperty rdf:about="http://purl.org/net/def/metashare#licenseCategory">
    <rdfs:comment xml:lang="en">A way of categorising licences into three main categories: PUB, ACA or RES, according to CLARIN recommendations (cf. https://kitwiki.csc.fi/twiki/bin/view/FinCLARIN/ClarinLC)</rdfs:comment>
    <rdfs:domain rdf:resource="http://purl.org/net/def/metashare#License"/>
    <rdfs:label xml:lang="en">License Category</rdfs:label>
    <rdfs:range rdf:resource="http://purl.org/net/def/metashare#LicenseCategory"/>
  </owl:ObjectProperty>
  <rdf:Description rdf:about="http://purl.org/net/def/metashare#licenseInfo">
    <rdfs:comment xml:lang="en">Links a resource to the licence under which it is distributed; values are taken from a list of standard licences</rdfs:comment>
  </rdf:Description>
  <owl:ObjectProperty rdf:about="http://purl.org/net/def/metashare#licensor">
    <rdfs:comment xml:lang="en">Groups information on the person who is legally eligible to licence and actually licenses the resource. The licensor could be different from the creator, the distributor or the IP rightsholder. The licensor has the necessary rights or licences to license the work and is the party that actually licenses the resource that enters the META-SHARE network. She will have obtained the necessary rights or licences from the IPR holder and she may have a distribution agreement with a distributor that disseminates the work under a set of conditions defined in the specific licence and collects revenue on the licensor's behalf. The attribution of the creator, separately from the attribution of the licensor, may be part of the licence under which the resource is distributed (as e.g. is the case with Creative Commons Licences)</rdfs:comment>
    <rdfs:comment xml:lang="en">The person who is legally eligible to license and actually licenses the resource. The licensor could be different from the creator, the distributor or the IPR holder. The licensor has the necessary rights or licences to license the work and is the party that actually licenses the resource that is distributed via the specific channel. She will have obtained the necessary rights or licences from the IPR holder and she may have a distribution agreement with a distributor that disseminates the work under a set of conditions defined in the specific  licence and collects revenue on the licensor's behalf. The attribution of the creator, separately from the attribution of the licensor, may be part of the licence under which the resource is distributed (as e.g. is the case with Creative Commons Licences).</rdfs:comment>
    <rdfs:domain rdf:resource="http://purl.org/net/def/metashare#LicenceInfo"/>
    <rdfs:range rdf:resource="http://purl.org/net/def/metashare#Actor"/>
  </owl:ObjectProperty>
  <ns:SignalEncoding rdf:about="http://purl.org/net/def/metashare#linearPCM"/>
  <owl:ObjectProperty rdf:about="http://purl.org/net/def/metashare#lingualityType">
    <rdfs:comment xml:lang="en">Indicates whether the resource includes one, two or more languages</rdfs:comment>
    <rdfs:domain>
      <owl:Class>
        <owl:unionOf>
          <rdf:Description>
            <rdf:first rdf:resource="http://purl.org/net/def/metashare#CorpusAudioInfo"/>
            <rdf:rest>
              <rdf:Description>
                <rdf:first rdf:resource="http://purl.org/net/def/metashare#LanguageDescriptionVideoInfo"/>
                <rdf:rest>
                  <rdf:Description>
                    <rdf:first rdf:resource="http://purl.org/net/def/metashare#CorpusVideoInfo"/>
                    <rdf:rest>
                      <rdf:Description>
                        <rdf:first rdf:resource="http://purl.org/net/def/metashare#LexicalConceptualResourceVideoInfo"/>
                        <rdf:rest>
                          <rdf:Description>
                            <rdf:first rdf:resource="http://purl.org/net/def/metashare#LexicalConceptualResourceAudioInfo"/>
                            <rdf:rest>
                              <rdf:Description>
                                <rdf:first rdf:resource="http://purl.org/net/def/metashare#CorpusImageInfo"/>
                                <rdf:rest>
                                  <rdf:Description>
                                    <rdf:first rdf:resource="http://purl.org/net/def/metashare#LanguageDescriptionImageInfo"/>
                                    <rdf:rest>
                                      <rdf:Description>
                                        <rdf:first rdf:resource="http://purl.org/net/def/metashare#LanguageDescriptionTextInfo"/>
                                        <rdf:rest>
                                          <rdf:Description>
                                            <rdf:first rdf:resource="http://purl.org/net/def/metashare#CorpusTextNgramInfo"/>
                                            <rdf:rest>
                                              <rdf:Description>
                                                <rdf:first rdf:resource="http://purl.org/net/def/metashare#CorpusTextInfo"/>
                                                <rdf:rest>
                                                  <rdf:Description>
                                                    <rdf:first rdf:resource="http://purl.org/net/def/metashare#LexicalConceptualResourceImageInfo"/>
                                                    <rdf:rest>
                                                      <rdf:Description>
                                                        <rdf:first rdf:resource="http://purl.org/net/def/metashare#LexicalConceptualResourceTextInfo"/>
                                                        <rdf:rest rdf:resource="http://www.w3.org/1999/02/22-rdf-syntax-ns#nil"/>
                                                      </rdf:Description>
                                                    </rdf:rest>
                                                  </rdf:Description>
                                                </rdf:rest>
                                              </rdf:Description>
                                            </rdf:rest>
                                          </rdf:Description>
                                        </rdf:rest>
                                      </rdf:Description>
                                    </rdf:rest>
                                  </rdf:Description>
                                </rdf:rest>
                              </rdf:Description>
                            </rdf:rest>
                          </rdf:Description>
                        </rdf:rest>
                      </rdf:Description>
                    </rdf:rest>
                  </rdf:Description>
                </rdf:rest>
              </rdf:Description>
            </rdf:rest>
          </rdf:Description>
        </owl:unionOf>
      </owl:Class>
    </rdfs:domain>
    <rdfs:range>
      <owl:Class>
        <owl:unionOf>
          <rdf:Description>
            <rdf:first rdf:resource="http://purl.org/net/def/metashare#LingualityType"/>
            <rdf:rest>
              <rdf:Description>
                <rdf:first rdf:resource="http://purl.org/net/def/metashare#LingualityType"/>
                <rdf:rest>
                  <rdf:Description>
                    <rdf:first rdf:resource="http://purl.org/net/def/metashare#LingualityType"/>
                    <rdf:rest>
                      <rdf:Description>
                        <rdf:first rdf:resource="http://purl.org/net/def/metashare#LingualityType"/>
                        <rdf:rest>
                          <rdf:Description>
                            <rdf:first rdf:resource="http://purl.org/net/def/metashare#LingualityType"/>
                            <rdf:rest>
                              <rdf:Description>
                                <rdf:first rdf:resource="http://purl.org/net/def/metashare#LingualityType"/>
                                <rdf:rest>
                                  <rdf:Description>
                                    <rdf:first rdf:resource="http://purl.org/net/def/metashare#LingualityType"/>
                                    <rdf:rest>
                                      <rdf:Description>
                                        <rdf:first rdf:resource="http://purl.org/net/def/metashare#LingualityType"/>
                                        <rdf:rest>
                                          <rdf:Description>
                                            <rdf:first rdf:resource="http://purl.org/net/def/metashare#LingualityType"/>
                                            <rdf:rest>
                                              <rdf:Description>
                                                <rdf:first rdf:resource="http://purl.org/net/def/metashare#LingualityType"/>
                                                <rdf:rest>
                                                  <rdf:Description>
                                                    <rdf:first rdf:resource="http://purl.org/net/def/metashare#LingualityType"/>
                                                    <rdf:rest>
                                                      <rdf:Description>
                                                        <rdf:first rdf:resource="http://purl.org/net/def/metashare#LingualityType"/>
                                                        <rdf:rest rdf:resource="http://www.w3.org/1999/02/22-rdf-syntax-ns#nil"/>
                                                      </rdf:Description>
                                                    </rdf:rest>
                                                  </rdf:Description>
                                                </rdf:rest>
                                              </rdf:Description>
                                            </rdf:rest>
                                          </rdf:Description>
                                        </rdf:rest>
                                      </rdf:Description>
                                    </rdf:rest>
                                  </rdf:Description>
                                </rdf:rest>
                              </rdf:Description>
                            </rdf:rest>
                          </rdf:Description>
                        </rdf:rest>
                      </rdf:Description>
                    </rdf:rest>
                  </rdf:Description>
                </rdf:rest>
              </rdf:Description>
            </rdf:rest>
          </rdf:Description>
        </owl:unionOf>
      </owl:Class>
    </rdfs:range>
  </owl:ObjectProperty>
  <owl:ObjectProperty rdf:about="http://purl.org/net/def/metashare#linguisticInformation">
    <rdfs:comment xml:lang="en">A more detailed account of the linguistic information contained in the lexicalConceptualResource</rdfs:comment>
    <rdfs:domain rdf:resource="http://purl.org/net/def/metashare#LexicalConceptualResourceInfo"/>
    <rdfs:range rdf:resource="http://purl.org/net/def/metashare#LinguisticInformation"/>
  </owl:ObjectProperty>
  <ns:UseNLPSpecific rdf:about="http://purl.org/net/def/metashare#linguisticResearch"/>
  <owl:ObjectProperty rdf:about="http://purl.org/net/def/metashare#linkToOtherMediaInfo">
    <rdfs:comment xml:lang="en">Groups information on the way different media of the resource interact with or link to each other. To be used for multimodal resources or for resources representing sensorimotor data</rdfs:comment>
    <rdfs:domain>
      <owl:Class>
        <owl:unionOf>
          <rdf:Description>
            <rdf:first rdf:resource="http://purl.org/net/def/metashare#CorpusTextNumericalInfo"/>
            <rdf:rest>
              <rdf:Description>
                <rdf:first rdf:resource="http://purl.org/net/def/metashare#LanguageDescriptionTextInfo"/>
                <rdf:rest>
                  <rdf:Description>
                    <rdf:first rdf:resource="http://purl.org/net/def/metashare#CorpusImageInfo"/>
                    <rdf:rest>
                      <rdf:Description>
                        <rdf:first rdf:resource="http://purl.org/net/def/metashare#LanguageDescriptionVideoInfo"/>
                        <rdf:rest>
                          <rdf:Description>
                            <rdf:first rdf:resource="http://purl.org/net/def/metashare#CorpusVideoInfo"/>
                            <rdf:rest>
                              <rdf:Description>
                                <rdf:first rdf:resource="http://purl.org/net/def/metashare#CorpusTextInfo"/>
                                <rdf:rest>
                                  <rdf:Description>
                                    <rdf:first rdf:resource="http://purl.org/net/def/metashare#CorpusAudioInfo"/>
                                    <rdf:rest>
                                      <rdf:Description>
                                        <rdf:first rdf:resource="http://purl.org/net/def/metashare#LanguageDescriptionImageInfo"/>
                                        <rdf:rest rdf:resource="http://www.w3.org/1999/02/22-rdf-syntax-ns#nil"/>
                                      </rdf:Description>
                                    </rdf:rest>
                                  </rdf:Description>
                                </rdf:rest>
                              </rdf:Description>
                            </rdf:rest>
                          </rdf:Description>
                        </rdf:rest>
                      </rdf:Description>
                    </rdf:rest>
                  </rdf:Description>
                </rdf:rest>
              </rdf:Description>
            </rdf:rest>
          </rdf:Description>
        </owl:unionOf>
      </owl:Class>
    </rdfs:domain>
    <rdfs:range>
      <owl:Class>
        <owl:unionOf>
          <rdf:Description>
            <rdf:first rdf:resource="http://purl.org/net/def/metashare#LinkToOtherMediaInfo"/>
            <rdf:rest>
              <rdf:Description>
                <rdf:first rdf:resource="http://purl.org/net/def/metashare#LinkToOtherMediaInfo"/>
                <rdf:rest>
                  <rdf:Description>
                    <rdf:first rdf:resource="http://purl.org/net/def/metashare#LinkToOtherMediaInfo"/>
                    <rdf:rest>
                      <rdf:Description>
                        <rdf:first rdf:resource="http://purl.org/net/def/metashare#LinkToOtherMediaInfo"/>
                        <rdf:rest>
                          <rdf:Description>
                            <rdf:first rdf:resource="http://purl.org/net/def/metashare#LinkToOtherMediaInfo"/>
                            <rdf:rest>
                              <rdf:Description>
                                <rdf:first rdf:resource="http://purl.org/net/def/metashare#LinkToOtherMediaInfo"/>
                                <rdf:rest>
                                  <rdf:Description>
                                    <rdf:first rdf:resource="http://purl.org/net/def/metashare#LinkToOtherMediaInfo"/>
                                    <rdf:rest>
                                      <rdf:Description>
                                        <rdf:first rdf:resource="http://purl.org/net/def/metashare#LinkToOtherMediaInfo"/>
                                        <rdf:rest rdf:resource="http://www.w3.org/1999/02/22-rdf-syntax-ns#nil"/>
                                      </rdf:Description>
                                    </rdf:rest>
                                  </rdf:Description>
                                </rdf:rest>
                              </rdf:Description>
                            </rdf:rest>
                          </rdf:Description>
                        </rdf:rest>
                      </rdf:Description>
                    </rdf:rest>
                  </rdf:Description>
                </rdf:rest>
              </rdf:Description>
            </rdf:rest>
          </rdf:Description>
        </owl:unionOf>
      </owl:Class>
    </rdfs:range>
  </owl:ObjectProperty>
  <ns:OperatingSystem rdf:about="http://purl.org/net/def/metashare#linux"/>
  <ns:UseNLPSpecific rdf:about="http://purl.org/net/def/metashare#lipTrackingAnalysis"/>
  <ns:ByteOrder rdf:about="http://purl.org/net/def/metashare#littleEndian"/>
  <ns:NoiseLevel rdf:about="http://purl.org/net/def/metashare#low">
    <rdf:type rdf:resource="http://purl.org/net/def/metashare#Quality"/>
    <rdf:type rdf:resource="http://purl.org/net/def/metashare#RecordingQuality"/>
  </ns:NoiseLevel>
  <ns:OperatingSystem rdf:about="http://purl.org/net/def/metashare#mac-OS"/>
  <ns:CompatibleLexiconType rdf:about="http://purl.org/net/def/metashare#machineReadableDictionary">
    <rdf:type rdf:resource="http://purl.org/net/def/metashare#LexicalConceptualResourceType"/>
  </ns:CompatibleLexiconType>
  <ns:UseNLPSpecific rdf:about="http://purl.org/net/def/metashare#machineTranslation"/>
  <ns:SexOfPersons rdf:about="http://purl.org/net/def/metashare#male"/>
  <ns:AnnotationMode rdf:about="http://purl.org/net/def/metashare#manual">
    <rdf:type rdf:resource="http://purl.org/net/def/metashare#CreationMode"/>
    <rdf:type rdf:resource="http://purl.org/net/def/metashare#ToolDocumentationType"/>
    <rdf:type rdf:resource="http://purl.org/net/def/metashare#ValidationMode"/>
  </ns:AnnotationMode>
  <ns:ScenarioType rdf:about="http://purl.org/net/def/metashare#mapTask"/>
  <ns:SizeUnit rdf:about="http://purl.org/net/def/metashare#mb"/>
  <owl:ObjectProperty rdf:about="http://purl.org/net/def/metashare#mediaPartInfo"/>
  <owl:ObjectProperty rdf:about="http://purl.org/net/def/metashare#mediaType">
    <rdfs:comment xml:lang="en">Specifies the media type of the resource and basically corresponds to the physical medium of the content representation. Each media type is described through a 				distinctive set of features. A resource may consist of parts attributed to different types of media.</rdfs:comment>
    <rdfs:domain>
      <owl:Class>
        <owl:unionOf>
          <rdf:Description>
            <rdf:first rdf:resource="http://purl.org/net/def/metashare#LanguageDescriptionVideoInfo"/>
            <rdf:rest>
              <rdf:Description>
                <rdf:first rdf:resource="http://purl.org/net/def/metashare#CorpusTextNumericalInfo"/>
                <rdf:rest>
                  <rdf:Description>
                    <rdf:first rdf:resource="http://purl.org/net/def/metashare#LexicalConceptualResourceTextInfo"/>
                    <rdf:rest>
                      <rdf:Description>
                        <rdf:first rdf:resource="http://purl.org/net/def/metashare#LexicalConceptualResourceAudioInfo"/>
                        <rdf:rest>
                          <rdf:Description>
                            <rdf:first rdf:resource="http://purl.org/net/def/metashare#CorpusTextNgramInfo"/>
                            <rdf:rest>
                              <rdf:Description>
                                <rdf:first rdf:resource="http://purl.org/net/def/metashare#LanguageDescriptionTextInfo"/>
                                <rdf:rest>
                                  <rdf:Description>
                                    <rdf:first rdf:resource="http://purl.org/net/def/metashare#LexicalConceptualResourceImageInfo"/>
                                    <rdf:rest>
                                      <rdf:Description>
                                        <rdf:first rdf:resource="http://purl.org/net/def/metashare#CorpusImageInfo"/>
                                        <rdf:rest>
                                          <rdf:Description>
                                            <rdf:first rdf:resource="http://purl.org/net/def/metashare#CorpusVideoInfo"/>
                                            <rdf:rest>
                                              <rdf:Description>
                                                <rdf:first rdf:resource="http://purl.org/net/def/metashare#OutputInfo"/>
                                                <rdf:rest>
                                                  <rdf:Description>
                                                    <rdf:first rdf:resource="http://purl.org/net/def/metashare#CorpusAudioInfo"/>
                                                    <rdf:rest>
                                                      <rdf:Description>
                                                        <rdf:first rdf:resource="http://purl.org/net/def/metashare#InputInfo"/>
                                                        <rdf:rest>
                                                          <rdf:Description>
                                                            <rdf:first rdf:resource="http://purl.org/net/def/metashare#CorpusTextInfo"/>
                                                            <rdf:rest>
                                                              <rdf:Description>
                                                                <rdf:first rdf:resource="http://purl.org/net/def/metashare#LexicalConceptualResourceVideoInfo"/>
                                                                <rdf:rest>
                                                                  <rdf:Description>
                                                                    <rdf:first rdf:resource="http://purl.org/net/def/metashare#LanguageDescriptionImageInfo"/>
                                                                    <rdf:rest rdf:resource="http://www.w3.org/1999/02/22-rdf-syntax-ns#nil"/>
                                                                  </rdf:Description>
                                                                </rdf:rest>
                                                              </rdf:Description>
                                                            </rdf:rest>
                                                          </rdf:Description>
                                                        </rdf:rest>
                                                      </rdf:Description>
                                                    </rdf:rest>
                                                  </rdf:Description>
                                                </rdf:rest>
                                              </rdf:Description>
                                            </rdf:rest>
                                          </rdf:Description>
                                        </rdf:rest>
                                      </rdf:Description>
                                    </rdf:rest>
                                  </rdf:Description>
                                </rdf:rest>
                              </rdf:Description>
                            </rdf:rest>
                          </rdf:Description>
                        </rdf:rest>
                      </rdf:Description>
                    </rdf:rest>
                  </rdf:Description>
                </rdf:rest>
              </rdf:Description>
            </rdf:rest>
          </rdf:Description>
        </owl:unionOf>
      </owl:Class>
    </rdfs:domain>
    <rdfs:range>
      <owl:Class>
        <owl:unionOf>
          <rdf:Description>
            <rdf:first rdf:resource="http://purl.org/net/def/metashare#MediaType"/>
            <rdf:rest>
              <rdf:Description>
                <rdf:first rdf:resource="http://purl.org/net/def/metashare#MediaType"/>
                <rdf:rest>
                  <rdf:Description>
                    <rdf:first rdf:resource="http://purl.org/net/def/metashare#MediaType"/>
                    <rdf:rest>
                      <rdf:Description>
                        <rdf:first rdf:resource="http://purl.org/net/def/metashare#MediaType"/>
                        <rdf:rest>
                          <rdf:Description>
                            <rdf:first rdf:resource="http://purl.org/net/def/metashare#MediaType"/>
                            <rdf:rest>
                              <rdf:Description>
                                <rdf:first rdf:resource="http://purl.org/net/def/metashare#MediaType"/>
                                <rdf:rest>
                                  <rdf:Description>
                                    <rdf:first rdf:resource="http://purl.org/net/def/metashare#MediaType"/>
                                    <rdf:rest>
                                      <rdf:Description>
                                        <rdf:first rdf:resource="http://purl.org/net/def/metashare#MediaType"/>
                                        <rdf:rest>
                                          <rdf:Description>
                                            <rdf:first rdf:resource="http://purl.org/net/def/metashare#MediaType"/>
                                            <rdf:rest>
                                              <rdf:Description>
                                                <rdf:first rdf:resource="http://purl.org/net/def/metashare#MediaType"/>
                                                <rdf:rest>
                                                  <rdf:Description>
                                                    <rdf:first rdf:resource="http://purl.org/net/def/metashare#MediaType"/>
                                                    <rdf:rest>
                                                      <rdf:Description>
                                                        <rdf:first rdf:resource="http://purl.org/net/def/metashare#MediaType"/>
                                                        <rdf:rest>
                                                          <rdf:Description>
                                                            <rdf:first rdf:resource="http://purl.org/net/def/metashare#MediaType"/>
                                                            <rdf:rest>
                                                              <rdf:Description>
                                                                <rdf:first rdf:resource="http://purl.org/net/def/metashare#MediaType"/>
                                                                <rdf:rest>
                                                                  <rdf:Description>
                                                                    <rdf:first rdf:resource="http://purl.org/net/def/metashare#MediaType"/>
                                                                    <rdf:rest rdf:resource="http://www.w3.org/1999/02/22-rdf-syntax-ns#nil"/>
                                                                  </rdf:Description>
                                                                </rdf:rest>
                                                              </rdf:Description>
                                                            </rdf:rest>
                                                          </rdf:Description>
                                                        </rdf:rest>
                                                      </rdf:Description>
                                                    </rdf:rest>
                                                  </rdf:Description>
                                                </rdf:rest>
                                              </rdf:Description>
                                            </rdf:rest>
                                          </rdf:Description>
                                        </rdf:rest>
                                      </rdf:Description>
                                    </rdf:rest>
                                  </rdf:Description>
                                </rdf:rest>
                              </rdf:Description>
                            </rdf:rest>
                          </rdf:Description>
                        </rdf:rest>
                      </rdf:Description>
                    </rdf:rest>
                  </rdf:Description>
                </rdf:rest>
              </rdf:Description>
            </rdf:rest>
          </rdf:Description>
        </owl:unionOf>
      </owl:Class>
    </rdfs:range>
  </owl:ObjectProperty>
  <owl:DatatypeProperty rdf:about="http://purl.org/net/def/metashare#mediaTypeDetails">
    <rdfs:comment xml:lang="en">Provides further information on the way the media types are linked and/or synchronized with each other within the same resource</rdfs:comment>
    <rdfs:domain rdf:resource="http://purl.org/net/def/metashare#LinkToOtherMediaInfo"/>
    <rdfs:range rdf:resource="http://www.w3.org/2001/XMLSchema#string"/>
  </owl:DatatypeProperty>
  <ns:SpeechInfluences rdf:about="http://purl.org/net/def/metashare#medication"/>
  <ns:NoiseLevel rdf:about="http://purl.org/net/def/metashare#medium">
    <rdf:type rdf:resource="http://purl.org/net/def/metashare#Quality"/>
    <rdf:type rdf:resource="http://purl.org/net/def/metashare#RecordingQuality"/>
  </ns:NoiseLevel>
  <owl:DatatypeProperty rdf:about="http://purl.org/net/def/metashare#member">
    <rdfs:comment xml:lang="en">Whether the user is a member or not</rdfs:comment>
    <rdfs:domain rdf:resource="http://purl.org/net/def/metashare#MembershipInfo"/>
    <rdfs:range rdf:resource="http://www.w3.org/2001/XMLSchema#boolean"/>
  </owl:DatatypeProperty>
  <ns:UserNature rdf:about="http://purl.org/net/def/metashare#memberOfELRA">
    <rdfs:comment xml:lang="en">Used for stating pricing privileges for members of ELRA with regard to the distribution of a resource</rdfs:comment>
  </ns:UserNature>
  <ns:UserNature rdf:about="http://purl.org/net/def/metashare#memberOfLDC">
    <rdfs:comment xml:lang="en">Used for stating pricing privileges for members of LDC with regard to the distribution of a resource</rdfs:comment>
  </ns:UserNature>
  <ns:UserNature rdf:about="http://purl.org/net/def/metashare#memberOfTST-Centrale">
    <rdfs:comment xml:lang="en">Used for stating pricing privileges for members of TST-Centrale with regard to the distribution of a resource</rdfs:comment>
  </ns:UserNature>
  <owl:ObjectProperty rdf:about="http://purl.org/net/def/metashare#membershipInfo">
    <rdfs:comment xml:lang="en">The conditions imposed by the user being member of some association/institution (e.g., ELRA, LDC) distributing the resource. This indicates the availability conditions (and prices) for users who are members or not</rdfs:comment>
    <rdfs:domain rdf:resource="http://purl.org/net/def/metashare#LicenceInfo"/>
    <rdfs:range rdf:resource="http://purl.org/net/def/metashare#MembershipInfo"/>
  </owl:ObjectProperty>
  <owl:ObjectProperty rdf:about="http://purl.org/net/def/metashare#membershipInstitution">
    <rdfs:comment xml:lang="en">This lists the different institutions releasing the resources and establishing membership conditions</rdfs:comment>
    <rdfs:domain rdf:resource="http://purl.org/net/def/metashare#MembershipInfo"/>
    <rdfs:range rdf:resource="http://purl.org/net/def/metashare#MembershipInstitution"/>
  </owl:ObjectProperty>
  <owl:DatatypeProperty rdf:about="http://purl.org/net/def/metashare#metaShareId">
    <rdfs:comment xml:lang="en">An unambiguous referent to the resource within META-SHARE; it reflects to the unique system id provided automatically by the MetaShare software</rdfs:comment>
    <rdfs:domain rdf:resource="http://purl.org/net/def/metashare#LanguageResource"/>
    <rdfs:range rdf:resource="http://www.w3.org/2001/XMLSchema#string"/>
  </owl:DatatypeProperty>
  <owl:DatatypeProperty rdf:about="http://purl.org/net/def/metashare#metadataSource">
    <rdfs:comment xml:lang="en">Refers to the catalogue or repository from which the metadata has been originated.</rdfs:comment>
    <rdfs:domain rdf:resource="http://purl.org/net/def/metashare#LanguageResource"/>
    <rdfs:range rdf:resource="http://www.w3.org/2001/XMLSchema#anyURI"/>
  </owl:DatatypeProperty>
  <ns:CapturingDeviceType rdf:about="http://purl.org/net/def/metashare#microphone">
    <rdf:type rdf:resource="http://purl.org/net/def/metashare#RequiredHardware"/>
  </ns:CapturingDeviceType>
  <ns:CapturingDeviceType rdf:about="http://purl.org/net/def/metashare#microphoneArray"/>
  <owl:DatatypeProperty rdf:about="http://purl.org/net/def/metashare#mimeType">
    <rdfs:comment xml:lang="en">The mime-type of the resource which is a formalized specifier for the format included or a mime-type that the tool/service accepts; value to be taken from a subset of the official mime types of the Internet Assigned Numbers Authority (http://www.iana.org/)</rdfs:comment>
    <rdfs:domain>
      <owl:Class>
        <owl:unionOf>
          <rdf:Description>
            <rdf:first rdf:resource="http://purl.org/net/def/metashare#OutputInfo"/>
            <rdf:rest>
              <rdf:Description>
                <rdf:first rdf:resource="http://purl.org/net/def/metashare#InputInfo"/>
                <rdf:rest rdf:resource="http://www.w3.org/1999/02/22-rdf-syntax-ns#nil"/>
              </rdf:Description>
            </rdf:rest>
          </rdf:Description>
        </owl:unionOf>
      </owl:Class>
    </rdfs:domain>
    <rdfs:range rdf:resource="http://www.w3.org/2001/XMLSchema#string"/>
  </owl:DatatypeProperty>
  <ns:DurationOfAudioInfoUnit rdf:about="http://purl.org/net/def/metashare#minutes">
    <rdf:type rdf:resource="http://purl.org/net/def/metashare#DurationOfEffectiveSpeechInfoUnit"/>
    <rdf:type rdf:resource="http://purl.org/net/def/metashare#SizeUnit"/>
  </ns:DurationOfAudioInfoUnit>
  <ns:AnnotatedElements rdf:about="http://purl.org/net/def/metashare#mispronunciations"/>
  <ns:AnnotationMode rdf:about="http://purl.org/net/def/metashare#mixed">
    <rdf:type rdf:resource="http://purl.org/net/def/metashare#CreationMode"/>
    <rdf:type rdf:resource="http://purl.org/net/def/metashare#HearingImpairmentOfPersons"/>
    <rdf:type rdf:resource="http://purl.org/net/def/metashare#OriginOfPersons"/>
    <rdf:type rdf:resource="http://purl.org/net/def/metashare#SexOfPersons"/>
    <rdf:type rdf:resource="http://purl.org/net/def/metashare#SpeakingImpairmentOfPersons"/>
    <rdf:type rdf:resource="http://purl.org/net/def/metashare#ValidationMode"/>
  </ns:AnnotationMode>
  <ns:ModalityAnnotation rdf:about="http://purl.org/net/def/metashare#modalityAnnotation-bodyMovements">
    <rdf:type rdf:resource="http://purl.org/net/def/metashare#AnnotationType"/>
  </ns:ModalityAnnotation>
  <ns:ModalityAnnotation rdf:about="http://purl.org/net/def/metashare#modalityAnnotation-facialExpressions">
    <rdf:type rdf:resource="http://purl.org/net/def/metashare#AnnotationType"/>
  </ns:ModalityAnnotation>
  <ns:ModalityAnnotation rdf:about="http://purl.org/net/def/metashare#modalityAnnotation-gazeEyeMovements">
    <rdf:type rdf:resource="http://purl.org/net/def/metashare#AnnotationType"/>
  </ns:ModalityAnnotation>
  <ns:ModalityAnnotation rdf:about="http://purl.org/net/def/metashare#modalityAnnotation-handArmGestures">
    <rdf:type rdf:resource="http://purl.org/net/def/metashare#AnnotationType"/>
  </ns:ModalityAnnotation>
  <ns:ModalityAnnotation rdf:about="http://purl.org/net/def/metashare#modalityAnnotation-handManipulationOfObjects">
    <rdf:type rdf:resource="http://purl.org/net/def/metashare#AnnotationType"/>
  </ns:ModalityAnnotation>
  <ns:ModalityAnnotation rdf:about="http://purl.org/net/def/metashare#modalityAnnotation-headMovements">
    <rdf:type rdf:resource="http://purl.org/net/def/metashare#AnnotationType"/>
  </ns:ModalityAnnotation>
  <ns:ModalityAnnotation rdf:about="http://purl.org/net/def/metashare#modalityAnnotation-lipMovements">
    <rdf:type rdf:resource="http://purl.org/net/def/metashare#AnnotationType"/>
  </ns:ModalityAnnotation>
  <owl:ObjectProperty rdf:about="http://purl.org/net/def/metashare#modalityInfo">
    <rdfs:comment xml:lang="en">Groups information on the modalities represented in the resource</rdfs:comment>
    <rdfs:domain>
      <owl:Class>
        <owl:unionOf>
          <rdf:Description>
            <rdf:first rdf:resource="http://purl.org/net/def/metashare#LexicalConceptualResourceAudioInfo"/>
            <rdf:rest>
              <rdf:Description>
                <rdf:first rdf:resource="http://purl.org/net/def/metashare#LexicalConceptualResourceVideoInfo"/>
                <rdf:rest>
                  <rdf:Description>
                    <rdf:first rdf:resource="http://purl.org/net/def/metashare#CorpusTextNumericalInfo"/>
                    <rdf:rest>
                      <rdf:Description>
                        <rdf:first rdf:resource="http://purl.org/net/def/metashare#LexicalConceptualResourceImageInfo"/>
                        <rdf:rest>
                          <rdf:Description>
                            <rdf:first rdf:resource="http://purl.org/net/def/metashare#CorpusTextInfo"/>
                            <rdf:rest>
                              <rdf:Description>
                                <rdf:first rdf:resource="http://purl.org/net/def/metashare#CorpusTextNgramInfo"/>
                                <rdf:rest>
                                  <rdf:Description>
                                    <rdf:first rdf:resource="http://purl.org/net/def/metashare#CorpusVideoInfo"/>
                                    <rdf:rest>
                                      <rdf:Description>
                                        <rdf:first rdf:resource="http://purl.org/net/def/metashare#LanguageDescriptionImageInfo"/>
                                        <rdf:rest>
                                          <rdf:Description>
                                            <rdf:first rdf:resource="http://purl.org/net/def/metashare#LanguageDescriptionTextInfo"/>
                                            <rdf:rest>
                                              <rdf:Description>
                                                <rdf:first rdf:resource="http://purl.org/net/def/metashare#CorpusAudioInfo"/>
                                                <rdf:rest>
                                                  <rdf:Description>
                                                    <rdf:first rdf:resource="http://purl.org/net/def/metashare#LexicalConceptualResourceTextInfo"/>
                                                    <rdf:rest>
                                                      <rdf:Description>
                                                        <rdf:first rdf:resource="http://purl.org/net/def/metashare#CorpusImageInfo"/>
                                                        <rdf:rest>
                                                          <rdf:Description>
                                                            <rdf:first rdf:resource="http://purl.org/net/def/metashare#LanguageDescriptionVideoInfo"/>
                                                            <rdf:rest rdf:resource="http://www.w3.org/1999/02/22-rdf-syntax-ns#nil"/>
                                                          </rdf:Description>
                                                        </rdf:rest>
                                                      </rdf:Description>
                                                    </rdf:rest>
                                                  </rdf:Description>
                                                </rdf:rest>
                                              </rdf:Description>
                                            </rdf:rest>
                                          </rdf:Description>
                                        </rdf:rest>
                                      </rdf:Description>
                                    </rdf:rest>
                                  </rdf:Description>
                                </rdf:rest>
                              </rdf:Description>
                            </rdf:rest>
                          </rdf:Description>
                        </rdf:rest>
                      </rdf:Description>
                    </rdf:rest>
                  </rdf:Description>
                </rdf:rest>
              </rdf:Description>
            </rdf:rest>
          </rdf:Description>
        </owl:unionOf>
      </owl:Class>
    </rdfs:domain>
    <rdfs:range>
      <owl:Class>
        <owl:unionOf>
          <rdf:Description>
            <rdf:first rdf:resource="http://purl.org/net/def/metashare#ModalityInfo"/>
            <rdf:rest>
              <rdf:Description>
                <rdf:first rdf:resource="http://purl.org/net/def/metashare#ModalityInfo"/>
                <rdf:rest>
                  <rdf:Description>
                    <rdf:first rdf:resource="http://purl.org/net/def/metashare#ModalityInfo"/>
                    <rdf:rest>
                      <rdf:Description>
                        <rdf:first rdf:resource="http://purl.org/net/def/metashare#ModalityInfo"/>
                        <rdf:rest>
                          <rdf:Description>
                            <rdf:first rdf:resource="http://purl.org/net/def/metashare#ModalityInfo"/>
                            <rdf:rest>
                              <rdf:Description>
                                <rdf:first rdf:resource="http://purl.org/net/def/metashare#ModalityInfo"/>
                                <rdf:rest>
                                  <rdf:Description>
                                    <rdf:first rdf:resource="http://purl.org/net/def/metashare#ModalityInfo"/>
                                    <rdf:rest>
                                      <rdf:Description>
                                        <rdf:first rdf:resource="http://purl.org/net/def/metashare#ModalityInfo"/>
                                        <rdf:rest>
                                          <rdf:Description>
                                            <rdf:first rdf:resource="http://purl.org/net/def/metashare#ModalityInfo"/>
                                            <rdf:rest>
                                              <rdf:Description>
                                                <rdf:first rdf:resource="http://purl.org/net/def/metashare#ModalityInfo"/>
                                                <rdf:rest>
                                                  <rdf:Description>
                                                    <rdf:first rdf:resource="http://purl.org/net/def/metashare#ModalityInfo"/>
                                                    <rdf:rest>
                                                      <rdf:Description>
                                                        <rdf:first rdf:resource="http://purl.org/net/def/metashare#ModalityInfo"/>
                                                        <rdf:rest>
                                                          <rdf:Description>
                                                            <rdf:first rdf:resource="http://purl.org/net/def/metashare#ModalityInfo"/>
                                                            <rdf:rest rdf:resource="http://www.w3.org/1999/02/22-rdf-syntax-ns#nil"/>
                                                          </rdf:Description>
                                                        </rdf:rest>
                                                      </rdf:Description>
                                                    </rdf:rest>
                                                  </rdf:Description>
                                                </rdf:rest>
                                              </rdf:Description>
                                            </rdf:rest>
                                          </rdf:Description>
                                        </rdf:rest>
                                      </rdf:Description>
                                    </rdf:rest>
                                  </rdf:Description>
                                </rdf:rest>
                              </rdf:Description>
                            </rdf:rest>
                          </rdf:Description>
                        </rdf:rest>
                      </rdf:Description>
                    </rdf:rest>
                  </rdf:Description>
                </rdf:rest>
              </rdf:Description>
            </rdf:rest>
          </rdf:Description>
        </owl:unionOf>
      </owl:Class>
    </rdfs:range>
  </owl:ObjectProperty>
  <owl:ObjectProperty rdf:about="http://purl.org/net/def/metashare#modalityType">
    <rdfs:comment xml:lang="en">Specifies the type of the modality represented in the resource or processed by a tool/service</rdfs:comment>
    <rdfs:domain>
      <owl:Class>
        <owl:unionOf>
          <rdf:Description>
            <rdf:first rdf:resource="http://purl.org/net/def/metashare#ModalityInfo"/>
            <rdf:rest>
              <rdf:Description>
                <rdf:first rdf:resource="http://purl.org/net/def/metashare#OutputInfo"/>
                <rdf:rest>
                  <rdf:Description>
                    <rdf:first rdf:resource="http://purl.org/net/def/metashare#InputInfo"/>
                    <rdf:rest rdf:resource="http://www.w3.org/1999/02/22-rdf-syntax-ns#nil"/>
                  </rdf:Description>
                </rdf:rest>
              </rdf:Description>
            </rdf:rest>
          </rdf:Description>
        </owl:unionOf>
      </owl:Class>
    </rdfs:domain>
    <rdfs:range>
      <owl:Class>
        <owl:unionOf>
          <rdf:Description>
            <rdf:first rdf:resource="http://purl.org/net/def/metashare#ModalityType"/>
            <rdf:rest>
              <rdf:Description>
                <rdf:first rdf:resource="http://purl.org/net/def/metashare#ModalityType"/>
                <rdf:rest>
                  <rdf:Description>
                    <rdf:first rdf:resource="http://purl.org/net/def/metashare#ModalityType"/>
                    <rdf:rest rdf:resource="http://www.w3.org/1999/02/22-rdf-syntax-ns#nil"/>
                  </rdf:Description>
                </rdf:rest>
              </rdf:Description>
            </rdf:rest>
          </rdf:Description>
        </owl:unionOf>
      </owl:Class>
    </rdfs:range>
  </owl:ObjectProperty>
  <owl:DatatypeProperty rdf:about="http://purl.org/net/def/metashare#modalityTypeDetails">
    <rdfs:comment xml:lang="en">Provides further information on modalities</rdfs:comment>
    <rdfs:domain rdf:resource="http://purl.org/net/def/metashare#ModalityInfo"/>
    <rdfs:range rdf:resource="http://www.w3.org/2001/XMLSchema#string"/>
  </owl:DatatypeProperty>
  <ns:SpeechItems rdf:about="http://purl.org/net/def/metashare#moneyAmounts"/>
  <ns:LingualityType rdf:about="http://purl.org/net/def/metashare#monolingual"/>
  <ns:ConversationalType rdf:about="http://purl.org/net/def/metashare#monologue"/>
  <ns:LinguisticInformation rdf:about="http://purl.org/net/def/metashare#morpho-Aspect"/>
  <ns:LinguisticInformation rdf:about="http://purl.org/net/def/metashare#morpho-Auxiliary"/>
  <ns:LinguisticInformation rdf:about="http://purl.org/net/def/metashare#morpho-Case"/>
  <ns:LinguisticInformation rdf:about="http://purl.org/net/def/metashare#morpho-Degree"/>
  <ns:LinguisticInformation rdf:about="http://purl.org/net/def/metashare#morpho-Derivation"/>
  <ns:LinguisticInformation rdf:about="http://purl.org/net/def/metashare#morpho-Gender"/>
  <ns:LinguisticInformation rdf:about="http://purl.org/net/def/metashare#morpho-Inflection"/>
  <ns:LinguisticInformation rdf:about="http://purl.org/net/def/metashare#morpho-IrregularForms"/>
  <ns:LinguisticInformation rdf:about="http://purl.org/net/def/metashare#morpho-Mood"/>
  <ns:LinguisticInformation rdf:about="http://purl.org/net/def/metashare#morpho-Number"/>
  <ns:LinguisticInformation rdf:about="http://purl.org/net/def/metashare#morpho-Person"/>
  <ns:LinguisticInformation rdf:about="http://purl.org/net/def/metashare#morpho-Reflexivity"/>
  <ns:LinguisticInformation rdf:about="http://purl.org/net/def/metashare#morpho-Tense"/>
  <ns:LinguisticInformation rdf:about="http://purl.org/net/def/metashare#morpho-Voice"/>
  <ns:UseNLPSpecific rdf:about="http://purl.org/net/def/metashare#morphologicalAnalysis"/>
  <ns:CompatibleLexiconType rdf:about="http://purl.org/net/def/metashare#morphologicalLexicon">
    <rdf:type rdf:resource="http://purl.org/net/def/metashare#LexicalConceptualResourceType"/>
  </ns:CompatibleLexiconType>
  <ns:EncodingLevel rdf:about="http://purl.org/net/def/metashare#morphology"/>
  <ns:MorphosyntacticAnnotation rdf:about="http://purl.org/net/def/metashare#morphosyntacticAnnotation-bPosTagging">
    <rdf:type rdf:resource="http://purl.org/net/def/metashare#AnnotationType"/>
  </ns:MorphosyntacticAnnotation>
  <ns:MorphosyntacticAnnotation rdf:about="http://purl.org/net/def/metashare#morphosyntacticAnnotation-posTagging">
    <rdf:type rdf:resource="http://purl.org/net/def/metashare#AnnotationType"/>
  </ns:MorphosyntacticAnnotation>
  <ns:UseNLPSpecific rdf:about="http://purl.org/net/def/metashare#morphosyntacticTagging"/>
  <ns:BodyParts rdf:about="http://purl.org/net/def/metashare#mouth"/>
  <ns:CompressionName rdf:about="http://purl.org/net/def/metashare#mov"/>
  <ns:CompressionName rdf:about="http://purl.org/net/def/metashare#mp3"/>
  <ns:CompressionName rdf:about="http://purl.org/net/def/metashare#mpeg"/>
  <ns:CompressionName rdf:about="http://purl.org/net/def/metashare#mpg"/>
  <ns:SignalEncoding rdf:about="http://purl.org/net/def/metashare#mu-law"/>
  <ns:SizeUnit rdf:about="http://purl.org/net/def/metashare#multiWordUnits"/>
  <ns:LingualityType rdf:about="http://purl.org/net/def/metashare#multilingual"/>
  <ns:MultilingualityType rdf:about="http://purl.org/net/def/metashare#multilingualSingleText"/>
  <owl:ObjectProperty rdf:about="http://purl.org/net/def/metashare#multilingualityType">
    <rdfs:comment xml:lang="en">Indicates whether the corpus is parallel, comparable or mixed</rdfs:comment>
    <rdfs:domain>
      <owl:Class>
        <owl:unionOf>
          <rdf:Description>
            <rdf:first rdf:resource="http://purl.org/net/def/metashare#CorpusVideoInfo"/>
            <rdf:rest>
              <rdf:Description>
                <rdf:first rdf:resource="http://purl.org/net/def/metashare#LexicalConceptualResourceAudioInfo"/>
                <rdf:rest>
                  <rdf:Description>
                    <rdf:first rdf:resource="http://purl.org/net/def/metashare#LanguageDescriptionImageInfo"/>
                    <rdf:rest>
                      <rdf:Description>
                        <rdf:first rdf:resource="http://purl.org/net/def/metashare#LanguageDescriptionTextInfo"/>
                        <rdf:rest>
                          <rdf:Description>
                            <rdf:first rdf:resource="http://purl.org/net/def/metashare#CorpusTextInfo"/>
                            <rdf:rest>
                              <rdf:Description>
                                <rdf:first rdf:resource="http://purl.org/net/def/metashare#CorpusAudioInfo"/>
                                <rdf:rest>
                                  <rdf:Description>
                                    <rdf:first rdf:resource="http://purl.org/net/def/metashare#CorpusTextNgramInfo"/>
                                    <rdf:rest>
                                      <rdf:Description>
                                        <rdf:first rdf:resource="http://purl.org/net/def/metashare#LexicalConceptualResourceVideoInfo"/>
                                        <rdf:rest>
                                          <rdf:Description>
                                            <rdf:first rdf:resource="http://purl.org/net/def/metashare#LexicalConceptualResourceImageInfo"/>
                                            <rdf:rest>
                                              <rdf:Description>
                                                <rdf:first rdf:resource="http://purl.org/net/def/metashare#LexicalConceptualResourceTextInfo"/>
                                                <rdf:rest>
                                                  <rdf:Description>
                                                    <rdf:first rdf:resource="http://purl.org/net/def/metashare#CorpusImageInfo"/>
                                                    <rdf:rest>
                                                      <rdf:Description>
                                                        <rdf:first rdf:resource="http://purl.org/net/def/metashare#LanguageDescriptionVideoInfo"/>
                                                        <rdf:rest rdf:resource="http://www.w3.org/1999/02/22-rdf-syntax-ns#nil"/>
                                                      </rdf:Description>
                                                    </rdf:rest>
                                                  </rdf:Description>
                                                </rdf:rest>
                                              </rdf:Description>
                                            </rdf:rest>
                                          </rdf:Description>
                                        </rdf:rest>
                                      </rdf:Description>
                                    </rdf:rest>
                                  </rdf:Description>
                                </rdf:rest>
                              </rdf:Description>
                            </rdf:rest>
                          </rdf:Description>
                        </rdf:rest>
                      </rdf:Description>
                    </rdf:rest>
                  </rdf:Description>
                </rdf:rest>
              </rdf:Description>
            </rdf:rest>
          </rdf:Description>
        </owl:unionOf>
      </owl:Class>
    </rdfs:domain>
    <rdfs:range>
      <owl:Class>
        <owl:unionOf>
          <rdf:Description>
            <rdf:first rdf:resource="http://purl.org/net/def/metashare#MultilingualityType"/>
            <rdf:rest>
              <rdf:Description>
                <rdf:first rdf:resource="http://purl.org/net/def/metashare#MultilingualityType"/>
                <rdf:rest>
                  <rdf:Description>
                    <rdf:first rdf:resource="http://purl.org/net/def/metashare#MultilingualityType"/>
                    <rdf:rest>
                      <rdf:Description>
                        <rdf:first rdf:resource="http://purl.org/net/def/metashare#MultilingualityType"/>
                        <rdf:rest>
                          <rdf:Description>
                            <rdf:first rdf:resource="http://purl.org/net/def/metashare#MultilingualityType"/>
                            <rdf:rest>
                              <rdf:Description>
                                <rdf:first rdf:resource="http://purl.org/net/def/metashare#MultilingualityType"/>
                                <rdf:rest>
                                  <rdf:Description>
                                    <rdf:first rdf:resource="http://purl.org/net/def/metashare#MultilingualityType"/>
                                    <rdf:rest>
                                      <rdf:Description>
                                        <rdf:first rdf:resource="http://purl.org/net/def/metashare#MultilingualityType"/>
                                        <rdf:rest>
                                          <rdf:Description>
                                            <rdf:first rdf:resource="http://purl.org/net/def/metashare#MultilingualityType"/>
                                            <rdf:rest>
                                              <rdf:Description>
                                                <rdf:first rdf:resource="http://purl.org/net/def/metashare#MultilingualityType"/>
                                                <rdf:rest>
                                                  <rdf:Description>
                                                    <rdf:first rdf:resource="http://purl.org/net/def/metashare#MultilingualityType"/>
                                                    <rdf:rest>
                                                      <rdf:Description>
                                                        <rdf:first rdf:resource="http://purl.org/net/def/metashare#MultilingualityType"/>
                                                        <rdf:rest rdf:resource="http://www.w3.org/1999/02/22-rdf-syntax-ns#nil"/>
                                                      </rdf:Description>
                                                    </rdf:rest>
                                                  </rdf:Description>
                                                </rdf:rest>
                                              </rdf:Description>
                                            </rdf:rest>
                                          </rdf:Description>
                                        </rdf:rest>
                                      </rdf:Description>
                                    </rdf:rest>
                                  </rdf:Description>
                                </rdf:rest>
                              </rdf:Description>
                            </rdf:rest>
                          </rdf:Description>
                        </rdf:rest>
                      </rdf:Description>
                    </rdf:rest>
                  </rdf:Description>
                </rdf:rest>
              </rdf:Description>
            </rdf:rest>
          </rdf:Description>
        </owl:unionOf>
      </owl:Class>
    </rdfs:range>
  </owl:ObjectProperty>
  <owl:DatatypeProperty rdf:about="http://purl.org/net/def/metashare#multilingualityTypeDetails">
    <rdfs:comment xml:lang="en">Provides further information on multilinguality of a resource in free text</rdfs:comment>
    <rdfs:domain>
      <owl:Class>
        <owl:unionOf>
          <rdf:Description>
            <rdf:first rdf:resource="http://purl.org/net/def/metashare#LanguageDescriptionImageInfo"/>
            <rdf:rest>
              <rdf:Description>
                <rdf:first rdf:resource="http://purl.org/net/def/metashare#LexicalConceptualResourceImageInfo"/>
                <rdf:rest>
                  <rdf:Description>
                    <rdf:first rdf:resource="http://purl.org/net/def/metashare#CorpusAudioInfo"/>
                    <rdf:rest>
                      <rdf:Description>
                        <rdf:first rdf:resource="http://purl.org/net/def/metashare#LexicalConceptualResourceVideoInfo"/>
                        <rdf:rest>
                          <rdf:Description>
                            <rdf:first rdf:resource="http://purl.org/net/def/metashare#CorpusImageInfo"/>
                            <rdf:rest>
                              <rdf:Description>
                                <rdf:first rdf:resource="http://purl.org/net/def/metashare#LexicalConceptualResourceTextInfo"/>
                                <rdf:rest>
                                  <rdf:Description>
                                    <rdf:first rdf:resource="http://purl.org/net/def/metashare#LanguageDescriptionVideoInfo"/>
                                    <rdf:rest>
                                      <rdf:Description>
                                        <rdf:first rdf:resource="http://purl.org/net/def/metashare#LanguageDescriptionTextInfo"/>
                                        <rdf:rest>
                                          <rdf:Description>
                                            <rdf:first rdf:resource="http://purl.org/net/def/metashare#CorpusVideoInfo"/>
                                            <rdf:rest>
                                              <rdf:Description>
                                                <rdf:first rdf:resource="http://purl.org/net/def/metashare#CorpusTextInfo"/>
                                                <rdf:rest>
                                                  <rdf:Description>
                                                    <rdf:first rdf:resource="http://purl.org/net/def/metashare#LexicalConceptualResourceAudioInfo"/>
                                                    <rdf:rest>
                                                      <rdf:Description>
                                                        <rdf:first rdf:resource="http://purl.org/net/def/metashare#CorpusTextNgramInfo"/>
                                                        <rdf:rest rdf:resource="http://www.w3.org/1999/02/22-rdf-syntax-ns#nil"/>
                                                      </rdf:Description>
                                                    </rdf:rest>
                                                  </rdf:Description>
                                                </rdf:rest>
                                              </rdf:Description>
                                            </rdf:rest>
                                          </rdf:Description>
                                        </rdf:rest>
                                      </rdf:Description>
                                    </rdf:rest>
                                  </rdf:Description>
                                </rdf:rest>
                              </rdf:Description>
                            </rdf:rest>
                          </rdf:Description>
                        </rdf:rest>
                      </rdf:Description>
                    </rdf:rest>
                  </rdf:Description>
                </rdf:rest>
              </rdf:Description>
            </rdf:rest>
          </rdf:Description>
        </owl:unionOf>
      </owl:Class>
    </rdfs:domain>
    <rdfs:range rdf:resource="http://www.w3.org/2001/XMLSchema#string"/>
  </owl:DatatypeProperty>
  <ns:ConversationalType rdf:about="http://purl.org/net/def/metashare#multilogue"/>
  <ns:UseNLPSpecific rdf:about="http://purl.org/net/def/metashare#multimediaDevelopment"/>
  <ns:UseNLPSpecific rdf:about="http://purl.org/net/def/metashare#multimediaDocumentProcessing"/>
  <ns:ConformanceToStandardsBestPractices rdf:about="http://purl.org/net/def/metashare#multimodalInteractionFramework"/>
  <ns:SceneIllumination rdf:about="http://purl.org/net/def/metashare#multipleSources"/>
  <ns:NonSpeechItems rdf:about="http://purl.org/net/def/metashare#music"/>
  <ns:UseNLPSpecific rdf:about="http://purl.org/net/def/metashare#namedEntityRecognition"/>
  <ns:FundingType rdf:about="http://purl.org/net/def/metashare#nationalFunds"/>
  <ns:Origin rdf:about="http://purl.org/net/def/metashare#native">
    <rdf:type rdf:resource="http://purl.org/net/def/metashare#OriginOfPersons"/>
  </ns:Origin>
  <ns:Naturality rdf:about="http://purl.org/net/def/metashare#natural"/>
  <ns:UseNLPSpecific rdf:about="http://purl.org/net/def/metashare#naturalLanguageGeneration"/>
  <ns:UseNLPSpecific rdf:about="http://purl.org/net/def/metashare#naturalLanguageUnderstanding"/>
  <ns:SpeechItems rdf:about="http://purl.org/net/def/metashare#naturalNumbers"/>
  <owl:ObjectProperty rdf:about="http://purl.org/net/def/metashare#naturality">
    <rdfs:comment xml:lang="en">Specifies the level of naturality for multimodal/multimedia resources</rdfs:comment>
    <rdfs:domain>
      <owl:Class>
        <owl:unionOf>
          <rdf:Description>
            <rdf:first rdf:resource="http://purl.org/net/def/metashare#CorpusVideoInfo"/>
            <rdf:rest>
              <rdf:Description>
                <rdf:first rdf:resource="http://purl.org/net/def/metashare#CorpusAudioInfo"/>
                <rdf:rest rdf:resource="http://www.w3.org/1999/02/22-rdf-syntax-ns#nil"/>
              </rdf:Description>
            </rdf:rest>
          </rdf:Description>
        </owl:unionOf>
      </owl:Class>
    </rdfs:domain>
    <rdfs:range>
      <owl:Class>
        <owl:unionOf>
          <rdf:Description>
            <rdf:first rdf:resource="http://purl.org/net/def/metashare#Naturality"/>
            <rdf:rest>
              <rdf:Description>
                <rdf:first rdf:resource="http://purl.org/net/def/metashare#Naturality"/>
                <rdf:rest rdf:resource="http://www.w3.org/1999/02/22-rdf-syntax-ns#nil"/>
              </rdf:Description>
            </rdf:rest>
          </rdf:Description>
        </owl:unionOf>
      </owl:Class>
    </rdfs:range>
  </owl:ObjectProperty>
  <ns:SizeUnit rdf:about="http://purl.org/net/def/metashare#neologisms"/>
  <owl:ObjectProperty rdf:about="http://purl.org/net/def/metashare#ngramInfo">
    <rdfs:comment xml:lang="en">Groups information specific to n-gram resources (e.g. range of n-grams, base item etc.)</rdfs:comment>
    <rdfs:domain rdf:resource="http://purl.org/net/def/metashare#CorpusTextNgramInfo"/>
    <rdfs:range rdf:resource="http://purl.org/net/def/metashare#NgramInfo"/>
  </owl:ObjectProperty>
  <ns:Use rdf:about="http://purl.org/net/def/metashare#nlpApplications"/>
  <ns:ToolServiceType rdf:about="http://purl.org/net/def/metashare#nlpDevelopmentEnvironment"/>
  <ns:Audience rdf:about="http://purl.org/net/def/metashare#no">
    <rdf:type rdf:resource="http://purl.org/net/def/metashare#HearingImpairmentOfPersons"/>
    <rdf:type rdf:resource="http://purl.org/net/def/metashare#SpeakingImpairmentOfPersons"/>
  </ns:Audience>
  <odrl:Set rdf:about="http://purl.org/net/def/metashare#noDerivatives">
    <rdf:type rdf:resource="http://purl.org/net/def/metashare#ConditionsOfUse"/>
    <rdfs:comment xml:lang="en">No Derivatives refers to a kind of 'ConditionsOfUse' imposed by the licence; users are not allow to share derivatives of the resource</rdfs:comment>
    <odrl:prohibition>
      <rdf:Description>
        <odrl:action rdf:resource="http://creativecommons.org/ns#DerivativeWorks"/>
      </rdf:Description>
    </odrl:prohibition>
  </odrl:Set>
  <ns:ConditionsOfUse rdf:about="http://purl.org/net/def/metashare#noRedistribution">
    <rdfs:comment xml:lang="en">No Redistribution refers to a kind of 'ConditionsOfUse' imposed by the licence; users are not allowed to redistribute the resource</rdfs:comment>
  </ns:ConditionsOfUse>
  <odrl:Set rdf:about="http://purl.org/net/def/metashare#noRedistriubtion">
    <odrl:prohibition>
      <rdf:Description>
        <odrl:action rdf:resource="http://creativecommons.org/ns#Reproduction"/>
      </rdf:Description>
    </odrl:prohibition>
  </odrl:Set>
  <ns:NonSpeechItems rdf:about="http://purl.org/net/def/metashare#noise"/>
  <owl:ObjectProperty rdf:about="http://purl.org/net/def/metashare#noiseLevel">
    <rdfs:comment xml:lang="en">Specifies the  level of background noise</rdfs:comment>
    <rdfs:domain>
      <owl:Class>
        <owl:unionOf>
          <rdf:Description>
            <rdf:first rdf:resource="http://purl.org/net/def/metashare#CorpusAudioInfo"/>
            <rdf:rest>
              <rdf:Description>
                <rdf:first rdf:resource="http://purl.org/net/def/metashare#LexicalConceptualResourceAudioInfo"/>
                <rdf:rest rdf:resource="http://www.w3.org/1999/02/22-rdf-syntax-ns#nil"/>
              </rdf:Description>
            </rdf:rest>
          </rdf:Description>
        </owl:unionOf>
      </owl:Class>
    </rdfs:domain>
    <rdfs:range>
      <owl:Class>
        <owl:unionOf>
          <rdf:Description>
            <rdf:first rdf:resource="http://purl.org/net/def/metashare#NoiseLevel"/>
            <rdf:rest>
              <rdf:Description>
                <rdf:first rdf:resource="http://purl.org/net/def/metashare#NoiseLevel"/>
                <rdf:rest rdf:resource="http://www.w3.org/1999/02/22-rdf-syntax-ns#nil"/>
              </rdf:Description>
            </rdf:rest>
          </rdf:Description>
        </owl:unionOf>
      </owl:Class>
    </rdfs:range>
  </owl:ObjectProperty>
  <rdf:Description rdf:about="http://purl.org/net/def/metashare#nonCommercialUse">
    <rdfs:comment xml:lang="en">Non-commercial use refers to a kind of 'ConditionsOfUse' imposed by the licence; use for non commercial purposes, such as research and education by academic users</rdfs:comment>
  </rdf:Description>
  <ns:Interactivity rdf:about="http://purl.org/net/def/metashare#nonInteractive"/>
  <ns:Origin rdf:about="http://purl.org/net/def/metashare#nonNative">
    <rdf:type rdf:resource="http://purl.org/net/def/metashare#OriginOfPersons"/>
  </ns:Origin>
  <owl:ObjectProperty rdf:about="http://purl.org/net/def/metashare#nonSpeechItems">
    <rdfs:comment xml:lang="en">Specifies the distinct elements that maybe included in the audio corpus</rdfs:comment>
    <rdfs:domain>
      <owl:Class>
        <owl:unionOf>
          <rdf:Description>
            <rdf:first rdf:resource="http://purl.org/net/def/metashare#CorpusAudioInfo"/>
            <rdf:rest>
              <rdf:Description>
                <rdf:first rdf:resource="http://purl.org/net/def/metashare#LexicalConceptualResourceAudioInfo"/>
                <rdf:rest rdf:resource="http://www.w3.org/1999/02/22-rdf-syntax-ns#nil"/>
              </rdf:Description>
            </rdf:rest>
          </rdf:Description>
        </owl:unionOf>
      </owl:Class>
    </rdfs:domain>
    <rdfs:range>
      <owl:Class>
        <owl:unionOf>
          <rdf:Description>
            <rdf:first rdf:resource="http://purl.org/net/def/metashare#NonSpeechItems"/>
            <rdf:rest>
              <rdf:Description>
                <rdf:first rdf:resource="http://purl.org/net/def/metashare#NonSpeechItems"/>
                <rdf:rest rdf:resource="http://www.w3.org/1999/02/22-rdf-syntax-ns#nil"/>
              </rdf:Description>
            </rdf:rest>
          </rdf:Description>
        </owl:unionOf>
      </owl:Class>
    </rdfs:range>
  </owl:ObjectProperty>
  <ns:BodyParts rdf:about="http://purl.org/net/def/metashare#none">
    <rdf:type rdf:resource="http://purl.org/net/def/metashare#RelatedLexiconType"/>
    <rdf:type rdf:resource="http://purl.org/net/def/metashare#RequiredHardware"/>
    <rdf:type rdf:resource="http://purl.org/net/def/metashare#TextIncludedInImage"/>
    <rdf:type rdf:resource="http://purl.org/net/def/metashare#TextIncludedInVideo"/>
    <rdf:type rdf:resource="http://purl.org/net/def/metashare#ToolDocumentationType"/>
  </ns:BodyParts>
  <ns:NonSpeechItems rdf:about="http://purl.org/net/def/metashare#notes"/>
  <ns:Task rdf:about="http://purl.org/net/def/metashare#npRecognition"/>
  <ns:GrammaticalPhenomenaCoverage rdf:about="http://purl.org/net/def/metashare#npStructure"/>
  <owl:DatatypeProperty rdf:about="http://purl.org/net/def/metashare#numberOfPersons">
    <rdfs:comment xml:lang="en">The number of the persons participating in the audio or video part of the resource</rdfs:comment>
    <rdfs:domain>
      <owl:Class>
        <owl:unionOf>
          <rdf:Description>
            <rdf:first rdf:resource="http://purl.org/net/def/metashare#CorpusTextNumericalInfo"/>
            <rdf:rest>
              <rdf:Description>
                <rdf:first rdf:resource="http://purl.org/net/def/metashare#CorpusImageInfo"/>
                <rdf:rest>
                  <rdf:Description>
                    <rdf:first rdf:resource="http://purl.org/net/def/metashare#CorpusVideoInfo"/>
                    <rdf:rest>
                      <rdf:Description>
                        <rdf:first rdf:resource="http://purl.org/net/def/metashare#CorpusAudioInfo"/>
                        <rdf:rest rdf:resource="http://www.w3.org/1999/02/22-rdf-syntax-ns#nil"/>
                      </rdf:Description>
                    </rdf:rest>
                  </rdf:Description>
                </rdf:rest>
              </rdf:Description>
            </rdf:rest>
          </rdf:Description>
        </owl:unionOf>
      </owl:Class>
    </rdfs:domain>
    <rdfs:range rdf:resource="http://www.w3.org/2001/XMLSchema#int"/>
  </owl:DatatypeProperty>
  <owl:DatatypeProperty rdf:about="http://purl.org/net/def/metashare#numberOfTrainedSpeakers">
    <rdfs:comment xml:lang="en">The number of participants that have been trained for the specific task</rdfs:comment>
    <rdfs:domain>
      <owl:Class>
        <owl:unionOf>
          <rdf:Description>
            <rdf:first rdf:resource="http://purl.org/net/def/metashare#CorpusTextNumericalInfo"/>
            <rdf:rest>
              <rdf:Description>
                <rdf:first rdf:resource="http://purl.org/net/def/metashare#CorpusVideoInfo"/>
                <rdf:rest>
                  <rdf:Description>
                    <rdf:first rdf:resource="http://purl.org/net/def/metashare#CorpusImageInfo"/>
                    <rdf:rest>
                      <rdf:Description>
                        <rdf:first rdf:resource="http://purl.org/net/def/metashare#CorpusAudioInfo"/>
                        <rdf:rest rdf:resource="http://www.w3.org/1999/02/22-rdf-syntax-ns#nil"/>
                      </rdf:Description>
                    </rdf:rest>
                  </rdf:Description>
                </rdf:rest>
              </rdf:Description>
            </rdf:rest>
          </rdf:Description>
        </owl:unionOf>
      </owl:Class>
    </rdfs:domain>
    <rdfs:range rdf:resource="http://www.w3.org/2001/XMLSchema#int"/>
  </owl:DatatypeProperty>
  <ns:RequiredHardware rdf:about="http://purl.org/net/def/metashare#ocrSystem"/>
  <ns:RecordingEnvironment rdf:about="http://purl.org/net/def/metashare#office"/>
  <ns:CompressionName rdf:about="http://purl.org/net/def/metashare#oggVorbis"/>
  <ns:ToolDocumentationType rdf:about="http://purl.org/net/def/metashare#online"/>
  <ns:ScenarioType rdf:about="http://purl.org/net/def/metashare#onlineEducationalGame"/>
  <odrl:Set rdf:about="http://purl.org/net/def/metashare#onlyMSmembers">
    <rdf:type rdf:resource="http://purl.org/net/def/metashare#ConditionsOfUse"/>
    <rdfs:comment xml:lang="en">Only Meta Share members refers to a kind of 'ConditionsOfUse' imposed by the licence; the resource can only be used by members of the MetaShare network</rdfs:comment>
    <odrl:permission>
      <rdf:Description>
        <odrl:constraint>
          <rdf:Description>
            <odrl:operator rdf:resource="http://www.w3.org/ns/odrl/2/eq"/>
            <odrl:recipient rdf:resource="http://purl.org/net/def/metashare#onlyMSmembers"/>
          </rdf:Description>
        </odrl:constraint>
      </rdf:Description>
    </odrl:permission>
  </odrl:Set>
  <ns:CompatibleLexiconType rdf:about="http://purl.org/net/def/metashare#ontology">
    <rdf:type rdf:resource="http://purl.org/net/def/metashare#LexicalConceptualResourceType"/>
  </ns:CompatibleLexiconType>
  <ns:License rdf:about="http://purl.org/net/def/metashare#openForReuseWithRestrictions">
    <rdf:type rdf:resource="http://www.w3.org/2002/07/owl#NamedIndividual"/>
    <rdfs:comment xml:lang="en">It refers to any kind of license that governs the use of a resource permitting certain automatic processing procedures but with specific restrictions; the end user is advised to check the conditionsOfUse metadata element for a quick overview of the rights granted for the use of the resource and to read carefully the full license text</rdfs:comment>
    <rdfs:label xml:lang="en">Open For Reuse With Restrictions</rdfs:label>
  </ns:License>
  <ns:RecordingEnvironment rdf:about="http://purl.org/net/def/metashare#openPublicPlace"/>
  <owl:ObjectProperty rdf:about="http://purl.org/net/def/metashare#operatingSystem">
    <rdfs:comment xml:lang="en">The operating system on which the tool will be running</rdfs:comment>
    <rdfs:domain rdf:resource="http://purl.org/net/def/metashare#ToolServiceInfo"/>
    <rdfs:range rdf:resource="http://purl.org/net/def/metashare#OperatingSystem"/>
  </owl:ObjectProperty>
  <ns:UseNLPSpecific rdf:about="http://purl.org/net/def/metashare#opinionMining"/>
  <owl:DatatypeProperty rdf:about="http://purl.org/net/def/metashare#order">
    <rdfs:comment xml:lang="en">The maximum number of items in the sequence</rdfs:comment>
    <rdfs:domain rdf:resource="http://purl.org/net/def/metashare#NgramInfo"/>
    <rdfs:range rdf:resource="http://www.w3.org/2001/XMLSchema#int"/>
  </owl:DatatypeProperty>
  <owl:DatatypeProperty rdf:about="http://purl.org/net/def/metashare#organizationDescription">
    <rdfs:comment xml:lang="en">Provides description of the organizations that may appear in the image corpus</rdfs:comment>
    <rdfs:domain rdf:resource="http://purl.org/net/def/metashare#StaticElementInfo"/>
    <rdfs:range rdf:resource="http://www.w3.org/2001/XMLSchema#string"/>
  </owl:DatatypeProperty>
  <owl:ObjectProperty rdf:about="http://purl.org/net/def/metashare#organizationInfo">
    <rdfs:comment xml:lang="en">Groups information on organizations related to the resource</rdfs:comment>
    <rdfs:domain rdf:resource="http://purl.org/net/def/metashare#Actor"/>
    <rdfs:range rdf:resource="http://purl.org/net/def/metashare#Organization"/>
  </owl:ObjectProperty>
  <owl:DatatypeProperty rdf:about="http://purl.org/net/def/metashare#organizationName">
    <rdfs:comment xml:lang="en">The full name of an organization</rdfs:comment>
    <rdfs:domain rdf:resource="http://purl.org/net/def/metashare#Organization"/>
    <rdfs:range rdf:resource="http://www.w3.org/1999/02/22-rdf-syntax-ns#langString"/>
  </owl:DatatypeProperty>
  <owl:DatatypeProperty rdf:about="http://purl.org/net/def/metashare#organizationShortName">
    <rdfs:comment xml:lang="en">The short name (abbreviation, acronym etc.) used for an organization</rdfs:comment>
    <rdfs:domain rdf:resource="http://purl.org/net/def/metashare#Organization"/>
    <rdfs:range rdf:resource="http://www.w3.org/1999/02/22-rdf-syntax-ns#langString"/>
  </owl:DatatypeProperty>
  <owl:ObjectProperty rdf:about="http://purl.org/net/def/metashare#origin">
    <rdfs:comment xml:lang="en">The language origin of the participant</rdfs:comment>
    <rdfs:domain rdf:resource="http://purl.org/net/def/metashare#ParticipantInfo"/>
    <rdfs:range rdf:resource="http://purl.org/net/def/metashare#Origin"/>
  </owl:ObjectProperty>
  <owl:ObjectProperty rdf:about="http://purl.org/net/def/metashare#originOfPersons">
    <rdfs:comment xml:lang="en">The language origin of the group of participants</rdfs:comment>
    <rdfs:domain>
      <owl:Class>
        <owl:unionOf>
          <rdf:Description>
            <rdf:first rdf:resource="http://purl.org/net/def/metashare#CorpusTextNumericalInfo"/>
            <rdf:rest>
              <rdf:Description>
                <rdf:first rdf:resource="http://purl.org/net/def/metashare#CorpusImageInfo"/>
                <rdf:rest>
                  <rdf:Description>
                    <rdf:first rdf:resource="http://purl.org/net/def/metashare#CorpusAudioInfo"/>
                    <rdf:rest>
                      <rdf:Description>
                        <rdf:first rdf:resource="http://purl.org/net/def/metashare#CorpusVideoInfo"/>
                        <rdf:rest rdf:resource="http://www.w3.org/1999/02/22-rdf-syntax-ns#nil"/>
                      </rdf:Description>
                    </rdf:rest>
                  </rdf:Description>
                </rdf:rest>
              </rdf:Description>
            </rdf:rest>
          </rdf:Description>
        </owl:unionOf>
      </owl:Class>
    </rdfs:domain>
    <rdfs:range>
      <owl:Class>
        <owl:unionOf>
          <rdf:Description>
            <rdf:first rdf:resource="http://purl.org/net/def/metashare#OriginOfPersons"/>
            <rdf:rest>
              <rdf:Description>
                <rdf:first rdf:resource="http://purl.org/net/def/metashare#OriginOfPersons"/>
                <rdf:rest>
                  <rdf:Description>
                    <rdf:first rdf:resource="http://purl.org/net/def/metashare#OriginOfPersons"/>
                    <rdf:rest>
                      <rdf:Description>
                        <rdf:first rdf:resource="http://purl.org/net/def/metashare#OriginOfPersons"/>
                        <rdf:rest rdf:resource="http://www.w3.org/1999/02/22-rdf-syntax-ns#nil"/>
                      </rdf:Description>
                    </rdf:rest>
                  </rdf:Description>
                </rdf:rest>
              </rdf:Description>
            </rdf:rest>
          </rdf:Description>
        </owl:unionOf>
      </owl:Class>
    </rdfs:range>
  </owl:ObjectProperty>
  <owl:DatatypeProperty rdf:about="http://purl.org/net/def/metashare#originalMetadataLink">
    <rdfs:comment xml:lang="en">A link to the original metadata record, in cases of harvesting</rdfs:comment>
    <rdfs:domain rdf:resource="http://purl.org/net/def/metashare#MetadataInfo"/>
    <rdfs:range rdf:resource="http://www.w3.org/2001/XMLSchema#string"/>
  </owl:DatatypeProperty>
  <owl:DatatypeProperty rdf:about="http://purl.org/net/def/metashare#originalMetadataSchema">
    <rdfs:comment xml:lang="en">Refers to the metadata schema originally used for the description of the resource</rdfs:comment>
    <rdfs:domain rdf:resource="http://purl.org/net/def/metashare#MetadataInfo"/>
    <rdfs:range rdf:resource="http://www.w3.org/2001/XMLSchema#string"/>
  </owl:DatatypeProperty>
  <owl:DatatypeProperty rdf:about="http://purl.org/net/def/metashare#originalSource">
    <rdfs:comment xml:lang="en">The name, the identifier or the url of thethe original resources that were at the base of the creation process of the resource</rdfs:comment>
    <rdfs:domain>
      <owl:Class>
        <owl:unionOf>
          <rdf:Description>
            <rdf:first rdf:resource="http://purl.org/net/def/metashare#CorpusVideoInfo"/>
            <rdf:rest>
              <rdf:Description>
                <rdf:first rdf:resource="http://purl.org/net/def/metashare#CorpusTextInfo"/>
                <rdf:rest>
                  <rdf:Description>
                    <rdf:first rdf:resource="http://purl.org/net/def/metashare#CorpusImageInfo"/>
                    <rdf:rest>
                      <rdf:Description>
                        <rdf:first rdf:resource="http://purl.org/net/def/metashare#CorpusTextNumericalInfo"/>
                        <rdf:rest>
                          <rdf:Description>
                            <rdf:first rdf:resource="http://purl.org/net/def/metashare#LanguageDescriptionVideoInfo"/>
                            <rdf:rest>
                              <rdf:Description>
                                <rdf:first rdf:resource="http://purl.org/net/def/metashare#LanguageDescriptionImageInfo"/>
                                <rdf:rest>
                                  <rdf:Description>
                                    <rdf:first rdf:resource="http://purl.org/net/def/metashare#ToolServiceInfo"/>
                                    <rdf:rest>
                                      <rdf:Description>
                                        <rdf:first rdf:resource="http://purl.org/net/def/metashare#CorpusTextNgramInfo"/>
                                        <rdf:rest>
                                          <rdf:Description>
                                            <rdf:first rdf:resource="http://purl.org/net/def/metashare#LanguageDescriptionTextInfo"/>
                                            <rdf:rest>
                                              <rdf:Description>
                                                <rdf:first rdf:resource="http://purl.org/net/def/metashare#LexicalConceptualResourceInfo"/>
                                                <rdf:rest>
                                                  <rdf:Description>
                                                    <rdf:first rdf:resource="http://purl.org/net/def/metashare#LanguageDescriptionInfo"/>
                                                    <rdf:rest>
                                                      <rdf:Description>
                                                        <rdf:first rdf:resource="http://purl.org/net/def/metashare#CorpusAudioInfo"/>
                                                        <rdf:rest rdf:resource="http://www.w3.org/1999/02/22-rdf-syntax-ns#nil"/>
                                                      </rdf:Description>
                                                    </rdf:rest>
                                                  </rdf:Description>
                                                </rdf:rest>
                                              </rdf:Description>
                                            </rdf:rest>
                                          </rdf:Description>
                                        </rdf:rest>
                                      </rdf:Description>
                                    </rdf:rest>
                                  </rdf:Description>
                                </rdf:rest>
                              </rdf:Description>
                            </rdf:rest>
                          </rdf:Description>
                        </rdf:rest>
                      </rdf:Description>
                    </rdf:rest>
                  </rdf:Description>
                </rdf:rest>
              </rdf:Description>
            </rdf:rest>
          </rdf:Description>
        </owl:unionOf>
      </owl:Class>
    </rdfs:domain>
    <rdfs:range rdf:resource="http://www.w3.org/2001/XMLSchema#string"/>
  </owl:DatatypeProperty>
  <ns:OperatingSystem rdf:about="http://purl.org/net/def/metashare#os-independent"/>
  <ns:AnnotatedElements rdf:about="http://purl.org/net/def/metashare#other">
    <rdf:type rdf:resource="http://purl.org/net/def/metashare#AnnotationType"/>
    <rdf:type rdf:resource="http://purl.org/net/def/metashare#AudioQualityMeasuresIncluded"/>
    <rdf:type rdf:resource="http://purl.org/net/def/metashare#BaseItem"/>
    <rdf:type rdf:resource="http://purl.org/net/def/metashare#CapturingDeviceType"/>
    <rdf:type rdf:resource="http://purl.org/net/def/metashare#CompatibleLexiconType"/>
    <rdf:type rdf:resource="http://purl.org/net/def/metashare#CompressionName"/>
    <rdf:type rdf:resource="http://purl.org/net/def/metashare#ConditionsOfUse"/>
    <rdf:type rdf:resource="http://purl.org/net/def/metashare#ConformanceToClassificationScheme"/>
    <rdf:type rdf:resource="http://purl.org/net/def/metashare#ConformanceToStandardsBestPractices"/>
    <rdf:type rdf:resource="http://purl.org/net/def/metashare#EncodingLevel"/>
    <rdf:type rdf:resource="http://purl.org/net/def/metashare#ExtraTextualInformationUnit"/>
    <rdf:type rdf:resource="http://purl.org/net/def/metashare#ExtratextualInformation"/>
    <rdf:type rdf:resource="http://purl.org/net/def/metashare#FundingType"/>
    <rdf:type rdf:resource="http://purl.org/net/def/metashare#GrammaticalPhenomenaCoverage"/>
    <rdf:type rdf:resource="http://purl.org/net/def/metashare#Interactivity"/>
    <rdf:type rdf:resource="http://purl.org/net/def/metashare#LanguageDescriptionType"/>
    <rdf:type rdf:resource="http://purl.org/net/def/metashare#LanguageVarietyType"/>
    <rdf:type rdf:resource="http://purl.org/net/def/metashare#LexicalConceptualResourceType"/>
    <rdf:type rdf:resource="http://purl.org/net/def/metashare#LicenceInfo"/>
    <rdf:type rdf:resource="http://purl.org/net/def/metashare#LinguisticInformation"/>
    <rdf:type rdf:resource="http://purl.org/net/def/metashare#MembershipInstitution"/>
    <rdf:type rdf:resource="http://purl.org/net/def/metashare#ModalityType"/>
    <rdf:type rdf:resource="http://purl.org/net/def/metashare#MultilingualityType"/>
    <rdf:type rdf:resource="http://purl.org/net/def/metashare#Naturality"/>
    <rdf:type rdf:resource="http://purl.org/net/def/metashare#NonSpeechItems"/>
    <rdf:type rdf:resource="http://purl.org/net/def/metashare#OperatingSystem"/>
    <rdf:type rdf:resource="http://purl.org/net/def/metashare#RecordingDeviceType"/>
    <rdf:type rdf:resource="http://purl.org/net/def/metashare#RecordingEnvironment"/>
    <rdf:type rdf:resource="http://purl.org/net/def/metashare#RequiredHardware"/>
    <rdf:type rdf:resource="http://purl.org/net/def/metashare#ScenarioType"/>
    <rdf:type rdf:resource="http://purl.org/net/def/metashare#SceneIllumination"/>
    <rdf:type rdf:resource="http://purl.org/net/def/metashare#SegmentationLevel"/>
    <rdf:type rdf:resource="http://purl.org/net/def/metashare#SignalEncoding"/>
    <rdf:type rdf:resource="http://purl.org/net/def/metashare#SizeUnit"/>
    <rdf:type rdf:resource="http://purl.org/net/def/metashare#SourceChannel"/>
    <rdf:type rdf:resource="http://purl.org/net/def/metashare#SourceChannelType"/>
    <rdf:type rdf:resource="http://purl.org/net/def/metashare#SpeechInfluences"/>
    <rdf:type rdf:resource="http://purl.org/net/def/metashare#SpeechItems"/>
    <rdf:type rdf:resource="http://purl.org/net/def/metashare#Task"/>
    <rdf:type rdf:resource="http://purl.org/net/def/metashare#ToolDocumentationType"/>
    <rdf:type rdf:resource="http://purl.org/net/def/metashare#ToolServiceType"/>
    <rdf:type rdf:resource="http://purl.org/net/def/metashare#UseNLPSpecific"/>
  </ns:AnnotatedElements>
  <owl:ObjectProperty rdf:about="http://purl.org/net/def/metashare#otherMedia">
    <rdfs:comment xml:lang="en">Specifies the media types that are linked to the media type described within the same resource</rdfs:comment>
    <rdfs:domain rdf:resource="http://purl.org/net/def/metashare#LinkToOtherMediaInfo"/>
    <rdfs:range rdf:resource="http://purl.org/net/def/metashare#OtherMedia"/>
  </owl:ObjectProperty>
  <owl:DatatypeProperty rdf:about="http://purl.org/net/def/metashare#output">
    <rdfs:comment xml:lang="en">Indicates whether the output of the operation of the grammar is a statement of grammaticality (grammatical/ungrammatical) or structures (interpretation of the input)</rdfs:comment>
    <rdfs:domain rdf:resource="http://purl.org/net/def/metashare#LanguageDescriptionInfo"/>
    <rdfs:range rdf:resource="http://www.w3.org/2001/XMLSchema#string"/>
  </owl:DatatypeProperty>
  <owl:ObjectProperty rdf:about="http://purl.org/net/def/metashare#outputInfo">
    <rdfs:comment xml:lang="en">Groups together information on the requirements set on the output of a tool or service</rdfs:comment>
    <rdfs:domain rdf:resource="http://purl.org/net/def/metashare#ToolServiceInfo"/>
    <rdfs:range rdf:resource="http://purl.org/net/def/metashare#OutputInfo"/>
  </owl:ObjectProperty>
  <ns:Interactivity rdf:about="http://purl.org/net/def/metashare#overlapping"/>
  <ns:FundingType rdf:about="http://purl.org/net/def/metashare#ownFunds"/>
  <ns:DistributionAccessMedium rdf:about="http://purl.org/net/def/metashare#paperCopy"/>
  <ns:SegmentationLevel rdf:about="http://purl.org/net/def/metashare#paragraph"/>
  <ns:MultilingualityType rdf:about="http://purl.org/net/def/metashare#parallel"/>
  <ns:Task rdf:about="http://purl.org/net/def/metashare#parsing">
    <rdf:type rdf:resource="http://purl.org/net/def/metashare#UseNLPSpecific"/>
  </ns:Task>
  <ns:LinguisticInformation rdf:about="http://purl.org/net/def/metashare#partOfSpeech"/>
  <ns:ValidationExtent rdf:about="http://purl.org/net/def/metashare#partial"/>
  <owl:ObjectProperty rdf:about="http://purl.org/net/def/metashare#participantInfo">
    <rdfs:comment xml:lang="en">Groups information on the individual person(s) participating in the audio, video, sensorimotor (textNumerical) part of the resource</rdfs:comment>
    <rdfs:domain>
      <owl:Class>
        <owl:unionOf>
          <rdf:Description>
            <rdf:first rdf:resource="http://purl.org/net/def/metashare#CorpusVideoInfo"/>
            <rdf:rest>
              <rdf:Description>
                <rdf:first rdf:resource="http://purl.org/net/def/metashare#CorpusAudioInfo"/>
                <rdf:rest>
                  <rdf:Description>
                    <rdf:first rdf:resource="http://purl.org/net/def/metashare#CorpusImageInfo"/>
                    <rdf:rest>
                      <rdf:Description>
                        <rdf:first rdf:resource="http://purl.org/net/def/metashare#CorpusTextNumericalInfo"/>
                        <rdf:rest rdf:resource="http://www.w3.org/1999/02/22-rdf-syntax-ns#nil"/>
                      </rdf:Description>
                    </rdf:rest>
                  </rdf:Description>
                </rdf:rest>
              </rdf:Description>
            </rdf:rest>
          </rdf:Description>
        </owl:unionOf>
      </owl:Class>
    </rdfs:domain>
    <rdfs:range>
      <owl:Class>
        <owl:unionOf>
          <rdf:Description>
            <rdf:first rdf:resource="http://purl.org/net/def/metashare#ParticipantInfo"/>
            <rdf:rest>
              <rdf:Description>
                <rdf:first rdf:resource="http://purl.org/net/def/metashare#ParticipantInfo"/>
                <rdf:rest>
                  <rdf:Description>
                    <rdf:first rdf:resource="http://purl.org/net/def/metashare#ParticipantInfo"/>
                    <rdf:rest>
                      <rdf:Description>
                        <rdf:first rdf:resource="http://purl.org/net/def/metashare#ParticipantInfo"/>
                        <rdf:rest rdf:resource="http://www.w3.org/1999/02/22-rdf-syntax-ns#nil"/>
                      </rdf:Description>
                    </rdf:rest>
                  </rdf:Description>
                </rdf:rest>
              </rdf:Description>
            </rdf:rest>
          </rdf:Description>
        </owl:unionOf>
      </owl:Class>
    </rdfs:range>
  </owl:ObjectProperty>
  <ns:ScenarioType rdf:about="http://purl.org/net/def/metashare#pearStory"/>
  <ns:ConformanceToStandardsBestPractices rdf:about="http://purl.org/net/def/metashare#pennTreeBank"/>
  <owl:DatatypeProperty rdf:about="http://purl.org/net/def/metashare#perplexity">
    <rdfs:comment xml:lang="en">Derived from running on test set taken from the same corpus</rdfs:comment>
    <rdfs:domain rdf:resource="http://purl.org/net/def/metashare#NgramInfo"/>
    <rdfs:range rdf:resource="http://www.w3.org/2001/XMLSchema#decimal"/>
  </owl:DatatypeProperty>
  <owl:DatatypeProperty rdf:about="http://purl.org/net/def/metashare#personDescription">
    <rdfs:comment xml:lang="en">Provides descriptive features for the persons represented in the image corpus</rdfs:comment>
    <rdfs:domain rdf:resource="http://purl.org/net/def/metashare#StaticElementInfo"/>
    <rdfs:range rdf:resource="http://www.w3.org/2001/XMLSchema#string"/>
  </owl:DatatypeProperty>
  <ns:UseNLPSpecific rdf:about="http://purl.org/net/def/metashare#personIdentification"/>
  <owl:ObjectProperty rdf:about="http://purl.org/net/def/metashare#personInfo">
    <rdfs:comment xml:lang="en">Groups information relevant to personsrelated to the resource; to be used mainly for contact persons, resource creators, validators, annotators etc. for whom personal data can be provided</rdfs:comment>
    <rdfs:domain rdf:resource="http://purl.org/net/def/metashare#Actor"/>
    <rdfs:range rdf:resource="http://purl.org/net/def/metashare#Person"/>
  </owl:ObjectProperty>
  <ns:UseNLPSpecific rdf:about="http://purl.org/net/def/metashare#personRecognition"/>
  <ns:ConditionsOfUse rdf:about="http://purl.org/net/def/metashare#personalDataIncluded">
    <rdf:type rdf:resource="http://www.w3.org/2002/07/owl#NamedIndividual"/>
    <rdfs:comment xml:lang="en">PersonalDataIncluded refers to a kind of 'ConditionsOfUse' imposed by the licence; it's a privacy warning for resources that include personal data.</rdfs:comment>
    <rdfs:label xml:lang="en">Personal Data Included</rdfs:label>
  </ns:ConditionsOfUse>
  <ns:UseNLPSpecific rdf:about="http://purl.org/net/def/metashare#persuasiveExpressionMining"/>
  <ns:BaseItem rdf:about="http://purl.org/net/def/metashare#phoneme">
    <rdf:type rdf:resource="http://purl.org/net/def/metashare#SegmentationLevel"/>
  </ns:BaseItem>
  <ns:SizeUnit rdf:about="http://purl.org/net/def/metashare#phonemes"/>
  <ns:SizeUnit rdf:about="http://purl.org/net/def/metashare#phoneticUnits"/>
  <ns:SpeechItems rdf:about="http://purl.org/net/def/metashare#phoneticallyBalancedSentences"/>
  <ns:SpeechItems rdf:about="http://purl.org/net/def/metashare#phoneticallyRichSentences"/>
  <ns:SpeechItems rdf:about="http://purl.org/net/def/metashare#phoneticallyRichWords"/>
  <ns:EncodingLevel rdf:about="http://purl.org/net/def/metashare#phonetics"/>
  <ns:LinguisticInformation rdf:about="http://purl.org/net/def/metashare#phonetics-Transcription"/>
  <ns:EncodingLevel rdf:about="http://purl.org/net/def/metashare#phonology"/>
  <ns:SegmentationLevel rdf:about="http://purl.org/net/def/metashare#phrase"/>
  <owl:DatatypeProperty rdf:about="http://purl.org/net/def/metashare#placeOfBirth">
    <rdfs:comment xml:lang="en">The place in which the participant has been born</rdfs:comment>
    <rdfs:domain rdf:resource="http://purl.org/net/def/metashare#ParticipantInfo"/>
    <rdfs:range rdf:resource="http://www.w3.org/2001/XMLSchema#string"/>
  </owl:DatatypeProperty>
  <owl:DatatypeProperty rdf:about="http://purl.org/net/def/metashare#placeOfChildhood">
    <rdfs:comment xml:lang="en">The place in which the participant lived as a child</rdfs:comment>
    <rdfs:domain rdf:resource="http://purl.org/net/def/metashare#ParticipantInfo"/>
    <rdfs:range rdf:resource="http://www.w3.org/2001/XMLSchema#string"/>
  </owl:DatatypeProperty>
  <owl:DatatypeProperty rdf:about="http://purl.org/net/def/metashare#placeOfSecondEducation">
    <rdfs:comment xml:lang="en">Specifies the place of the secondary education of the participant</rdfs:comment>
    <rdfs:domain rdf:resource="http://purl.org/net/def/metashare#ParticipantInfo"/>
    <rdfs:range rdf:resource="http://www.w3.org/2001/XMLSchema#string"/>
  </owl:DatatypeProperty>
  <ns:CapturingEnvironment rdf:about="http://purl.org/net/def/metashare#plain"/>
  <ns:Naturality rdf:about="http://purl.org/net/def/metashare#planned"/>
  <ns:ToolServiceType rdf:about="http://purl.org/net/def/metashare#platform"/>
  <ns:UseNLPSpecific rdf:about="http://purl.org/net/def/metashare#posTagging"/>
  <owl:DatatypeProperty rdf:about="http://purl.org/net/def/metashare#posesPerSubject">
    <rdfs:comment xml:lang="en">The number of poses per subject that participates in the video part of the resource</rdfs:comment>
    <rdfs:domain rdf:resource="http://purl.org/net/def/metashare#DynamicElementInfo"/>
    <rdfs:range rdf:resource="http://www.w3.org/2001/XMLSchema#int"/>
  </owl:DatatypeProperty>
  <owl:DatatypeProperty rdf:about="http://purl.org/net/def/metashare#position">
    <rdfs:comment xml:lang="en">The position or the title of a person if affiliated to an organization </rdfs:comment>
    <rdfs:domain rdf:resource="http://purl.org/net/def/metashare#Person"/>
    <rdfs:range rdf:resource="http://www.w3.org/2001/XMLSchema#string"/>
  </owl:DatatypeProperty>
  <ns:GrammaticalPhenomenaCoverage rdf:about="http://purl.org/net/def/metashare#ppAttachment"/>
  <ns:EncodingLevel rdf:about="http://purl.org/net/def/metashare#pragmatics"/>
  <ns:ConformanceToStandardsBestPractices rdf:about="http://purl.org/net/def/metashare#pragueTreebank"/>
  <ns:SizeUnit rdf:about="http://purl.org/net/def/metashare#predicates"/>
  <owl:DatatypeProperty rdf:about="http://purl.org/net/def/metashare#profession">
    <rdfs:comment xml:lang="en">Provides information on the participant's profession</rdfs:comment>
    <rdfs:domain rdf:resource="http://purl.org/net/def/metashare#ParticipantInfo"/>
    <rdfs:range rdf:resource="http://www.w3.org/2001/XMLSchema#string"/>
  </owl:DatatypeProperty>
  <owl:DatatypeProperty rdf:about="http://purl.org/net/def/metashare#projectEndDate">
    <rdfs:comment xml:lang="en">The end date of a project related to the resources</rdfs:comment>
    <rdfs:domain rdf:resource="http://purl.org/net/def/metashare#Project"/>
    <rdfs:range rdf:resource="http://www.w3.org/2001/XMLSchema#date"/>
  </owl:DatatypeProperty>
  <owl:DatatypeProperty rdf:about="http://purl.org/net/def/metashare#projectID">
    <rdfs:comment xml:lang="en">An unambiguous referent to a project related to the resource</rdfs:comment>
    <rdfs:domain rdf:resource="http://purl.org/net/def/metashare#Project"/>
    <rdfs:range rdf:resource="http://www.w3.org/2001/XMLSchema#string"/>
  </owl:DatatypeProperty>
  <owl:DatatypeProperty rdf:about="http://purl.org/net/def/metashare#projectName">
    <rdfs:comment xml:lang="en">The full name of a project related to the resource</rdfs:comment>
    <rdfs:domain rdf:resource="http://purl.org/net/def/metashare#Project"/>
    <rdfs:range rdf:resource="http://www.w3.org/1999/02/22-rdf-syntax-ns#langString"/>
  </owl:DatatypeProperty>
  <owl:DatatypeProperty rdf:about="http://purl.org/net/def/metashare#projectShortName">
    <rdfs:comment xml:lang="en">A short name or abbreviation of a project related to the resource</rdfs:comment>
    <rdfs:domain rdf:resource="http://purl.org/net/def/metashare#Project"/>
    <rdfs:range rdf:resource="http://www.w3.org/1999/02/22-rdf-syntax-ns#langString"/>
  </owl:DatatypeProperty>
  <owl:DatatypeProperty rdf:about="http://purl.org/net/def/metashare#projectStartDate">
    <rdfs:comment xml:lang="en">The starting date of a project related to the resource</rdfs:comment>
    <rdfs:domain rdf:resource="http://purl.org/net/def/metashare#Project"/>
    <rdfs:range rdf:resource="http://www.w3.org/2001/XMLSchema#date"/>
  </owl:DatatypeProperty>
  <ns:Naturality rdf:about="http://purl.org/net/def/metashare#prompted"/>
  <ns:SpeechItems rdf:about="http://purl.org/net/def/metashare#properNouns"/>
  <ns:LicenceInfo rdf:about="http://purl.org/net/def/metashare#proprietary">
    <rdfs:comment xml:lang="en">It refers to any kind of proprietary license meant to govern the use of a resource; the rights holder has exclusive legal rights over the license itself; the end user is advised to check the conditionsOfUse metadata element for a quick overview of the rights granted for the use of the resource and pay attention to the full license text; </rdfs:comment>
  </ns:LicenceInfo>
  <ns:SegmentationLevel rdf:about="http://purl.org/net/def/metashare#prosodicBoundaries"/>
  <owl:ObjectProperty rdf:about="http://purl.org/net/def/metashare#publications">
    <rdfs:comment xml:lang="en">Takes publications from DBLP.</rdfs:comment>
    <rdfs:domain rdf:resource="http://purl.org/net/def/metashare#Actor"/>
  </owl:ObjectProperty>
  <ns:UseNLPSpecific rdf:about="http://purl.org/net/def/metashare#qualitativeAnalysis"/>
  <owl:ObjectProperty rdf:about="http://purl.org/net/def/metashare#quality">
    <rdfs:comment xml:lang="en">Specifies the quality level of image resource</rdfs:comment>
    <rdfs:domain rdf:resource="http://purl.org/net/def/metashare#ImageFormatInfo"/>
    <rdfs:range rdf:resource="http://purl.org/net/def/metashare#Quality"/>
  </owl:ObjectProperty>
  <ns:UseNLPSpecific rdf:about="http://purl.org/net/def/metashare#questionAnswering"/>
  <ns:SizeUnit rdf:about="http://purl.org/net/def/metashare#questions"/>
  <ns:SourceChannel rdf:about="http://purl.org/net/def/metashare#radio"/>
  <ns:RasterOrVectorGraphics rdf:about="http://purl.org/net/def/metashare#raster"/>
  <owl:ObjectProperty rdf:about="http://purl.org/net/def/metashare#rasterOrVectorGraphics">
    <rdfs:comment xml:lang="en">Indicates if the image is stored as raster or vector graphics</rdfs:comment>
    <rdfs:domain rdf:resource="http://purl.org/net/def/metashare#ImageFormatInfo"/>
    <rdfs:range rdf:resource="http://purl.org/net/def/metashare#RasterOrVectorGraphics"/>
  </owl:ObjectProperty>
  <ns:SizeUnit rdf:about="http://purl.org/net/def/metashare#rb"/>
  <ns:Naturality rdf:about="http://purl.org/net/def/metashare#readSpeech"/>
  <ns:UseNLPSpecific rdf:about="http://purl.org/net/def/metashare#readingAndWritingAidApplications"/>
  <ns:CompressionName rdf:about="http://purl.org/net/def/metashare#realAudio"/>
  <owl:ObjectProperty rdf:about="http://purl.org/net/def/metashare#recorder">
    <rdfs:comment xml:lang="en">Information on the recorder(s) of the audio or video part of the resource</rdfs:comment>
    <rdfs:domain>
      <owl:Class>
        <owl:unionOf>
          <rdf:Description>
            <rdf:first rdf:resource="http://purl.org/net/def/metashare#CorpusVideoInfo"/>
            <rdf:rest>
              <rdf:Description>
                <rdf:first rdf:resource="http://purl.org/net/def/metashare#CorpusTextNumericalInfo"/>
                <rdf:rest>
                  <rdf:Description>
                    <rdf:first rdf:resource="http://purl.org/net/def/metashare#CorpusAudioInfo"/>
                    <rdf:rest rdf:resource="http://www.w3.org/1999/02/22-rdf-syntax-ns#nil"/>
                  </rdf:Description>
                </rdf:rest>
              </rdf:Description>
            </rdf:rest>
          </rdf:Description>
        </owl:unionOf>
      </owl:Class>
    </rdfs:domain>
    <rdfs:range>
      <owl:Class>
        <owl:unionOf>
          <rdf:Description>
            <rdf:first rdf:resource="http://purl.org/net/def/metashare#Actor"/>
            <rdf:rest>
              <rdf:Description>
                <rdf:first rdf:resource="http://purl.org/net/def/metashare#Actor"/>
                <rdf:rest>
                  <rdf:Description>
                    <rdf:first rdf:resource="http://purl.org/net/def/metashare#Actor"/>
                    <rdf:rest rdf:resource="http://www.w3.org/1999/02/22-rdf-syntax-ns#nil"/>
                  </rdf:Description>
                </rdf:rest>
              </rdf:Description>
            </rdf:rest>
          </rdf:Description>
        </owl:unionOf>
      </owl:Class>
    </rdfs:range>
  </owl:ObjectProperty>
  <owl:ObjectProperty rdf:about="http://purl.org/net/def/metashare#recordingDeviceType">
    <rdfs:comment xml:lang="en">The nature of the recording platform hardware and the storage medium</rdfs:comment>
    <rdfs:domain>
      <owl:Class>
        <owl:unionOf>
          <rdf:Description>
            <rdf:first rdf:resource="http://purl.org/net/def/metashare#CorpusTextNumericalInfo"/>
            <rdf:rest>
              <rdf:Description>
                <rdf:first rdf:resource="http://purl.org/net/def/metashare#CorpusAudioInfo"/>
                <rdf:rest>
                  <rdf:Description>
                    <rdf:first rdf:resource="http://purl.org/net/def/metashare#CorpusVideoInfo"/>
                    <rdf:rest rdf:resource="http://www.w3.org/1999/02/22-rdf-syntax-ns#nil"/>
                  </rdf:Description>
                </rdf:rest>
              </rdf:Description>
            </rdf:rest>
          </rdf:Description>
        </owl:unionOf>
      </owl:Class>
    </rdfs:domain>
    <rdfs:range>
      <owl:Class>
        <owl:unionOf>
          <rdf:Description>
            <rdf:first rdf:resource="http://purl.org/net/def/metashare#RecordingDeviceType"/>
            <rdf:rest>
              <rdf:Description>
                <rdf:first rdf:resource="http://purl.org/net/def/metashare#RecordingDeviceType"/>
                <rdf:rest>
                  <rdf:Description>
                    <rdf:first rdf:resource="http://purl.org/net/def/metashare#RecordingDeviceType"/>
                    <rdf:rest rdf:resource="http://www.w3.org/1999/02/22-rdf-syntax-ns#nil"/>
                  </rdf:Description>
                </rdf:rest>
              </rdf:Description>
            </rdf:rest>
          </rdf:Description>
        </owl:unionOf>
      </owl:Class>
    </rdfs:range>
  </owl:ObjectProperty>
  <owl:DatatypeProperty rdf:about="http://purl.org/net/def/metashare#recordingDeviceTypeDetails">
    <rdfs:comment xml:lang="en">Free text description of the recoding device</rdfs:comment>
    <rdfs:domain>
      <owl:Class>
        <owl:unionOf>
          <rdf:Description>
            <rdf:first rdf:resource="http://purl.org/net/def/metashare#CorpusTextNumericalInfo"/>
            <rdf:rest>
              <rdf:Description>
                <rdf:first rdf:resource="http://purl.org/net/def/metashare#CorpusAudioInfo"/>
                <rdf:rest>
                  <rdf:Description>
                    <rdf:first rdf:resource="http://purl.org/net/def/metashare#CorpusVideoInfo"/>
                    <rdf:rest rdf:resource="http://www.w3.org/1999/02/22-rdf-syntax-ns#nil"/>
                  </rdf:Description>
                </rdf:rest>
              </rdf:Description>
            </rdf:rest>
          </rdf:Description>
        </owl:unionOf>
      </owl:Class>
    </rdfs:domain>
    <rdfs:range rdf:resource="http://www.w3.org/2001/XMLSchema#string"/>
  </owl:DatatypeProperty>
  <owl:ObjectProperty rdf:about="http://purl.org/net/def/metashare#recordingEnvironment">
    <rdfs:comment xml:lang="en">Where the recording took place</rdfs:comment>
    <rdfs:domain>
      <owl:Class>
        <owl:unionOf>
          <rdf:Description>
            <rdf:first rdf:resource="http://purl.org/net/def/metashare#CorpusAudioInfo"/>
            <rdf:rest>
              <rdf:Description>
                <rdf:first rdf:resource="http://purl.org/net/def/metashare#CorpusVideoInfo"/>
                <rdf:rest>
                  <rdf:Description>
                    <rdf:first rdf:resource="http://purl.org/net/def/metashare#CorpusTextNumericalInfo"/>
                    <rdf:rest rdf:resource="http://www.w3.org/1999/02/22-rdf-syntax-ns#nil"/>
                  </rdf:Description>
                </rdf:rest>
              </rdf:Description>
            </rdf:rest>
          </rdf:Description>
        </owl:unionOf>
      </owl:Class>
    </rdfs:domain>
    <rdfs:range>
      <owl:Class>
        <owl:unionOf>
          <rdf:Description>
            <rdf:first rdf:resource="http://purl.org/net/def/metashare#RecordingEnvironment"/>
            <rdf:rest>
              <rdf:Description>
                <rdf:first rdf:resource="http://purl.org/net/def/metashare#RecordingEnvironment"/>
                <rdf:rest>
                  <rdf:Description>
                    <rdf:first rdf:resource="http://purl.org/net/def/metashare#RecordingEnvironment"/>
                    <rdf:rest rdf:resource="http://www.w3.org/1999/02/22-rdf-syntax-ns#nil"/>
                  </rdf:Description>
                </rdf:rest>
              </rdf:Description>
            </rdf:rest>
          </rdf:Description>
        </owl:unionOf>
      </owl:Class>
    </rdfs:range>
  </owl:ObjectProperty>
  <owl:DatatypeProperty rdf:about="http://purl.org/net/def/metashare#recordingPlatformSoftware">
    <rdfs:comment xml:lang="en">The software used for the recording platform</rdfs:comment>
    <rdfs:domain>
      <owl:Class>
        <owl:unionOf>
          <rdf:Description>
            <rdf:first rdf:resource="http://purl.org/net/def/metashare#CorpusVideoInfo"/>
            <rdf:rest>
              <rdf:Description>
                <rdf:first rdf:resource="http://purl.org/net/def/metashare#CorpusTextNumericalInfo"/>
                <rdf:rest>
                  <rdf:Description>
                    <rdf:first rdf:resource="http://purl.org/net/def/metashare#CorpusAudioInfo"/>
                    <rdf:rest rdf:resource="http://www.w3.org/1999/02/22-rdf-syntax-ns#nil"/>
                  </rdf:Description>
                </rdf:rest>
              </rdf:Description>
            </rdf:rest>
          </rdf:Description>
        </owl:unionOf>
      </owl:Class>
    </rdfs:domain>
    <rdfs:range rdf:resource="http://www.w3.org/2001/XMLSchema#string"/>
  </owl:DatatypeProperty>
  <owl:ObjectProperty rdf:about="http://purl.org/net/def/metashare#recordingQuality">
    <rdfs:comment xml:lang="en">Indication of the audio or video recording quality</rdfs:comment>
    <rdfs:domain rdf:resource="http://purl.org/net/def/metashare#AudioFormatInfo"/>
    <rdfs:range rdf:resource="http://purl.org/net/def/metashare#RecordingQuality"/>
  </owl:ObjectProperty>
  <odrl:Set rdf:about="http://purl.org/net/def/metashare#redeposit">
    <rdf:type rdf:resource="http://purl.org/net/def/metashare#ConditionsOfUse"/>
    <rdfs:comment xml:lang="en">Redeposit refers to a kind of 'ConditionsOfUse' imposed by the licence; users are encouraged to deposit any modified versions of the resource they make to the distribution channel through which they have acquired the resource</rdfs:comment>
    <odrl:permission>
      <rdf:Description>
        <odrl:duty>
          <rdf:Description>
            <odrl:action rdf:resource="http://purl.org/net/def/metashare#redeposit"/>
          </rdf:Description>
        </odrl:duty>
      </rdf:Description>
    </odrl:permission>
  </odrl:Set>
  <owl:DatatypeProperty rdf:about="http://purl.org/net/def/metashare#region">
    <rdfs:comment xml:lang="en">The name of the region, county or department as mentioned in the postal address of a person or organization</rdfs:comment>
    <rdfs:domain>
      <owl:Class>
        <owl:unionOf>
          <rdf:Description>
            <rdf:first rdf:resource="http://purl.org/net/def/metashare#Organization"/>
            <rdf:rest>
              <rdf:Description>
                <rdf:first rdf:resource="http://purl.org/net/def/metashare#Person"/>
                <rdf:rest rdf:resource="http://www.w3.org/1999/02/22-rdf-syntax-ns#nil"/>
              </rdf:Description>
            </rdf:rest>
          </rdf:Description>
        </owl:unionOf>
      </owl:Class>
    </rdfs:domain>
    <rdfs:range rdf:resource="http://www.w3.org/2001/XMLSchema#string"/>
  </owl:DatatypeProperty>
  <owl:DatatypeProperty rdf:about="http://purl.org/net/def/metashare#register">
    <rdfs:comment xml:lang="en">For corpora that have already been using register classification</rdfs:comment>
    <rdfs:domain>
      <owl:Class>
        <owl:unionOf>
          <rdf:Description>
            <rdf:first rdf:resource="http://purl.org/net/def/metashare#TextClassificationInfo"/>
            <rdf:rest>
              <rdf:Description>
                <rdf:first rdf:resource="http://purl.org/net/def/metashare#AudioClassificationInfo"/>
                <rdf:rest rdf:resource="http://www.w3.org/1999/02/22-rdf-syntax-ns#nil"/>
              </rdf:Description>
            </rdf:rest>
          </rdf:Description>
        </owl:unionOf>
      </owl:Class>
    </rdfs:domain>
    <rdfs:range rdf:resource="http://www.w3.org/2001/XMLSchema#string"/>
  </owl:DatatypeProperty>
  <owl:ObjectProperty rdf:about="http://purl.org/net/def/metashare#relatedLexiconType">
    <rdfs:comment xml:lang="en">Indicates the position of the lexica that must or can be used with the grammar</rdfs:comment>
    <rdfs:domain rdf:resource="http://purl.org/net/def/metashare#LanguageDescriptionInfo"/>
    <rdfs:range rdf:resource="http://purl.org/net/def/metashare#RelatedLexiconType"/>
  </owl:ObjectProperty>
  <owl:DatatypeProperty rdf:about="http://purl.org/net/def/metashare#relatedResource">
    <rdfs:comment xml:lang="en">The full name, the identifier or the url of the related resource</rdfs:comment>
    <rdfs:domain rdf:resource="http://purl.org/net/def/metashare#RelationInfo"/>
    <rdfs:range rdf:resource="http://www.w3.org/2001/XMLSchema#string"/>
  </owl:DatatypeProperty>
  <owl:ObjectProperty rdf:about="http://purl.org/net/def/metashare#relationInfo">
    <rdfs:domain rdf:resource="http://purl.org/net/def/metashare#LanguageResource"/>
    <rdfs:range rdf:resource="http://purl.org/net/def/metashare#RelationInfo"/>
  </owl:ObjectProperty>
  <owl:DatatypeProperty rdf:about="http://purl.org/net/def/metashare#relationType">
    <rdfs:comment xml:lang="en">Specifies the type of relation not covered by the ones proposed by META-SHARE</rdfs:comment>
    <rdfs:domain rdf:resource="http://purl.org/net/def/metashare#RelationInfo"/>
    <rdfs:range rdf:resource="http://www.w3.org/2001/XMLSchema#string"/>
  </owl:DatatypeProperty>
  <ns:ConditionsOfUse rdf:about="http://purl.org/net/def/metashare#requestPlan">
    <rdf:type rdf:resource="http://www.w3.org/2002/07/owl#NamedIndividual"/>
    <rdfs:comment xml:lang="en">RequestPlan refers to a kind of 'ConditionsOfUse' imposed by the licence; the licensor requires a research plan for granting access.</rdfs:comment>
    <rdfs:label xml:lang="en">Request Plan</rdfs:label>
  </ns:ConditionsOfUse>
  <owl:ObjectProperty rdf:about="http://purl.org/net/def/metashare#requiredHardware">
    <rdfs:comment xml:lang="en">Hardware required for running a tool and/or computational grammar</rdfs:comment>
    <rdfs:domain>
      <owl:Class>
        <owl:unionOf>
          <rdf:Description>
            <rdf:first rdf:resource="http://purl.org/net/def/metashare#LanguageDescriptionInfo"/>
            <rdf:rest>
              <rdf:Description>
                <rdf:first rdf:resource="http://purl.org/net/def/metashare#ToolServiceInfo"/>
                <rdf:rest rdf:resource="http://www.w3.org/1999/02/22-rdf-syntax-ns#nil"/>
              </rdf:Description>
            </rdf:rest>
          </rdf:Description>
        </owl:unionOf>
      </owl:Class>
    </rdfs:domain>
    <rdfs:range>
      <owl:Class>
        <owl:unionOf>
          <rdf:Description>
            <rdf:first rdf:resource="http://purl.org/net/def/metashare#RequiredHardware"/>
            <rdf:rest>
              <rdf:Description>
                <rdf:first rdf:resource="http://purl.org/net/def/metashare#RequiredHardware"/>
                <rdf:rest rdf:resource="http://www.w3.org/1999/02/22-rdf-syntax-ns#nil"/>
              </rdf:Description>
            </rdf:rest>
          </rdf:Description>
        </owl:unionOf>
      </owl:Class>
    </rdfs:range>
  </owl:ObjectProperty>
  <owl:DatatypeProperty rdf:about="http://purl.org/net/def/metashare#requiredLRs">
    <rdfs:comment xml:lang="en">If for running a tool and/or computational grammar, specific LRs (e.g. a grammar, a list of words etc.) are required</rdfs:comment>
    <rdfs:domain>
      <owl:Class>
        <owl:unionOf>
          <rdf:Description>
            <rdf:first rdf:resource="http://purl.org/net/def/metashare#ToolServiceInfo"/>
            <rdf:rest>
              <rdf:Description>
                <rdf:first rdf:resource="http://purl.org/net/def/metashare#LanguageDescriptionInfo"/>
                <rdf:rest rdf:resource="http://www.w3.org/1999/02/22-rdf-syntax-ns#nil"/>
              </rdf:Description>
            </rdf:rest>
          </rdf:Description>
        </owl:unionOf>
      </owl:Class>
    </rdfs:domain>
    <rdfs:range rdf:resource="http://www.w3.org/2001/XMLSchema#string"/>
  </owl:DatatypeProperty>
  <owl:DatatypeProperty rdf:about="http://purl.org/net/def/metashare#requiredSoftware">
    <rdfs:comment xml:lang="en">Additional software required for running a tool and/or computational grammar</rdfs:comment>
    <rdfs:domain>
      <owl:Class>
        <owl:unionOf>
          <rdf:Description>
            <rdf:first rdf:resource="http://purl.org/net/def/metashare#ToolServiceInfo"/>
            <rdf:rest>
              <rdf:Description>
                <rdf:first rdf:resource="http://purl.org/net/def/metashare#LanguageDescriptionInfo"/>
                <rdf:rest rdf:resource="http://www.w3.org/1999/02/22-rdf-syntax-ns#nil"/>
              </rdf:Description>
            </rdf:rest>
          </rdf:Description>
        </owl:unionOf>
      </owl:Class>
    </rdfs:domain>
    <rdfs:range rdf:resource="http://www.w3.org/2001/XMLSchema#string"/>
  </owl:DatatypeProperty>
  <ns:ConditionsOfUse rdf:about="http://purl.org/net/def/metashare#research">
    <rdf:type rdf:resource="http://www.w3.org/2002/07/owl#NamedIndividual"/>
    <rdfs:comment xml:lang="en">Research refers to a kind of 'ConditionsOfUse' imposed by the licence; the resource can only be used for research purposes.</rdfs:comment>
    <rdfs:label xml:lang="en">Research</rdfs:label>
  </ns:ConditionsOfUse>
  <owl:ObjectProperty rdf:about="http://purl.org/net/def/metashare#resolutionInfo">
    <rdfs:comment xml:lang="en">Groups together information on the image resolution</rdfs:comment>
    <rdfs:domain>
      <owl:Class>
        <owl:unionOf>
          <rdf:Description>
            <rdf:first rdf:resource="http://purl.org/net/def/metashare#ImageFormatInfo"/>
            <rdf:rest>
              <rdf:Description>
                <rdf:first rdf:resource="http://purl.org/net/def/metashare#VideoFormatInfo"/>
                <rdf:rest rdf:resource="http://www.w3.org/1999/02/22-rdf-syntax-ns#nil"/>
              </rdf:Description>
            </rdf:rest>
          </rdf:Description>
        </owl:unionOf>
      </owl:Class>
    </rdfs:domain>
    <rdfs:range>
      <owl:Class>
        <owl:unionOf>
          <rdf:Description>
            <rdf:first rdf:resource="http://purl.org/net/def/metashare#ResolutionInfo"/>
            <rdf:rest>
              <rdf:Description>
                <rdf:first rdf:resource="http://purl.org/net/def/metashare#ResolutionInfo"/>
                <rdf:rest rdf:resource="http://www.w3.org/1999/02/22-rdf-syntax-ns#nil"/>
              </rdf:Description>
            </rdf:rest>
          </rdf:Description>
        </owl:unionOf>
      </owl:Class>
    </rdfs:range>
  </owl:ObjectProperty>
  <owl:ObjectProperty rdf:about="http://purl.org/net/def/metashare#resolutionStandard">
    <rdfs:comment xml:lang="en">The standard to which  the resolution conforms</rdfs:comment>
    <rdfs:domain rdf:resource="http://purl.org/net/def/metashare#ResolutionInfo"/>
    <rdfs:range rdf:resource="http://purl.org/net/def/metashare#ResolutionStandard"/>
  </owl:ObjectProperty>
  <owl:DatatypeProperty rdf:about="http://purl.org/net/def/metashare#resourceAssociatedWith">
    <rdfs:comment xml:lang="en">Refers to another resource that the resource described uses for its operation</rdfs:comment>
    <rdfs:domain rdf:resource="http://purl.org/net/def/metashare#LanguageResource"/>
    <rdfs:range rdf:resource="http://www.w3.org/2001/XMLSchema#string"/>
  </owl:DatatypeProperty>
  <owl:DatatypeProperty rdf:about="http://purl.org/net/def/metashare#resourceShortName">
    <rdfs:comment xml:lang="en">The short form (abbreviation, acronym etc.) used to identify the resource; the element can be repeated for the different language versions using the "lang" attribute to specify the language.</rdfs:comment>
    <rdfs:domain rdf:resource="http://purl.org/net/def/metashare#LanguageResource"/>
    <rdfs:range rdf:resource="http://www.w3.org/1999/02/22-rdf-syntax-ns#langString"/>
  </owl:DatatypeProperty>
  <owl:ObjectProperty rdf:about="http://purl.org/net/def/metashare#resourceType">
    <rdfs:comment xml:lang="en">Specifies the type of the resource being described</rdfs:comment>
    <rdfs:domain>
      <owl:Class>
        <owl:unionOf>
          <rdf:Description>
            <rdf:first rdf:resource="http://purl.org/net/def/metashare#OutputInfo"/>
            <rdf:rest>
              <rdf:Description>
                <rdf:first rdf:resource="http://purl.org/net/def/metashare#InputInfo"/>
                <rdf:rest>
                  <rdf:Description>
                    <rdf:first rdf:resource="http://purl.org/net/def/metashare#LanguageDescriptionInfo"/>
                    <rdf:rest>
                      <rdf:Description>
                        <rdf:first rdf:resource="http://purl.org/net/def/metashare#ToolServiceInfo"/>
                        <rdf:rest>
                          <rdf:Description>
                            <rdf:first rdf:resource="http://purl.org/net/def/metashare#CorpusInfo"/>
                            <rdf:rest rdf:resource="http://www.w3.org/1999/02/22-rdf-syntax-ns#nil"/>
                          </rdf:Description>
                        </rdf:rest>
                      </rdf:Description>
                    </rdf:rest>
                  </rdf:Description>
                </rdf:rest>
              </rdf:Description>
            </rdf:rest>
          </rdf:Description>
        </owl:unionOf>
      </owl:Class>
    </rdfs:domain>
    <rdfs:range>
      <owl:Class>
        <owl:unionOf>
          <rdf:Description>
            <rdf:first rdf:resource="http://purl.org/net/def/metashare#ResourceType"/>
            <rdf:rest>
              <rdf:Description>
                <rdf:first rdf:resource="http://purl.org/net/def/metashare#ResourceType"/>
                <rdf:rest>
                  <rdf:Description>
                    <rdf:first rdf:resource="http://purl.org/net/def/metashare#ResourceType"/>
                    <rdf:rest>
                      <rdf:Description>
                        <rdf:first rdf:resource="http://purl.org/net/def/metashare#ResourceType"/>
                        <rdf:rest>
                          <rdf:Description>
                            <rdf:first rdf:resource="http://purl.org/net/def/metashare#ResourceType"/>
                            <rdf:rest rdf:resource="http://www.w3.org/1999/02/22-rdf-syntax-ns#nil"/>
                          </rdf:Description>
                        </rdf:rest>
                      </rdf:Description>
                    </rdf:rest>
                  </rdf:Description>
                </rdf:rest>
              </rdf:Description>
            </rdf:rest>
          </rdf:Description>
        </owl:unionOf>
      </owl:Class>
    </rdfs:range>
  </owl:ObjectProperty>
  <owl:DatatypeProperty rdf:about="http://purl.org/net/def/metashare#revision">
    <rdfs:comment xml:lang="en">Provides an account of the revisions in free text or a link to a document with revisions</rdfs:comment>
    <rdfs:domain>
      <owl:Class>
        <owl:unionOf>
          <rdf:Description>
            <rdf:first rdf:resource="http://purl.org/net/def/metashare#LanguageResource"/>
            <rdf:rest>
              <rdf:Description>
                <rdf:first rdf:resource="http://purl.org/net/def/metashare#MetadataInfo"/>
                <rdf:rest rdf:resource="http://www.w3.org/1999/02/22-rdf-syntax-ns#nil"/>
              </rdf:Description>
            </rdf:rest>
          </rdf:Description>
        </owl:unionOf>
      </owl:Class>
    </rdfs:domain>
    <rdfs:range rdf:resource="http://www.w3.org/2001/XMLSchema#string"/>
  </owl:DatatypeProperty>
  <owl:DatatypeProperty rdf:about="http://purl.org/net/def/metashare#robustness">
    <rdfs:comment xml:lang="en">Free text statement on the robustness of the grammar (how well the grammar can cope with misspelt/unknown etc. input, i.e. whether it can produce even partial interpretations of the input)</rdfs:comment>
    <rdfs:domain rdf:resource="http://purl.org/net/def/metashare#LanguageDescriptionInfo"/>
    <rdfs:range rdf:resource="http://www.w3.org/2001/XMLSchema#string"/>
  </owl:DatatypeProperty>
  <ns:ScenarioType rdf:about="http://purl.org/net/def/metashare#rolePlay"/>
  <ns:SizeUnit rdf:about="http://purl.org/net/def/metashare#rules"/>
  <owl:DatatypeProperty rdf:about="http://purl.org/net/def/metashare#runningEnvironmentDetails">
    <rdfs:comment xml:lang="en">Provides further information on the running environment</rdfs:comment>
    <rdfs:domain>
      <owl:Class>
        <owl:unionOf>
          <rdf:Description>
            <rdf:first rdf:resource="http://purl.org/net/def/metashare#ToolServiceInfo"/>
            <rdf:rest>
              <rdf:Description>
                <rdf:first rdf:resource="http://purl.org/net/def/metashare#LanguageDescriptionInfo"/>
                <rdf:rest rdf:resource="http://www.w3.org/1999/02/22-rdf-syntax-ns#nil"/>
              </rdf:Description>
            </rdf:rest>
          </rdf:Description>
        </owl:unionOf>
      </owl:Class>
    </rdfs:domain>
    <rdfs:range rdf:resource="http://www.w3.org/2001/XMLSchema#string"/>
  </owl:DatatypeProperty>
  <owl:DatatypeProperty rdf:about="http://purl.org/net/def/metashare#runningTime">
    <rdfs:comment xml:lang="en">Gives information on the running time of a tool or service</rdfs:comment>
    <rdfs:domain rdf:resource="http://purl.org/net/def/metashare#ToolServiceInfo"/>
    <rdfs:range rdf:resource="http://www.w3.org/2001/XMLSchema#string"/>
  </owl:DatatypeProperty>
  <owl:DatatypeProperty rdf:about="http://purl.org/net/def/metashare#samplesLocation">
    <rdfs:comment xml:lang="en">A url with samples of the resource or, in the case of tools, of samples of the output</rdfs:comment>
    <rdfs:domain rdf:resource="http://purl.org/net/def/metashare#LanguageResource"/>
    <rdfs:range rdf:resource="http://www.w3.org/2001/XMLSchema#string"/>
  </owl:DatatypeProperty>
  <owl:ObjectProperty rdf:about="http://purl.org/net/def/metashare#scenarioType">
    <rdfs:comment xml:lang="en">Indicates the task defined for the conversation or the interaction of participants</rdfs:comment>
    <rdfs:domain>
      <owl:Class>
        <owl:unionOf>
          <rdf:Description>
            <rdf:first rdf:resource="http://purl.org/net/def/metashare#CorpusVideoInfo"/>
            <rdf:rest>
              <rdf:Description>
                <rdf:first rdf:resource="http://purl.org/net/def/metashare#CorpusAudioInfo"/>
                <rdf:rest rdf:resource="http://www.w3.org/1999/02/22-rdf-syntax-ns#nil"/>
              </rdf:Description>
            </rdf:rest>
          </rdf:Description>
        </owl:unionOf>
      </owl:Class>
    </rdfs:domain>
    <rdfs:range>
      <owl:Class>
        <owl:unionOf>
          <rdf:Description>
            <rdf:first rdf:resource="http://purl.org/net/def/metashare#ScenarioType"/>
            <rdf:rest>
              <rdf:Description>
                <rdf:first rdf:resource="http://purl.org/net/def/metashare#ScenarioType"/>
                <rdf:rest rdf:resource="http://www.w3.org/1999/02/22-rdf-syntax-ns#nil"/>
              </rdf:Description>
            </rdf:rest>
          </rdf:Description>
        </owl:unionOf>
      </owl:Class>
    </rdfs:range>
  </owl:ObjectProperty>
  <ns:SegmentationLevel rdf:about="http://purl.org/net/def/metashare#scene"/>
  <owl:ObjectProperty rdf:about="http://purl.org/net/def/metashare#sceneIllumination">
    <rdfs:comment xml:lang="en">Information on the illumination of the scene</rdfs:comment>
    <rdfs:domain>
      <owl:Class>
        <owl:unionOf>
          <rdf:Description>
            <rdf:first rdf:resource="http://purl.org/net/def/metashare#CorpusAudioInfo"/>
            <rdf:rest>
              <rdf:Description>
                <rdf:first rdf:resource="http://purl.org/net/def/metashare#CorpusTextNumericalInfo"/>
                <rdf:rest>
                  <rdf:Description>
                    <rdf:first rdf:resource="http://purl.org/net/def/metashare#CorpusImageInfo"/>
                    <rdf:rest>
                      <rdf:Description>
                        <rdf:first rdf:resource="http://purl.org/net/def/metashare#CorpusVideoInfo"/>
                        <rdf:rest rdf:resource="http://www.w3.org/1999/02/22-rdf-syntax-ns#nil"/>
                      </rdf:Description>
                    </rdf:rest>
                  </rdf:Description>
                </rdf:rest>
              </rdf:Description>
            </rdf:rest>
          </rdf:Description>
        </owl:unionOf>
      </owl:Class>
    </rdfs:domain>
    <rdfs:range>
      <owl:Class>
        <owl:unionOf>
          <rdf:Description>
            <rdf:first rdf:resource="http://purl.org/net/def/metashare#SceneIllumination"/>
            <rdf:rest>
              <rdf:Description>
                <rdf:first rdf:resource="http://purl.org/net/def/metashare#SceneIllumination"/>
                <rdf:rest>
                  <rdf:Description>
                    <rdf:first rdf:resource="http://purl.org/net/def/metashare#SceneIllumination"/>
                    <rdf:rest>
                      <rdf:Description>
                        <rdf:first rdf:resource="http://purl.org/net/def/metashare#SceneIllumination"/>
                        <rdf:rest rdf:resource="http://www.w3.org/1999/02/22-rdf-syntax-ns#nil"/>
                      </rdf:Description>
                    </rdf:rest>
                  </rdf:Description>
                </rdf:rest>
              </rdf:Description>
            </rdf:rest>
          </rdf:Description>
        </owl:unionOf>
      </owl:Class>
    </rdfs:range>
  </owl:ObjectProperty>
  <ns:DurationOfAudioInfoUnit rdf:about="http://purl.org/net/def/metashare#seconds">
    <rdf:type rdf:resource="http://purl.org/net/def/metashare#DurationOfEffectiveSpeechInfoUnit"/>
    <rdf:type rdf:resource="http://purl.org/net/def/metashare#SizeUnit"/>
  </ns:DurationOfAudioInfoUnit>
  <ns:AnnotationType rdf:about="http://purl.org/net/def/metashare#segmentation"/>
  <owl:ObjectProperty rdf:about="http://purl.org/net/def/metashare#segmentationLevel">
    <rdfs:comment xml:lang="en">Specifies the segmentation unit in terms of which the resource has been segmented or the level of segmentation a tool/service requires/outputs</rdfs:comment>
    <rdfs:domain>
      <owl:Class>
        <owl:unionOf>
          <rdf:Description>
            <rdf:first rdf:resource="http://purl.org/net/def/metashare#AnnotationInfo"/>
            <rdf:rest>
              <rdf:Description>
                <rdf:first rdf:resource="http://purl.org/net/def/metashare#OutputInfo"/>
                <rdf:rest>
                  <rdf:Description>
                    <rdf:first rdf:resource="http://purl.org/net/def/metashare#InputInfo"/>
                    <rdf:rest rdf:resource="http://www.w3.org/1999/02/22-rdf-syntax-ns#nil"/>
                  </rdf:Description>
                </rdf:rest>
              </rdf:Description>
            </rdf:rest>
          </rdf:Description>
        </owl:unionOf>
      </owl:Class>
    </rdfs:domain>
    <rdfs:range>
      <owl:Class>
        <owl:unionOf>
          <rdf:Description>
            <rdf:first rdf:resource="http://purl.org/net/def/metashare#SegmentationLevel"/>
            <rdf:rest>
              <rdf:Description>
                <rdf:first rdf:resource="http://purl.org/net/def/metashare#SegmentationLevel"/>
                <rdf:rest>
                  <rdf:Description>
                    <rdf:first rdf:resource="http://purl.org/net/def/metashare#SegmentationLevel"/>
                    <rdf:rest rdf:resource="http://www.w3.org/1999/02/22-rdf-syntax-ns#nil"/>
                  </rdf:Description>
                </rdf:rest>
              </rdf:Description>
            </rdf:rest>
          </rdf:Description>
        </owl:unionOf>
      </owl:Class>
    </rdfs:range>
  </owl:ObjectProperty>
  <ns:SemanticAnnotation rdf:about="http://purl.org/net/def/metashare#semanticAnnotation">
    <rdf:type rdf:resource="http://purl.org/net/def/metashare#AnnotationType"/>
  </ns:SemanticAnnotation>
  <ns:SemanticAnnotation rdf:about="http://purl.org/net/def/metashare#semanticAnnotation-certaintyLevel">
    <rdf:type rdf:resource="http://purl.org/net/def/metashare#AnnotationType"/>
  </ns:SemanticAnnotation>
  <ns:SemanticAnnotation rdf:about="http://purl.org/net/def/metashare#semanticAnnotation-emotions">
    <rdf:type rdf:resource="http://purl.org/net/def/metashare#AnnotationType"/>
  </ns:SemanticAnnotation>
  <ns:SemanticAnnotation rdf:about="http://purl.org/net/def/metashare#semanticAnnotation-entityMentions">
    <rdf:type rdf:resource="http://purl.org/net/def/metashare#AnnotationType"/>
  </ns:SemanticAnnotation>
  <ns:SemanticAnnotation rdf:about="http://purl.org/net/def/metashare#semanticAnnotation-events">
    <rdf:type rdf:resource="http://purl.org/net/def/metashare#AnnotationType"/>
  </ns:SemanticAnnotation>
  <ns:SemanticAnnotation rdf:about="http://purl.org/net/def/metashare#semanticAnnotation-namedEntities">
    <rdf:type rdf:resource="http://purl.org/net/def/metashare#AnnotationType"/>
  </ns:SemanticAnnotation>
  <ns:SemanticAnnotation rdf:about="http://purl.org/net/def/metashare#semanticAnnotation-polarity">
    <rdf:type rdf:resource="http://purl.org/net/def/metashare#AnnotationType"/>
  </ns:SemanticAnnotation>
  <ns:SemanticAnnotation rdf:about="http://purl.org/net/def/metashare#semanticAnnotation-questionTopicalTarget">
    <rdf:type rdf:resource="http://purl.org/net/def/metashare#AnnotationType"/>
  </ns:SemanticAnnotation>
  <ns:SemanticAnnotation rdf:about="http://purl.org/net/def/metashare#semanticAnnotation-semanticClasses">
    <rdf:type rdf:resource="http://purl.org/net/def/metashare#AnnotationType"/>
  </ns:SemanticAnnotation>
  <ns:SemanticAnnotation rdf:about="http://purl.org/net/def/metashare#semanticAnnotation-semanticRelations">
    <rdf:type rdf:resource="http://purl.org/net/def/metashare#AnnotationType"/>
  </ns:SemanticAnnotation>
  <ns:SemanticAnnotation rdf:about="http://purl.org/net/def/metashare#semanticAnnotation-semanticRoles">
    <rdf:type rdf:resource="http://purl.org/net/def/metashare#AnnotationType"/>
  </ns:SemanticAnnotation>
  <ns:SemanticAnnotation rdf:about="http://purl.org/net/def/metashare#semanticAnnotation-speechActs">
    <rdf:type rdf:resource="http://purl.org/net/def/metashare#AnnotationType"/>
  </ns:SemanticAnnotation>
  <ns:SemanticAnnotation rdf:about="http://purl.org/net/def/metashare#semanticAnnotation-temporalExpressions">
    <rdf:type rdf:resource="http://purl.org/net/def/metashare#AnnotationType"/>
  </ns:SemanticAnnotation>
  <ns:SemanticAnnotation rdf:about="http://purl.org/net/def/metashare#semanticAnnotation-textualEntailment">
    <rdf:type rdf:resource="http://purl.org/net/def/metashare#AnnotationType"/>
  </ns:SemanticAnnotation>
  <ns:SemanticAnnotation rdf:about="http://purl.org/net/def/metashare#semanticAnnotation-wordSenses">
    <rdf:type rdf:resource="http://purl.org/net/def/metashare#AnnotationType"/>
  </ns:SemanticAnnotation>
  <ns:UseNLPSpecific rdf:about="http://purl.org/net/def/metashare#semanticRoleLabelling"/>
  <ns:SizeUnit rdf:about="http://purl.org/net/def/metashare#semanticUnits"/>
  <ns:UseNLPSpecific rdf:about="http://purl.org/net/def/metashare#semanticWeb"/>
  <ns:EncodingLevel rdf:about="http://purl.org/net/def/metashare#semantics">
    <rdf:type rdf:resource="http://purl.org/net/def/metashare#ExtraTextualInformationUnit"/>
  </ns:EncodingLevel>
  <ns:LinguisticInformation rdf:about="http://purl.org/net/def/metashare#semantics-CrossReferences"/>
  <ns:LinguisticInformation rdf:about="http://purl.org/net/def/metashare#semantics-Domain"/>
  <ns:LinguisticInformation rdf:about="http://purl.org/net/def/metashare#semantics-EventType"/>
  <ns:LinguisticInformation rdf:about="http://purl.org/net/def/metashare#semantics-QualiaStructure"/>
  <ns:LinguisticInformation rdf:about="http://purl.org/net/def/metashare#semantics-Relations"/>
  <ns:LinguisticInformation rdf:about="http://purl.org/net/def/metashare#semantics-Relations-Antonyms"/>
  <ns:LinguisticInformation rdf:about="http://purl.org/net/def/metashare#semantics-Relations-Hyperonyms"/>
  <ns:LinguisticInformation rdf:about="http://purl.org/net/def/metashare#semantics-Relations-Hyponyms"/>
  <ns:LinguisticInformation rdf:about="http://purl.org/net/def/metashare#semantics-Relations-Meronyms"/>
  <ns:LinguisticInformation rdf:about="http://purl.org/net/def/metashare#semantics-Relations-Synonyms"/>
  <ns:LinguisticInformation rdf:about="http://purl.org/net/def/metashare#semantics-Relations-Troponyms"/>
  <ns:LinguisticInformation rdf:about="http://purl.org/net/def/metashare#semantics-SemanticClass"/>
  <ns:LinguisticInformation rdf:about="http://purl.org/net/def/metashare#semantics-SemanticRoles"/>
  <ns:LinguisticInformation rdf:about="http://purl.org/net/def/metashare#semantics-Traits"/>
  <ns:Interactivity rdf:about="http://purl.org/net/def/metashare#semiInteractive"/>
  <ns:Naturality rdf:about="http://purl.org/net/def/metashare#semiPlanned"/>
  <owl:DatatypeProperty rdf:about="http://purl.org/net/def/metashare#sensorTechnology">
    <rdfs:comment xml:lang="en">Specifies either the type of image sensor or the sensing method used in the camera or the image-capture device</rdfs:comment>
    <rdfs:domain>
      <owl:Class>
        <owl:unionOf>
          <rdf:Description>
            <rdf:first rdf:resource="http://purl.org/net/def/metashare#CorpusImageInfo"/>
            <rdf:rest>
              <rdf:Description>
                <rdf:first rdf:resource="http://purl.org/net/def/metashare#CorpusVideoInfo"/>
                <rdf:rest>
                  <rdf:Description>
                    <rdf:first rdf:resource="http://purl.org/net/def/metashare#CorpusTextNumericalInfo"/>
                    <rdf:rest>
                      <rdf:Description>
                        <rdf:first rdf:resource="http://purl.org/net/def/metashare#CorpusAudioInfo"/>
                        <rdf:rest rdf:resource="http://www.w3.org/1999/02/22-rdf-syntax-ns#nil"/>
                      </rdf:Description>
                    </rdf:rest>
                  </rdf:Description>
                </rdf:rest>
              </rdf:Description>
            </rdf:rest>
          </rdf:Description>
        </owl:unionOf>
      </owl:Class>
    </rdfs:domain>
    <rdfs:range rdf:resource="http://www.w3.org/2001/XMLSchema#string"/>
  </owl:DatatypeProperty>
  <ns:SegmentationLevel rdf:about="http://purl.org/net/def/metashare#sentence"/>
  <ns:SizeUnit rdf:about="http://purl.org/net/def/metashare#sentences"/>
  <ns:UseNLPSpecific rdf:about="http://purl.org/net/def/metashare#sentimentAnalysis"/>
  <ns:ToolServiceType rdf:about="http://purl.org/net/def/metashare#service"/>
  <owl:ObjectProperty rdf:about="http://purl.org/net/def/metashare#sexOfPersons">
    <rdfs:comment xml:lang="en">The gender of the group of participants</rdfs:comment>
    <rdfs:domain>
      <owl:Class>
        <owl:unionOf>
          <rdf:Description>
            <rdf:first rdf:resource="http://purl.org/net/def/metashare#CorpusAudioInfo"/>
            <rdf:rest>
              <rdf:Description>
                <rdf:first rdf:resource="http://purl.org/net/def/metashare#CorpusTextNumericalInfo"/>
                <rdf:rest>
                  <rdf:Description>
                    <rdf:first rdf:resource="http://purl.org/net/def/metashare#CorpusImageInfo"/>
                    <rdf:rest>
                      <rdf:Description>
                        <rdf:first rdf:resource="http://purl.org/net/def/metashare#CorpusVideoInfo"/>
                        <rdf:rest rdf:resource="http://www.w3.org/1999/02/22-rdf-syntax-ns#nil"/>
                      </rdf:Description>
                    </rdf:rest>
                  </rdf:Description>
                </rdf:rest>
              </rdf:Description>
            </rdf:rest>
          </rdf:Description>
        </owl:unionOf>
      </owl:Class>
    </rdfs:domain>
    <rdfs:range>
      <owl:Class>
        <owl:unionOf>
          <rdf:Description>
            <rdf:first rdf:resource="http://purl.org/net/def/metashare#SexOfPersons"/>
            <rdf:rest>
              <rdf:Description>
                <rdf:first rdf:resource="http://purl.org/net/def/metashare#SexOfPersons"/>
                <rdf:rest>
                  <rdf:Description>
                    <rdf:first rdf:resource="http://purl.org/net/def/metashare#SexOfPersons"/>
                    <rdf:rest>
                      <rdf:Description>
                        <rdf:first rdf:resource="http://purl.org/net/def/metashare#SexOfPersons"/>
                        <rdf:rest rdf:resource="http://www.w3.org/1999/02/22-rdf-syntax-ns#nil"/>
                      </rdf:Description>
                    </rdf:rest>
                  </rdf:Description>
                </rdf:rest>
              </rdf:Description>
            </rdf:rest>
          </rdf:Description>
        </owl:unionOf>
      </owl:Class>
    </rdfs:range>
  </owl:ObjectProperty>
  <owl:DatatypeProperty rdf:about="http://purl.org/net/def/metashare#shallowness">
    <rdfs:comment xml:lang="en">Free text statement on the shallowness of the grammar (how deep the syntactic analysis performed by the grammar can be)</rdfs:comment>
    <rdfs:domain rdf:resource="http://purl.org/net/def/metashare#LanguageDescriptionInfo"/>
    <rdfs:range rdf:resource="http://www.w3.org/2001/XMLSchema#string"/>
  </owl:DatatypeProperty>
  <odrl:Set rdf:about="http://purl.org/net/def/metashare#shareAlike">
    <rdf:type rdf:resource="http://purl.org/net/def/metashare#ConditionsOfUse"/>
    <odrl:permission>
      <rdf:Description>
        <odrl:duty>
          <rdf:Description>
            <odrl:action rdf:resource="http://creativecommons.org/ns#ShareALike"/>
          </rdf:Description>
        </odrl:duty>
      </rdf:Description>
    </odrl:permission>
  </odrl:Set>
  <ns:CompressionName rdf:about="http://purl.org/net/def/metashare#shorten"/>
  <ns:SegmentationLevel rdf:about="http://purl.org/net/def/metashare#shot"/>
  <ns:SizeUnit rdf:about="http://purl.org/net/def/metashare#shots"/>
  <owl:ObjectProperty rdf:about="http://purl.org/net/def/metashare#signConvention">
    <rdfs:comment xml:lang="en">Binary representation of numbers</rdfs:comment>
    <rdfs:domain rdf:resource="http://purl.org/net/def/metashare#AudioFormatInfo"/>
    <rdfs:range rdf:resource="http://purl.org/net/def/metashare#SignConvention"/>
  </owl:ObjectProperty>
  <ns:ModalityType rdf:about="http://purl.org/net/def/metashare#signLanguage"/>
  <ns:UseNLPSpecific rdf:about="http://purl.org/net/def/metashare#signLanguageGeneration"/>
  <ns:UseNLPSpecific rdf:about="http://purl.org/net/def/metashare#signLanguageRecognition"/>
  <ns:SegmentationLevel rdf:about="http://purl.org/net/def/metashare#signal"/>
  <owl:ObjectProperty rdf:about="http://purl.org/net/def/metashare#signalEncoding">
    <rdfs:comment xml:lang="en">Specifies the  encoding the audio type uses</rdfs:comment>
    <rdfs:domain rdf:resource="http://purl.org/net/def/metashare#AudioFormatInfo"/>
    <rdfs:range rdf:resource="http://purl.org/net/def/metashare#SignalEncoding"/>
  </owl:ObjectProperty>
  <ns:SignConvention rdf:about="http://purl.org/net/def/metashare#signedInteger"/>
  <ns:SceneIllumination rdf:about="http://purl.org/net/def/metashare#singleSource"/>
  <owl:DatatypeProperty rdf:about="http://purl.org/net/def/metashare#size">
    <rdfs:comment xml:lang="en">Specifies the size of the resource with regard to the SizeUnit measurement in form of a number</rdfs:comment>
    <rdfs:domain rdf:resource="http://purl.org/net/def/metashare#Size"/>
    <rdfs:range rdf:resource="http://www.w3.org/2001/XMLSchema#string"/>
  </owl:DatatypeProperty>
  <owl:DatatypeProperty rdf:about="http://purl.org/net/def/metashare#sizeHeight">
    <rdfs:comment xml:lang="en">The frame height in pixels</rdfs:comment>
    <rdfs:domain rdf:resource="http://purl.org/net/def/metashare#ResolutionInfo"/>
    <rdfs:range rdf:resource="http://www.w3.org/2001/XMLSchema#int"/>
  </owl:DatatypeProperty>
  <owl:ObjectProperty rdf:about="http://purl.org/net/def/metashare#sizeInfo">
    <rdfs:comment xml:lang="en">Groups information on the size of the resource or of resource parts</rdfs:comment>
    <rdfs:domain>
      <owl:Class>
        <owl:unionOf>
          <rdf:Description>
            <rdf:first rdf:resource="http://purl.org/net/def/metashare#CorpusTextNumericalInfo"/>
            <rdf:rest>
              <rdf:Description>
                <rdf:first rdf:resource="http://purl.org/net/def/metashare#CorpusImageInfo"/>
                <rdf:rest>
                  <rdf:Description>
                    <rdf:first rdf:resource="http://purl.org/net/def/metashare#LanguageDescriptionTextInfo"/>
                    <rdf:rest>
                      <rdf:Description>
                        <rdf:first rdf:resource="http://purl.org/net/def/metashare#LexicalConceptualResourceImageInfo"/>
                        <rdf:rest>
                          <rdf:Description>
                            <rdf:first rdf:resource="http://purl.org/net/def/metashare#LexicalConceptualResourceAudioInfo"/>
                            <rdf:rest>
                              <rdf:Description>
                                <rdf:first rdf:resource="http://purl.org/net/def/metashare#CorpusTextInfo"/>
                                <rdf:rest>
                                  <rdf:Description>
                                    <rdf:first rdf:resource="http://purl.org/net/def/metashare#AudioSizeInfo"/>
                                    <rdf:rest>
                                      <rdf:Description>
                                        <rdf:first rdf:resource="http://purl.org/net/def/metashare#CorpusTextNgramInfo"/>
                                        <rdf:rest>
                                          <rdf:Description>
                                            <rdf:first rdf:resource="http://purl.org/net/def/metashare#LexicalConceptualResourceTextInfo"/>
                                            <rdf:rest>
                                              <rdf:Description>
                                                <rdf:first rdf:resource="http://purl.org/net/def/metashare#LexicalConceptualResourceVideoInfo"/>
                                                <rdf:rest>
                                                  <rdf:Description>
                                                    <rdf:first rdf:resource="http://purl.org/net/def/metashare#LanguageDescriptionVideoInfo"/>
                                                    <rdf:rest>
                                                      <rdf:Description>
                                                        <rdf:first rdf:resource="http://purl.org/net/def/metashare#LanguageDescriptionImageInfo"/>
                                                        <rdf:rest>
                                                          <rdf:Description>
                                                            <rdf:first rdf:resource="http://purl.org/net/def/metashare#CorpusVideoInfo"/>
                                                            <rdf:rest rdf:resource="http://www.w3.org/1999/02/22-rdf-syntax-ns#nil"/>
                                                          </rdf:Description>
                                                        </rdf:rest>
                                                      </rdf:Description>
                                                    </rdf:rest>
                                                  </rdf:Description>
                                                </rdf:rest>
                                              </rdf:Description>
                                            </rdf:rest>
                                          </rdf:Description>
                                        </rdf:rest>
                                      </rdf:Description>
                                    </rdf:rest>
                                  </rdf:Description>
                                </rdf:rest>
                              </rdf:Description>
                            </rdf:rest>
                          </rdf:Description>
                        </rdf:rest>
                      </rdf:Description>
                    </rdf:rest>
                  </rdf:Description>
                </rdf:rest>
              </rdf:Description>
            </rdf:rest>
          </rdf:Description>
        </owl:unionOf>
      </owl:Class>
    </rdfs:domain>
    <rdfs:range>
      <owl:Class>
        <owl:unionOf>
          <rdf:Description>
            <rdf:first rdf:resource="http://purl.org/net/def/metashare#Size"/>
            <rdf:rest>
              <rdf:Description>
                <rdf:first rdf:resource="http://purl.org/net/def/metashare#Size"/>
                <rdf:rest>
                  <rdf:Description>
                    <rdf:first rdf:resource="http://purl.org/net/def/metashare#Size"/>
                    <rdf:rest>
                      <rdf:Description>
                        <rdf:first rdf:resource="http://purl.org/net/def/metashare#Size"/>
                        <rdf:rest>
                          <rdf:Description>
                            <rdf:first rdf:resource="http://purl.org/net/def/metashare#Size"/>
                            <rdf:rest>
                              <rdf:Description>
                                <rdf:first rdf:resource="http://purl.org/net/def/metashare#Size"/>
                                <rdf:rest>
                                  <rdf:Description>
                                    <rdf:first rdf:resource="http://purl.org/net/def/metashare#Size"/>
                                    <rdf:rest>
                                      <rdf:Description>
                                        <rdf:first rdf:resource="http://purl.org/net/def/metashare#Size"/>
                                        <rdf:rest>
                                          <rdf:Description>
                                            <rdf:first rdf:resource="http://purl.org/net/def/metashare#Size"/>
                                            <rdf:rest>
                                              <rdf:Description>
                                                <rdf:first rdf:resource="http://purl.org/net/def/metashare#Size"/>
                                                <rdf:rest>
                                                  <rdf:Description>
                                                    <rdf:first rdf:resource="http://purl.org/net/def/metashare#Size"/>
                                                    <rdf:rest>
                                                      <rdf:Description>
                                                        <rdf:first rdf:resource="http://purl.org/net/def/metashare#Size"/>
                                                        <rdf:rest>
                                                          <rdf:Description>
                                                            <rdf:first rdf:resource="http://purl.org/net/def/metashare#Size"/>
                                                            <rdf:rest rdf:resource="http://www.w3.org/1999/02/22-rdf-syntax-ns#nil"/>
                                                          </rdf:Description>
                                                        </rdf:rest>
                                                      </rdf:Description>
                                                    </rdf:rest>
                                                  </rdf:Description>
                                                </rdf:rest>
                                              </rdf:Description>
                                            </rdf:rest>
                                          </rdf:Description>
                                        </rdf:rest>
                                      </rdf:Description>
                                    </rdf:rest>
                                  </rdf:Description>
                                </rdf:rest>
                              </rdf:Description>
                            </rdf:rest>
                          </rdf:Description>
                        </rdf:rest>
                      </rdf:Description>
                    </rdf:rest>
                  </rdf:Description>
                </rdf:rest>
              </rdf:Description>
            </rdf:rest>
          </rdf:Description>
        </owl:unionOf>
      </owl:Class>
    </rdfs:range>
  </owl:ObjectProperty>
  <owl:ObjectProperty rdf:about="http://purl.org/net/def/metashare#sizePerAnnotation">
    <rdfs:comment xml:lang="en">Provides information on size for the annotated parts of the resource</rdfs:comment>
    <rdfs:domain rdf:resource="http://purl.org/net/def/metashare#AnnotationInfo"/>
    <rdfs:range rdf:resource="http://purl.org/net/def/metashare#Size"/>
  </owl:ObjectProperty>
  <owl:ObjectProperty rdf:about="http://purl.org/net/def/metashare#sizePerAudioClassification">
    <rdfs:comment xml:lang="en">The size of the audio subparts of the resource in terms of classification criteria</rdfs:comment>
    <rdfs:domain rdf:resource="http://purl.org/net/def/metashare#AudioClassificationInfo"/>
    <rdfs:range rdf:resource="http://purl.org/net/def/metashare#Size"/>
  </owl:ObjectProperty>
  <owl:ObjectProperty rdf:about="http://purl.org/net/def/metashare#sizePerAudioFormat">
    <rdfs:comment xml:lang="en">Used to give info on size of parts of a resource that differ as to the format</rdfs:comment>
    <rdfs:domain rdf:resource="http://purl.org/net/def/metashare#AudioFormatInfo"/>
    <rdfs:range rdf:resource="http://purl.org/net/def/metashare#Size"/>
  </owl:ObjectProperty>
  <owl:ObjectProperty rdf:about="http://purl.org/net/def/metashare#sizePerCharacterEncoding">
    <rdfs:comment xml:lang="en">Provides information on the size of the resource parts with different character encoding</rdfs:comment>
    <rdfs:domain rdf:resource="http://purl.org/net/def/metashare#CharacterEncodingInfo"/>
    <rdfs:range rdf:resource="http://purl.org/net/def/metashare#Size"/>
  </owl:ObjectProperty>
  <owl:ObjectProperty rdf:about="http://purl.org/net/def/metashare#sizePerDomain">
    <rdfs:comment xml:lang="en">Specifies the size of resource parts per domain</rdfs:comment>
    <rdfs:domain rdf:resource="http://purl.org/net/def/metashare#DomainInfo"/>
    <rdfs:range rdf:resource="http://purl.org/net/def/metashare#Size"/>
  </owl:ObjectProperty>
  <owl:ObjectProperty rdf:about="http://purl.org/net/def/metashare#sizePerGeographicCoverage">
    <rdfs:comment xml:lang="en">Provides information on size per geographically distinct section of the resource</rdfs:comment>
    <rdfs:domain rdf:resource="http://purl.org/net/def/metashare#GeographicCoverageInfo"/>
    <rdfs:range rdf:resource="http://purl.org/net/def/metashare#Size"/>
  </owl:ObjectProperty>
  <owl:ObjectProperty rdf:about="http://purl.org/net/def/metashare#sizePerImageClassification">
    <rdfs:comment xml:lang="en">Provides information on size of parts with different image classification</rdfs:comment>
    <rdfs:domain rdf:resource="http://purl.org/net/def/metashare#ImageClassificationInfo"/>
    <rdfs:range rdf:resource="http://purl.org/net/def/metashare#Size"/>
  </owl:ObjectProperty>
  <owl:ObjectProperty rdf:about="http://purl.org/net/def/metashare#sizePerImageFormat">
    <rdfs:comment xml:lang="en">Used to give info on size of parts of a resource that differ as to the format</rdfs:comment>
    <rdfs:domain rdf:resource="http://purl.org/net/def/metashare#ImageFormatInfo"/>
    <rdfs:range rdf:resource="http://purl.org/net/def/metashare#Size"/>
  </owl:ObjectProperty>
  <owl:ObjectProperty rdf:about="http://purl.org/net/def/metashare#sizePerLanguage">
    <rdfs:comment xml:lang="en">Provides information on the size per language component</rdfs:comment>
    <rdfs:domain rdf:resource="http://purl.org/net/def/metashare#LanguageInfo"/>
    <rdfs:range rdf:resource="http://purl.org/net/def/metashare#Size"/>
  </owl:ObjectProperty>
  <owl:ObjectProperty rdf:about="http://purl.org/net/def/metashare#sizePerLanguageVariety">
    <rdfs:comment xml:lang="en">Provides information on the size per language variety component</rdfs:comment>
    <rdfs:domain rdf:resource="http://purl.org/net/def/metashare#LanguageVarietyInfo"/>
    <rdfs:range rdf:resource="http://purl.org/net/def/metashare#Size"/>
  </owl:ObjectProperty>
  <owl:ObjectProperty rdf:about="http://purl.org/net/def/metashare#sizePerModality">
    <rdfs:comment xml:lang="en">Provides information on the size per modality component</rdfs:comment>
    <rdfs:domain rdf:resource="http://purl.org/net/def/metashare#ModalityInfo"/>
    <rdfs:range rdf:resource="http://purl.org/net/def/metashare#Size"/>
  </owl:ObjectProperty>
  <owl:ObjectProperty rdf:about="http://purl.org/net/def/metashare#sizePerTextClassification">
    <rdfs:comment xml:lang="en">Provides information on size of resource parts with different text classification</rdfs:comment>
    <rdfs:domain rdf:resource="http://purl.org/net/def/metashare#TextClassificationInfo"/>
    <rdfs:range rdf:resource="http://purl.org/net/def/metashare#Size"/>
  </owl:ObjectProperty>
  <owl:ObjectProperty rdf:about="http://purl.org/net/def/metashare#sizePerTextFormat">
    <rdfs:comment xml:lang="en">Provides information on the size of the resource parts with different format</rdfs:comment>
    <rdfs:domain rdf:resource="http://purl.org/net/def/metashare#TextFormatInfo"/>
    <rdfs:range rdf:resource="http://purl.org/net/def/metashare#Size"/>
  </owl:ObjectProperty>
  <owl:ObjectProperty rdf:about="http://purl.org/net/def/metashare#sizePerTextNumericalFormat">
    <rdfs:comment xml:lang="en">Gives information on the size of textNumerical resource parts with different format</rdfs:comment>
    <rdfs:domain rdf:resource="http://purl.org/net/def/metashare#TextNumericalFormatInfo"/>
    <rdfs:range rdf:resource="http://purl.org/net/def/metashare#Size"/>
  </owl:ObjectProperty>
  <owl:ObjectProperty rdf:about="http://purl.org/net/def/metashare#sizePerTimeCoverage">
    <rdfs:comment xml:lang="en">Provides information on size per time period represented in the resource</rdfs:comment>
    <rdfs:domain rdf:resource="http://purl.org/net/def/metashare#TimeCoverageInfo"/>
    <rdfs:range rdf:resource="http://purl.org/net/def/metashare#Size"/>
  </owl:ObjectProperty>
  <owl:ObjectProperty rdf:about="http://purl.org/net/def/metashare#sizePerValidation">
    <rdfs:comment xml:lang="en">Specifies the size of the validated part of a resource</rdfs:comment>
    <rdfs:domain rdf:resource="http://purl.org/net/def/metashare#ValidationInfo"/>
    <rdfs:range rdf:resource="http://purl.org/net/def/metashare#Size"/>
  </owl:ObjectProperty>
  <owl:ObjectProperty rdf:about="http://purl.org/net/def/metashare#sizePerVideoClassification">
    <rdfs:comment xml:lang="en">Used to give info on size of parts with different video classification</rdfs:comment>
    <rdfs:domain rdf:resource="http://purl.org/net/def/metashare#VideoClassificationInfo"/>
    <rdfs:range rdf:resource="http://purl.org/net/def/metashare#Size"/>
  </owl:ObjectProperty>
  <owl:ObjectProperty rdf:about="http://purl.org/net/def/metashare#sizePerVideoFormat">
    <rdfs:comment xml:lang="en">Used to give info on size of parts of a resource that differ as to the format</rdfs:comment>
    <rdfs:domain rdf:resource="http://purl.org/net/def/metashare#VideoFormatInfo"/>
    <rdfs:range rdf:resource="http://purl.org/net/def/metashare#Size"/>
  </owl:ObjectProperty>
  <owl:ObjectProperty rdf:about="http://purl.org/net/def/metashare#sizeUnit">
    <rdfs:comment xml:lang="en">Specifies the unit that is used when providing information on the size of the resource or of resource parts</rdfs:comment>
    <rdfs:domain rdf:resource="http://purl.org/net/def/metashare#Size"/>
    <rdfs:range rdf:resource="http://purl.org/net/def/metashare#SizeUnit"/>
  </owl:ObjectProperty>
  <owl:DatatypeProperty rdf:about="http://purl.org/net/def/metashare#sizeWidth">
    <rdfs:comment xml:lang="en">The frame width in pixels</rdfs:comment>
    <rdfs:domain rdf:resource="http://purl.org/net/def/metashare#ResolutionInfo"/>
    <rdfs:range rdf:resource="http://www.w3.org/2001/XMLSchema#int"/>
  </owl:DatatypeProperty>
  <ns:SpeechInfluences rdf:about="http://purl.org/net/def/metashare#sleepDeprivation"/>
  <owl:DatatypeProperty rdf:about="http://purl.org/net/def/metashare#smokingHabits">
    <rdfs:comment xml:lang="en">Provides information on whether the participants smokes and on his/her smoking habits in general</rdfs:comment>
    <rdfs:domain rdf:resource="http://purl.org/net/def/metashare#ParticipantInfo"/>
    <rdfs:range rdf:resource="http://www.w3.org/2001/XMLSchema#string"/>
  </owl:DatatypeProperty>
  <owl:DatatypeProperty rdf:about="http://purl.org/net/def/metashare#smoothing">
    <rdfs:comment xml:lang="en">The technique used for giving unseen items some probability</rdfs:comment>
    <rdfs:domain rdf:resource="http://purl.org/net/def/metashare#NgramInfo"/>
    <rdfs:range rdf:resource="http://www.w3.org/2001/XMLSchema#string"/>
  </owl:DatatypeProperty>
  <ns:Audience rdf:about="http://purl.org/net/def/metashare#some"/>
  <ns:RecordingDeviceType rdf:about="http://purl.org/net/def/metashare#soundBlasterCard"/>
  <ns:ExtratextualInformation rdf:about="http://purl.org/net/def/metashare#soundRecordings"/>
  <ns:NonSpeechItems rdf:about="http://purl.org/net/def/metashare#sounds"/>
  <owl:ObjectProperty rdf:about="http://purl.org/net/def/metashare#sourceChannel">
    <rdfs:comment xml:lang="en">Information on the source channel</rdfs:comment>
    <rdfs:domain>
      <owl:Class>
        <owl:unionOf>
          <rdf:Description>
            <rdf:first rdf:resource="http://purl.org/net/def/metashare#CorpusAudioInfo"/>
            <rdf:rest>
              <rdf:Description>
                <rdf:first rdf:resource="http://purl.org/net/def/metashare#CorpusTextNumericalInfo"/>
                <rdf:rest>
                  <rdf:Description>
                    <rdf:first rdf:resource="http://purl.org/net/def/metashare#CorpusVideoInfo"/>
                    <rdf:rest rdf:resource="http://www.w3.org/1999/02/22-rdf-syntax-ns#nil"/>
                  </rdf:Description>
                </rdf:rest>
              </rdf:Description>
            </rdf:rest>
          </rdf:Description>
        </owl:unionOf>
      </owl:Class>
    </rdfs:domain>
    <rdfs:range>
      <owl:Class>
        <owl:unionOf>
          <rdf:Description>
            <rdf:first rdf:resource="http://purl.org/net/def/metashare#SourceChannel"/>
            <rdf:rest>
              <rdf:Description>
                <rdf:first rdf:resource="http://purl.org/net/def/metashare#SourceChannel"/>
                <rdf:rest>
                  <rdf:Description>
                    <rdf:first rdf:resource="http://purl.org/net/def/metashare#SourceChannel"/>
                    <rdf:rest rdf:resource="http://www.w3.org/1999/02/22-rdf-syntax-ns#nil"/>
                  </rdf:Description>
                </rdf:rest>
              </rdf:Description>
            </rdf:rest>
          </rdf:Description>
        </owl:unionOf>
      </owl:Class>
    </rdfs:range>
  </owl:ObjectProperty>
  <owl:DatatypeProperty rdf:about="http://purl.org/net/def/metashare#sourceChannelDetails">
    <rdfs:comment xml:lang="en">The details of the channel equipment used (brand, type etc.)</rdfs:comment>
    <rdfs:domain>
      <owl:Class>
        <owl:unionOf>
          <rdf:Description>
            <rdf:first rdf:resource="http://purl.org/net/def/metashare#CorpusAudioInfo"/>
            <rdf:rest>
              <rdf:Description>
                <rdf:first rdf:resource="http://purl.org/net/def/metashare#CorpusTextNumericalInfo"/>
                <rdf:rest>
                  <rdf:Description>
                    <rdf:first rdf:resource="http://purl.org/net/def/metashare#CorpusVideoInfo"/>
                    <rdf:rest rdf:resource="http://www.w3.org/1999/02/22-rdf-syntax-ns#nil"/>
                  </rdf:Description>
                </rdf:rest>
              </rdf:Description>
            </rdf:rest>
          </rdf:Description>
        </owl:unionOf>
      </owl:Class>
    </rdfs:domain>
    <rdfs:range rdf:resource="http://www.w3.org/2001/XMLSchema#string"/>
  </owl:DatatypeProperty>
  <owl:DatatypeProperty rdf:about="http://purl.org/net/def/metashare#sourceChannelName">
    <rdfs:comment xml:lang="en">The name of the specific source recorded</rdfs:comment>
    <rdfs:domain>
      <owl:Class>
        <owl:unionOf>
          <rdf:Description>
            <rdf:first rdf:resource="http://purl.org/net/def/metashare#CorpusVideoInfo"/>
            <rdf:rest>
              <rdf:Description>
                <rdf:first rdf:resource="http://purl.org/net/def/metashare#CorpusAudioInfo"/>
                <rdf:rest>
                  <rdf:Description>
                    <rdf:first rdf:resource="http://purl.org/net/def/metashare#CorpusTextNumericalInfo"/>
                    <rdf:rest rdf:resource="http://www.w3.org/1999/02/22-rdf-syntax-ns#nil"/>
                  </rdf:Description>
                </rdf:rest>
              </rdf:Description>
            </rdf:rest>
          </rdf:Description>
        </owl:unionOf>
      </owl:Class>
    </rdfs:domain>
    <rdfs:range rdf:resource="http://www.w3.org/2001/XMLSchema#string"/>
  </owl:DatatypeProperty>
  <owl:ObjectProperty rdf:about="http://purl.org/net/def/metashare#sourceChannelType">
    <rdfs:comment xml:lang="en">Type of the source channel</rdfs:comment>
    <rdfs:domain>
      <owl:Class>
        <owl:unionOf>
          <rdf:Description>
            <rdf:first rdf:resource="http://purl.org/net/def/metashare#CorpusTextNumericalInfo"/>
            <rdf:rest>
              <rdf:Description>
                <rdf:first rdf:resource="http://purl.org/net/def/metashare#CorpusVideoInfo"/>
                <rdf:rest>
                  <rdf:Description>
                    <rdf:first rdf:resource="http://purl.org/net/def/metashare#CorpusAudioInfo"/>
                    <rdf:rest rdf:resource="http://www.w3.org/1999/02/22-rdf-syntax-ns#nil"/>
                  </rdf:Description>
                </rdf:rest>
              </rdf:Description>
            </rdf:rest>
          </rdf:Description>
        </owl:unionOf>
      </owl:Class>
    </rdfs:domain>
    <rdfs:range>
      <owl:Class>
        <owl:unionOf>
          <rdf:Description>
            <rdf:first rdf:resource="http://purl.org/net/def/metashare#SourceChannelType"/>
            <rdf:rest>
              <rdf:Description>
                <rdf:first rdf:resource="http://purl.org/net/def/metashare#SourceChannelType"/>
                <rdf:rest>
                  <rdf:Description>
                    <rdf:first rdf:resource="http://purl.org/net/def/metashare#SourceChannelType"/>
                    <rdf:rest rdf:resource="http://www.w3.org/1999/02/22-rdf-syntax-ns#nil"/>
                  </rdf:Description>
                </rdf:rest>
              </rdf:Description>
            </rdf:rest>
          </rdf:Description>
        </owl:unionOf>
      </owl:Class>
    </rdfs:range>
  </owl:ObjectProperty>
  <ns:ConditionsOfUse rdf:about="http://purl.org/net/def/metashare#spatialConstraint">
    <rdf:type rdf:resource="http://www.w3.org/2002/07/owl#NamedIndividual"/>
    <rdfs:comment xml:lang="en">Spatial constraint refers to a kind of 'ConditionsOfUse' imposed by the licence; used for resources with spatial restrictions, e.g. the content is available or can be used only at a single location, center, or site.</rdfs:comment>
    <rdfs:label xml:lang="en">Spatial Constraint</rdfs:label>
  </ns:ConditionsOfUse>
  <ns:UseNLPSpecific rdf:about="http://purl.org/net/def/metashare#speakerIdentification"/>
  <ns:AnnotatedElements rdf:about="http://purl.org/net/def/metashare#speakerNoise"/>
  <ns:UseNLPSpecific rdf:about="http://purl.org/net/def/metashare#speakerVerification"/>
  <owl:DatatypeProperty rdf:about="http://purl.org/net/def/metashare#speakingImpairment">
    <rdfs:comment xml:lang="en">Provides information on any speaking impairment the participant may have</rdfs:comment>
    <rdfs:domain rdf:resource="http://purl.org/net/def/metashare#ParticipantInfo"/>
    <rdfs:range rdf:resource="http://www.w3.org/2001/XMLSchema#string"/>
  </owl:DatatypeProperty>
  <owl:ObjectProperty rdf:about="http://purl.org/net/def/metashare#speakingImpairmentOfPersons">
    <rdfs:comment xml:lang="en">Whether the group of participants contains persons withwith speakingimpairments</rdfs:comment>
    <rdfs:domain>
      <owl:Class>
        <owl:unionOf>
          <rdf:Description>
            <rdf:first rdf:resource="http://purl.org/net/def/metashare#CorpusVideoInfo"/>
            <rdf:rest>
              <rdf:Description>
                <rdf:first rdf:resource="http://purl.org/net/def/metashare#CorpusAudioInfo"/>
                <rdf:rest>
                  <rdf:Description>
                    <rdf:first rdf:resource="http://purl.org/net/def/metashare#CorpusTextNumericalInfo"/>
                    <rdf:rest>
                      <rdf:Description>
                        <rdf:first rdf:resource="http://purl.org/net/def/metashare#CorpusImageInfo"/>
                        <rdf:rest rdf:resource="http://www.w3.org/1999/02/22-rdf-syntax-ns#nil"/>
                      </rdf:Description>
                    </rdf:rest>
                  </rdf:Description>
                </rdf:rest>
              </rdf:Description>
            </rdf:rest>
          </rdf:Description>
        </owl:unionOf>
      </owl:Class>
    </rdfs:domain>
    <rdfs:range>
      <owl:Class>
        <owl:unionOf>
          <rdf:Description>
            <rdf:first rdf:resource="http://purl.org/net/def/metashare#SpeakingImpairmentOfPersons"/>
            <rdf:rest>
              <rdf:Description>
                <rdf:first rdf:resource="http://purl.org/net/def/metashare#SpeakingImpairmentOfPersons"/>
                <rdf:rest>
                  <rdf:Description>
                    <rdf:first rdf:resource="http://purl.org/net/def/metashare#SpeakingImpairmentOfPersons"/>
                    <rdf:rest>
                      <rdf:Description>
                        <rdf:first rdf:resource="http://purl.org/net/def/metashare#SpeakingImpairmentOfPersons"/>
                        <rdf:rest rdf:resource="http://www.w3.org/1999/02/22-rdf-syntax-ns#nil"/>
                      </rdf:Description>
                    </rdf:rest>
                  </rdf:Description>
                </rdf:rest>
              </rdf:Description>
            </rdf:rest>
          </rdf:Description>
        </owl:unionOf>
      </owl:Class>
    </rdfs:range>
  </owl:ObjectProperty>
  <ns:RequiredHardware rdf:about="http://purl.org/net/def/metashare#specialHardwareEquipment"/>
  <ns:UseNLPSpecific rdf:about="http://purl.org/net/def/metashare#speechAnalysis"/>
  <ns:SpeechAnnotation rdf:about="http://purl.org/net/def/metashare#speechAnnotation">
    <rdf:type rdf:resource="http://purl.org/net/def/metashare#AnnotationType"/>
  </ns:SpeechAnnotation>
  <ns:SpeechAnnotation rdf:about="http://purl.org/net/def/metashare#speechAnnotation-orthographicTranscription">
    <rdf:type rdf:resource="http://purl.org/net/def/metashare#AnnotationType"/>
  </ns:SpeechAnnotation>
  <ns:SpeechAnnotation rdf:about="http://purl.org/net/def/metashare#speechAnnotation-paralanguageAnnotation">
    <rdf:type rdf:resource="http://purl.org/net/def/metashare#AnnotationType"/>
  </ns:SpeechAnnotation>
  <ns:SpeechAnnotation rdf:about="http://purl.org/net/def/metashare#speechAnnotation-phoneticTranscription">
    <rdf:type rdf:resource="http://purl.org/net/def/metashare#AnnotationType"/>
  </ns:SpeechAnnotation>
  <ns:SpeechAnnotation rdf:about="http://purl.org/net/def/metashare#speechAnnotation-prosodicAnnotation">
    <rdf:type rdf:resource="http://purl.org/net/def/metashare#AnnotationType"/>
  </ns:SpeechAnnotation>
  <ns:SpeechAnnotation rdf:about="http://purl.org/net/def/metashare#speechAnnotation-soundEvents">
    <rdf:type rdf:resource="http://purl.org/net/def/metashare#AnnotationType"/>
  </ns:SpeechAnnotation>
  <ns:AnnotationType rdf:about="http://purl.org/net/def/metashare#speechAnnotation-soundToTextAlignment"/>
  <ns:SpeechAnnotation rdf:about="http://purl.org/net/def/metashare#speechAnnotation-speakerIdentification">
    <rdf:type rdf:resource="http://purl.org/net/def/metashare#AnnotationType"/>
  </ns:SpeechAnnotation>
  <ns:SpeechAnnotation rdf:about="http://purl.org/net/def/metashare#speechAnnotation-speakerTurns">
    <rdf:type rdf:resource="http://purl.org/net/def/metashare#AnnotationType"/>
  </ns:SpeechAnnotation>
  <ns:UseNLPSpecific rdf:about="http://purl.org/net/def/metashare#speechAssistedVideoControl"/>
  <owl:DatatypeProperty rdf:about="http://purl.org/net/def/metashare#speechGenre">
    <rdfs:comment xml:lang="en">The conventionalized discourse of the content of the resource, based on extra-linguistic and internal linguistic criteria; the values here are intended only for speech</rdfs:comment>
    <rdfs:domain rdf:resource="http://purl.org/net/def/metashare#AudioClassificationInfo"/>
    <rdfs:range rdf:resource="http://www.w3.org/2001/XMLSchema#string"/>
    <rdfs:subPropertyOf rdf:resource="http://purl.org/net/def/metashare#genre"/>
  </owl:DatatypeProperty>
  <owl:ObjectProperty rdf:about="http://purl.org/net/def/metashare#speechInfluences">
    <rdfs:comment xml:lang="en">Specifies the factors influencing speech</rdfs:comment>
    <rdfs:domain>
      <owl:Class>
        <owl:unionOf>
          <rdf:Description>
            <rdf:first rdf:resource="http://purl.org/net/def/metashare#CorpusAudioInfo"/>
            <rdf:rest>
              <rdf:Description>
                <rdf:first rdf:resource="http://purl.org/net/def/metashare#CorpusImageInfo"/>
                <rdf:rest>
                  <rdf:Description>
                    <rdf:first rdf:resource="http://purl.org/net/def/metashare#CorpusTextNumericalInfo"/>
                    <rdf:rest>
                      <rdf:Description>
                        <rdf:first rdf:resource="http://purl.org/net/def/metashare#CorpusVideoInfo"/>
                        <rdf:rest rdf:resource="http://www.w3.org/1999/02/22-rdf-syntax-ns#nil"/>
                      </rdf:Description>
                    </rdf:rest>
                  </rdf:Description>
                </rdf:rest>
              </rdf:Description>
            </rdf:rest>
          </rdf:Description>
        </owl:unionOf>
      </owl:Class>
    </rdfs:domain>
    <rdfs:range>
      <owl:Class>
        <owl:unionOf>
          <rdf:Description>
            <rdf:first rdf:resource="http://purl.org/net/def/metashare#SpeechInfluences"/>
            <rdf:rest>
              <rdf:Description>
                <rdf:first rdf:resource="http://purl.org/net/def/metashare#SpeechInfluences"/>
                <rdf:rest>
                  <rdf:Description>
                    <rdf:first rdf:resource="http://purl.org/net/def/metashare#SpeechInfluences"/>
                    <rdf:rest>
                      <rdf:Description>
                        <rdf:first rdf:resource="http://purl.org/net/def/metashare#SpeechInfluences"/>
                        <rdf:rest rdf:resource="http://www.w3.org/1999/02/22-rdf-syntax-ns#nil"/>
                      </rdf:Description>
                    </rdf:rest>
                  </rdf:Description>
                </rdf:rest>
              </rdf:Description>
            </rdf:rest>
          </rdf:Description>
        </owl:unionOf>
      </owl:Class>
    </rdfs:range>
  </owl:ObjectProperty>
  <owl:ObjectProperty rdf:about="http://purl.org/net/def/metashare#speechItems">
    <rdfs:comment xml:lang="en">Specifies the distinct elements that are pronounced and annotated as such</rdfs:comment>
    <rdfs:domain>
      <owl:Class>
        <owl:unionOf>
          <rdf:Description>
            <rdf:first rdf:resource="http://purl.org/net/def/metashare#LexicalConceptualResourceAudioInfo"/>
            <rdf:rest>
              <rdf:Description>
                <rdf:first rdf:resource="http://purl.org/net/def/metashare#CorpusAudioInfo"/>
                <rdf:rest rdf:resource="http://www.w3.org/1999/02/22-rdf-syntax-ns#nil"/>
              </rdf:Description>
            </rdf:rest>
          </rdf:Description>
        </owl:unionOf>
      </owl:Class>
    </rdfs:domain>
    <rdfs:range>
      <owl:Class>
        <owl:unionOf>
          <rdf:Description>
            <rdf:first rdf:resource="http://purl.org/net/def/metashare#SpeechItems"/>
            <rdf:rest>
              <rdf:Description>
                <rdf:first rdf:resource="http://purl.org/net/def/metashare#SpeechItems"/>
                <rdf:rest rdf:resource="http://www.w3.org/1999/02/22-rdf-syntax-ns#nil"/>
              </rdf:Description>
            </rdf:rest>
          </rdf:Description>
        </owl:unionOf>
      </owl:Class>
    </rdfs:range>
  </owl:ObjectProperty>
  <ns:UseNLPSpecific rdf:about="http://purl.org/net/def/metashare#speechLipsCorrelationAnalysis"/>
  <ns:UseNLPSpecific rdf:about="http://purl.org/net/def/metashare#speechRecognition"/>
  <ns:UseNLPSpecific rdf:about="http://purl.org/net/def/metashare#speechSynthesis"/>
  <ns:UseNLPSpecific rdf:about="http://purl.org/net/def/metashare#speechToSpeechTranslation"/>
  <ns:UseNLPSpecific rdf:about="http://purl.org/net/def/metashare#speechUnderstanding"/>
  <ns:UseNLPSpecific rdf:about="http://purl.org/net/def/metashare#speechVerification"/>
  <ns:UseNLPSpecific rdf:about="http://purl.org/net/def/metashare#spellChecking"/>
  <ns:UseNLPSpecific rdf:about="http://purl.org/net/def/metashare#spokenDialogueSystems"/>
  <ns:ModalityType rdf:about="http://purl.org/net/def/metashare#spokenLanguage"/>
  <ns:Naturality rdf:about="http://purl.org/net/def/metashare#spontaneous"/>
  <owl:ObjectProperty rdf:about="http://purl.org/net/def/metashare#staticElementInfo">
    <rdfs:comment xml:lang="en">Groups information on the static element visible on the images</rdfs:comment>
    <rdfs:domain>
      <owl:Class>
        <owl:unionOf>
          <rdf:Description>
            <rdf:first rdf:resource="http://purl.org/net/def/metashare#LanguageDescriptionImageInfo"/>
            <rdf:rest>
              <rdf:Description>
                <rdf:first rdf:resource="http://purl.org/net/def/metashare#LexicalConceptualResourceImageInfo"/>
                <rdf:rest>
                  <rdf:Description>
                    <rdf:first rdf:resource="http://purl.org/net/def/metashare#CorpusImageInfo"/>
                    <rdf:rest rdf:resource="http://www.w3.org/1999/02/22-rdf-syntax-ns#nil"/>
                  </rdf:Description>
                </rdf:rest>
              </rdf:Description>
            </rdf:rest>
          </rdf:Description>
        </owl:unionOf>
      </owl:Class>
    </rdfs:domain>
    <rdfs:range>
      <owl:Class>
        <owl:unionOf>
          <rdf:Description>
            <rdf:first rdf:resource="http://purl.org/net/def/metashare#StaticElementInfo"/>
            <rdf:rest>
              <rdf:Description>
                <rdf:first rdf:resource="http://purl.org/net/def/metashare#StaticElementInfo"/>
                <rdf:rest>
                  <rdf:Description>
                    <rdf:first rdf:resource="http://purl.org/net/def/metashare#StaticElementInfo"/>
                    <rdf:rest rdf:resource="http://www.w3.org/1999/02/22-rdf-syntax-ns#nil"/>
                  </rdf:Description>
                </rdf:rest>
              </rdf:Description>
            </rdf:rest>
          </rdf:Description>
        </owl:unionOf>
      </owl:Class>
    </rdfs:range>
  </owl:ObjectProperty>
  <ns:LinguisticInformation rdf:about="http://purl.org/net/def/metashare#statisticalProperties"/>
  <ns:AnnotationType rdf:about="http://purl.org/net/def/metashare#stemming"/>
  <ns:AnnotationType rdf:about="http://purl.org/net/def/metashare#structuralAnnotation"/>
  <ns:RecordingEnvironment rdf:about="http://purl.org/net/def/metashare#studio"/>
  <ns:CapturingDeviceType rdf:about="http://purl.org/net/def/metashare#studioEquipment"/>
  <ns:TextIncludedInImage rdf:about="http://purl.org/net/def/metashare#subtitles">
    <rdf:type rdf:resource="http://purl.org/net/def/metashare#TextIncludedInVideo"/>
  </ns:TextIncludedInImage>
  <ns:ToolServiceType rdf:about="http://purl.org/net/def/metashare#suiteOfTools"/>
  <ns:UseNLPSpecific rdf:about="http://purl.org/net/def/metashare#summarisation"/>
  <ns:BaseItem rdf:about="http://purl.org/net/def/metashare#syllable">
    <rdf:type rdf:resource="http://purl.org/net/def/metashare#SegmentationLevel"/>
  </ns:BaseItem>
  <ns:SizeUnit rdf:about="http://purl.org/net/def/metashare#syllables"/>
  <owl:DatatypeProperty rdf:about="http://purl.org/net/def/metashare#synchronizedWithAudio">
    <rdfs:comment xml:lang="en">Whether text, video or textNumerical media type is synchronized with audio within the same resource</rdfs:comment>
    <rdfs:domain rdf:resource="http://purl.org/net/def/metashare#LinkToOtherMediaInfo"/>
    <rdfs:range rdf:resource="http://www.w3.org/2001/XMLSchema#boolean"/>
  </owl:DatatypeProperty>
  <owl:DatatypeProperty rdf:about="http://purl.org/net/def/metashare#synchronizedWithImage">
    <rdfs:domain rdf:resource="http://purl.org/net/def/metashare#LinkToOtherMediaInfo"/>
    <rdfs:range rdf:resource="http://www.w3.org/2001/XMLSchema#boolean"/>
  </owl:DatatypeProperty>
  <owl:DatatypeProperty rdf:about="http://purl.org/net/def/metashare#synchronizedWithText">
    <rdfs:comment xml:lang="en">Whether video, text and textNumerical media type is synchronized with text within the same resource</rdfs:comment>
    <rdfs:domain rdf:resource="http://purl.org/net/def/metashare#LinkToOtherMediaInfo"/>
    <rdfs:range rdf:resource="http://www.w3.org/2001/XMLSchema#boolean"/>
  </owl:DatatypeProperty>
  <owl:DatatypeProperty rdf:about="http://purl.org/net/def/metashare#synchronizedWithTextNumerical">
    <rdfs:comment xml:lang="en">Whether video or audio media type is synchronized with the textNumerical (representation of sensorimotor measurements) within the same resource </rdfs:comment>
    <rdfs:domain rdf:resource="http://purl.org/net/def/metashare#LinkToOtherMediaInfo"/>
    <rdfs:range rdf:resource="http://www.w3.org/2001/XMLSchema#boolean"/>
  </owl:DatatypeProperty>
  <owl:DatatypeProperty rdf:about="http://purl.org/net/def/metashare#synchronizedWithVideo">
    <rdfs:comment xml:lang="en">Whether text or textNumerical media type is synchronized with video within the same resource</rdfs:comment>
    <rdfs:domain rdf:resource="http://purl.org/net/def/metashare#LinkToOtherMediaInfo"/>
    <rdfs:range rdf:resource="http://www.w3.org/2001/XMLSchema#boolean"/>
  </owl:DatatypeProperty>
  <ns:SizeUnit rdf:about="http://purl.org/net/def/metashare#synsets"/>
  <ns:SyntacticAnnotation rdf:about="http://purl.org/net/def/metashare#syntacticAnnotation-shallowParsing">
    <rdf:type rdf:resource="http://purl.org/net/def/metashare#AnnotationType"/>
  </ns:SyntacticAnnotation>
  <ns:SyntacticAnnotation rdf:about="http://purl.org/net/def/metashare#syntacticAnnotation-subcategorizationFrames">
    <rdf:type rdf:resource="http://purl.org/net/def/metashare#AnnotationType"/>
  </ns:SyntacticAnnotation>
  <ns:SyntacticAnnotation rdf:about="http://purl.org/net/def/metashare#syntacticAnnotation-treebanks">
    <rdf:type rdf:resource="http://purl.org/net/def/metashare#AnnotationType"/>
  </ns:SyntacticAnnotation>
  <ns:SizeUnit rdf:about="http://purl.org/net/def/metashare#syntacticUnits"/>
  <ns:LinguisticInformation rdf:about="http://purl.org/net/def/metashare#syntacticoSemanticLinks"/>
  <ns:SyntacticAnnotation rdf:about="http://purl.org/net/def/metashare#syntacticosemanticAnnotation-links">
    <rdf:type rdf:resource="http://purl.org/net/def/metashare#AnnotationType"/>
  </ns:SyntacticAnnotation>
  <ns:EncodingLevel rdf:about="http://purl.org/net/def/metashare#syntax">
    <rdf:type rdf:resource="http://purl.org/net/def/metashare#ExtraTextualInformationUnit"/>
  </ns:EncodingLevel>
  <ns:LinguisticInformation rdf:about="http://purl.org/net/def/metashare#syntax-SubcatFrame"/>
  <owl:DatatypeProperty rdf:about="http://purl.org/net/def/metashare#tagset">
    <rdfs:comment xml:lang="en">A name or a url reference to the tagset used in the annotation of the resource or used by the tool/service</rdfs:comment>
    <rdfs:domain>
      <owl:Class>
        <owl:unionOf>
          <rdf:Description>
            <rdf:first rdf:resource="http://purl.org/net/def/metashare#InputInfo"/>
            <rdf:rest>
              <rdf:Description>
                <rdf:first rdf:resource="http://purl.org/net/def/metashare#AnnotationInfo"/>
                <rdf:rest>
                  <rdf:Description>
                    <rdf:first rdf:resource="http://purl.org/net/def/metashare#OutputInfo"/>
                    <rdf:rest rdf:resource="http://www.w3.org/1999/02/22-rdf-syntax-ns#nil"/>
                  </rdf:Description>
                </rdf:rest>
              </rdf:Description>
            </rdf:rest>
          </rdf:Description>
        </owl:unionOf>
      </owl:Class>
    </rdfs:domain>
    <rdfs:range rdf:resource="http://www.w3.org/2001/XMLSchema#string"/>
  </owl:DatatypeProperty>
  <owl:DatatypeProperty rdf:about="http://purl.org/net/def/metashare#tagsetLanguageId">
    <rdfs:comment xml:lang="en">The identifier of the tagset language; an autocompletion mechanism with values from the ISO 639 is provided in the editor, but the values can be subsequently edited for further specification (according to the IETF BCP47 guidelines)</rdfs:comment>
    <rdfs:domain rdf:resource="http://purl.org/net/def/metashare#AnnotationInfo"/>
    <rdfs:range rdf:resource="http://www.w3.org/2001/XMLSchema#string"/>
  </owl:DatatypeProperty>
  <owl:DatatypeProperty rdf:about="http://purl.org/net/def/metashare#tagsetLanguageName">
    <rdfs:comment xml:lang="en">The name of the tagset language; an autocompletion mechanism with values from the ISO 639 is provided in the editor, but the values can be subsequently edited for further specification (according to the IETF BCP47 guidelines)</rdfs:comment>
    <rdfs:domain rdf:resource="http://purl.org/net/def/metashare#AnnotationInfo"/>
    <rdfs:range rdf:resource="http://www.w3.org/2001/XMLSchema#string"/>
  </owl:DatatypeProperty>
  <ns:UseNLPSpecific rdf:about="http://purl.org/net/def/metashare#talkingHeadSynthesis"/>
  <ns:RecordingDeviceType rdf:about="http://purl.org/net/def/metashare#tapeVHS"/>
  <owl:ObjectProperty rdf:about="http://purl.org/net/def/metashare#task">
    <rdfs:comment xml:lang="en">An indication of the task performed by the grammar</rdfs:comment>
    <rdfs:domain rdf:resource="http://purl.org/net/def/metashare#LanguageDescriptionInfo"/>
    <rdfs:range rdf:resource="http://purl.org/net/def/metashare#Task"/>
  </owl:ObjectProperty>
  <ns:EvaluationLevel rdf:about="http://purl.org/net/def/metashare#technological"/>
  <ns:AgeGroup rdf:about="http://purl.org/net/def/metashare#teenager">
    <rdf:type rdf:resource="http://purl.org/net/def/metashare#AgeOfPersons"/>
  </ns:AgeGroup>
  <ns:SourceChannel rdf:about="http://purl.org/net/def/metashare#telephone"/>
  <ns:CapturingDeviceType rdf:about="http://purl.org/net/def/metashare#telephoneFixed"/>
  <ns:CapturingDeviceType rdf:about="http://purl.org/net/def/metashare#telephoneIP"/>
  <ns:CapturingDeviceType rdf:about="http://purl.org/net/def/metashare#telephoneMobile"/>
  <owl:DatatypeProperty rdf:about="http://purl.org/net/def/metashare#telephoneNumber">
    <rdfs:comment xml:lang="en">The telephone number of a person or an organization; recommended format: +_international code_city code_number</rdfs:comment>
    <rdfs:domain>
      <owl:Class>
        <owl:unionOf>
          <rdf:Description>
            <rdf:first rdf:resource="http://purl.org/net/def/metashare#Person"/>
            <rdf:rest>
              <rdf:Description>
                <rdf:first rdf:resource="http://purl.org/net/def/metashare#Organization"/>
                <rdf:rest rdf:resource="http://www.w3.org/1999/02/22-rdf-syntax-ns#nil"/>
              </rdf:Description>
            </rdf:rest>
          </rdf:Description>
        </owl:unionOf>
      </owl:Class>
    </rdfs:domain>
    <rdfs:range rdf:resource="http://www.w3.org/2001/XMLSchema#string"/>
  </owl:DatatypeProperty>
  <ns:SpeechItems rdf:about="http://purl.org/net/def/metashare#telephoneNumbers"/>
  <ns:NonSpeechItems rdf:about="http://purl.org/net/def/metashare#tempo"/>
  <ns:UseNLPSpecific rdf:about="http://purl.org/net/def/metashare#temporalExpressionRecognition"/>
  <ns:CompatibleLexiconType rdf:about="http://purl.org/net/def/metashare#terminologicalResource">
    <rdf:type rdf:resource="http://purl.org/net/def/metashare#LexicalConceptualResourceType"/>
  </ns:CompatibleLexiconType>
  <ns:UseNLPSpecific rdf:about="http://purl.org/net/def/metashare#terminologyExtraction"/>
  <ns:SizeUnit rdf:about="http://purl.org/net/def/metashare#terms"/>
  <ns:UseNLPSpecific rdf:about="http://purl.org/net/def/metashare#texToSpeechSynthesis"/>
  <ns:MediaType rdf:about="http://purl.org/net/def/metashare#text">
    <rdf:type rdf:resource="http://purl.org/net/def/metashare#OtherMedia"/>
  </ns:MediaType>
  <ns:UseNLPSpecific rdf:about="http://purl.org/net/def/metashare#textCategorisation"/>
  <owl:ObjectProperty rdf:about="http://purl.org/net/def/metashare#textClassificationInfo">
    <rdfs:comment xml:lang="en">Groups together information on text type/genre of the resource</rdfs:comment>
    <rdfs:domain>
      <owl:Class>
        <owl:unionOf>
          <rdf:Description>
            <rdf:first rdf:resource="http://purl.org/net/def/metashare#CorpusTextNgramInfo"/>
            <rdf:rest>
              <rdf:Description>
                <rdf:first rdf:resource="http://purl.org/net/def/metashare#CorpusTextInfo"/>
                <rdf:rest rdf:resource="http://www.w3.org/1999/02/22-rdf-syntax-ns#nil"/>
              </rdf:Description>
            </rdf:rest>
          </rdf:Description>
        </owl:unionOf>
      </owl:Class>
    </rdfs:domain>
    <rdfs:range>
      <owl:Class>
        <owl:unionOf>
          <rdf:Description>
            <rdf:first rdf:resource="http://purl.org/net/def/metashare#TextClassificationInfo"/>
            <rdf:rest>
              <rdf:Description>
                <rdf:first rdf:resource="http://purl.org/net/def/metashare#TextClassificationInfo"/>
                <rdf:rest rdf:resource="http://www.w3.org/1999/02/22-rdf-syntax-ns#nil"/>
              </rdf:Description>
            </rdf:rest>
          </rdf:Description>
        </owl:unionOf>
      </owl:Class>
    </rdfs:range>
  </owl:ObjectProperty>
  <owl:ObjectProperty rdf:about="http://purl.org/net/def/metashare#textFormatInfo">
    <rdfs:comment xml:lang="en">Groups information on the text format(s) of a resource</rdfs:comment>
    <rdfs:domain>
      <owl:Class>
        <owl:unionOf>
          <rdf:Description>
            <rdf:first rdf:resource="http://purl.org/net/def/metashare#CorpusTextNgramInfo"/>
            <rdf:rest>
              <rdf:Description>
                <rdf:first rdf:resource="http://purl.org/net/def/metashare#CorpusTextInfo"/>
                <rdf:rest>
                  <rdf:Description>
                    <rdf:first rdf:resource="http://purl.org/net/def/metashare#LexicalConceptualResourceTextInfo"/>
                    <rdf:rest>
                      <rdf:Description>
                        <rdf:first rdf:resource="http://purl.org/net/def/metashare#LanguageDescriptionTextInfo"/>
                        <rdf:rest rdf:resource="http://www.w3.org/1999/02/22-rdf-syntax-ns#nil"/>
                      </rdf:Description>
                    </rdf:rest>
                  </rdf:Description>
                </rdf:rest>
              </rdf:Description>
            </rdf:rest>
          </rdf:Description>
        </owl:unionOf>
      </owl:Class>
    </rdfs:domain>
    <rdfs:range>
      <owl:Class>
        <owl:unionOf>
          <rdf:Description>
            <rdf:first rdf:resource="http://purl.org/net/def/metashare#TextFormatInfo"/>
            <rdf:rest>
              <rdf:Description>
                <rdf:first rdf:resource="http://purl.org/net/def/metashare#TextFormatInfo"/>
                <rdf:rest>
                  <rdf:Description>
                    <rdf:first rdf:resource="http://purl.org/net/def/metashare#TextFormatInfo"/>
                    <rdf:rest>
                      <rdf:Description>
                        <rdf:first rdf:resource="http://purl.org/net/def/metashare#TextFormatInfo"/>
                        <rdf:rest rdf:resource="http://www.w3.org/1999/02/22-rdf-syntax-ns#nil"/>
                      </rdf:Description>
                    </rdf:rest>
                  </rdf:Description>
                </rdf:rest>
              </rdf:Description>
            </rdf:rest>
          </rdf:Description>
        </owl:unionOf>
      </owl:Class>
    </rdfs:range>
  </owl:ObjectProperty>
  <ns:UseNLPSpecific rdf:about="http://purl.org/net/def/metashare#textGeneration"/>
  <owl:DatatypeProperty rdf:about="http://purl.org/net/def/metashare#textGenre">
    <rdfs:comment xml:lang="en">Genre: The conventionalized discourse or text types of the content of the resource, based on extra-linguistic and internal linguistic criteria</rdfs:comment>
    <rdfs:domain rdf:resource="http://purl.org/net/def/metashare#TextClassificationInfo"/>
    <rdfs:range rdf:resource="http://www.w3.org/2001/XMLSchema#string"/>
    <rdfs:subPropertyOf rdf:resource="http://purl.org/net/def/metashare#genre"/>
  </owl:DatatypeProperty>
  <owl:ObjectProperty rdf:about="http://purl.org/net/def/metashare#textIncludedInImage">
    <rdfs:comment xml:lang="en">Provides information on the type of text that may be on the image</rdfs:comment>
    <rdfs:domain>
      <owl:Class>
        <owl:unionOf>
          <rdf:Description>
            <rdf:first rdf:resource="http://purl.org/net/def/metashare#LexicalConceptualResourceImageInfo"/>
            <rdf:rest>
              <rdf:Description>
                <rdf:first rdf:resource="http://purl.org/net/def/metashare#CorpusImageInfo"/>
                <rdf:rest>
                  <rdf:Description>
                    <rdf:first rdf:resource="http://purl.org/net/def/metashare#LanguageDescriptionImageInfo"/>
                    <rdf:rest rdf:resource="http://www.w3.org/1999/02/22-rdf-syntax-ns#nil"/>
                  </rdf:Description>
                </rdf:rest>
              </rdf:Description>
            </rdf:rest>
          </rdf:Description>
        </owl:unionOf>
      </owl:Class>
    </rdfs:domain>
    <rdfs:range>
      <owl:Class>
        <owl:unionOf>
          <rdf:Description>
            <rdf:first rdf:resource="http://purl.org/net/def/metashare#TextIncludedInImage"/>
            <rdf:rest>
              <rdf:Description>
                <rdf:first rdf:resource="http://purl.org/net/def/metashare#TextIncludedInImage"/>
                <rdf:rest>
                  <rdf:Description>
                    <rdf:first rdf:resource="http://purl.org/net/def/metashare#TextIncludedInImage"/>
                    <rdf:rest rdf:resource="http://www.w3.org/1999/02/22-rdf-syntax-ns#nil"/>
                  </rdf:Description>
                </rdf:rest>
              </rdf:Description>
            </rdf:rest>
          </rdf:Description>
        </owl:unionOf>
      </owl:Class>
    </rdfs:range>
  </owl:ObjectProperty>
  <owl:ObjectProperty rdf:about="http://purl.org/net/def/metashare#textIncludedInVideo">
    <rdfs:comment xml:lang="en">Indicates if text is present in or in conjunction with the video</rdfs:comment>
    <rdfs:domain>
      <owl:Class>
        <owl:unionOf>
          <rdf:Description>
            <rdf:first rdf:resource="http://purl.org/net/def/metashare#LexicalConceptualResourceVideoInfo"/>
            <rdf:rest>
              <rdf:Description>
                <rdf:first rdf:resource="http://purl.org/net/def/metashare#LanguageDescriptionVideoInfo"/>
                <rdf:rest>
                  <rdf:Description>
                    <rdf:first rdf:resource="http://purl.org/net/def/metashare#CorpusVideoInfo"/>
                    <rdf:rest rdf:resource="http://www.w3.org/1999/02/22-rdf-syntax-ns#nil"/>
                  </rdf:Description>
                </rdf:rest>
              </rdf:Description>
            </rdf:rest>
          </rdf:Description>
        </owl:unionOf>
      </owl:Class>
    </rdfs:domain>
    <rdfs:range>
      <owl:Class>
        <owl:unionOf>
          <rdf:Description>
            <rdf:first rdf:resource="http://purl.org/net/def/metashare#TextIncludedInVideo"/>
            <rdf:rest>
              <rdf:Description>
                <rdf:first rdf:resource="http://purl.org/net/def/metashare#TextIncludedInVideo"/>
                <rdf:rest>
                  <rdf:Description>
                    <rdf:first rdf:resource="http://purl.org/net/def/metashare#TextIncludedInVideo"/>
                    <rdf:rest rdf:resource="http://www.w3.org/1999/02/22-rdf-syntax-ns#nil"/>
                  </rdf:Description>
                </rdf:rest>
              </rdf:Description>
            </rdf:rest>
          </rdf:Description>
        </owl:unionOf>
      </owl:Class>
    </rdfs:range>
  </owl:ObjectProperty>
  <ns:UseNLPSpecific rdf:about="http://purl.org/net/def/metashare#textMining"/>
  <ns:MediaType rdf:about="http://purl.org/net/def/metashare#textNgram"/>
  <ns:MediaType rdf:about="http://purl.org/net/def/metashare#textNumerical">
    <rdf:type rdf:resource="http://purl.org/net/def/metashare#OtherMedia"/>
  </ns:MediaType>
  <owl:ObjectProperty rdf:about="http://purl.org/net/def/metashare#textNumericalFormatInfo">
    <rdfs:comment xml:lang="en">Groups information on the format(s) of the textNumerical part of the resource</rdfs:comment>
    <rdfs:domain rdf:resource="http://purl.org/net/def/metashare#CorpusTextNumericalInfo"/>
    <rdfs:range rdf:resource="http://purl.org/net/def/metashare#TextNumericalFormatInfo"/>
  </owl:ObjectProperty>
  <ns:SizeUnit rdf:about="http://purl.org/net/def/metashare#texts"/>
  <ns:UseNLPSpecific rdf:about="http://purl.org/net/def/metashare#textualEntailment"/>
  <owl:DatatypeProperty rdf:about="http://purl.org/net/def/metashare#theoreticModel">
    <rdfs:comment xml:lang="en">Name of the theoretic model applied for the creation/enrichment of the resource, and/or reference (URL or bibliographic reference) to informative material about the theoretic model used</rdfs:comment>
    <rdfs:domain>
      <owl:Class>
        <owl:unionOf>
          <rdf:Description>
            <rdf:first rdf:resource="http://purl.org/net/def/metashare#LanguageDescriptionInfo"/>
            <rdf:rest>
              <rdf:Description>
                <rdf:first rdf:resource="http://purl.org/net/def/metashare#AnnotationInfo"/>
                <rdf:rest>
                  <rdf:Description>
                    <rdf:first rdf:resource="http://purl.org/net/def/metashare#LexicalConceptualResourceInfo"/>
                    <rdf:rest rdf:resource="http://www.w3.org/1999/02/22-rdf-syntax-ns#nil"/>
                  </rdf:Description>
                </rdf:rest>
              </rdf:Description>
            </rdf:rest>
          </rdf:Description>
        </owl:unionOf>
      </owl:Class>
    </rdfs:domain>
    <rdfs:range rdf:resource="http://www.w3.org/2001/XMLSchema#string"/>
  </owl:DatatypeProperty>
  <ns:CompatibleLexiconType rdf:about="http://purl.org/net/def/metashare#thesaurus">
    <rdf:type rdf:resource="http://purl.org/net/def/metashare#LexicalConceptualResourceType"/>
  </ns:CompatibleLexiconType>
  <owl:DatatypeProperty rdf:about="http://purl.org/net/def/metashare#thingDescription">
    <rdfs:comment xml:lang="en">Provides description of the things represented in the image corpus</rdfs:comment>
    <rdfs:domain rdf:resource="http://purl.org/net/def/metashare#StaticElementInfo"/>
    <rdfs:range rdf:resource="http://www.w3.org/2001/XMLSchema#string"/>
  </owl:DatatypeProperty>
  <owl:DatatypeProperty rdf:about="http://purl.org/net/def/metashare#timeCoverage">
    <rdfs:comment xml:lang="en">The time period that the content of a resource is about</rdfs:comment>
    <rdfs:domain rdf:resource="http://purl.org/net/def/metashare#TimeCoverageInfo"/>
    <rdfs:range rdf:resource="http://www.w3.org/2001/XMLSchema#string"/>
  </owl:DatatypeProperty>
  <owl:ObjectProperty rdf:about="http://purl.org/net/def/metashare#timeCoverageInfo">
    <rdfs:comment xml:lang="en">Groups together information on time classification of the resource</rdfs:comment>
    <rdfs:domain>
      <owl:Class>
        <owl:unionOf>
          <rdf:Description>
            <rdf:first rdf:resource="http://purl.org/net/def/metashare#LexicalConceptualResourceAudioInfo"/>
            <rdf:rest>
              <rdf:Description>
                <rdf:first rdf:resource="http://purl.org/net/def/metashare#LanguageDescriptionTextInfo"/>
                <rdf:rest>
                  <rdf:Description>
                    <rdf:first rdf:resource="http://purl.org/net/def/metashare#CorpusTextNgramInfo"/>
                    <rdf:rest>
                      <rdf:Description>
                        <rdf:first rdf:resource="http://purl.org/net/def/metashare#CorpusImageInfo"/>
                        <rdf:rest>
                          <rdf:Description>
                            <rdf:first rdf:resource="http://purl.org/net/def/metashare#CorpusVideoInfo"/>
                            <rdf:rest>
                              <rdf:Description>
                                <rdf:first rdf:resource="http://purl.org/net/def/metashare#LanguageDescriptionImageInfo"/>
                                <rdf:rest>
                                  <rdf:Description>
                                    <rdf:first rdf:resource="http://purl.org/net/def/metashare#LexicalConceptualResourceTextInfo"/>
                                    <rdf:rest>
                                      <rdf:Description>
                                        <rdf:first rdf:resource="http://purl.org/net/def/metashare#LexicalConceptualResourceVideoInfo"/>
                                        <rdf:rest>
                                          <rdf:Description>
                                            <rdf:first rdf:resource="http://purl.org/net/def/metashare#LexicalConceptualResourceImageInfo"/>
                                            <rdf:rest>
                                              <rdf:Description>
                                                <rdf:first rdf:resource="http://purl.org/net/def/metashare#CorpusAudioInfo"/>
                                                <rdf:rest>
                                                  <rdf:Description>
                                                    <rdf:first rdf:resource="http://purl.org/net/def/metashare#CorpusTextInfo"/>
                                                    <rdf:rest>
                                                      <rdf:Description>
                                                        <rdf:first rdf:resource="http://purl.org/net/def/metashare#LanguageDescriptionVideoInfo"/>
                                                        <rdf:rest rdf:resource="http://www.w3.org/1999/02/22-rdf-syntax-ns#nil"/>
                                                      </rdf:Description>
                                                    </rdf:rest>
                                                  </rdf:Description>
                                                </rdf:rest>
                                              </rdf:Description>
                                            </rdf:rest>
                                          </rdf:Description>
                                        </rdf:rest>
                                      </rdf:Description>
                                    </rdf:rest>
                                  </rdf:Description>
                                </rdf:rest>
                              </rdf:Description>
                            </rdf:rest>
                          </rdf:Description>
                        </rdf:rest>
                      </rdf:Description>
                    </rdf:rest>
                  </rdf:Description>
                </rdf:rest>
              </rdf:Description>
            </rdf:rest>
          </rdf:Description>
        </owl:unionOf>
      </owl:Class>
    </rdfs:domain>
    <rdfs:range>
      <owl:Class>
        <owl:unionOf>
          <rdf:Description>
            <rdf:first rdf:resource="http://purl.org/net/def/metashare#TimeCoverageInfo"/>
            <rdf:rest>
              <rdf:Description>
                <rdf:first rdf:resource="http://purl.org/net/def/metashare#TimeCoverageInfo"/>
                <rdf:rest>
                  <rdf:Description>
                    <rdf:first rdf:resource="http://purl.org/net/def/metashare#TimeCoverageInfo"/>
                    <rdf:rest>
                      <rdf:Description>
                        <rdf:first rdf:resource="http://purl.org/net/def/metashare#TimeCoverageInfo"/>
                        <rdf:rest>
                          <rdf:Description>
                            <rdf:first rdf:resource="http://purl.org/net/def/metashare#TimeCoverageInfo"/>
                            <rdf:rest>
                              <rdf:Description>
                                <rdf:first rdf:resource="http://purl.org/net/def/metashare#TimeCoverageInfo"/>
                                <rdf:rest>
                                  <rdf:Description>
                                    <rdf:first rdf:resource="http://purl.org/net/def/metashare#TimeCoverageInfo"/>
                                    <rdf:rest>
                                      <rdf:Description>
                                        <rdf:first rdf:resource="http://purl.org/net/def/metashare#TimeCoverageInfo"/>
                                        <rdf:rest>
                                          <rdf:Description>
                                            <rdf:first rdf:resource="http://purl.org/net/def/metashare#TimeCoverageInfo"/>
                                            <rdf:rest>
                                              <rdf:Description>
                                                <rdf:first rdf:resource="http://purl.org/net/def/metashare#TimeCoverageInfo"/>
                                                <rdf:rest>
                                                  <rdf:Description>
                                                    <rdf:first rdf:resource="http://purl.org/net/def/metashare#TimeCoverageInfo"/>
                                                    <rdf:rest>
                                                      <rdf:Description>
                                                        <rdf:first rdf:resource="http://purl.org/net/def/metashare#TimeCoverageInfo"/>
                                                        <rdf:rest rdf:resource="http://www.w3.org/1999/02/22-rdf-syntax-ns#nil"/>
                                                      </rdf:Description>
                                                    </rdf:rest>
                                                  </rdf:Description>
                                                </rdf:rest>
                                              </rdf:Description>
                                            </rdf:rest>
                                          </rdf:Description>
                                        </rdf:rest>
                                      </rdf:Description>
                                    </rdf:rest>
                                  </rdf:Description>
                                </rdf:rest>
                              </rdf:Description>
                            </rdf:rest>
                          </rdf:Description>
                        </rdf:rest>
                      </rdf:Description>
                    </rdf:rest>
                  </rdf:Description>
                </rdf:rest>
              </rdf:Description>
            </rdf:rest>
          </rdf:Description>
        </owl:unionOf>
      </owl:Class>
    </rdfs:range>
  </owl:ObjectProperty>
  <ns:Task rdf:about="http://purl.org/net/def/metashare#titlesParsing"/>
  <ns:SizeUnit rdf:about="http://purl.org/net/def/metashare#tokens"/>
  <ns:ToolServiceType rdf:about="http://purl.org/net/def/metashare#tool"/>
  <owl:ObjectProperty rdf:about="http://purl.org/net/def/metashare#toolDocumentationType">
    <rdfs:comment xml:lang="en">Specifies the type of documentation for tool or service</rdfs:comment>
    <rdfs:domain rdf:resource="http://purl.org/net/def/metashare#LanguageResource"/>
    <rdfs:range rdf:resource="http://purl.org/net/def/metashare#ToolDocumentationType"/>
  </owl:ObjectProperty>
  <ns:ResourceType rdf:about="http://purl.org/net/def/metashare#toolService"/>
  <owl:ObjectProperty rdf:about="http://purl.org/net/def/metashare#toolServiceInfo">
    <rdfs:comment xml:lang="en">Groups together elements required for the description of tools and services</rdfs:comment>
    <rdfs:domain rdf:resource="http://purl.org/net/def/metashare#LanguageResource"/>
    <rdfs:range rdf:resource="http://purl.org/net/def/metashare#ToolServiceInfo"/>
  </owl:ObjectProperty>
  <owl:DatatypeProperty rdf:about="http://purl.org/net/def/metashare#toolServiceSubtype">
    <rdfs:comment xml:lang="en">Specifies the subtype of tool or service</rdfs:comment>
    <rdfs:domain rdf:resource="http://purl.org/net/def/metashare#ToolServiceInfo"/>
    <rdfs:range rdf:resource="http://www.w3.org/2001/XMLSchema#string"/>
  </owl:DatatypeProperty>
  <owl:ObjectProperty rdf:about="http://purl.org/net/def/metashare#toolServiceType">
    <rdfs:comment xml:lang="en">Specifies the type of the tool or service</rdfs:comment>
    <rdfs:domain rdf:resource="http://purl.org/net/def/metashare#ToolServiceInfo"/>
    <rdfs:range rdf:resource="http://purl.org/net/def/metashare#ToolServiceType"/>
  </owl:ObjectProperty>
  <ns:SegmentationLevel rdf:about="http://purl.org/net/def/metashare#topic"/>
  <ns:UseNLPSpecific rdf:about="http://purl.org/net/def/metashare#topicDetection_Tracking"/>
  <owl:DatatypeProperty rdf:about="http://purl.org/net/def/metashare#trainedSpeaker">
    <rdfs:comment xml:lang="en">Provides information on whether the participant is trained in a specific task</rdfs:comment>
    <rdfs:domain rdf:resource="http://purl.org/net/def/metashare#ParticipantInfo"/>
    <rdfs:range rdf:resource="http://www.w3.org/2001/XMLSchema#boolean"/>
  </owl:DatatypeProperty>
  <ns:AnnotationType rdf:about="http://purl.org/net/def/metashare#translation"/>
  <ns:LinguisticInformation rdf:about="http://purl.org/net/def/metashare#translationEquivalent"/>
  <ns:AnnotationType rdf:about="http://purl.org/net/def/metashare#transliteration"/>
  <ns:RecordingEnvironment rdf:about="http://purl.org/net/def/metashare#transport"/>
  <ns:SizeUnit rdf:about="http://purl.org/net/def/metashare#trigrams"/>
  <ns:AnnotatedElements rdf:about="http://purl.org/net/def/metashare#truncation"/>
  <ns:SizeUnit rdf:about="http://purl.org/net/def/metashare#turns"/>
  <ns:SourceChannel rdf:about="http://purl.org/net/def/metashare#tv"/>
  <owl:DatatypeProperty rdf:about="http://purl.org/net/def/metashare#typeOfImageContent">
    <rdfs:comment xml:lang="en">The main types of object or people represented in the image corpus</rdfs:comment>
    <rdfs:domain>
      <owl:Class>
        <owl:unionOf>
          <rdf:Description>
            <rdf:first rdf:resource="http://purl.org/net/def/metashare#CorpusImageInfo"/>
            <rdf:rest>
              <rdf:Description>
                <rdf:first rdf:resource="http://purl.org/net/def/metashare#LexicalConceptualResourceImageInfo"/>
                <rdf:rest>
                  <rdf:Description>
                    <rdf:first rdf:resource="http://purl.org/net/def/metashare#LanguageDescriptionImageInfo"/>
                    <rdf:rest rdf:resource="http://www.w3.org/1999/02/22-rdf-syntax-ns#nil"/>
                  </rdf:Description>
                </rdf:rest>
              </rdf:Description>
            </rdf:rest>
          </rdf:Description>
        </owl:unionOf>
      </owl:Class>
    </rdfs:domain>
    <rdfs:range rdf:resource="http://www.w3.org/2001/XMLSchema#string"/>
  </owl:DatatypeProperty>
  <owl:DatatypeProperty rdf:about="http://purl.org/net/def/metashare#typeOfTextNumericalContent">
    <rdfs:comment xml:lang="en">Specifies the content that is represented in the textNumerical part of the resource</rdfs:comment>
    <rdfs:domain rdf:resource="http://purl.org/net/def/metashare#CorpusTextNumericalInfo"/>
    <rdfs:range rdf:resource="http://www.w3.org/2001/XMLSchema#string"/>
  </owl:DatatypeProperty>
  <ns:Availability rdf:about="http://purl.org/net/def/metashare#underNegotiation">
    <rdf:type rdf:resource="http://purl.org/net/def/metashare#LicenceInfo"/>
    <rdfs:comment xml:lang="en">For resources whose availability is still pending.</rdfs:comment>
  </ns:Availability>
  <ns:SizeUnit rdf:about="http://purl.org/net/def/metashare#unigrams"/>
  <ns:SizeUnit rdf:about="http://purl.org/net/def/metashare#units"/>
  <ns:OperatingSystem rdf:about="http://purl.org/net/def/metashare#unix"/>
  <ns:Origin rdf:about="http://purl.org/net/def/metashare#unknown">
    <rdf:type rdf:resource="http://purl.org/net/def/metashare#OriginOfPersons"/>
    <rdf:type rdf:resource="http://purl.org/net/def/metashare#SexOfPersons"/>
  </ns:Origin>
  <ns:SignConvention rdf:about="http://purl.org/net/def/metashare#unsignedInteger"/>
  <owl:DatatypeProperty rdf:about="http://purl.org/net/def/metashare#updateFrequency">
    <rdfs:comment xml:lang="en">Specifies the frequency with which the resource is updated</rdfs:comment>
    <rdfs:domain rdf:resource="http://purl.org/net/def/metashare#LanguageResource"/>
    <rdfs:range rdf:resource="http://www.w3.org/2001/XMLSchema#string"/>
  </owl:DatatypeProperty>
  <owl:DatatypeProperty rdf:about="http://purl.org/net/def/metashare#url">
    <rdfs:comment xml:lang="en">A URL used as homepage of an entity (e.g. of a person, organization, resource etc.) and/or where an entity (e.g.LR, document etc.) is located</rdfs:comment>
    <rdfs:domain>
      <owl:Class>
        <owl:unionOf>
          <rdf:Description>
            <rdf:first rdf:resource="http://purl.org/net/def/metashare#LanguageResource"/>
            <rdf:rest>
              <rdf:Description>
                <rdf:first rdf:resource="http://purl.org/net/def/metashare#Organization"/>
                <rdf:rest>
                  <rdf:Description>
                    <rdf:first rdf:resource="http://purl.org/net/def/metashare#Project"/>
                    <rdf:rest>
                      <rdf:Description>
                        <rdf:first rdf:resource="http://purl.org/net/def/metashare#Person"/>
                        <rdf:rest rdf:resource="http://www.w3.org/1999/02/22-rdf-syntax-ns#nil"/>
                      </rdf:Description>
                    </rdf:rest>
                  </rdf:Description>
                </rdf:rest>
              </rdf:Description>
            </rdf:rest>
          </rdf:Description>
        </owl:unionOf>
      </owl:Class>
    </rdfs:domain>
    <rdfs:range rdf:resource="http://www.w3.org/2001/XMLSchema#string"/>
  </owl:DatatypeProperty>
  <ns:EvaluationLevel rdf:about="http://purl.org/net/def/metashare#usage"/>
  <ns:LinguisticInformation rdf:about="http://purl.org/net/def/metashare#usage-Collocations"/>
  <ns:LinguisticInformation rdf:about="http://purl.org/net/def/metashare#usage-Examples"/>
  <ns:LinguisticInformation rdf:about="http://purl.org/net/def/metashare#usage-Frequency"/>
  <ns:LinguisticInformation rdf:about="http://purl.org/net/def/metashare#usage-Notes"/>
  <ns:LinguisticInformation rdf:about="http://purl.org/net/def/metashare#usage-Register"/>
  <owl:ObjectProperty rdf:about="http://purl.org/net/def/metashare#usageProject">
    <rdfs:comment xml:lang="en">Groups information on the project in which the resource has been used</rdfs:comment>
    <rdfs:domain rdf:resource="http://purl.org/net/def/metashare#ActualUseInfo"/>
    <rdfs:range rdf:resource="http://purl.org/net/def/metashare#Project"/>
  </owl:ObjectProperty>
  <owl:ObjectProperty rdf:about="http://purl.org/net/def/metashare#usageReport">
    <rdfs:comment xml:lang="en">Reports on the research papers documenting the usage of a resource, either in a structured form or in free text</rdfs:comment>
    <rdfs:domain rdf:resource="http://purl.org/net/def/metashare#ActualUseInfo"/>
    <rdfs:range rdf:resource="http://purl.org/net/def/metashare#Documentation"/>
  </owl:ObjectProperty>
  <owl:ObjectProperty rdf:about="http://purl.org/net/def/metashare#use">
    <dct:replaces rdf:resource="http://www.ilsp.gr/META-XMLSchema#actualUse"/>
    <dct:replaces rdf:resource="http://www.ilsp.gr/META-XMLSchema#foreseenUse"/>
    <rdfs:domain>
      <owl:Class>
        <owl:unionOf>
          <rdf:Description>
            <rdf:first rdf:resource="http://purl.org/net/def/metashare#ActualUseInfo"/>
            <rdf:rest>
              <rdf:Description>
                <rdf:first rdf:resource="http://purl.org/net/def/metashare#ForeseenUseInfo"/>
                <rdf:rest rdf:resource="http://www.w3.org/1999/02/22-rdf-syntax-ns#nil"/>
              </rdf:Description>
            </rdf:rest>
          </rdf:Description>
        </owl:unionOf>
      </owl:Class>
    </rdfs:domain>
    <rdfs:range>
      <owl:Class>
        <owl:unionOf>
          <rdf:Description>
            <rdf:first rdf:resource="http://purl.org/net/def/metashare#Use"/>
            <rdf:rest>
              <rdf:Description>
                <rdf:first rdf:resource="http://purl.org/net/def/metashare#Use"/>
                <rdf:rest rdf:resource="http://www.w3.org/1999/02/22-rdf-syntax-ns#nil"/>
              </rdf:Description>
            </rdf:rest>
          </rdf:Description>
        </owl:unionOf>
      </owl:Class>
    </rdfs:range>
  </owl:ObjectProperty>
  <owl:ObjectProperty rdf:about="http://purl.org/net/def/metashare#useNLPSpecific">
    <rdfs:comment xml:lang="en">Specifies the NLP application for which the resource iscreated or the application in which it has actually been used.</rdfs:comment>
    <rdfs:domain>
      <owl:Class>
        <owl:unionOf>
          <rdf:Description>
            <rdf:first rdf:resource="http://purl.org/net/def/metashare#ForeseenUseInfo"/>
            <rdf:rest>
              <rdf:Description>
                <rdf:first rdf:resource="http://purl.org/net/def/metashare#ActualUseInfo"/>
                <rdf:rest rdf:resource="http://www.w3.org/1999/02/22-rdf-syntax-ns#nil"/>
              </rdf:Description>
            </rdf:rest>
          </rdf:Description>
        </owl:unionOf>
      </owl:Class>
    </rdfs:domain>
    <rdfs:range>
      <owl:Class>
        <owl:unionOf>
          <rdf:Description>
            <rdf:first rdf:resource="http://purl.org/net/def/metashare#UseNLPSpecific"/>
            <rdf:rest>
              <rdf:Description>
                <rdf:first rdf:resource="http://purl.org/net/def/metashare#UseNLPSpecific"/>
                <rdf:rest rdf:resource="http://www.w3.org/1999/02/22-rdf-syntax-ns#nil"/>
              </rdf:Description>
            </rdf:rest>
          </rdf:Description>
        </owl:unionOf>
      </owl:Class>
    </rdfs:range>
  </owl:ObjectProperty>
  <ns:UseNLPSpecific rdf:about="http://purl.org/net/def/metashare#userAuthentication"/>
  <ns:ConditionsOfUse rdf:about="http://purl.org/net/def/metashare#userIdentified">
    <rdf:type rdf:resource="http://www.w3.org/2002/07/owl#NamedIndividual"/>
    <rdfs:comment xml:lang="en">UserIdentified refers to a kind of 'ConditionsOfUse' imposed by the licence; the resource can only be accessed by users that are identified/authenticated.</rdfs:comment>
    <rdfs:label xml:lang="en">User Identified</rdfs:label>
  </ns:ConditionsOfUse>
  <owl:ObjectProperty rdf:about="http://purl.org/net/def/metashare#userManual">
    <rdfs:comment xml:lang="en">Points to the User Manual.</rdfs:comment>
    <rdfs:domain rdf:resource="http://purl.org/net/def/metashare#LanguageResource"/>
    <rdfs:range rdf:resource="http://purl.org/net/def/metashare#DocumentInfo"/>
  </owl:ObjectProperty>
  <owl:ObjectProperty rdf:about="http://purl.org/net/def/metashare#userNature">
    <rdfs:comment xml:lang="en">The conditions imposed by the nature of the user (for instance, a research use may have different implications depending on this)</rdfs:comment>
    <rdfs:comment xml:lang="en">Used to identify the type of user of the resource (affiliated with a commercial vs. academic institution)</rdfs:comment>
    <rdfs:domain rdf:resource="http://purl.org/net/def/metashare#LicenceInfo"/>
    <rdfs:range rdf:resource="http://purl.org/net/def/metashare#UserNature"/>
  </owl:ObjectProperty>
  <ns:SegmentationLevel rdf:about="http://purl.org/net/def/metashare#utterance"/>
  <ns:SizeUnit rdf:about="http://purl.org/net/def/metashare#utterances"/>
  <owl:DatatypeProperty rdf:about="http://purl.org/net/def/metashare#validated">
    <rdfs:comment xml:lang="en">Specifies the validation status of the resource</rdfs:comment>
    <rdfs:domain rdf:resource="http://purl.org/net/def/metashare#ValidationInfo"/>
    <rdfs:range rdf:resource="http://www.w3.org/2001/XMLSchema#boolean"/>
  </owl:DatatypeProperty>
  <owl:ObjectProperty rdf:about="http://purl.org/net/def/metashare#validationExtent">
    <rdfs:comment xml:lang="en">The resource coverage in terms of validated data</rdfs:comment>
    <rdfs:domain rdf:resource="http://purl.org/net/def/metashare#ValidationInfo"/>
    <rdfs:range rdf:resource="http://purl.org/net/def/metashare#ValidationExtent"/>
  </owl:ObjectProperty>
  <owl:DatatypeProperty rdf:about="http://purl.org/net/def/metashare#validationExtentDetails">
    <rdfs:comment xml:lang="en">Provides information on size or other details of partially validated data; to be used if only part of the resource has been validated and as an alternative to SizeInfo if the validated part cannot be counted otherwise</rdfs:comment>
    <rdfs:domain rdf:resource="http://purl.org/net/def/metashare#ValidationInfo"/>
    <rdfs:range rdf:resource="http://www.w3.org/2001/XMLSchema#string"/>
  </owl:DatatypeProperty>
  <owl:ObjectProperty rdf:about="http://purl.org/net/def/metashare#validationInfo">
    <rdfs:comment xml:lang="en">Groups information on validation of a resource; it can be repeated to allow for different validations (e.g. formal validation of the whole resource; content validation of one part of the resource etc.). </rdfs:comment>
    <rdfs:domain rdf:resource="http://purl.org/net/def/metashare#LanguageResource"/>
    <rdfs:range rdf:resource="http://purl.org/net/def/metashare#ValidationInfo"/>
  </owl:ObjectProperty>
  <owl:ObjectProperty rdf:about="http://purl.org/net/def/metashare#validationMode">
    <rdfs:comment xml:lang="en">Specifies the validation methodology applied</rdfs:comment>
    <rdfs:domain rdf:resource="http://purl.org/net/def/metashare#ValidationInfo"/>
    <rdfs:range rdf:resource="http://purl.org/net/def/metashare#ValidationMode"/>
  </owl:ObjectProperty>
  <owl:DatatypeProperty rdf:about="http://purl.org/net/def/metashare#validationModeDetails">
    <rdfs:comment xml:lang="en">Textual field for additional information on validation</rdfs:comment>
    <rdfs:domain rdf:resource="http://purl.org/net/def/metashare#ValidationInfo"/>
    <rdfs:range rdf:resource="http://www.w3.org/2001/XMLSchema#string"/>
  </owl:DatatypeProperty>
  <owl:ObjectProperty rdf:about="http://purl.org/net/def/metashare#validationReport">
    <rdfs:comment xml:lang="en">A short account of the validation details or a bibliographic reference to a document with detailed information on the validation process and results</rdfs:comment>
    <rdfs:domain rdf:resource="http://purl.org/net/def/metashare#ValidationInfo"/>
    <rdfs:range rdf:resource="http://purl.org/net/def/metashare#Documentation"/>
  </owl:ObjectProperty>
  <owl:DatatypeProperty rdf:about="http://purl.org/net/def/metashare#validationTool">
    <rdfs:comment xml:lang="en">The name, the identifier or the url of the tool used for the validation of the resource</rdfs:comment>
    <rdfs:domain rdf:resource="http://purl.org/net/def/metashare#ValidationInfo"/>
    <rdfs:range rdf:resource="http://www.w3.org/2001/XMLSchema#string"/>
  </owl:DatatypeProperty>
  <owl:ObjectProperty rdf:about="http://purl.org/net/def/metashare#validationType">
    <rdfs:comment xml:lang="en">Specifies the type of the validation that have been performed </rdfs:comment>
    <rdfs:domain rdf:resource="http://purl.org/net/def/metashare#ValidationInfo"/>
    <rdfs:range rdf:resource="http://purl.org/net/def/metashare#ValidationType"/>
  </owl:ObjectProperty>
  <owl:ObjectProperty rdf:about="http://purl.org/net/def/metashare#validator">
    <rdfs:comment xml:lang="en">Groups information on the person(s) or the organization(s) that validated the resource</rdfs:comment>
    <rdfs:domain rdf:resource="http://purl.org/net/def/metashare#ValidationInfo"/>
    <rdfs:range rdf:resource="http://purl.org/net/def/metashare#Actor"/>
  </owl:ObjectProperty>
  <ns:SceneIllumination rdf:about="http://purl.org/net/def/metashare#variable"/>
  <ns:SpeechItems rdf:about="http://purl.org/net/def/metashare#vcvSequences"/>
  <ns:RasterOrVectorGraphics rdf:about="http://purl.org/net/def/metashare#vector"/>
  <ns:Quality rdf:about="http://purl.org/net/def/metashare#veryHigh">
    <rdf:type rdf:resource="http://purl.org/net/def/metashare#RecordingQuality"/>
  </ns:Quality>
  <ns:Quality rdf:about="http://purl.org/net/def/metashare#veryLow">
    <rdf:type rdf:resource="http://purl.org/net/def/metashare#RecordingQuality"/>
  </ns:Quality>
  <ns:MediaType rdf:about="http://purl.org/net/def/metashare#video">
    <rdf:type rdf:resource="http://purl.org/net/def/metashare#OtherMedia"/>
  </ns:MediaType>
  <owl:ObjectProperty rdf:about="http://purl.org/net/def/metashare#videoClassificationInfo">
    <rdfs:comment xml:lang="en">Groups together information on video genre of the resource</rdfs:comment>
    <rdfs:domain rdf:resource="http://purl.org/net/def/metashare#CorpusVideoInfo"/>
    <rdfs:range rdf:resource="http://purl.org/net/def/metashare#VideoClassificationInfo"/>
  </owl:ObjectProperty>
  <owl:ObjectProperty rdf:about="http://purl.org/net/def/metashare#videoFormatInfo">
    <rdfs:comment xml:lang="en">Groups information on the format(s) of a resource; repeated if parts of the resource are in different formats</rdfs:comment>
    <rdfs:domain>
      <owl:Class>
        <owl:unionOf>
          <rdf:Description>
            <rdf:first rdf:resource="http://purl.org/net/def/metashare#LanguageDescriptionVideoInfo"/>
            <rdf:rest>
              <rdf:Description>
                <rdf:first rdf:resource="http://purl.org/net/def/metashare#LexicalConceptualResourceVideoInfo"/>
                <rdf:rest>
                  <rdf:Description>
                    <rdf:first rdf:resource="http://purl.org/net/def/metashare#CorpusVideoInfo"/>
                    <rdf:rest rdf:resource="http://www.w3.org/1999/02/22-rdf-syntax-ns#nil"/>
                  </rdf:Description>
                </rdf:rest>
              </rdf:Description>
            </rdf:rest>
          </rdf:Description>
        </owl:unionOf>
      </owl:Class>
    </rdfs:domain>
    <rdfs:range>
      <owl:Class>
        <owl:unionOf>
          <rdf:Description>
            <rdf:first rdf:resource="http://purl.org/net/def/metashare#VideoFormatInfo"/>
            <rdf:rest>
              <rdf:Description>
                <rdf:first rdf:resource="http://purl.org/net/def/metashare#VideoFormatInfo"/>
                <rdf:rest>
                  <rdf:Description>
                    <rdf:first rdf:resource="http://purl.org/net/def/metashare#VideoFormatInfo"/>
                    <rdf:rest rdf:resource="http://www.w3.org/1999/02/22-rdf-syntax-ns#nil"/>
                  </rdf:Description>
                </rdf:rest>
              </rdf:Description>
            </rdf:rest>
          </rdf:Description>
        </owl:unionOf>
      </owl:Class>
    </rdfs:range>
  </owl:ObjectProperty>
  <owl:DatatypeProperty rdf:about="http://purl.org/net/def/metashare#videoGenre">
    <rdfs:comment xml:lang="en">A first indication of type of video recorded</rdfs:comment>
    <rdfs:domain rdf:resource="http://purl.org/net/def/metashare#VideoClassificationInfo"/>
    <rdfs:range rdf:resource="http://www.w3.org/2001/XMLSchema#string"/>
    <rdfs:subPropertyOf rdf:resource="http://purl.org/net/def/metashare#genre"/>
  </owl:DatatypeProperty>
  <ns:ExtratextualInformation rdf:about="http://purl.org/net/def/metashare#videos"/>
  <owl:ObjectProperty rdf:about="http://purl.org/net/def/metashare#visualModelling">
    <rdfs:comment xml:lang="en">The dimensional form applied on video or image corpus</rdfs:comment>
    <rdfs:domain>
      <owl:Class>
        <owl:unionOf>
          <rdf:Description>
            <rdf:first rdf:resource="http://purl.org/net/def/metashare#ImageFormatInfo"/>
            <rdf:rest>
              <rdf:Description>
                <rdf:first rdf:resource="http://purl.org/net/def/metashare#VideoFormatInfo"/>
                <rdf:rest rdf:resource="http://www.w3.org/1999/02/22-rdf-syntax-ns#nil"/>
              </rdf:Description>
            </rdf:rest>
          </rdf:Description>
        </owl:unionOf>
      </owl:Class>
    </rdfs:domain>
    <rdfs:range>
      <owl:Class>
        <owl:unionOf>
          <rdf:Description>
            <rdf:first rdf:resource="http://purl.org/net/def/metashare#VisualModelling"/>
            <rdf:rest>
              <rdf:Description>
                <rdf:first rdf:resource="http://purl.org/net/def/metashare#VisualModelling"/>
                <rdf:rest rdf:resource="http://www.w3.org/1999/02/22-rdf-syntax-ns#nil"/>
              </rdf:Description>
            </rdf:rest>
          </rdf:Description>
        </owl:unionOf>
      </owl:Class>
    </rdfs:range>
  </owl:ObjectProperty>
  <ns:UseNLPSpecific rdf:about="http://purl.org/net/def/metashare#visualSceneUnderstanding"/>
  <owl:DatatypeProperty rdf:about="http://purl.org/net/def/metashare#vocalTractConditions">
    <rdfs:comment xml:lang="en">Provides information on the vocal tract conditions that may influence the speech of the participant</rdfs:comment>
    <rdfs:domain rdf:resource="http://purl.org/net/def/metashare#ParticipantInfo"/>
    <rdfs:range rdf:resource="http://www.w3.org/2001/XMLSchema#string"/>
  </owl:DatatypeProperty>
  <ns:ModalityType rdf:about="http://purl.org/net/def/metashare#voice"/>
  <ns:UseNLPSpecific rdf:about="http://purl.org/net/def/metashare#voiceControl"/>
  <ns:SourceChannel rdf:about="http://purl.org/net/def/metashare#webCam"/>
  <ns:DistributionAccessMedium rdf:about="http://purl.org/net/def/metashare#webExecutable"/>
  <ns:UseNLPSpecific rdf:about="http://purl.org/net/def/metashare#webServices"/>
  <ns:CapturingDeviceType rdf:about="http://purl.org/net/def/metashare#webcam"/>
  <owl:DatatypeProperty rdf:about="http://purl.org/net/def/metashare#weight">
    <rdfs:comment xml:lang="en">Provides information on the weight of the participant</rdfs:comment>
    <rdfs:domain rdf:resource="http://purl.org/net/def/metashare#ParticipantInfo"/>
    <rdfs:range rdf:resource="http://www.w3.org/2001/XMLSchema#int"/>
  </owl:DatatypeProperty>
  <owl:DatatypeProperty rdf:about="http://purl.org/net/def/metashare#weightedGrammar">
    <rdfs:comment xml:lang="en">Indicates whether the grammar contains numerical weights (incl. probabilities)</rdfs:comment>
    <rdfs:domain rdf:resource="http://purl.org/net/def/metashare#LanguageDescriptionInfo"/>
    <rdfs:range rdf:resource="http://www.w3.org/2001/XMLSchema#boolean"/>
  </owl:DatatypeProperty>
  <ns:BodyParts rdf:about="http://purl.org/net/def/metashare#wholeBody"/>
  <ns:OperatingSystem rdf:about="http://purl.org/net/def/metashare#windows"/>
  <ns:CharacterEncoding rdf:about="http://purl.org/net/def/metashare#windows-1250"/>
  <ns:CharacterEncoding rdf:about="http://purl.org/net/def/metashare#windows-1251"/>
  <ns:CharacterEncoding rdf:about="http://purl.org/net/def/metashare#windows-1252"/>
  <ns:CharacterEncoding rdf:about="http://purl.org/net/def/metashare#windows-1253"/>
  <ns:CharacterEncoding rdf:about="http://purl.org/net/def/metashare#windows-1254"/>
  <ns:CharacterEncoding rdf:about="http://purl.org/net/def/metashare#windows-1255"/>
  <ns:CharacterEncoding rdf:about="http://purl.org/net/def/metashare#windows-1256"/>
  <ns:CharacterEncoding rdf:about="http://purl.org/net/def/metashare#windows-1257"/>
  <ns:CharacterEncoding rdf:about="http://purl.org/net/def/metashare#windows-1258"/>
  <ns:CharacterEncoding rdf:about="http://purl.org/net/def/metashare#windows-31j"/>
  <ns:ScenarioType rdf:about="http://purl.org/net/def/metashare#wizardOfOz"/>
  <ns:BaseItem rdf:about="http://purl.org/net/def/metashare#word">
    <rdf:type rdf:resource="http://purl.org/net/def/metashare#ExtraTextualInformationUnit"/>
    <rdf:type rdf:resource="http://purl.org/net/def/metashare#SegmentationLevel"/>
  </ns:BaseItem>
  <ns:ScenarioType rdf:about="http://purl.org/net/def/metashare#wordGame"/>
  <ns:SegmentationLevel rdf:about="http://purl.org/net/def/metashare#wordGroup"/>
  <ns:CompatibleLexiconType rdf:about="http://purl.org/net/def/metashare#wordList">
    <rdf:type rdf:resource="http://purl.org/net/def/metashare#LexicalConceptualResourceType"/>
  </ns:CompatibleLexiconType>
  <rdf:Description rdf:about="http://purl.org/net/def/metashare#wordNet">
    <dct:replaces rdf:resource="http://www.ilsp.gr/META-XMLSchema#wordnet"/>
  </rdf:Description>
  <ns:UseNLPSpecific rdf:about="http://purl.org/net/def/metashare#wordSenseDisambiguation"/>
  <ns:CompatibleLexiconType rdf:about="http://purl.org/net/def/metashare#wordlist"/>
  <ns:CompatibleLexiconType rdf:about="http://purl.org/net/def/metashare#wordnet">
    <rdf:type rdf:resource="http://purl.org/net/def/metashare#LexicalConceptualResourceType"/>
  </ns:CompatibleLexiconType>
  <ns:SizeUnit rdf:about="http://purl.org/net/def/metashare#words"/>
  <ns:ModalityType rdf:about="http://purl.org/net/def/metashare#writtenLanguage"/>
  <ns:CharacterEncoding rdf:about="http://purl.org/net/def/metashare#x-EUC-CN"/>
  <ns:CharacterEncoding rdf:about="http://purl.org/net/def/metashare#x-EUC-JP-LINUX"/>
  <ns:CharacterEncoding rdf:about="http://purl.org/net/def/metashare#x-EUC-TW"/>
  <ns:CharacterEncoding rdf:about="http://purl.org/net/def/metashare#x-MS950-HKSCS"/>
  <ns:CharacterEncoding rdf:about="http://purl.org/net/def/metashare#x-mswin-936"/>
  <ns:CharacterEncoding rdf:about="http://purl.org/net/def/metashare#x-windows-949"/>
  <ns:CharacterEncoding rdf:about="http://purl.org/net/def/metashare#x-windows-950"/>
  <ns:HearingImpairmentOfPersons rdf:about="http://purl.org/net/def/metashare#yes">
    <rdf:type rdf:resource="http://purl.org/net/def/metashare#SpeakingImpairmentOfPersons"/>
  </ns:HearingImpairmentOfPersons>
  <ns:SpeechItems rdf:about="http://purl.org/net/def/metashare#yesNoQuestions"/>
  <owl:DatatypeProperty rdf:about="http://purl.org/net/def/metashare#zipCode">
    <rdfs:comment xml:lang="en">The zip code of the postal address of a person or organization </rdfs:comment>
    <rdfs:domain>
      <owl:Class>
        <owl:unionOf>
          <rdf:Description>
            <rdf:first rdf:resource="http://purl.org/net/def/metashare#Person"/>
            <rdf:rest>
              <rdf:Description>
                <rdf:first rdf:resource="http://purl.org/net/def/metashare#Organization"/>
                <rdf:rest rdf:resource="http://www.w3.org/1999/02/22-rdf-syntax-ns#nil"/>
              </rdf:Description>
            </rdf:rest>
          </rdf:Description>
        </owl:unionOf>
      </owl:Class>
    </rdfs:domain>
    <rdfs:range rdf:resource="http://www.w3.org/2001/XMLSchema#string"/>
  </owl:DatatypeProperty>
  <ns:SpeechAnnotation rdf:about="http://purl.org/net/def/speechAnnotation-soundToTextAlignment"/>
  <rdfs:Datatype rdf:about="http://www.w3.org/1999/02/22-rdf-syntax-ns#langString"/>
</rdf:RDF>
